@prefix schema: <http://schema.org/> .
@prefix void:  <http://rdfs.org/ns/void#> .
@prefix obda:  <https://w3id.org/obda/vocabulary#> .
@prefix data:  <http://destination.example.org/data/> .
@prefix owl:   <http://www.w3.org/2002/07/owl#> .
@prefix gml:   <http://www.opengis.net/ont/gml#> .
@prefix xsd:   <http://www.w3.org/2001/XMLSchema#> .
@prefix dcmitype: <http://purl.org/dc/dcmitype/> .
@prefix rdfs:  <http://www.w3.org/2000/01/rdf-schema#> .
@prefix voc:   <http://destination.example.org/ontology/dest#> .
@prefix ns1:   <http://www.w3.org/2004/02/skos/core#> .
@prefix ssn:   <http://www.w3.org/ns/ssn/> .
@prefix geo:   <http://www.opengis.net/ont/geosparql#> .
@prefix cdt:   <http://w3id.org/lindt/custom_datatypes#> .
@prefix sf:    <http://www.opengis.net/ont/sf#> .
@prefix rdf:   <http://www.w3.org/1999/02/22-rdf-syntax-ns#> .
@prefix xml:   <http://www.w3.org/XML/1998/namespace> .
@prefix bibo:  <http://purl.org/ontology/bibo/> .
@prefix dcat:  <http://www.w3.org/ns/dcat#> .
@prefix foaf:  <http://xmlns.com/foaf/0.1/> .
@prefix sosa:  <http://www.w3.org/ns/sosa/> .

schema:Sculpture  a      rdfs:Class ;
        rdfs:comment     "A piece of sculpture." ;
        rdfs:label       "Sculpture" ;
        rdfs:subClassOf  schema:CreativeWork .

schema:contentRating  a  rdf:Property ;
        rdfs:comment  "Official rating of a piece of content&#x2014;for example,'MPAA PG-13'." ;
        rdfs:label    "contentRating" .

schema:Recipe  a         rdfs:Class ;
        rdfs:comment     "A recipe. For dietary restrictions covered by the recipe, a few common restrictions are enumerated via [[suitableForDiet]]. The [[keywords]] property can also be used to add more detail." ;
        rdfs:label       "Recipe" ;
        rdfs:subClassOf  schema:HowTo .

schema:Brand  a          rdfs:Class ;
        rdfs:comment     "A brand is a name used by an organization or business person for labeling a product, product group, or similar." ;
        rdfs:label       "Brand" ;
        rdfs:subClassOf  schema:Intangible .

schema:creator  a     rdf:Property ;
        rdfs:comment  "The creator/author of this CreativeWork. This is the same as the Author property for CreativeWork." ;
        rdfs:label    "creator" .

schema:Barcode  a        rdfs:Class ;
        rdfs:comment     "An image of a visual machine-readable code such as a barcode or QR code." ;
        rdfs:label       "Barcode" ;
        rdfs:subClassOf  schema:ImageObject .

schema:ReturnAction  a   rdfs:Class ;
        rdfs:comment     "The act of returning to the origin that which was previously received (concrete objects) or taken (ownership)." ;
        rdfs:label       "ReturnAction" ;
        rdfs:subClassOf  schema:TransferAction .

schema:departureStation
        a             rdf:Property ;
        rdfs:comment  "The station from which the train departs." ;
        rdfs:label    "departureStation" .

schema:PathologyTest  a  rdfs:Class ;
        rdfs:comment     "A medical test performed by a laboratory that typically involves examination of a tissue sample by a pathologist." ;
        rdfs:label       "PathologyTest" ;
        rdfs:subClassOf  schema:MedicalTest .

schema:Nerve  a          rdfs:Class ;
        rdfs:comment     "A common pathway for the electrochemical nerve impulses that are transmitted along each of the axons." ;
        rdfs:label       "Nerve" ;
        rdfs:subClassOf  schema:AnatomicalStructure .

schema:sdPublisher  a  rdf:Property ;
        rdfs:comment  "Indicates the party responsible for generating and publishing the current structured data markup, typically in cases where the structured data is derived automatically from existing published content but published on a different site. For example, student projects and open data initiatives often re-publish existing content with more explicitly structured metadata. The\n[[sdPublisher]] property helps make such practices more explicit." ;
        rdfs:label    "sdPublisher" .

schema:trackingUrl  a  rdf:Property ;
        rdfs:comment  "Tracking url for the parcel delivery." ;
        rdfs:label    "trackingUrl" .

schema:suitableForDiet
        a             rdf:Property ;
        rdfs:comment  "Indicates a dietary restriction or guideline for which this recipe or menu item is suitable, e.g. diabetic, halal etc." ;
        rdfs:label    "suitableForDiet" .

schema:linkRelationship
        a             rdf:Property ;
        rdfs:comment  "Indicates the relationship type of a Web link. " ;
        rdfs:label    "linkRelationship" .

schema:foodEvent  a         rdf:Property ;
        rdfs:comment        "A sub property of location. The specific food event where the action occurred." ;
        rdfs:label          "foodEvent" ;
        rdfs:subPropertyOf  schema:location .

schema:course  a            rdf:Property ;
        rdfs:comment        "A sub property of location. The course where this action was taken." ;
        rdfs:label          "course" ;
        rdfs:subPropertyOf  schema:location .

schema:Optometric  a     rdfs:Class ;
        rdfs:comment     "The science or practice of testing visual acuity and prescribing corrective lenses." ;
        rdfs:label       "Optometric" ;
        rdfs:subClassOf  schema:MedicalBusiness .

schema:CookAction  a     rdfs:Class ;
        rdfs:comment     "The act of producing/preparing food." ;
        rdfs:label       "CookAction" ;
        rdfs:subClassOf  schema:CreateAction .

schema:maximumAttendeeCapacity
        a             rdf:Property ;
        rdfs:comment  "The total number of individuals that may attend an event or venue." ;
        rdfs:label    "maximumAttendeeCapacity" .

schema:ViewAction  a     rdfs:Class ;
        rdfs:comment     "The act of consuming static visual content." ;
        rdfs:label       "ViewAction" ;
        rdfs:subClassOf  schema:ConsumeAction .

schema:firstPerformance
        a             rdf:Property ;
        rdfs:comment  "The date and place the work was first performed." ;
        rdfs:label    "firstPerformance" .

schema:bitrate  a     rdf:Property ;
        rdfs:comment  "The bitrate of the media object." ;
        rdfs:label    "bitrate" .

schema:MusicVideoObject
        a                rdfs:Class ;
        rdfs:comment     "A music video file." ;
        rdfs:label       "MusicVideoObject" ;
        rdfs:subClassOf  schema:MediaObject .

schema:paymentStatus  a  rdf:Property ;
        rdfs:comment  "The status of payment; whether the invoice has been paid or not." ;
        rdfs:label    "paymentStatus" .

schema:manufacturer  a  rdf:Property ;
        rdfs:comment  "The manufacturer of the product." ;
        rdfs:label    "manufacturer" .

schema:Dermatology  a    rdfs:Class ;
        rdfs:comment     "A specific branch of medical science that pertains to diagnosis and treatment of disorders of skin." ;
        rdfs:label       "Dermatology" ;
        rdfs:subClassOf  schema:MedicalBusiness .

schema:author  a      rdf:Property ;
        rdfs:comment  "The author of this content or rating. Please note that author is special in that HTML 5 provides a special mechanism for indicating authorship via the rel tag. That is equivalent to this and may be used interchangeably." ;
        rdfs:label    "author" .

schema:ReviewNewsArticle
        a                rdfs:Class ;
        rdfs:comment     "A [[NewsArticle]] and [[CriticReview]] providing a professional critic's assessment of a service, product, performance, or artistic or literary work." ;
        rdfs:label       "ReviewNewsArticle" ;
        rdfs:subClassOf  schema:CriticReview , schema:NewsArticle .

schema:AmpStory  a       rdfs:Class ;
        rdfs:comment     "A creative work with a visual storytelling format intended to be viewed online, particularly on mobile devices." ;
        rdfs:label       "AmpStory" ;
        rdfs:subClassOf  schema:CreativeWork .

schema:UserInteraction
        a                rdfs:Class ;
        rdfs:comment     "UserInteraction and its subtypes is an old way of talking about users interacting with pages. It is generally better to use [[Action]]-based vocabulary, alongside types such as [[Comment]]." ;
        rdfs:label       "UserInteraction" ;
        rdfs:subClassOf  schema:Event .

schema:OrderStatus  a    rdfs:Class ;
        rdfs:comment     "Enumerated status values for Order." ;
        rdfs:label       "OrderStatus" ;
        rdfs:subClassOf  schema:StatusEnumeration .

schema:nonEqual  a    rdf:Property ;
        rdfs:comment  "This ordering relation for qualitative values indicates that the subject is not equal to the object." ;
        rdfs:label    "nonEqual" .

schema:School  a         rdfs:Class ;
        rdfs:comment     "A school." ;
        rdfs:label       "School" ;
        rdfs:subClassOf  schema:EducationalOrganization .

schema:BusinessFunction
        a                rdfs:Class ;
        rdfs:comment     "The business function specifies the type of activity or access (i.e., the bundle of rights) offered by the organization or business person through the offer. Typical are sell, rental or lease, maintenance or repair, manufacture / produce, recycle / dispose, engineering / construction, or installation. Proprietary specifications of access rights are also instances of this class.\\n\\nCommonly used values:\\n\\n* http://purl.org/goodrelations/v1#ConstructionInstallation\\n* http://purl.org/goodrelations/v1#Dispose\\n* http://purl.org/goodrelations/v1#LeaseOut\\n* http://purl.org/goodrelations/v1#Maintain\\n* http://purl.org/goodrelations/v1#ProvideService\\n* http://purl.org/goodrelations/v1#Repair\\n* http://purl.org/goodrelations/v1#Sell\\n* http://purl.org/goodrelations/v1#Buy\n        " ;
        rdfs:label       "BusinessFunction" ;
        rdfs:subClassOf  schema:Enumeration .

schema:recipient  a         rdf:Property ;
        rdfs:comment        "A sub property of participant. The participant who is at the receiving end of the action." ;
        rdfs:label          "recipient" ;
        rdfs:subPropertyOf  schema:participant .

schema:reviewAspect  a  rdf:Property ;
        rdfs:comment  "This Review or Rating is relevant to this part or facet of the itemReviewed." ;
        rdfs:label    "reviewAspect" .

schema:step  a        rdf:Property ;
        rdfs:comment  "A single step item (as HowToStep, text, document, video, etc.) or a HowToSection." ;
        rdfs:label    "step" .

schema:children  a    rdf:Property ;
        rdfs:comment  "A child of the person." ;
        rdfs:label    "children" .

schema:proteinContent
        a             rdf:Property ;
        rdfs:comment  "The number of grams of protein." ;
        rdfs:label    "proteinContent" .

schema:applicantLocationRequirements
        a             rdf:Property ;
        rdfs:comment  "The location(s) applicants can apply from. This is usually used for telecommuting jobs where the applicant does not need to be in a physical office. Note: This should not be used for citizenship or work visa requirements." ;
        rdfs:label    "applicantLocationRequirements" .

schema:RegisterAction
        a                rdfs:Class ;
        rdfs:comment     "The act of registering to be a user of a service, product or web page.\\n\\nRelated actions:\\n\\n* [[JoinAction]]: Unlike JoinAction, RegisterAction implies you are registering to be a user of a service, *not* a group/team of people.\\n* [FollowAction]]: Unlike FollowAction, RegisterAction doesn't imply that the agent is expecting to poll for updates from the object.\\n* [[SubscribeAction]]: Unlike SubscribeAction, RegisterAction doesn't imply that the agent is expecting updates from the object." ;
        rdfs:label       "RegisterAction" ;
        rdfs:subClassOf  schema:InteractAction .

schema:WarrantyPromise
        a                rdfs:Class ;
        rdfs:comment     "A structured value representing the duration and scope of services that will be provided to a customer free of charge in case of a defect or malfunction of a product." ;
        rdfs:label       "WarrantyPromise" ;
        rdfs:subClassOf  schema:StructuredValue .

schema:Guide  a          rdfs:Class ;
        rdfs:comment     "[[Guide]] is a page or article that recommend specific products or services, or aspects of a thing for a user to consider. A [[Guide]] may represent a Buying Guide and detail aspects of products or services for a user to consider. A [[Guide]] may represent a Product Guide and recommend specific products or services. A [[Guide]] may represent a Ranked List and recommend specific products or services with ranking." ;
        rdfs:label       "Guide" ;
        rdfs:subClassOf  schema:CreativeWork .

schema:roleName  a    rdf:Property ;
        rdfs:comment  "A role played, performed or filled by a person or organization. For example, the team of creators for a comic book might fill the roles named 'inker', 'penciller', and 'letterer'; or an athlete in a SportsTeam might play in the position named 'Quarterback'." ;
        rdfs:label    "roleName" .

schema:AssessAction  a   rdfs:Class ;
        rdfs:comment     "The act of forming one's opinion, reaction or sentiment." ;
        rdfs:label       "AssessAction" ;
        rdfs:subClassOf  schema:Action .

schema:contactPoints  a  rdf:Property ;
        rdfs:comment  "A contact point for a person or organization." ;
        rdfs:label    "contactPoints" .

schema:ReturnFeesEnumeration
        a                rdfs:Class ;
        rdfs:comment     "ReturnFeesEnumeration expresses policies for return fees." ;
        rdfs:label       "ReturnFeesEnumeration" ;
        rdfs:subClassOf  schema:Enumeration .

schema:BikeStore  a      rdfs:Class ;
        rdfs:comment     "A bike store." ;
        rdfs:label       "BikeStore" ;
        rdfs:subClassOf  schema:Store .

schema:DrawAction  a     rdfs:Class ;
        rdfs:comment     "The act of producing a visual/graphical representation of an object, typically with a pen/pencil and paper as instruments." ;
        rdfs:label       "DrawAction" ;
        rdfs:subClassOf  schema:CreateAction .

schema:yearlyRevenue  a  rdf:Property ;
        rdfs:comment  "The size of the business in annual revenue." ;
        rdfs:label    "yearlyRevenue" .

schema:PropertyValueSpecification
        a                rdfs:Class ;
        rdfs:comment     "A Property value specification." ;
        rdfs:label       "PropertyValueSpecification" ;
        rdfs:subClassOf  schema:Intangible .

schema:vatID  a       rdf:Property ;
        rdfs:comment  "The Value-added Tax ID of the organization or person." ;
        rdfs:label    "vatID" .

schema:MedicalIntangible
        a                rdfs:Class ;
        rdfs:comment     "A utility class that serves as the umbrella for a number of 'intangible' things in the medical space." ;
        rdfs:label       "MedicalIntangible" ;
        rdfs:subClassOf  schema:MedicalEntity .

schema:broadcastSignalModulation
        a             rdf:Property ;
        rdfs:comment  "The modulation (e.g. FM, AM, etc) used by a particular broadcast service." ;
        rdfs:label    "broadcastSignalModulation" .

schema:workHours  a   rdf:Property ;
        rdfs:comment  "The typical working hours for this job (e.g. 1st shift, night shift, 8am-5pm)." ;
        rdfs:label    "workHours" .

schema:EndorseAction  a  rdfs:Class ;
        rdfs:comment     "An agent approves/certifies/likes/supports/sanction an object." ;
        rdfs:label       "EndorseAction" ;
        rdfs:subClassOf  schema:ReactAction .

schema:HinduTemple  a    rdfs:Class ;
        rdfs:comment     "A Hindu temple." ;
        rdfs:label       "HinduTemple" ;
        rdfs:subClassOf  schema:PlaceOfWorship .

schema:commentText  a  rdf:Property ;
        rdfs:comment  "The text of the UserComment." ;
        rdfs:label    "commentText" .

schema:contentType  a  rdf:Property ;
        rdfs:comment  "The supported content type(s) for an EntryPoint response." ;
        rdfs:label    "contentType" .

schema:requiredMinAge
        a             rdf:Property ;
        rdfs:comment  "Audiences defined by a person's minimum age." ;
        rdfs:label    "requiredMinAge" .

schema:DanceEvent  a     rdfs:Class ;
        rdfs:comment     "Event type: A social dance." ;
        rdfs:label       "DanceEvent" ;
        rdfs:subClassOf  schema:Event .

schema:honorificSuffix
        a             rdf:Property ;
        rdfs:comment  "An honorific suffix following a Person's name such as M.D. /PhD/MSCSW." ;
        rdfs:label    "honorificSuffix" .

schema:WatchAction  a    rdfs:Class ;
        rdfs:comment     "The act of consuming dynamic/moving visual content." ;
        rdfs:label       "WatchAction" ;
        rdfs:subClassOf  schema:ConsumeAction .

schema:domiciledMortgage
        a             rdf:Property ;
        rdfs:comment  "Whether borrower is a resident of the jurisdiction where the property is located." ;
        rdfs:label    "domiciledMortgage" .

schema:productionCompany
        a             rdf:Property ;
        rdfs:comment  "The production company or studio responsible for the item e.g. series, video game, episode etc." ;
        rdfs:label    "productionCompany" .

schema:typeOfBed  a   rdf:Property ;
        rdfs:comment  "The type of bed to which the BedDetail refers, i.e. the type of bed available in the quantity indicated by quantity." ;
        rdfs:label    "typeOfBed" .

schema:SportsActivityLocation
        a                rdfs:Class ;
        rdfs:comment     "A sports location, such as a playing field." ;
        rdfs:label       "SportsActivityLocation" ;
        rdfs:subClassOf  schema:LocalBusiness .

schema:sampleType  a  rdf:Property ;
        rdfs:comment  "What type of code sample: full (compile ready) solution, code snippet, inline code, scripts, template." ;
        rdfs:label    "sampleType" .

schema:RealEstateAgent
        a                rdfs:Class ;
        rdfs:comment     "A real-estate agent." ;
        rdfs:label       "RealEstateAgent" ;
        rdfs:subClassOf  schema:LocalBusiness .

schema:TextDigitalDocument
        a                rdfs:Class ;
        rdfs:comment     "A file composed primarily of text." ;
        rdfs:label       "TextDigitalDocument" ;
        rdfs:subClassOf  schema:DigitalDocument .

schema:payload  a     rdf:Property ;
        rdfs:comment  "The permitted weight of passengers and cargo, EXCLUDING the weight of the empty vehicle.\\n\\nTypical unit code(s): KGM for kilogram, LBR for pound\\n\\n* Note 1: Many databases specify the permitted TOTAL weight instead, which is the sum of [[weight]] and [[payload]]\\n* Note 2: You can indicate additional information in the [[name]] of the [[QuantitativeValue]] node.\\n* Note 3: You may also link to a [[QualitativeValue]] node that provides additional information using [[valueReference]].\\n* Note 4: Note that you can use [[minValue]] and [[maxValue]] to indicate ranges." ;
        rdfs:label    "payload" .

schema:broadcastOfEvent
        a             rdf:Property ;
        rdfs:comment  "The event being broadcast such as a sporting event or awards ceremony." ;
        rdfs:label    "broadcastOfEvent" .

schema:LegislationObject
        a                rdfs:Class ;
        rdfs:comment     "A specific object or file containing a Legislation. Note that the same Legislation can be published in multiple files. For example, a digitally signed PDF, a plain PDF and an HTML version." ;
        rdfs:label       "LegislationObject" ;
        rdfs:subClassOf  schema:MediaObject , schema:Legislation .

schema:departureBusStop
        a             rdf:Property ;
        rdfs:comment  "The stop or station from which the bus departs." ;
        rdfs:label    "departureBusStop" .

schema:numTracks  a   rdf:Property ;
        rdfs:comment  "The number of tracks in this album or playlist." ;
        rdfs:label    "numTracks" .

schema:percentile25  a  rdf:Property ;
        rdfs:comment  "The 25th percentile value." ;
        rdfs:label    "percentile25" .

schema:suggestedMaxAge
        a             rdf:Property ;
        rdfs:comment  "Maximum recommended age in years for the audience or user." ;
        rdfs:label    "suggestedMaxAge" .

schema:tocEntry  a          rdf:Property ;
        rdfs:comment        "Indicates a [[HyperTocEntry]] in a [[HyperToc]]." ;
        rdfs:label          "tocEntry" ;
        rdfs:subPropertyOf  schema:hasPart .

schema:hasCategoryCode
        a                   rdf:Property ;
        rdfs:comment        "A Category code contained in this code set." ;
        rdfs:label          "hasCategoryCode" ;
        rdfs:subPropertyOf  schema:hasDefinedTerm .

schema:partOfTVSeries
        a                   rdf:Property ;
        rdfs:comment        "The TV series to which this episode or season belongs." ;
        rdfs:label          "partOfTVSeries" ;
        rdfs:subPropertyOf  schema:isPartOf .

schema:ParkingFacility
        a                rdfs:Class ;
        rdfs:comment     "A parking lot or other parking facility." ;
        rdfs:label       "ParkingFacility" ;
        rdfs:subClassOf  schema:CivicStructure .

schema:softwareVersion
        a             rdf:Property ;
        rdfs:comment  "Version of the software instance." ;
        rdfs:label    "softwareVersion" .

schema:study  a       rdf:Property ;
        rdfs:comment  "A medical study or trial related to this entity." ;
        rdfs:label    "study" .

schema:inverseOf  a   rdf:Property ;
        rdfs:comment  "Relates a property to a property that is its inverse. Inverse properties relate the same pairs of items to each other, but in reversed direction. For example, the 'alumni' and 'alumniOf' properties are inverseOf each other. Some properties don't have explicit inverses; in these situations RDFa and JSON-LD syntax for reverse properties can be used." ;
        rdfs:label    "inverseOf" .

schema:RadioClip  a      rdfs:Class ;
        rdfs:comment     "A short radio program or a segment/part of a radio program." ;
        rdfs:label       "RadioClip" ;
        rdfs:subClassOf  schema:Clip .

schema:referenceQuantity
        a             rdf:Property ;
        rdfs:comment  "The reference quantity for which a certain price applies, e.g. 1 EUR per 4 kWh of electricity. This property is a replacement for unitOfMeasurement for the advanced cases where the price does not relate to a standard unit." ;
        rdfs:label    "referenceQuantity" .

schema:healthPlanCopayOption
        a             rdf:Property ;
        rdfs:comment  "Whether the copay is before or after deductible, etc. TODO: Is this a closed set?" ;
        rdfs:label    "healthPlanCopayOption" .

schema:VisualArtwork  a  rdfs:Class ;
        rdfs:comment     "A work of art that is primarily visual in character." ;
        rdfs:label       "VisualArtwork" ;
        rdfs:subClassOf  schema:CreativeWork .

schema:membershipNumber
        a             rdf:Property ;
        rdfs:comment  "A unique identifier for the membership." ;
        rdfs:label    "membershipNumber" .

schema:byMonthWeek  a  rdf:Property ;
        rdfs:comment  "Defines the week(s) of the month on which a recurring Event takes place. Specified as an Integer between 1-5. For clarity, byMonthWeek is best used in conjunction with byDay to indicate concepts like the first and third Mondays of a month." ;
        rdfs:label    "byMonthWeek" .

schema:monthsOfExperience
        a             rdf:Property ;
        rdfs:comment  "Indicates the minimal number of months of experience required for a position." ;
        rdfs:label    "monthsOfExperience" .

schema:DiscussionForumPosting
        a                rdfs:Class ;
        rdfs:comment     "A posting to a discussion forum." ;
        rdfs:label       "DiscussionForumPosting" ;
        rdfs:subClassOf  schema:SocialMediaPosting .

schema:ticketToken  a  rdf:Property ;
        rdfs:comment  "Reference to an asset (e.g., Barcode, QR code image or PDF) usable for entrance." ;
        rdfs:label    "ticketToken" .

schema:numberOfBathroomsTotal
        a             rdf:Property ;
        rdfs:comment  "The total integer number of bathrooms in a some [[Accommodation]], following real estate conventions as [documented in RESO](https://ddwiki.reso.org/display/DDW17/BathroomsTotalInteger+Field): \"The simple sum of the number of bathrooms. For example for a property with two Full Bathrooms and one Half Bathroom, the Bathrooms Total Integer will be 3.\". See also [[numberOfRooms]]." ;
        rdfs:label    "numberOfBathroomsTotal" .

schema:restPeriods  a  rdf:Property ;
        rdfs:comment  "How often one should break from the activity." ;
        rdfs:label    "restPeriods" .

schema:salaryCurrency
        a             rdf:Property ;
        rdfs:comment  "The currency (coded using [ISO 4217](http://en.wikipedia.org/wiki/ISO_4217) ) used for the main salary information in this job posting or for this employee." ;
        rdfs:label    "salaryCurrency" .

schema:numberOfItems  a  rdf:Property ;
        rdfs:comment  "The number of items in an ItemList. Note that some descriptions might not fully describe all items in a list (e.g., multi-page pagination); in such cases, the numberOfItems would be for the entire list." ;
        rdfs:label    "numberOfItems" .

schema:doseUnit  a    rdf:Property ;
        rdfs:comment  "The unit of the dose, e.g. 'mg'." ;
        rdfs:label    "doseUnit" .

schema:LifestyleModification
        a                rdfs:Class ;
        rdfs:comment     "A process of care involving exercise, changes to diet, fitness routines, and other lifestyle changes aimed at improving a health condition." ;
        rdfs:label       "LifestyleModification" ;
        rdfs:subClassOf  schema:MedicalEntity .

schema:memoryRequirements
        a             rdf:Property ;
        rdfs:comment  "Minimum memory requirements." ;
        rdfs:label    "memoryRequirements" .

schema:sku  a               rdf:Property ;
        rdfs:comment        "The Stock Keeping Unit (SKU), i.e. a merchant-specific identifier for a product or service, or the product to which the offer refers." ;
        rdfs:label          "sku" ;
        rdfs:subPropertyOf  schema:identifier .

schema:height  a      rdf:Property ;
        rdfs:comment  "The height of the item." ;
        rdfs:label    "height" .

schema:cvdNumBeds  a  rdf:Property ;
        rdfs:comment  "numbeds - HOSPITAL INPATIENT BEDS: Inpatient beds, including all staffed, licensed, and overflow (surge) beds used for inpatients." ;
        rdfs:label    "cvdNumBeds" .

schema:operatingSystem
        a             rdf:Property ;
        rdfs:comment  "Operating systems supported (Windows 7, OSX 10.6, Android 1.6)." ;
        rdfs:label    "operatingSystem" .

schema:geoCoveredBy  a  rdf:Property ;
        rdfs:comment  "Represents a relationship between two geometries (or the places they represent), relating a geometry to another that covers it. As defined in [DE-9IM](https://en.wikipedia.org/wiki/DE-9IM)." ;
        rdfs:label    "geoCoveredBy" .

schema:Park  a           rdfs:Class ;
        rdfs:comment     "A park." ;
        rdfs:label       "Park" ;
        rdfs:subClassOf  schema:CivicStructure .

schema:costPerUnit  a  rdf:Property ;
        rdfs:comment  "The cost per unit of the drug." ;
        rdfs:label    "costPerUnit" .

schema:educationalProgramMode
        a             rdf:Property ;
        rdfs:comment  "Similar to courseMode, The medium or means of delivery of the program as a whole. The value may either be a text label (e.g. \"online\", \"onsite\" or \"blended\"; \"synchronous\" or \"asynchronous\"; \"full-time\" or \"part-time\") or a URL reference to a term from a controlled vocabulary (e.g. https://ceds.ed.gov/element/001311#Asynchronous )." ;
        rdfs:label    "educationalProgramMode" .

schema:AutomotiveBusiness
        a                rdfs:Class ;
        rdfs:comment     "Car repair, sales, or parts." ;
        rdfs:label       "AutomotiveBusiness" ;
        rdfs:subClassOf  schema:LocalBusiness .

schema:BoatTerminal  a   rdfs:Class ;
        rdfs:comment     "A terminal for boats, ships, and other water vessels." ;
        rdfs:label       "BoatTerminal" ;
        rdfs:subClassOf  schema:CivicStructure .

schema:relatedTherapy
        a             rdf:Property ;
        rdfs:comment  "A medical therapy related to this anatomy." ;
        rdfs:label    "relatedTherapy" .

schema:speechToTextMarkup
        a             rdf:Property ;
        rdfs:comment  "Form of markup used. eg. [SSML](https://www.w3.org/TR/speech-synthesis11) or [IPA](https://www.wikidata.org/wiki/Property:P898)." ;
        rdfs:label    "speechToTextMarkup" .

schema:character  a   rdf:Property ;
        rdfs:comment  "Fictional person connected with a creative work." ;
        rdfs:label    "character" .

schema:subStructure  a  rdf:Property ;
        rdfs:comment  "Component (sub-)structure(s) that comprise this anatomical structure." ;
        rdfs:label    "subStructure" .

schema:actionableFeedbackPolicy
        a                   rdf:Property ;
        rdfs:comment        "For a [[NewsMediaOrganization]] or other news-related [[Organization]], a statement about public engagement activities (for news media, the newsroom’s), including involving the public - digitally or otherwise -- in coverage decisions, reporting and activities after publication." ;
        rdfs:label          "actionableFeedbackPolicy" ;
        rdfs:subPropertyOf  schema:publishingPrinciples .

schema:brand  a       rdf:Property ;
        rdfs:comment  "The brand(s) associated with a product or service, or the brand(s) maintained by an organization or business person." ;
        rdfs:label    "brand" .

schema:FinancialService
        a                rdfs:Class ;
        rdfs:comment     "Financial services business." ;
        rdfs:label       "FinancialService" ;
        rdfs:subClassOf  schema:LocalBusiness .

schema:enginePower  a  rdf:Property ;
        rdfs:comment  "The power of the vehicle's engine.\n    Typical unit code(s): KWT for kilowatt, BHP for brake horsepower, N12 for metric horsepower (PS, with 1 PS = 735,49875 W)\\n\\n* Note 1: There are many different ways of measuring an engine's power. For an overview, see  [http://en.wikipedia.org/wiki/Horsepower#Engine_power_test_codes](http://en.wikipedia.org/wiki/Horsepower#Engine_power_test_codes).\\n* Note 2: You can link to information about how the given value has been determined using the [[valueReference]] property.\\n* Note 3: You can use [[minValue]] and [[maxValue]] to indicate ranges." ;
        rdfs:label    "enginePower" .

schema:SizeSystemEnumeration
        a                rdfs:Class ;
        rdfs:comment     "Enumerates common size systems for different categories of products, for example \"EN-13402\" or \"UK\" for wearables or \"Imperial\" for screws." ;
        rdfs:label       "SizeSystemEnumeration" ;
        rdfs:subClassOf  schema:Enumeration .

schema:NGO  a            rdfs:Class ;
        rdfs:comment     "Organization: Non-governmental Organization." ;
        rdfs:label       "NGO" ;
        rdfs:subClassOf  schema:Organization .

schema:GeoShape  a       rdfs:Class ;
        rdfs:comment     "The geographic shape of a place. A GeoShape can be described using several properties whose values are based on latitude/longitude pairs. Either whitespace or commas can be used to separate latitude and longitude; whitespace should be used when writing a list of several such points." ;
        rdfs:label       "GeoShape" ;
        rdfs:subClassOf  schema:StructuredValue .

schema:Mosque  a         rdfs:Class ;
        rdfs:comment     "A mosque." ;
        rdfs:label       "Mosque" ;
        rdfs:subClassOf  schema:PlaceOfWorship .

schema:originAddress  a  rdf:Property ;
        rdfs:comment  "Shipper's address." ;
        rdfs:label    "originAddress" .

schema:nerve  a       rdf:Property ;
        rdfs:comment  "The underlying innervation associated with the muscle." ;
        rdfs:label    "nerve" .

schema:MusicAlbumProductionType
        a                rdfs:Class ;
        rdfs:comment     "Classification of the album by it's type of content: soundtrack, live album, studio album, etc." ;
        rdfs:label       "MusicAlbumProductionType" ;
        rdfs:subClassOf  schema:Enumeration .

schema:maintainer  a  rdf:Property ;
        rdfs:comment  "A maintainer of a [[Dataset]], software package ([[SoftwareApplication]]), or other [[Project]]. A maintainer is a [[Person]] or [[Organization]] that manages contributions to, and/or publication of, some (typically complex) artifact. It is common for distributions of software and data to be based on \"upstream\" sources. When [[maintainer]] is applied to a specific version of something e.g. a particular version or packaging of a [[Dataset]], it is always  possible that the upstream source has a different maintainer. The [[isBasedOn]] property can be used to indicate such relationships between datasets to make the different maintenance roles clear. Similarly in the case of software, a package may have dedicated maintainers working on integration into software distributions such as Ubuntu, as well as upstream maintainers of the underlying work.\n      " ;
        rdfs:label    "maintainer" .

schema:programName  a  rdf:Property ;
        rdfs:comment  "The program providing the membership." ;
        rdfs:label    "programName" .

schema:result  a      rdf:Property ;
        rdfs:comment  "The result produced in the action. e.g. John wrote *a book*." ;
        rdfs:label    "result" .

schema:MotorizedBicycle
        a                rdfs:Class ;
        rdfs:comment     "A motorized bicycle is a bicycle with an attached motor used to power the vehicle, or to assist with pedaling." ;
        rdfs:label       "MotorizedBicycle" ;
        rdfs:subClassOf  schema:Vehicle .

schema:validUntil  a  rdf:Property ;
        rdfs:comment  "The date when the item is no longer valid." ;
        rdfs:label    "validUntil" .

schema:partOfInvoice  a  rdf:Property ;
        rdfs:comment  "The order is being paid as part of the referenced Invoice." ;
        rdfs:label    "partOfInvoice" .

schema:HealthTopicContent
        a                rdfs:Class ;
        rdfs:comment     "[[HealthTopicContent]] is [[WebContent]] that is about some aspect of a health topic, e.g. a condition, its symptoms or treatments. Such content may be comprised of several parts or sections and use different types of media. Multiple instances of [[WebContent]] (and hence [[HealthTopicContent]]) can be related using [[hasPart]] / [[isPartOf]] where there is some kind of content hierarchy, and their content described with [[about]] and [[mentions]] e.g. building upon the existing [[MedicalCondition]] vocabulary.\n  " ;
        rdfs:label       "HealthTopicContent" ;
        rdfs:subClassOf  schema:WebContent .

schema:Hotel  a          rdfs:Class ;
        rdfs:comment     "A hotel is an establishment that provides lodging paid on a short-term basis (Source: Wikipedia, the free encyclopedia, see http://en.wikipedia.org/wiki/Hotel).\n<br /><br />\nSee also the <a href=\"/docs/hotels.html\">dedicated document on the use of schema.org for marking up hotels and other forms of accommodations</a>.\n" ;
        rdfs:label       "Hotel" ;
        rdfs:subClassOf  schema:LodgingBusiness .

schema:AskPublicNewsArticle
        a                rdfs:Class ;
        rdfs:comment     "A [[NewsArticle]] expressing an open call by a [[NewsMediaOrganization]] asking the public for input, insights, clarifications, anecdotes, documentation, etc., on an issue, for reporting purposes." ;
        rdfs:label       "AskPublicNewsArticle" ;
        rdfs:subClassOf  schema:NewsArticle .

schema:status  a      rdf:Property ;
        rdfs:comment  "The status of the study (enumerated)." ;
        rdfs:label    "status" .

schema:translator  a  rdf:Property ;
        rdfs:comment  "Organization or person who adapts a creative work to different languages, regional differences and technical requirements of a target market, or that translates during some event." ;
        rdfs:label    "translator" .

schema:modifiedTime  a  rdf:Property ;
        rdfs:comment  "The date and time the reservation was modified." ;
        rdfs:label    "modifiedTime" .

schema:mpn  a         rdf:Property ;
        rdfs:comment  "The Manufacturer Part Number (MPN) of the product, or the product to which the offer refers." ;
        rdfs:label    "mpn" .

schema:GroceryStore  a   rdfs:Class ;
        rdfs:comment     "A grocery store." ;
        rdfs:label       "GroceryStore" ;
        rdfs:subClassOf  schema:Store .

schema:subTest  a     rdf:Property ;
        rdfs:comment  "A component test of the panel." ;
        rdfs:label    "subTest" .

schema:publisherImprint
        a             rdf:Property ;
        rdfs:comment  "The publishing division which published the comic." ;
        rdfs:label    "publisherImprint" .

schema:geoRadius  a   rdf:Property ;
        rdfs:comment  "Indicates the approximate radius of a GeoCircle (metres unless indicated otherwise via Distance notation)." ;
        rdfs:label    "geoRadius" .

schema:startTime  a   rdf:Property ;
        rdfs:comment  "The startTime of something. For a reserved event or service (e.g. FoodEstablishmentReservation), the time that it is expected to start. For actions that span a period of time, when the action was performed. e.g. John wrote a book from *January* to December. For media, including audio and video, it's the time offset of the start of a clip within a larger file.\\n\\nNote that Event uses startDate/endDate instead of startTime/endTime, even when describing dates with times. This situation may be clarified in future revisions." ;
        rdfs:label    "startTime" .

schema:exampleOfWork  a  rdf:Property ;
        rdfs:comment  "A creative work that this work is an example/instance/realization/derivation of." ;
        rdfs:label    "exampleOfWork" .

schema:Gynecologic  a    rdfs:Class ;
        rdfs:comment     "A specific branch of medical science that pertains to the health care of women, particularly in the diagnosis and treatment of disorders affecting the female reproductive system." ;
        rdfs:label       "Gynecologic" ;
        rdfs:subClassOf  schema:MedicalBusiness .

schema:childMaxAge  a  rdf:Property ;
        rdfs:comment  "Maximal age of the child." ;
        rdfs:label    "childMaxAge" .

schema:DrugPregnancyCategory
        a                rdfs:Class ;
        rdfs:comment     "Categories that represent an assessment of the risk of fetal injury due to a drug or pharmaceutical used as directed by the mother during pregnancy." ;
        rdfs:label       "DrugPregnancyCategory" ;
        rdfs:subClassOf  schema:MedicalEnumeration .

schema:MedicalSignOrSymptom
        a                rdfs:Class ;
        rdfs:comment     "Any feature associated or not with a medical condition. In medicine a symptom is generally subjective while a sign is objective." ;
        rdfs:label       "MedicalSignOrSymptom" ;
        rdfs:subClassOf  schema:MedicalCondition .

schema:polygon  a     rdf:Property ;
        rdfs:comment  "A polygon is the area enclosed by a point-to-point path for which the starting and ending points are the same. A polygon is expressed as a series of four or more space delimited points where the first and final points are identical." ;
        rdfs:label    "polygon" .

schema:installUrl  a  rdf:Property ;
        rdfs:comment  "URL at which the app may be installed, if different from the URL of the item." ;
        rdfs:label    "installUrl" .

schema:legislationJurisdiction
        a                   rdf:Property ;
        rdfs:comment        "The jurisdiction from which the legislation originates." ;
        rdfs:label          "legislationJurisdiction" ;
        rdfs:subPropertyOf  schema:spatialCoverage , schema:jurisdiction .

schema:distinguishingSign
        a             rdf:Property ;
        rdfs:comment  "One of a set of signs and symptoms that can be used to distinguish this diagnosis from others in the differential diagnosis." ;
        rdfs:label    "distinguishingSign" .

schema:diet  a              rdf:Property ;
        rdfs:comment        "A sub property of instrument. The diet used in this action." ;
        rdfs:label          "diet" ;
        rdfs:subPropertyOf  schema:instrument .

schema:orderItemNumber
        a             rdf:Property ;
        rdfs:comment  "The identifier of the order item." ;
        rdfs:label    "orderItemNumber" .

schema:EntryPoint  a     rdfs:Class ;
        rdfs:comment     "An entry point, within some Web-based protocol." ;
        rdfs:label       "EntryPoint" ;
        rdfs:subClassOf  schema:Intangible .

schema:AssignAction  a   rdfs:Class ;
        rdfs:comment     "The act of allocating an action/event/task to some destination (someone or something)." ;
        rdfs:label       "AssignAction" ;
        rdfs:subClassOf  schema:AllocateAction .

schema:Drug  a           rdfs:Class ;
        rdfs:comment     "A chemical or biologic substance, used as a medical therapy, that has a physiological effect on an organism. Here the term drug is used interchangeably with the term medicine although clinical knowledge make a clear difference between them." ;
        rdfs:label       "Drug" ;
        rdfs:subClassOf  schema:Substance .

schema:LoanOrCredit  a   rdfs:Class ;
        rdfs:comment     "A financial product for the loaning of an amount of money, or line of credit, under agreed terms and charges." ;
        rdfs:label       "LoanOrCredit" ;
        rdfs:subClassOf  schema:FinancialProduct .

schema:dateModified  a  rdf:Property ;
        rdfs:comment  "The date on which the CreativeWork was most recently modified or when the item's entry was modified within a DataFeed." ;
        rdfs:label    "dateModified" .

schema:workLocation  a      rdf:Property ;
        rdfs:comment        "A contact location for a person's place of work." ;
        rdfs:label          "workLocation" ;
        rdfs:subPropertyOf  schema:location .

schema:Vessel  a         rdfs:Class ;
        rdfs:comment     "A component of the human body circulatory system comprised of an intricate network of hollow tubes that transport blood throughout the entire body." ;
        rdfs:label       "Vessel" ;
        rdfs:subClassOf  schema:AnatomicalStructure .

schema:ComedyClub  a     rdfs:Class ;
        rdfs:comment     "A comedy club." ;
        rdfs:label       "ComedyClub" ;
        rdfs:subClassOf  schema:EntertainmentBusiness .

schema:colorist  a    rdf:Property ;
        rdfs:comment  "The individual who adds color to inked drawings." ;
        rdfs:label    "colorist" .

schema:availableThrough
        a             rdf:Property ;
        rdfs:comment  "After this date, the item will no longer be available for pickup." ;
        rdfs:label    "availableThrough" .

schema:responsibilities
        a             rdf:Property ;
        rdfs:comment  "Responsibilities associated with this role or Occupation." ;
        rdfs:label    "responsibilities" .

schema:LiteraryEvent  a  rdfs:Class ;
        rdfs:comment     "Event type: Literary event." ;
        rdfs:label       "LiteraryEvent" ;
        rdfs:subClassOf  schema:Event .

schema:season  a            rdf:Property ;
        rdfs:comment        "A season in a media series." ;
        rdfs:label          "season" ;
        rdfs:subPropertyOf  schema:hasPart .

schema:ShoeStore  a      rdfs:Class ;
        rdfs:comment     "A shoe store." ;
        rdfs:label       "ShoeStore" ;
        rdfs:subClassOf  schema:Store .

schema:HowToSection  a   rdfs:Class ;
        rdfs:comment     "A sub-grouping of steps in the instructions for how to achieve a result (e.g. steps for making a pie crust within a pie recipe)." ;
        rdfs:label       "HowToSection" ;
        rdfs:subClassOf  schema:ListItem , schema:ItemList , schema:CreativeWork .

schema:LocalBusiness  a  rdfs:Class ;
        rdfs:comment     "A particular physical business or branch of an organization. Examples of LocalBusiness include a restaurant, a particular branch of a restaurant chain, a branch of a bank, a medical practice, a club, a bowling alley, etc." ;
        rdfs:label       "LocalBusiness" ;
        rdfs:subClassOf  schema:Place , schema:Organization .

schema:UserReview  a     rdfs:Class ;
        rdfs:comment     "A review created by an end-user (e.g. consumer, purchaser, attendee etc.), in contrast with [[CriticReview]]." ;
        rdfs:label       "UserReview" ;
        rdfs:subClassOf  schema:Review .

schema:isAccessoryOrSparePartFor
        a             rdf:Property ;
        rdfs:comment  "A pointer to another product (or multiple products) for which this product is an accessory or spare part." ;
        rdfs:label    "isAccessoryOrSparePartFor" .

schema:foundingLocation
        a             rdf:Property ;
        rdfs:comment  "The place where the Organization was founded." ;
        rdfs:label    "foundingLocation" .

schema:deliveryTime  a  rdf:Property ;
        rdfs:comment  "The total delay between the receipt of the order and the goods reaching the final customer." ;
        rdfs:label    "deliveryTime" .

schema:employee  a    rdf:Property ;
        rdfs:comment  "Someone working for this organization." ;
        rdfs:label    "employee" .

schema:cssSelector  a  rdf:Property ;
        rdfs:comment  "A CSS selector, e.g. of a [[SpeakableSpecification]] or [[WebPageElement]]. In the latter case, multiple matches within a page can constitute a single conceptual \"Web page element\"." ;
        rdfs:label    "cssSelector" .

schema:legislationChanges
        a             rdf:Property ;
        rdfs:comment  "Another legislation that this legislation changes. This encompasses the notions of amendment, replacement, correction, repeal, or other types of change. This may be a direct change (textual or non-textual amendment) or a consequential or indirect change. The property is to be used to express the existence of a change relationship between two acts rather than the existence of a consolidated version of the text that shows the result of the change. For consolidation relationships, use the <a href=\"/legislationConsolidates\">legislationConsolidates</a> property." ;
        rdfs:label    "legislationChanges" .

schema:followup  a    rdf:Property ;
        rdfs:comment  "Typical or recommended followup care after the procedure is performed." ;
        rdfs:label    "followup" .

schema:reservedTicket
        a             rdf:Property ;
        rdfs:comment  "A ticket associated with the reservation." ;
        rdfs:label    "reservedTicket" .

schema:procedure  a   rdf:Property ;
        rdfs:comment  "A description of the procedure involved in setting up, using, and/or installing the device." ;
        rdfs:label    "procedure" .

schema:borrower  a          rdf:Property ;
        rdfs:comment        "A sub property of participant. The person that borrows the object being lent." ;
        rdfs:label          "borrower" ;
        rdfs:subPropertyOf  schema:participant .

schema:workload  a    rdf:Property ;
        rdfs:comment  "Quantitative measure of the physiologic output of the exercise; also referred to as energy expenditure." ;
        rdfs:label    "workload" .

schema:Muscle  a         rdfs:Class ;
        rdfs:comment     "A muscle is an anatomical structure consisting of a contractile form of tissue that animals use to effect movement." ;
        rdfs:label       "Muscle" ;
        rdfs:subClassOf  schema:AnatomicalStructure .

schema:containedIn  a  owl:ObjectProperty ;
        rdfs:comment  "The basic containment relation between a place and one that contains it." ;
        rdfs:label    "containedIn" .

schema:bodyLocation  a  rdf:Property ;
        rdfs:comment  "Location in the body of the anatomical structure." ;
        rdfs:label    "bodyLocation" .

schema:callSign  a          rdf:Property ;
        rdfs:comment        "A [callsign](https://en.wikipedia.org/wiki/Call_sign), as used in broadcasting and radio communications to identify people, radio and TV stations, or vehicles." ;
        rdfs:label          "callSign" ;
        rdfs:subPropertyOf  schema:identifier .

schema:DeliveryEvent  a  rdfs:Class ;
        rdfs:comment     "An event involving the delivery of an item." ;
        rdfs:label       "DeliveryEvent" ;
        rdfs:subClassOf  schema:Event .

schema:HowToItem  a      rdfs:Class ;
        rdfs:comment     "An item used as either a tool or supply when performing the instructions for how to to achieve a result." ;
        rdfs:label       "HowToItem" ;
        rdfs:subClassOf  schema:ListItem .

schema:SomeProducts  a   rdfs:Class ;
        rdfs:comment     "A placeholder for multiple similar products of the same kind." ;
        rdfs:label       "SomeProducts" ;
        rdfs:subClassOf  schema:Product .

schema:processingTime
        a             rdf:Property ;
        rdfs:comment  "Estimated processing time for the service using this channel." ;
        rdfs:label    "processingTime" .

schema:trainName  a   rdf:Property ;
        rdfs:comment  "The name of the train (e.g. The Orient Express)." ;
        rdfs:label    "trainName" .

schema:pagination  a  rdf:Property ;
        rdfs:comment  "Any description of pages that is not separated into pageStart and pageEnd; for example, \"1-6, 9, 55\" or \"10-12, 46-49\"." ;
        rdfs:label    "pagination" .

schema:ownedFrom  a   rdf:Property ;
        rdfs:comment  "The date and time of obtaining the product." ;
        rdfs:label    "ownedFrom" .

schema:AutoWash  a       rdfs:Class ;
        rdfs:comment     "A car wash business." ;
        rdfs:label       "AutoWash" ;
        rdfs:subClassOf  schema:AutomotiveBusiness .

schema:MedicalTrial  a   rdfs:Class ;
        rdfs:comment     "A medical trial is a type of medical study that uses scientific process used to compare the safety and efficacy of medical therapies or medical procedures. In general, medical trials are controlled and subjects are allocated at random to the different treatment and/or control groups." ;
        rdfs:label       "MedicalTrial" ;
        rdfs:subClassOf  schema:MedicalStudy .

schema:text  a        rdf:Property ;
        rdfs:comment  "The textual content of this CreativeWork." ;
        rdfs:label    "text" .

schema:opens  a       rdf:Property ;
        rdfs:comment  "The opening hour of the place or service on the given day(s) of the week." ;
        rdfs:label    "opens" .

schema:foodWarning  a  rdf:Property ;
        rdfs:comment  "Any precaution, guidance, contraindication, etc. related to consumption of specific foods while taking this drug." ;
        rdfs:label    "foodWarning" .

schema:Observation  a    rdfs:Class ;
        rdfs:comment     "Instances of the class [[Observation]] are used to specify observations about an entity (which may or may not be an instance of a [[StatisticalPopulation]]), at a particular time. The principal properties of an [[Observation]] are [[observedNode]], [[measuredProperty]], [[measuredValue]] (or [[median]], etc.) and [[observationDate]] ([[measuredProperty]] properties can, but need not always, be W3C RDF Data Cube \"measure properties\", as in the [lifeExpectancy example](https://www.w3.org/TR/vocab-data-cube/#dsd-example)).\nSee also [[StatisticalPopulation]], and the [data and datasets](/docs/data-and-datasets.html) overview for more details.\n  " ;
        rdfs:label       "Observation" ;
        rdfs:subClassOf  schema:Intangible .

schema:BoatReservation
        a                rdfs:Class ;
        rdfs:comment     "A reservation for boat travel.\n\nNote: This type is for information about actual reservations, e.g. in confirmation emails or HTML pages with individual confirmations of reservations. For offers of tickets, use [[Offer]]." ;
        rdfs:label       "BoatReservation" ;
        rdfs:subClassOf  schema:Reservation .

schema:MonetaryAmount
        a                rdfs:Class ;
        rdfs:comment     "A monetary value or range. This type can be used to describe an amount of money such as $50 USD, or a range as in describing a bank account being suitable for a balance between £1,000 and £1,000,000 GBP, or the value of a salary, etc. It is recommended to use [[PriceSpecification]] Types to describe the price of an Offer, Invoice, etc." ;
        rdfs:label       "MonetaryAmount" ;
        rdfs:subClassOf  schema:StructuredValue .

schema:TaxiService  a    rdfs:Class ;
        rdfs:comment     "A service for a vehicle for hire with a driver for local travel. Fares are usually calculated based on distance traveled." ;
        rdfs:label       "TaxiService" ;
        rdfs:subClassOf  schema:Service .

schema:numberOfForwardGears
        a             rdf:Property ;
        rdfs:comment  "The total number of forward gears available for the transmission system of the vehicle.\\n\\nTypical unit code(s): C62" ;
        rdfs:label    "numberOfForwardGears" .

schema:valueMaxLength
        a             rdf:Property ;
        rdfs:comment  "Specifies the allowed range for number of characters in a literal value." ;
        rdfs:label    "valueMaxLength" .

schema:awards  a      rdf:Property ;
        rdfs:comment  "Awards won by or for this item." ;
        rdfs:label    "awards" .

schema:containedInPlace
        a             rdf:Property , owl:ObjectProperty ;
        rdfs:comment  "The basic containment relation between a place and one that contains it." ;
        rdfs:label    "containedInPlace" .

schema:ratingCount  a  rdf:Property ;
        rdfs:comment  "The count of total number of ratings." ;
        rdfs:label    "ratingCount" .

schema:owns  a        rdf:Property ;
        rdfs:comment  "Products owned by the organization or person." ;
        rdfs:label    "owns" .

schema:suggestedAge  a  rdf:Property ;
        rdfs:comment  "The age or age range for the intended audience or person, for example 3-12 months for infants, 1-5 years for toddlers." ;
        rdfs:label    "suggestedAge" .

schema:phoneticText  a  rdf:Property ;
        rdfs:comment  "Representation of a text [[textValue]] using the specified [[speechToTextMarkup]]. For example the city name of Houston in IPA: /ˈhjuːstən/." ;
        rdfs:label    "phoneticText" .

schema:clipNumber  a        rdf:Property ;
        rdfs:comment        "Position of the clip within an ordered group of clips." ;
        rdfs:label          "clipNumber" ;
        rdfs:subPropertyOf  schema:position .

schema:HealthInsurancePlan
        a                rdfs:Class ;
        rdfs:comment     "A US-style health insurance plan, including PPOs, EPOs, and HMOs. " ;
        rdfs:label       "HealthInsurancePlan" ;
        rdfs:subClassOf  schema:Intangible .

schema:browserRequirements
        a             rdf:Property ;
        rdfs:comment  "Specifies browser requirements in human-readable text. For example, 'requires HTML5 support'." ;
        rdfs:label    "browserRequirements" .

schema:foundingDate  a  rdf:Property ;
        rdfs:comment  "The date that this organization was founded." ;
        rdfs:label    "foundingDate" .

schema:AutoRental  a     rdfs:Class ;
        rdfs:comment     "A car rental business." ;
        rdfs:label       "AutoRental" ;
        rdfs:subClassOf  schema:AutomotiveBusiness .

schema:educationalUse
        a             rdf:Property ;
        rdfs:comment  "The purpose of a work in the context of education; for example, 'assignment', 'group work'." ;
        rdfs:label    "educationalUse" .

schema:MedicalTrialDesign
        a                rdfs:Class ;
        rdfs:comment     "Design models for medical trials. Enumerated type." ;
        rdfs:label       "MedicalTrialDesign" ;
        rdfs:subClassOf  schema:MedicalEnumeration .

schema:audience  a    rdf:Property ;
        rdfs:comment  "An intended audience, i.e. a group for whom something was created." ;
        rdfs:label    "audience" .

schema:Answer  a         rdfs:Class ;
        rdfs:comment     "An answer offered to a question; perhaps correct, perhaps opinionated or wrong." ;
        rdfs:label       "Answer" ;
        rdfs:subClassOf  schema:Comment .

schema:afterMedia  a  rdf:Property ;
        rdfs:comment  "A media object representing the circumstances after performing this direction." ;
        rdfs:label    "afterMedia" .

schema:cashBack  a    rdf:Property ;
        rdfs:comment  "A cardholder benefit that pays the cardholder a small percentage of their net expenditures." ;
        rdfs:label    "cashBack" .

schema:parent  a      rdf:Property ;
        rdfs:comment  "A parent of this person." ;
        rdfs:label    "parent" .

schema:InfectiousAgentClass
        a                rdfs:Class ;
        rdfs:comment     "Classes of agents or pathogens that transmit infectious diseases. Enumerated type." ;
        rdfs:label       "InfectiousAgentClass" ;
        rdfs:subClassOf  schema:MedicalEnumeration .

schema:image  a       rdf:Property ;
        rdfs:comment  "An image of the item. This can be a [[URL]] or a fully described [[ImageObject]]." ;
        rdfs:label    "image" .

schema:infectiousAgent
        a             rdf:Property ;
        rdfs:comment  "The actual infectious agent, such as a specific bacterium." ;
        rdfs:label    "infectiousAgent" .

schema:RepaymentSpecification
        a                rdfs:Class ;
        rdfs:comment     "A structured value representing repayment." ;
        rdfs:label       "RepaymentSpecification" ;
        rdfs:subClassOf  schema:StructuredValue .

schema:CreateAction  a   rdfs:Class ;
        rdfs:comment     "The act of deliberately creating/producing/generating/building a result out of the agent." ;
        rdfs:label       "CreateAction" ;
        rdfs:subClassOf  schema:Action .

schema:greater  a     rdf:Property ;
        rdfs:comment  "This ordering relation for qualitative values indicates that the subject is greater than the object." ;
        rdfs:label    "greater" .

schema:measurementTechnique
        a             rdf:Property ;
        rdfs:comment  "A technique or technology used in a [[Dataset]] (or [[DataDownload]], [[DataCatalog]]),\ncorresponding to the method used for measuring the corresponding variable(s) (described using [[variableMeasured]]). This is oriented towards scientific and scholarly dataset publication but may have broader applicability; it is not intended as a full representation of measurement, but rather as a high level summary for dataset discovery.\n\nFor example, if [[variableMeasured]] is: molecule concentration, [[measurementTechnique]] could be: \"mass spectrometry\" or \"nmr spectroscopy\" or \"colorimetry\" or \"immunofluorescence\".\n\nIf the [[variableMeasured]] is \"depression rating\", the [[measurementTechnique]] could be \"Zung Scale\" or \"HAM-D\" or \"Beck Depression Inventory\".\n\nIf there are several [[variableMeasured]] properties recorded for some given data object, use a [[PropertyValue]] for each [[variableMeasured]] and attach the corresponding [[measurementTechnique]].\n      " ;
        rdfs:label    "measurementTechnique" .

schema:dayOfWeek  a   rdf:Property ;
        rdfs:comment  "The day of the week for which these opening hours are valid." ;
        rdfs:label    "dayOfWeek" .

schema:targetPopulation
        a             rdf:Property ;
        rdfs:comment  "Characteristics of the population for which this is intended, or which typically uses it, e.g. 'adults'." ;
        rdfs:label    "targetPopulation" .

schema:director  a    rdf:Property ;
        rdfs:comment  "A director of e.g. tv, radio, movie, video gaming etc. content, or of an event. Directors can be associated with individual items or with a series, episode, clip." ;
        rdfs:label    "director" .

schema:paymentDue  a  rdf:Property ;
        rdfs:comment  "The date that payment is due." ;
        rdfs:label    "paymentDue" .

schema:broadcastFrequencyValue
        a             rdf:Property ;
        rdfs:comment  "The frequency in MHz for a particular broadcast." ;
        rdfs:label    "broadcastFrequencyValue" .

schema:identifier  a  rdf:Property ;
        rdfs:comment  "The identifier property represents any kind of identifier for any kind of [[Thing]], such as ISBNs, GTIN codes, UUIDs etc. Schema.org provides dedicated properties for representing many of these, either as textual strings or as URL (URI) links. See [background notes](/docs/datamodel.html#identifierBg) for more details.\n        " ;
        rdfs:label    "identifier" .

schema:repetitions  a  rdf:Property ;
        rdfs:comment  "Number of times one should repeat the activity." ;
        rdfs:label    "repetitions" .

schema:MediaSubscription
        a                rdfs:Class ;
        rdfs:comment     "A subscription which allows a user to access media including audio, video, books, etc." ;
        rdfs:label       "MediaSubscription" ;
        rdfs:subClassOf  schema:Intangible .

schema:doseSchedule  a  rdf:Property ;
        rdfs:comment  "A dosing schedule for the drug for a given population, either observed, recommended, or maximum dose based on the type used." ;
        rdfs:label    "doseSchedule" .

schema:candidate  a         rdf:Property ;
        rdfs:comment        "A sub property of object. The candidate subject of this action." ;
        rdfs:label          "candidate" ;
        rdfs:subPropertyOf  schema:object .

schema:OceanBodyOfWater
        a                rdfs:Class ;
        rdfs:comment     "An ocean (for example, the Pacific)." ;
        rdfs:label       "OceanBodyOfWater" ;
        rdfs:subClassOf  schema:BodyOfWater .

schema:ReplaceAction  a  rdfs:Class ;
        rdfs:comment     "The act of editing a recipient by replacing an old object with a new object." ;
        rdfs:label       "ReplaceAction" ;
        rdfs:subClassOf  schema:UpdateAction .

schema:governmentBenefitsInfo
        a             rdf:Property ;
        rdfs:comment  "governmentBenefitsInfo provides information about government benefits associated with a SpecialAnnouncement." ;
        rdfs:label    "governmentBenefitsInfo" .

schema:runsTo  a      rdf:Property ;
        rdfs:comment  "The vasculature the lymphatic structure runs, or efferents, to." ;
        rdfs:label    "runsTo" .

schema:educationalCredentialAwarded
        a             rdf:Property ;
        rdfs:comment  "A description of the qualification, award, certificate, diploma or other educational credential awarded as a consequence of successful completion of this course or program." ;
        rdfs:label    "educationalCredentialAwarded" .

schema:Series  a         rdfs:Class ;
        rdfs:comment     "A Series in schema.org is a group of related items, typically but not necessarily of the same kind. See also [[CreativeWorkSeries]], [[EventSeries]]." ;
        rdfs:label       "Series" ;
        rdfs:subClassOf  schema:Intangible .

schema:previousStartDate
        a             rdf:Property ;
        rdfs:comment  "Used in conjunction with eventStatus for rescheduled or cancelled events. This property contains the previously scheduled start date. For rescheduled events, the startDate property should be used for the newly scheduled start date. In the (rare) case of an event that has been postponed and rescheduled multiple times, this field may be repeated." ;
        rdfs:label    "previousStartDate" .

schema:AllocateAction
        a                rdfs:Class ;
        rdfs:comment     "The act of organizing tasks/objects/events by associating resources to it." ;
        rdfs:label       "AllocateAction" ;
        rdfs:subClassOf  schema:OrganizeAction .

schema:musicArrangement
        a             rdf:Property ;
        rdfs:comment  "An arrangement derived from the composition." ;
        rdfs:label    "musicArrangement" .

schema:BusinessAudience
        a                rdfs:Class ;
        rdfs:comment     "A set of characteristics belonging to businesses, e.g. who compose an item's target audience." ;
        rdfs:label       "BusinessAudience" ;
        rdfs:subClassOf  schema:Audience .

schema:sensoryUnit  a  rdf:Property ;
        rdfs:comment  "The neurological pathway extension that inputs and sends information to the brain or spinal cord." ;
        rdfs:label    "sensoryUnit" .

schema:GovernmentService
        a                rdfs:Class ;
        rdfs:comment     "A service provided by a government organization, e.g. food stamps, veterans benefits, etc." ;
        rdfs:label       "GovernmentService" ;
        rdfs:subClassOf  schema:Service .

schema:RiverBodyOfWater
        a                rdfs:Class ;
        rdfs:comment     "A river (for example, the broad majestic Shannon)." ;
        rdfs:label       "RiverBodyOfWater" ;
        rdfs:subClassOf  schema:BodyOfWater .

schema:referencesOrder
        a             rdf:Property ;
        rdfs:comment  "The Order(s) related to this Invoice. One or more Orders may be combined into a single Invoice." ;
        rdfs:label    "referencesOrder" .

schema:loanType  a    rdf:Property ;
        rdfs:comment  "The type of a loan or credit." ;
        rdfs:label    "loanType" .

schema:MedicalTherapy
        a                rdfs:Class ;
        rdfs:comment     "Any medical intervention designed to prevent, treat, and cure human diseases and medical conditions, including both curative and palliative therapies. Medical therapies are typically processes of care relying upon pharmacotherapy, behavioral therapy, supportive therapy (with fluid or nutrition for example), or detoxification (e.g. hemodialysis) aimed at improving or preventing a health condition." ;
        rdfs:label       "MedicalTherapy" ;
        rdfs:subClassOf  schema:TherapeuticProcedure .

schema:BookmarkAction
        a                rdfs:Class ;
        rdfs:comment     "An agent bookmarks/flags/labels/tags/marks an object." ;
        rdfs:label       "BookmarkAction" ;
        rdfs:subClassOf  schema:OrganizeAction .

schema:modelDate  a   rdf:Property ;
        rdfs:comment  "The release date of a vehicle model (often used to differentiate versions of the same make and model)." ;
        rdfs:label    "modelDate" .

schema:programType  a  rdf:Property ;
        rdfs:comment  "The type of educational or occupational program. For example, classroom, internship, alternance, etc.." ;
        rdfs:label    "programType" .

schema:SaleEvent  a      rdfs:Class ;
        rdfs:comment     "Event type: Sales event." ;
        rdfs:label       "SaleEvent" ;
        rdfs:subClassOf  schema:Event .

schema:travelBans  a  rdf:Property ;
        rdfs:comment  "Information about travel bans, e.g. in the context of a pandemic." ;
        rdfs:label    "travelBans" .

schema:coursePrerequisites
        a             rdf:Property ;
        rdfs:comment  "Requirements for taking the Course. May be completion of another [[Course]] or a textual description like \"permission of instructor\". Requirements may be a pre-requisite competency, referenced using [[AlignmentObject]]." ;
        rdfs:label    "coursePrerequisites" .

schema:EmergencyService
        a                rdfs:Class ;
        rdfs:comment     "An emergency service, such as a fire station or ER." ;
        rdfs:label       "EmergencyService" ;
        rdfs:subClassOf  schema:LocalBusiness .

schema:quest  a       rdf:Property ;
        rdfs:comment  "The task that a player-controlled character, or group of characters may complete in order to gain a reward." ;
        rdfs:label    "quest" .

schema:Occupation  a     rdfs:Class ;
        rdfs:comment     "A profession, may involve prolonged training and/or a formal qualification." ;
        rdfs:label       "Occupation" ;
        rdfs:subClassOf  schema:Intangible .

schema:CafeOrCoffeeShop
        a                rdfs:Class ;
        rdfs:comment     "A cafe or coffee shop." ;
        rdfs:label       "CafeOrCoffeeShop" ;
        rdfs:subClassOf  schema:FoodEstablishment .

schema:runtimePlatform
        a             rdf:Property ;
        rdfs:comment  "Runtime platform or script interpreter dependencies (Example - Java v1, Python2.3, .Net Framework 3.0)." ;
        rdfs:label    "runtimePlatform" .

schema:accommodationFloorPlan
        a             rdf:Property ;
        rdfs:comment  "A floorplan of some [[Accommodation]]." ;
        rdfs:label    "accommodationFloorPlan" .

schema:copyrightNotice
        a             rdf:Property ;
        rdfs:comment  "Text of a notice appropriate for describing the copyright aspects of this Creative Work, ideally indicating the owner of the copyright for the Work." ;
        rdfs:label    "copyrightNotice" .

schema:LendAction  a     rdfs:Class ;
        rdfs:comment     "The act of providing an object under an agreement that it will be returned at a later date. Reciprocal of BorrowAction.\\n\\nRelated actions:\\n\\n* [[BorrowAction]]: Reciprocal of LendAction." ;
        rdfs:label       "LendAction" ;
        rdfs:subClassOf  schema:TransferAction .

schema:TaxiStand  a      rdfs:Class ;
        rdfs:comment     "A taxi stand." ;
        rdfs:label       "TaxiStand" ;
        rdfs:subClassOf  schema:CivicStructure .

schema:QuantitativeValue
        a                rdfs:Class ;
        rdfs:comment     " A point value or interval for product characteristics and other purposes." ;
        rdfs:label       "QuantitativeValue" ;
        rdfs:subClassOf  schema:StructuredValue .

schema:AutomatedTeller
        a                rdfs:Class ;
        rdfs:comment     "ATM/cash machine." ;
        rdfs:label       "AutomatedTeller" ;
        rdfs:subClassOf  schema:FinancialService .

schema:expires  a     rdf:Property ;
        rdfs:comment  "Date the content expires and is no longer useful or available. For example a [[VideoObject]] or [[NewsArticle]] whose availability or relevance is time-limited, or a [[ClaimReview]] fact check whose publisher wants to indicate that it may no longer be relevant (or helpful to highlight) after some date." ;
        rdfs:label    "expires" .

schema:abstract  a    rdf:Property ;
        rdfs:comment  "An abstract is a short description that summarizes a [[CreativeWork]]." ;
        rdfs:label    "abstract" .

schema:availableChannel
        a             rdf:Property ;
        rdfs:comment  "A means of accessing the service (e.g. a phone bank, a web site, a location, etc.)." ;
        rdfs:label    "availableChannel" .

schema:roofLoad  a    rdf:Property ;
        rdfs:comment  "The permitted total weight of cargo and installations (e.g. a roof rack) on top of the vehicle.\\n\\nTypical unit code(s): KGM for kilogram, LBR for pound\\n\\n* Note 1: You can indicate additional information in the [[name]] of the [[QuantitativeValue]] node.\\n* Note 2: You may also link to a [[QualitativeValue]] node that provides additional information using [[valueReference]]\\n* Note 3: Note that you can use [[minValue]] and [[maxValue]] to indicate ranges." ;
        rdfs:label    "roofLoad" .

schema:Synagogue  a      rdfs:Class ;
        rdfs:comment     "A synagogue." ;
        rdfs:label       "Synagogue" ;
        rdfs:subClassOf  schema:PlaceOfWorship .

schema:availableDeliveryMethod
        a             rdf:Property ;
        rdfs:comment  "The delivery method(s) available for this offer." ;
        rdfs:label    "availableDeliveryMethod" .

schema:acceptedOffer  a  rdf:Property ;
        rdfs:comment  "The offer(s) -- e.g., product, quantity and price combinations -- included in the order." ;
        rdfs:label    "acceptedOffer" .

schema:broadcastSubChannel
        a             rdf:Property ;
        rdfs:comment  "The subchannel used for the broadcast." ;
        rdfs:label    "broadcastSubChannel" .

schema:ComicSeries  a    rdfs:Class ;
        rdfs:comment     "A sequential publication of comic stories under a\n    \tunifying title, for example \"The Amazing Spider-Man\" or \"Groo the\n    \tWanderer\"." ;
        rdfs:label       "ComicSeries" ;
        rdfs:subClassOf  schema:Periodical .

schema:ParentAudience
        a                rdfs:Class ;
        rdfs:comment     "A set of characteristics describing parents, who can be interested in viewing some content." ;
        rdfs:label       "ParentAudience" ;
        rdfs:subClassOf  schema:PeopleAudience .

schema:departureBoatTerminal
        a             rdf:Property ;
        rdfs:comment  "The terminal or port from which the boat departs." ;
        rdfs:label    "departureBoatTerminal" .

schema:lodgingUnitDescription
        a             rdf:Property ;
        rdfs:comment  "A full description of the lodging unit." ;
        rdfs:label    "lodgingUnitDescription" .

schema:numberedPosition
        a             rdf:Property ;
        rdfs:comment  "A number associated with a role in an organization, for example, the number on an athlete's jersey." ;
        rdfs:label    "numberedPosition" .

schema:carrier  a     rdf:Property ;
        rdfs:comment  "'carrier' is an out-dated term indicating the 'provider' for parcel delivery and flights." ;
        rdfs:label    "carrier" .

schema:catalogNumber  a  rdf:Property ;
        rdfs:comment  "The catalog number for the release." ;
        rdfs:label    "catalogNumber" .

schema:Chapter  a        rdfs:Class ;
        rdfs:comment     "One of the sections into which a book is divided. A chapter usually has a section number or a name." ;
        rdfs:label       "Chapter" ;
        rdfs:subClassOf  schema:CreativeWork .

schema:hasPart  a     rdf:Property ;
        rdfs:comment  "Indicates an item or CreativeWork that is part of this item, or CreativeWork (in some sense)." ;
        rdfs:label    "hasPart" .

schema:target  a      rdf:Property ;
        rdfs:comment  "Indicates a target EntryPoint for an Action." ;
        rdfs:label    "target" .

schema:departureTime  a  rdf:Property ;
        rdfs:comment  "The expected departure time." ;
        rdfs:label    "departureTime" .

schema:Course  a         rdfs:Class ;
        rdfs:comment     "A description of an educational course which may be offered as distinct instances at which take place at different times or take place at different locations, or be offered through different media or modes of study. An educational course is a sequence of one or more educational events and/or creative works which aims to build knowledge, competence or ability of learners." ;
        rdfs:label       "Course" ;
        rdfs:subClassOf  schema:LearningResource , schema:CreativeWork .

schema:feesAndCommissionsSpecification
        a             rdf:Property ;
        rdfs:comment  "Description of fees, commissions, and other terms applied either to a class of financial product, or by a financial service organization." ;
        rdfs:label    "feesAndCommissionsSpecification" .

schema:BefriendAction
        a                rdfs:Class ;
        rdfs:comment     "The act of forming a personal connection with someone (object) mutually/bidirectionally/symmetrically.\\n\\nRelated actions:\\n\\n* [[FollowAction]]: Unlike FollowAction, BefriendAction implies that the connection is reciprocal." ;
        rdfs:label       "BefriendAction" ;
        rdfs:subClassOf  schema:InteractAction .

schema:Bridge  a         rdfs:Class ;
        rdfs:comment     "A bridge." ;
        rdfs:label       "Bridge" ;
        rdfs:subClassOf  schema:CivicStructure .

schema:FAQPage  a        rdfs:Class ;
        rdfs:comment     "A [[FAQPage]] is a [[WebPage]] presenting one or more \"[Frequently asked questions](https://en.wikipedia.org/wiki/FAQ)\" (see also [[QAPage]])." ;
        rdfs:label       "FAQPage" ;
        rdfs:subClassOf  schema:WebPage .

schema:sizeGroup  a   rdf:Property ;
        rdfs:comment  "The size group (also known as \"size type\") for a product's size. Size groups are common in the fashion industry to define size segments and suggested audiences for wearable products. Multiple values can be combined, for example \"men's big and tall\", \"petite maternity\" or \"regular\"" ;
        rdfs:label    "sizeGroup" .

schema:ProductGroup  a   rdfs:Class ;
        rdfs:comment     "A ProductGroup represents a group of [[Product]]s that vary only in certain well-described ways, such as by [[size]], [[color]], [[material]] etc.\n\nWhile a ProductGroup itself is not directly offered for sale, the various varying products that it represents can be. The ProductGroup serves as a prototype or template, standing in for all of the products who have an [[isVariantOf]] relationship to it. As such, properties (including additional types) can be applied to the ProductGroup to represent characteristics shared by each of the (possibly very many) variants. Properties that reference a ProductGroup are not included in this mechanism; neither are the following specific properties [[variesBy]], [[hasVariant]], [[url]]. " ;
        rdfs:label       "ProductGroup" ;
        rdfs:subClassOf  schema:Product .

schema:albumRelease  a  rdf:Property ;
        rdfs:comment  "A release of this album." ;
        rdfs:label    "albumRelease" .

schema:clinicalPharmacology
        a             rdf:Property ;
        rdfs:comment  "Description of the absorption and elimination of drugs, including their concentration (pharmacokinetics, pK) and biological effects (pharmacodynamics, pD)." ;
        rdfs:label    "clinicalPharmacology" .

schema:prescribingInfo
        a             rdf:Property ;
        rdfs:comment  "Link to prescribing information for the drug." ;
        rdfs:label    "prescribingInfo" .

schema:commentCount  a  rdf:Property ;
        rdfs:comment  "The number of comments this CreativeWork (e.g. Article, Question or Answer) has received. This is most applicable to works published in Web sites with commenting system; additional comments may exist elsewhere." ;
        rdfs:label    "commentCount" .

schema:width  a       rdf:Property ;
        rdfs:comment  "The width of the item." ;
        rdfs:label    "width" .

schema:itemLocation  a      rdf:Property ;
        rdfs:comment        "Current location of the item."@en ;
        rdfs:label          "itemLocation"@en ;
        rdfs:subPropertyOf  schema:location .

schema:VideoGameClip  a  rdfs:Class ;
        rdfs:comment     "A short segment/part of a video game." ;
        rdfs:label       "VideoGameClip" ;
        rdfs:subClassOf  schema:Clip .

schema:Movie  a          rdfs:Class ;
        rdfs:comment     "A movie." ;
        rdfs:label       "Movie" ;
        rdfs:subClassOf  schema:CreativeWork .

schema:PhotographAction
        a                rdfs:Class ;
        rdfs:comment     "The act of capturing still images of objects using a camera." ;
        rdfs:label       "PhotographAction" ;
        rdfs:subClassOf  schema:CreateAction .

schema:DigitalDocumentPermission
        a                rdfs:Class ;
        rdfs:comment     "A permission for a particular person or group to access a particular file." ;
        rdfs:label       "DigitalDocumentPermission" ;
        rdfs:subClassOf  schema:Intangible .

schema:Emergency  a      rdfs:Class ;
        rdfs:comment     "A specific branch of medical science that deals with the evaluation and initial treatment of medical conditions caused by trauma or sudden illness." ;
        rdfs:label       "Emergency" ;
        rdfs:subClassOf  schema:MedicalBusiness .

schema:ListItem  a       rdfs:Class ;
        rdfs:comment     "An list item, e.g. a step in a checklist or how-to description." ;
        rdfs:label       "ListItem" ;
        rdfs:subClassOf  schema:Intangible .

schema:startDate  a   rdf:Property ;
        rdfs:comment  "The start date and time of the item (in [ISO 8601 date format](http://en.wikipedia.org/wiki/ISO_8601))." ;
        rdfs:label    "startDate" .

schema:servesCuisine  a  rdf:Property ;
        rdfs:comment  "The cuisine of the restaurant." ;
        rdfs:label    "servesCuisine" .

schema:replacee  a          rdf:Property ;
        rdfs:comment        "A sub property of object. The object that is being replaced." ;
        rdfs:label          "replacee" ;
        rdfs:subPropertyOf  schema:object .

schema:dosageForm  a  rdf:Property ;
        rdfs:comment  "A dosage form in which this drug/supplement is available, e.g. 'tablet', 'suspension', 'injection'." ;
        rdfs:label    "dosageForm" .

schema:variesBy  a    rdf:Property ;
        rdfs:comment  "Indicates the property or properties by which the variants in a [[ProductGroup]] vary, e.g. their size, color etc. Schema.org properties can be referenced by their short name e.g. \"color\"; terms defined elsewhere can be referenced with their URIs." ;
        rdfs:label    "variesBy" .

schema:experienceInPlaceOfEducation
        a             rdf:Property ;
        rdfs:comment  "Indicates whether a [[JobPosting]] will accept experience (as indicated by [[OccupationalExperienceRequirements]]) in place of its formal educational qualifications (as indicated by [[educationRequirements]]). If true, indicates that satisfying one of these requirements is sufficient." ;
        rdfs:label    "experienceInPlaceOfEducation" .

schema:description  a  rdf:Property ;
        rdfs:comment  "A description of the item." ;
        rdfs:label    "description" .

schema:prescriptionStatus
        a             rdf:Property ;
        rdfs:comment  "Indicates the status of drug prescription eg. local catalogs classifications or whether the drug is available by prescription or over-the-counter, etc." ;
        rdfs:label    "prescriptionStatus" .

schema:maximumEnrollment
        a             rdf:Property ;
        rdfs:comment  "The maximum number of students who may be enrolled in the program." ;
        rdfs:label    "maximumEnrollment" .

schema:availableIn  a  rdf:Property ;
        rdfs:comment  "The location in which the strength is available." ;
        rdfs:label    "availableIn" .

schema:Project  a        rdfs:Class ;
        rdfs:comment     "An enterprise (potentially individual but typically collaborative), planned to achieve a particular aim.\nUse properties from [[Organization]], [[subOrganization]]/[[parentOrganization]] to indicate project sub-structures. \n   " ;
        rdfs:label       "Project" ;
        rdfs:subClassOf  schema:Organization .

schema:Conversation  a   rdfs:Class ;
        rdfs:comment     "One or more messages between organizations or people on a particular topic. Individual messages can be linked to the conversation with isPartOf or hasPart properties." ;
        rdfs:label       "Conversation" ;
        rdfs:subClassOf  schema:CreativeWork .

schema:isbn  a              rdf:Property ;
        rdfs:comment        "The ISBN of the book." ;
        rdfs:label          "isbn" ;
        rdfs:subPropertyOf  schema:identifier .

schema:paymentUrl  a  rdf:Property ;
        rdfs:comment  "The URL for sending a payment." ;
        rdfs:label    "paymentUrl" .

schema:ReviewAction  a   rdfs:Class ;
        rdfs:comment     "The act of producing a balanced opinion about the object for an audience. An agent reviews an object with participants resulting in a review." ;
        rdfs:label       "ReviewAction" ;
        rdfs:subClassOf  schema:AssessAction .

schema:accessibilityHazard
        a             rdf:Property ;
        rdfs:comment  "A characteristic of the described resource that is physiologically dangerous to some users. Related to WCAG 2.0 guideline 2.3 ([WebSchemas wiki lists possible values](http://www.w3.org/wiki/WebSchemas/Accessibility))." ;
        rdfs:label    "accessibilityHazard" .

schema:timeToComplete
        a             rdf:Property ;
        rdfs:comment  "The expected length of time to complete the program if attending full-time." ;
        rdfs:label    "timeToComplete" .

schema:Ligament  a       rdfs:Class ;
        rdfs:comment     "A short band of tough, flexible, fibrous connective tissue that functions to connect multiple bones, cartilages, and structurally support joints." ;
        rdfs:label       "Ligament" ;
        rdfs:subClassOf  schema:AnatomicalStructure .

schema:OnDemandEvent  a  rdfs:Class ;
        rdfs:comment     "A publication event e.g. catch-up TV or radio podcast, during which a program is available on-demand." ;
        rdfs:label       "OnDemandEvent" ;
        rdfs:subClassOf  schema:PublicationEvent .

schema:priceValidUntil
        a             rdf:Property ;
        rdfs:comment  "The date after which the price is no longer available." ;
        rdfs:label    "priceValidUntil" .

schema:percentile75  a  rdf:Property ;
        rdfs:comment  "The 75th percentile value." ;
        rdfs:label    "percentile75" .

schema:TheaterEvent  a   rdfs:Class ;
        rdfs:comment     "Event type: Theater performance." ;
        rdfs:label       "TheaterEvent" ;
        rdfs:subClassOf  schema:Event .

schema:homeLocation  a      rdf:Property ;
        rdfs:comment        "A contact location for a person's residence." ;
        rdfs:label          "homeLocation" ;
        rdfs:subPropertyOf  schema:location .

schema:occupationalCredentialAwarded
        a             rdf:Property ;
        rdfs:comment  "A description of the qualification, award, certificate, diploma or other occupational credential awarded as a consequence of successful completion of this course or program." ;
        rdfs:label    "occupationalCredentialAwarded" .

schema:agent  a       rdf:Property ;
        rdfs:comment  "The direct performer or driver of the action (animate or inanimate). e.g. *John* wrote a book." ;
        rdfs:label    "agent" .

schema:AdministrativeArea
        a                rdfs:Class ;
        rdfs:comment     "A geographical region, typically under the jurisdiction of a particular government." ;
        rdfs:label       "AdministrativeArea" ;
        rdfs:subClassOf  schema:Place .

schema:defaultValue  a  rdf:Property ;
        rdfs:comment  "The default value of the input.  For properties that expect a literal, the default is a literal value, for properties that expect an object, it's an ID reference to one of the current values." ;
        rdfs:label    "defaultValue" .

schema:colleagues  a  rdf:Property ;
        rdfs:comment  "A colleague of the person." ;
        rdfs:label    "colleagues" .

schema:numConstraints
        a             rdf:Property ;
        rdfs:comment  "Indicates the number of constraints (not counting [[populationType]]) defined for a particular [[StatisticalPopulation]]. This helps applications understand if they have access to a sufficiently complete description of a [[StatisticalPopulation]]." ;
        rdfs:label    "numConstraints" .

schema:frequency  a   rdf:Property ;
        rdfs:comment  "How often the dose is taken, e.g. 'daily'." ;
        rdfs:label    "frequency" .

schema:isAccessibleForFree
        a             rdf:Property ;
        rdfs:comment  "A flag to signal that the item, event, or place is accessible for free." ;
        rdfs:label    "isAccessibleForFree" .

schema:MediaManipulationRatingEnumeration
        a                rdfs:Class ;
        rdfs:comment     " Codes for use with the [[mediaAuthenticityCategory]] property, indicating the authenticity of a media object (in the context of how it was published or shared). In general these codes are not mutually exclusive, although some combinations (such as 'original' versus 'transformed', 'edited' and 'staged') would be contradictory if applied in the same [[MediaReview]]. Note that the application of these codes is with regard to a piece of media shared or published in a particular context." ;
        rdfs:label       "MediaManipulationRatingEnumeration" ;
        rdfs:subClassOf  schema:Enumeration .

schema:numberOfFullBathrooms
        a             rdf:Property ;
        rdfs:comment  "Number of full bathrooms - The total number of full and ¾ bathrooms in an [[Accommodation]]. This corresponds to the [BathroomsFull field in RESO](https://ddwiki.reso.org/display/DDW17/BathroomsFull+Field)." ;
        rdfs:label    "numberOfFullBathrooms" .

schema:Preschool  a      rdfs:Class ;
        rdfs:comment     "A preschool." ;
        rdfs:label       "Preschool" ;
        rdfs:subClassOf  schema:EducationalOrganization .

schema:ItemList  a       rdfs:Class ;
        rdfs:comment     "A list of items of any sort&#x2014;for example, Top 10 Movies About Weathermen, or Top 100 Party Songs. Not to be confused with HTML lists, which are often used only for formatting." ;
        rdfs:label       "ItemList" ;
        rdfs:subClassOf  schema:Intangible .

schema:SocialEvent  a    rdfs:Class ;
        rdfs:comment     "Event type: Social event." ;
        rdfs:label       "SocialEvent" ;
        rdfs:subClassOf  schema:Event .

schema:ExhibitionEvent
        a                rdfs:Class ;
        rdfs:comment     "Event type: Exhibition event, e.g. at a museum, library, archive, tradeshow, ..." ;
        rdfs:label       "ExhibitionEvent" ;
        rdfs:subClassOf  schema:Event .

schema:ArchiveOrganization
        a                rdfs:Class ;
        rdfs:comment     "An organization with archival holdings. An organization which keeps and preserves archival material and typically makes it accessible to the public."@en ;
        rdfs:label       "ArchiveOrganization"@en ;
        rdfs:subClassOf  schema:LocalBusiness .

schema:engineType  a  rdf:Property ;
        rdfs:comment  "The type of engine or engines powering the vehicle." ;
        rdfs:label    "engineType" .

schema:FlightReservation
        a                rdfs:Class ;
        rdfs:comment     "A reservation for air travel.\\n\\nNote: This type is for information about actual reservations, e.g. in confirmation emails or HTML pages with individual confirmations of reservations. For offers of tickets, use [[Offer]]." ;
        rdfs:label       "FlightReservation" ;
        rdfs:subClassOf  schema:Reservation .

schema:sportsTeam  a        rdf:Property ;
        rdfs:comment        "A sub property of participant. The sports team that participated on this action." ;
        rdfs:label          "sportsTeam" ;
        rdfs:subPropertyOf  schema:participant .

schema:availableFrom  a  rdf:Property ;
        rdfs:comment  "When the item is available for pickup from the store, locker, etc." ;
        rdfs:label    "availableFrom" .

schema:MedicalDevicePurpose
        a                rdfs:Class ;
        rdfs:comment     "Categories of medical devices, organized by the purpose or intended use of the device." ;
        rdfs:label       "MedicalDevicePurpose" ;
        rdfs:subClassOf  schema:MedicalEnumeration .

schema:TechArticle  a    rdfs:Class ;
        rdfs:comment     "A technical article - Example: How-to (task) topics, step-by-step, procedural troubleshooting, specifications, etc." ;
        rdfs:label       "TechArticle" ;
        rdfs:subClassOf  schema:Article .

schema:code  a        rdf:Property ;
        rdfs:comment  "A medical code for the entity, taken from a controlled vocabulary or ontology such as ICD-9, DiseasesDB, MeSH, SNOMED-CT, RxNorm, etc." ;
        rdfs:label    "code" .

schema:InvestmentOrDeposit
        a                rdfs:Class ;
        rdfs:comment     "A type of financial product that typically requires the client to transfer funds to a financial service in return for potential beneficial financial return." ;
        rdfs:label       "InvestmentOrDeposit" ;
        rdfs:subClassOf  schema:FinancialProduct .

schema:valueName  a   rdf:Property ;
        rdfs:comment  "Indicates the name of the PropertyValueSpecification to be used in URL templates and form encoding in a manner analogous to HTML's input@name." ;
        rdfs:label    "valueName" .

schema:diseasePreventionInfo
        a             rdf:Property ;
        rdfs:comment  "Information about disease prevention." ;
        rdfs:label    "diseasePreventionInfo" .

schema:normalRange  a  rdf:Property ;
        rdfs:comment  "Range of acceptable values for a typical patient, when applicable." ;
        rdfs:label    "normalRange" .

schema:SoftwareApplication
        a                rdfs:Class ;
        rdfs:comment     "A software application." ;
        rdfs:label       "SoftwareApplication" ;
        rdfs:subClassOf  schema:CreativeWork .

schema:PublicToilet  a   rdfs:Class ;
        rdfs:comment     "A public toilet is a room or small building containing one or more toilets (and possibly also urinals) which is available for use by the general public, or by customers or employees of certain businesses." ;
        rdfs:label       "PublicToilet" ;
        rdfs:subClassOf  schema:CivicStructure .

schema:alumni  a      rdf:Property ;
        rdfs:comment  "Alumni of an organization." ;
        rdfs:label    "alumni" .

schema:billingStart  a  rdf:Property ;
        rdfs:comment  "Specifies after how much time this price (or price component) becomes valid and billing starts. Can be used, for example, to model a price increase after the first year of a subscription. The unit of measurement is specified by the unitCode property." ;
        rdfs:label    "billingStart" .

schema:publisher  a   rdf:Property ;
        rdfs:comment  "The publisher of the creative work." ;
        rdfs:label    "publisher" .

schema:totalJobOpenings
        a             rdf:Property ;
        rdfs:comment  "The number of positions open for this job posting. Use a positive integer. Do not use if the number of positions is unclear or not known." ;
        rdfs:label    "totalJobOpenings" .

schema:globalLocationNumber
        a                   rdf:Property ;
        rdfs:comment        "The [Global Location Number](http://www.gs1.org/gln) (GLN, sometimes also referred to as International Location Number or ILN) of the respective organization, person, or place. The GLN is a 13-digit number used to identify parties and physical locations." ;
        rdfs:label          "globalLocationNumber" ;
        rdfs:subPropertyOf  schema:identifier .

schema:Schedule  a       rdfs:Class ;
        rdfs:comment     "A schedule defines a repeating time period used to describe a regularly occurring [[Event]]. At a minimum a schedule will specify [[repeatFrequency]] which describes the interval between occurences of the event. Additional information can be provided to specify the schedule more precisely.\n      This includes identifying the day(s) of the week or month when the recurring event will take place, in addition to its start and end time. Schedules may also\n      have start and end dates to indicate when they are active, e.g. to define a limited calendar of events." ;
        rdfs:label       "Schedule" ;
        rdfs:subClassOf  schema:Intangible .

schema:CreativeWorkSeason
        a                rdfs:Class ;
        rdfs:comment     "A media season e.g. tv, radio, video game etc." ;
        rdfs:label       "CreativeWorkSeason" ;
        rdfs:subClassOf  schema:CreativeWork .

schema:termDuration  a  rdf:Property ;
        rdfs:comment  "The amount of time in a term as defined by the institution. A term is a length of time where students take one or more classes. Semesters and quarters are common units for term." ;
        rdfs:label    "termDuration" .

schema:MedicalEntity  a  rdfs:Class ;
        rdfs:comment     "The most generic type of entity related to health and the practice of medicine." ;
        rdfs:label       "MedicalEntity" ;
        rdfs:subClassOf  schema:Thing .

schema:productGroupID
        a             rdf:Property ;
        rdfs:comment  "Indicates a textual identifier for a ProductGroup." ;
        rdfs:label    "productGroupID" .

schema:ticketNumber  a  rdf:Property ;
        rdfs:comment  "The unique identifier for the ticket." ;
        rdfs:label    "ticketNumber" .

schema:Diet  a           rdfs:Class ;
        rdfs:comment     "A strategy of regulating the intake of food to achieve or maintain a specific health-related goal." ;
        rdfs:label       "Diet" ;
        rdfs:subClassOf  schema:LifestyleModification , schema:CreativeWork .

schema:isrcCode  a    rdf:Property ;
        rdfs:comment  "The International Standard Recording Code for the recording." ;
        rdfs:label    "isrcCode" .

schema:Map  a            rdfs:Class ;
        rdfs:comment     "A map." ;
        rdfs:label       "Map" ;
        rdfs:subClassOf  schema:CreativeWork .

schema:legislationLegalValue
        a             rdf:Property ;
        rdfs:comment  "The legal value of this legislation file. The same legislation can be written in multiple files with different legal values. Typically a digitally signed PDF have a \"stronger\" legal value than the HTML file of the same act." ;
        rdfs:label    "legislationLegalValue" .

schema:BusStop  a        rdfs:Class ;
        rdfs:comment     "A bus stop." ;
        rdfs:label       "BusStop" ;
        rdfs:subClassOf  schema:CivicStructure .

schema:Midwifery  a      rdfs:Class ;
        rdfs:comment     "A nurse-like health profession that deals with pregnancy, childbirth, and the postpartum period (including care of the newborn), besides sexual and reproductive health of women throughout their lives." ;
        rdfs:label       "Midwifery" ;
        rdfs:subClassOf  schema:MedicalBusiness .

schema:Courthouse  a     rdfs:Class ;
        rdfs:comment     "A courthouse." ;
        rdfs:label       "Courthouse" ;
        rdfs:subClassOf  schema:GovernmentBuilding .

schema:PerformAction  a  rdfs:Class ;
        rdfs:comment     "The act of participating in performance arts." ;
        rdfs:label       "PerformAction" ;
        rdfs:subClassOf  schema:PlayAction .

schema:ElementarySchool
        a                rdfs:Class ;
        rdfs:comment     "An elementary school." ;
        rdfs:label       "ElementarySchool" ;
        rdfs:subClassOf  schema:EducationalOrganization .

schema:recipeYield  a       rdf:Property ;
        rdfs:comment        "The quantity produced by the recipe (for example, number of people served, number of servings, etc)." ;
        rdfs:label          "recipeYield" ;
        rdfs:subPropertyOf  schema:yield .

schema:containsSeason
        a                   rdf:Property ;
        rdfs:comment        "A season that is part of the media series." ;
        rdfs:label          "containsSeason" ;
        rdfs:subPropertyOf  schema:hasPart .

schema:sourcedFrom  a  rdf:Property ;
        rdfs:comment  "The neurological pathway that originates the neurons." ;
        rdfs:label    "sourcedFrom" .

schema:downPayment  a  rdf:Property ;
        rdfs:comment  "a type of payment made in cash during the onset of the purchase of an expensive good/service. The payment typically represents only a percentage of the full purchase price." ;
        rdfs:label    "downPayment" .

schema:shippingDetails
        a             rdf:Property ;
        rdfs:comment  "Indicates information about the shipping policies and options associated with an [[Offer]]." ;
        rdfs:label    "shippingDetails" .

schema:softwareAddOn  a  rdf:Property ;
        rdfs:comment  "Additional content for a software application." ;
        rdfs:label    "softwareAddOn" .

schema:MedicalImagingTechnique
        a                rdfs:Class ;
        rdfs:comment     "Any medical imaging modality typically used for diagnostic purposes. Enumerated type." ;
        rdfs:label       "MedicalImagingTechnique" ;
        rdfs:subClassOf  schema:MedicalEnumeration .

schema:trialDesign  a  rdf:Property ;
        rdfs:comment  "Specifics about the trial design (enumerated)." ;
        rdfs:label    "trialDesign" .

schema:WPFooter  a       rdfs:Class ;
        rdfs:comment     "The footer section of the page." ;
        rdfs:label       "WPFooter" ;
        rdfs:subClassOf  schema:WebPageElement .

schema:merchantReturnLink
        a             rdf:Property ;
        rdfs:comment  "Indicates a Web page or service by URL, for product return." ;
        rdfs:label    "merchantReturnLink" .

schema:targetPlatform
        a             rdf:Property ;
        rdfs:comment  "Type of app development: phone, Metro style, desktop, XBox, etc." ;
        rdfs:label    "targetPlatform" .

schema:DrugStrength  a   rdfs:Class ;
        rdfs:comment     "A specific strength in which a medical drug is available in a specific country." ;
        rdfs:label       "DrugStrength" ;
        rdfs:subClassOf  schema:MedicalIntangible .

schema:ToyStore  a       rdfs:Class ;
        rdfs:comment     "A toy store." ;
        rdfs:label       "ToyStore" ;
        rdfs:subClassOf  schema:Store .

schema:encoding  a    rdf:Property ;
        rdfs:comment  "A media object that encodes this CreativeWork. This property is a synonym for associatedMedia." ;
        rdfs:label    "encoding" .

schema:VitalSign  a      rdfs:Class ;
        rdfs:comment     "Vital signs are measures of various physiological functions in order to assess the most basic body functions." ;
        rdfs:label       "VitalSign" ;
        rdfs:subClassOf  schema:MedicalSign .

schema:beneficiaryBank
        a             rdf:Property ;
        rdfs:comment  "A bank or bank’s branch, financial institution or international financial institution operating the beneficiary’s bank account or releasing funds for the beneficiary." ;
        rdfs:label    "beneficiaryBank" .

schema:saturatedFatContent
        a             rdf:Property ;
        rdfs:comment  "The number of grams of saturated fat." ;
        rdfs:label    "saturatedFatContent" .

schema:smokingAllowed
        a             rdf:Property ;
        rdfs:comment  "Indicates whether it is allowed to smoke in the place, e.g. in the restaurant, hotel or hotel room." ;
        rdfs:label    "smokingAllowed" .

schema:TakeAction  a     rdfs:Class ;
        rdfs:comment     "The act of gaining ownership of an object from an origin. Reciprocal of GiveAction.\\n\\nRelated actions:\\n\\n* [[GiveAction]]: The reciprocal of TakeAction.\\n* [[ReceiveAction]]: Unlike ReceiveAction, TakeAction implies that ownership has been transfered." ;
        rdfs:label       "TakeAction" ;
        rdfs:subClassOf  schema:TransferAction .

schema:GeoCircle  a      rdfs:Class ;
        rdfs:comment     "A GeoCircle is a GeoShape representing a circular geographic area. As it is a GeoShape\n          it provides the simple textual property 'circle', but also allows the combination of postalCode alongside geoRadius.\n          The center of the circle can be indicated via the 'geoMidpoint' property, or more approximately using 'address', 'postalCode'.\n       " ;
        rdfs:label       "GeoCircle" ;
        rdfs:subClassOf  schema:GeoShape .

schema:HealthClub  a     rdfs:Class ;
        rdfs:comment     "A health club." ;
        rdfs:label       "HealthClub" ;
        rdfs:subClassOf  schema:SportsActivityLocation , schema:HealthAndBeautyBusiness .

schema:insertion  a   rdf:Property ;
        rdfs:comment  "The place of attachment of a muscle, or what the muscle moves." ;
        rdfs:label    "insertion" .

schema:founders  a    rdf:Property ;
        rdfs:comment  "A person who founded this organization." ;
        rdfs:label    "founders" .

schema:familyName  a  rdf:Property ;
        rdfs:comment  "Family name. In the U.S., the last name of a Person." ;
        rdfs:label    "familyName" .

schema:Text  a        rdfs:Class ;
        rdfs:comment  "Data type: Text." ;
        rdfs:label    "Text" .

schema:mechanismOfAction
        a             rdf:Property ;
        rdfs:comment  "The specific biochemical interaction through which this drug or supplement produces its pharmacological effect." ;
        rdfs:label    "mechanismOfAction" .

schema:playerType  a  rdf:Property ;
        rdfs:comment  "Player type required&#x2014;for example, Flash or Silverlight." ;
        rdfs:label    "playerType" .

schema:Offer  a          rdfs:Class ;
        rdfs:comment     "An offer to transfer some rights to an item or to provide a service — for example, an offer to sell tickets to an event, to rent the DVD of a movie, to stream a TV show over the internet, to repair a motorcycle, or to loan a book.\\n\\nNote: As the [[businessFunction]] property, which identifies the form of offer (e.g. sell, lease, repair, dispose), defaults to http://purl.org/goodrelations/v1#Sell; an Offer without a defined businessFunction value can be assumed to be an offer to sell.\\n\\nFor [GTIN](http://www.gs1.org/barcodes/technical/idkeys/gtin)-related fields, see [Check Digit calculator](http://www.gs1.org/barcodes/support/check_digit_calculator) and [validation guide](http://www.gs1us.org/resources/standards/gtin-validation-guide) from [GS1](http://www.gs1.org/)." ;
        rdfs:label       "Offer" ;
        rdfs:subClassOf  schema:Intangible .

schema:ActionStatusType
        a                rdfs:Class ;
        rdfs:comment     "The status of an Action." ;
        rdfs:label       "ActionStatusType" ;
        rdfs:subClassOf  schema:StatusEnumeration .

schema:populationType
        a             rdf:Property ;
        rdfs:comment  "Indicates the populationType common to all members of a [[StatisticalPopulation]]." ;
        rdfs:label    "populationType" .

schema:WebSite  a        rdfs:Class ;
        rdfs:comment     "A WebSite is a set of related web pages and other items typically served from a single web domain and accessible via URLs." ;
        rdfs:label       "WebSite" ;
        rdfs:subClassOf  schema:CreativeWork .

schema:RespiratoryTherapy
        a                rdfs:Class ;
        rdfs:comment     "The therapy that is concerned with the maintenance or improvement of respiratory function (as in patients with pulmonary disease)." ;
        rdfs:label       "RespiratoryTherapy" ;
        rdfs:subClassOf  schema:MedicalTherapy .

schema:healthPlanMarketingUrl
        a             rdf:Property ;
        rdfs:comment  "The URL that goes directly to the plan brochure for the specific standard plan or plan variation." ;
        rdfs:label    "healthPlanMarketingUrl" .

schema:itemReviewed  a  rdf:Property ;
        rdfs:comment  "The item that is being reviewed/rated." ;
        rdfs:label    "itemReviewed" .

schema:MedicalStudy  a   rdfs:Class ;
        rdfs:comment     "A medical study is an umbrella type covering all kinds of research studies relating to human medicine or health, including observational studies and interventional trials and registries, randomized, controlled or not. When the specific type of study is known, use one of the extensions of this type, such as MedicalTrial or MedicalObservationalStudy. Also, note that this type should be used to mark up data that describes the study itself; to tag an article that publishes the results of a study, use MedicalScholarlyArticle. Note: use the code property of MedicalEntity to store study IDs, e.g. clinicaltrials.gov ID." ;
        rdfs:label       "MedicalStudy" ;
        rdfs:subClassOf  schema:MedicalEntity .

schema:CreativeWork  a   rdfs:Class ;
        rdfs:comment     "The most generic kind of creative work, including books, movies, photographs, software programs, etc." ;
        rdfs:label       "CreativeWork" ;
        rdfs:subClassOf  schema:Thing .

schema:iataCode  a    rdf:Property ;
        rdfs:comment  "IATA identifier for an airline or airport." ;
        rdfs:label    "iataCode" .

schema:MusicGroup  a     rdfs:Class ;
        rdfs:comment     "A musical group, such as a band, an orchestra, or a choir. Can also be a solo musician." ;
        rdfs:label       "MusicGroup" ;
        rdfs:subClassOf  schema:PerformingGroup .

bibo:Issue  a   rdfs:Class .

schema:orderQuantity  a  rdf:Property ;
        rdfs:comment  "The number of the item ordered. If the property is not set, assume the quantity is one." ;
        rdfs:label    "orderQuantity" .

schema:includedInHealthInsurancePlan
        a             rdf:Property ;
        rdfs:comment  "The insurance plans that cover this drug." ;
        rdfs:label    "includedInHealthInsurancePlan" .

schema:Embassy  a        rdfs:Class ;
        rdfs:comment     "An embassy." ;
        rdfs:label       "Embassy" ;
        rdfs:subClassOf  schema:GovernmentBuilding .

schema:nsn  a               rdf:Property ;
        rdfs:comment        "Indicates the [NATO stock number](https://en.wikipedia.org/wiki/NATO_Stock_Number) (nsn) of a [[Product]]. " ;
        rdfs:label          "nsn" ;
        rdfs:subPropertyOf  schema:identifier .

schema:reviewedBy  a  rdf:Property ;
        rdfs:comment  "People or organizations that have reviewed the content on this web page for accuracy and/or completeness." ;
        rdfs:label    "reviewedBy" .

schema:itemListOrder  a  rdf:Property ;
        rdfs:comment  "Type of ordering (e.g. Ascending, Descending, Unordered)." ;
        rdfs:label    "itemListOrder" .

schema:ReactAction  a    rdfs:Class ;
        rdfs:comment     "The act of responding instinctively and emotionally to an object, expressing a sentiment." ;
        rdfs:label       "ReactAction" ;
        rdfs:subClassOf  schema:AssessAction .

schema:EventStatusType
        a                rdfs:Class ;
        rdfs:comment     "EventStatusType is an enumeration type whose instances represent several states that an Event may be in." ;
        rdfs:label       "EventStatusType" ;
        rdfs:subClassOf  schema:StatusEnumeration .

schema:dateIssued  a  rdf:Property ;
        rdfs:comment  "The date the ticket was issued." ;
        rdfs:label    "dateIssued" .

schema:processorRequirements
        a             rdf:Property ;
        rdfs:comment  "Processor architecture required to run the application (e.g. IA64)." ;
        rdfs:label    "processorRequirements" .

schema:seatingType  a  rdf:Property ;
        rdfs:comment  "The type/class of the seat." ;
        rdfs:label    "seatingType" .

schema:MapCategoryType
        a                rdfs:Class ;
        rdfs:comment     "An enumeration of several kinds of Map." ;
        rdfs:label       "MapCategoryType" ;
        rdfs:subClassOf  schema:Enumeration .

schema:maximumIntake  a  rdf:Property ;
        rdfs:comment  "Recommended intake of this supplement for a given population as defined by a specific recommending authority." ;
        rdfs:label    "maximumIntake" .

schema:Room  a           rdfs:Class ;
        rdfs:comment     "A room is a distinguishable space within a structure, usually separated from other spaces by interior walls. (Source: Wikipedia, the free encyclopedia, see <a href=\"http://en.wikipedia.org/wiki/Room\">http://en.wikipedia.org/wiki/Room</a>).\n<br /><br />\nSee also the <a href=\"/docs/hotels.html\">dedicated document on the use of schema.org for marking up hotels and other forms of accommodations</a>.\n" ;
        rdfs:label       "Room" ;
        rdfs:subClassOf  schema:Accommodation .

schema:torque  a      rdf:Property ;
        rdfs:comment  "The torque (turning force) of the vehicle's engine.\\n\\nTypical unit code(s): NU for newton metre (N m), F17 for pound-force per foot, or F48 for pound-force per inch\\n\\n* Note 1: You can link to information about how the given value has been determined (e.g. reference RPM) using the [[valueReference]] property.\\n* Note 2: You can use [[minValue]] and [[maxValue]] to indicate ranges." ;
        rdfs:label    "torque" .

schema:geoContains  a  rdf:Property ;
        rdfs:comment  "Represents a relationship between two geometries (or the places they represent), relating a containing geometry to a contained geometry. \"a contains b iff no points of b lie in the exterior of a, and at least one point of the interior of b lies in the interior of a\". As defined in [DE-9IM](https://en.wikipedia.org/wiki/DE-9IM)." ;
        rdfs:label    "geoContains" .

schema:GovernmentBuilding
        a                rdfs:Class ;
        rdfs:comment     "A government building." ;
        rdfs:label       "GovernmentBuilding" ;
        rdfs:subClassOf  schema:CivicStructure .

schema:FoodService  a    rdfs:Class ;
        rdfs:comment     "A food service, like breakfast, lunch, or dinner." ;
        rdfs:label       "FoodService" ;
        rdfs:subClassOf  schema:Service .

schema:ReserveAction  a  rdfs:Class ;
        rdfs:comment     "Reserving a concrete object.\\n\\nRelated actions:\\n\\n* [[ScheduleAction]]: Unlike ScheduleAction, ReserveAction reserves concrete objects (e.g. a table, a hotel) towards a time slot / spatial allocation." ;
        rdfs:label       "ReserveAction" ;
        rdfs:subClassOf  schema:PlanAction .

schema:ArtGallery  a     rdfs:Class ;
        rdfs:comment     "An art gallery." ;
        rdfs:label       "ArtGallery" ;
        rdfs:subClassOf  schema:EntertainmentBusiness .

schema:GeneralContractor
        a                rdfs:Class ;
        rdfs:comment     "A general contractor." ;
        rdfs:label       "GeneralContractor" ;
        rdfs:subClassOf  schema:HomeAndConstructionBusiness .

schema:termsPerYear  a  rdf:Property ;
        rdfs:comment  "The number of times terms of study are offered per year. Semesters and quarters are common units for term. For example, if the student can only take 2 semesters for the program in one year, then termsPerYear should be 2." ;
        rdfs:label    "termsPerYear" .

schema:FloorPlan  a      rdfs:Class ;
        rdfs:comment     "A FloorPlan is an explicit representation of a collection of similar accommodations, allowing the provision of common information (room counts, sizes, layout diagrams) and offers for rental or sale. In typical use, some [[ApartmentComplex]] has an [[accommodationFloorPlan]] which is a [[FloorPlan]].  A FloorPlan is always in the context of a particular place, either a larger [[ApartmentComplex]] or a single [[Apartment]]. The visual/spatial aspects of a floor plan (i.e. room layout, [see wikipedia](https://en.wikipedia.org/wiki/Floor_plan)) can be indicated using [[image]]. " ;
        rdfs:label       "FloorPlan" ;
        rdfs:subClassOf  schema:Intangible .

schema:healthPlanCoinsuranceRate
        a             rdf:Property ;
        rdfs:comment  "Whether The rate of coinsurance expressed as a number between 0.0 and 1.0." ;
        rdfs:label    "healthPlanCoinsuranceRate" .

schema:applicationSubCategory
        a             rdf:Property ;
        rdfs:comment  "Subcategory of the application, e.g. 'Arcade Game'." ;
        rdfs:label    "applicationSubCategory" .

schema:leiCode  a           rdf:Property ;
        rdfs:comment        "An organization identifier that uniquely identifies a legal entity as defined in ISO 17442." ;
        rdfs:label          "leiCode" ;
        rdfs:subPropertyOf  schema:identifier .

schema:cvdNumC19Died  a  rdf:Property ;
        rdfs:comment  "numc19died - DEATHS: Patients with suspected or confirmed COVID-19 who died in the hospital, ED, or any overflow location." ;
        rdfs:label    "cvdNumC19Died" .

schema:vehicleSpecialUsage
        a             rdf:Property ;
        rdfs:comment  "Indicates whether the vehicle has been used for special purposes, like commercial rental, driving school, or as a taxi. The legislation in many countries requires this information to be revealed when offering a car for sale." ;
        rdfs:label    "vehicleSpecialUsage" .

schema:functionalClass
        a             rdf:Property ;
        rdfs:comment  "The degree of mobility the joint allows." ;
        rdfs:label    "functionalClass" .

schema:countriesNotSupported
        a             rdf:Property ;
        rdfs:comment  "Countries for which the application is not supported. You can also provide the two-letter ISO 3166-1 alpha-2 country code." ;
        rdfs:label    "countriesNotSupported" .

schema:lesserOrEqual  a  rdf:Property ;
        rdfs:comment  "This ordering relation for qualitative values indicates that the subject is lesser than or equal to the object." ;
        rdfs:label    "lesserOrEqual" .

schema:Drawing  a        rdfs:Class ;
        rdfs:comment     "A picture or diagram made with a pencil, pen, or crayon rather than paint." ;
        rdfs:label       "Drawing" ;
        rdfs:subClassOf  schema:CreativeWork .

schema:Car  a            rdfs:Class ;
        rdfs:comment     "A car is a wheeled, self-powered motor vehicle used for transportation." ;
        rdfs:label       "Car" ;
        rdfs:subClassOf  schema:Vehicle .

schema:HealthAspectEnumeration
        a                rdfs:Class ;
        rdfs:comment     "HealthAspectEnumeration enumerates several aspects of health content online, each of which might be described using [[hasHealthAspect]] and [[HealthTopicContent]]." ;
        rdfs:label       "HealthAspectEnumeration" ;
        rdfs:subClassOf  schema:Enumeration .

schema:accountMinimumInflow
        a             rdf:Property ;
        rdfs:comment  "A minimum amount that has to be paid in every month." ;
        rdfs:label    "accountMinimumInflow" .

schema:articleBody  a  rdf:Property ;
        rdfs:comment  "The actual body of the article." ;
        rdfs:label    "articleBody" .

schema:arrivalPlatform
        a             rdf:Property ;
        rdfs:comment  "The platform where the train arrives." ;
        rdfs:label    "arrivalPlatform" .

schema:broadcastFrequency
        a             rdf:Property ;
        rdfs:comment  "The frequency used for over-the-air broadcasts. Numeric values or simple ranges e.g. 87-99. In addition a shortcut idiom is supported for frequences of AM and FM radio channels, e.g. \"87 FM\"." ;
        rdfs:label    "broadcastFrequency" .

schema:MortgageLoan  a   rdfs:Class ;
        rdfs:comment     "A loan in which property or real estate is used as collateral. (A loan securitized against some real estate)." ;
        rdfs:label       "MortgageLoan" ;
        rdfs:subClassOf  schema:LoanOrCredit .

schema:codingSystem  a  rdf:Property ;
        rdfs:comment  "The coding system, e.g. 'ICD-10'." ;
        rdfs:label    "codingSystem" .

schema:diversityPolicy
        a             rdf:Property ;
        rdfs:comment  "Statement on diversity policy by an [[Organization]] e.g. a [[NewsMediaOrganization]]. For a [[NewsMediaOrganization]], a statement describing the newsroom’s diversity policy on both staffing and sources, typically providing staffing data." ;
        rdfs:label    "diversityPolicy" .

schema:ShoppingCenter
        a                rdfs:Class ;
        rdfs:comment     "A shopping center or mall." ;
        rdfs:label       "ShoppingCenter" ;
        rdfs:subClassOf  schema:LocalBusiness .

schema:MonetaryGrant  a  rdfs:Class ;
        rdfs:comment     "A monetary grant." ;
        rdfs:label       "MonetaryGrant" ;
        rdfs:subClassOf  schema:Grant .

schema:OpeningHoursSpecification
        a                rdfs:Class ;
        rdfs:comment     "A structured value providing information about the opening hours of a place or a certain service inside a place.\\n\\n\nThe place is __open__ if the [[opens]] property is specified, and __closed__ otherwise.\\n\\nIf the value for the [[closes]] property is less than the value for the [[opens]] property then the hour range is assumed to span over the next day.\n      " ;
        rdfs:label       "OpeningHoursSpecification" ;
        rdfs:subClassOf  schema:StructuredValue .

schema:storageRequirements
        a             rdf:Property ;
        rdfs:comment  "Storage requirements (free space required)." ;
        rdfs:label    "storageRequirements" .

schema:EUEnergyEfficiencyEnumeration
        a                rdfs:Class ;
        rdfs:comment     "Enumerates the EU energy efficiency classes A-G as well as A+, A++, and A+++ as defined in EU directive 2017/1369." ;
        rdfs:label       "EUEnergyEfficiencyEnumeration" ;
        rdfs:subClassOf  schema:EnergyEfficiencyEnumeration .

schema:partOfEpisode  a     rdf:Property ;
        rdfs:comment        "The episode to which this clip belongs." ;
        rdfs:label          "partOfEpisode" ;
        rdfs:subPropertyOf  schema:isPartOf .

schema:PerformanceRole
        a                rdfs:Class ;
        rdfs:comment     "A PerformanceRole is a Role that some entity places with regard to a theatrical performance, e.g. in a Movie, TVSeries etc." ;
        rdfs:label       "PerformanceRole" ;
        rdfs:subClassOf  schema:Role .

schema:RestrictedDiet
        a                rdfs:Class ;
        rdfs:comment     "A diet restricted to certain foods or preparations for cultural, religious, health or lifestyle reasons. " ;
        rdfs:label       "RestrictedDiet" ;
        rdfs:subClassOf  schema:Enumeration .

schema:Newspaper  a      rdfs:Class ;
        rdfs:comment     "A publication containing information about varied topics that are pertinent to general information, a geographic area, or a specific subject matter (i.e. business, culture, education). Often published daily." ;
        rdfs:label       "Newspaper" ;
        rdfs:subClassOf  schema:Periodical .

schema:EducationalOccupationalProgram
        a                rdfs:Class ;
        rdfs:comment     "A program offered by an institution which determines the learning progress to achieve an outcome, usually a credential like a degree or certificate. This would define a discrete set of opportunities (e.g., job, courses) that together constitute a program with a clear start, end, set of requirements, and transition to a new occupational opportunity (e.g., a job), or sometimes a higher educational opportunity (e.g., an advanced degree)." ;
        rdfs:label       "EducationalOccupationalProgram" ;
        rdfs:subClassOf  schema:Intangible .

geo:asWKT  a    rdf:Property .

schema:cvdNumC19OFMechVentPats
        a             rdf:Property ;
        rdfs:comment  "numc19ofmechventpats - ED/OVERFLOW and VENTILATED: Patients with suspected or confirmed COVID-19 who are in the ED or any overflow location awaiting an inpatient bed and on a mechanical ventilator." ;
        rdfs:label    "cvdNumC19OFMechVentPats" .

schema:contentLocation
        a             rdf:Property ;
        rdfs:comment  "The location depicted or described in the content. For example, the location in a photograph or painting." ;
        rdfs:label    "contentLocation" .

schema:longitude  a   rdf:Property ;
        rdfs:comment  "The longitude of a location. For example ```-122.08585``` ([WGS 84](https://en.wikipedia.org/wiki/World_Geodetic_System))." ;
        rdfs:label    "longitude" .

schema:broadcastChannelId
        a             rdf:Property ;
        rdfs:comment  "The unique address by which the BroadcastService can be identified in a provider lineup. In US, this is typically a number." ;
        rdfs:label    "broadcastChannelId" .

schema:pregnancyWarning
        a             rdf:Property ;
        rdfs:comment  "Any precaution, guidance, contraindication, etc. related to this drug's use during pregnancy." ;
        rdfs:label    "pregnancyWarning" .

schema:scheduledPaymentDate
        a             rdf:Property ;
        rdfs:comment  "The date the invoice is scheduled to be paid." ;
        rdfs:label    "scheduledPaymentDate" .

schema:CurrencyConversionService
        a                rdfs:Class ;
        rdfs:comment     "A service to convert funds from one currency to another currency." ;
        rdfs:label       "CurrencyConversionService" ;
        rdfs:subClassOf  schema:FinancialProduct .

schema:OfferForPurchase
        a                rdfs:Class ;
        rdfs:comment     "An [[OfferForPurchase]] in Schema.org represents an [[Offer]] to sell something, i.e. an [[Offer]] whose\n  [[businessFunction]] is [sell](http://purl.org/goodrelations/v1#Sell.). See [Good Relations](https://en.wikipedia.org/wiki/GoodRelations) for\n  background on the underlying concepts.\n  " ;
        rdfs:label       "OfferForPurchase" ;
        rdfs:subClassOf  schema:Offer .

schema:identifyingTest
        a             rdf:Property ;
        rdfs:comment  "A diagnostic test that can identify this sign." ;
        rdfs:label    "identifyingTest" .

schema:BusStation  a     rdfs:Class ;
        rdfs:comment     "A bus station." ;
        rdfs:label       "BusStation" ;
        rdfs:subClassOf  schema:CivicStructure .

schema:baseSalary  a  rdf:Property ;
        rdfs:comment  "The base salary of the job or of an employee in an EmployeeRole." ;
        rdfs:label    "baseSalary" .

schema:Corporation  a    rdfs:Class ;
        rdfs:comment     "Organization: A business corporation." ;
        rdfs:label       "Corporation" ;
        rdfs:subClassOf  schema:Organization .

schema:MerchantReturnPolicy
        a                rdfs:Class ;
        rdfs:comment     "A MerchantReturnPolicy provides information about product return policies associated with an [[Organization]] or [[Product]]." ;
        rdfs:label       "MerchantReturnPolicy" ;
        rdfs:subClassOf  schema:Intangible .

schema:MedicalTestPanel
        a                rdfs:Class ;
        rdfs:comment     "Any collection of tests commonly ordered together." ;
        rdfs:label       "MedicalTestPanel" ;
        rdfs:subClassOf  schema:MedicalTest .

schema:priceComponentType
        a             rdf:Property ;
        rdfs:comment  "Identifies a price component (for example, a line item on an invoice), part of the total price for an offer." ;
        rdfs:label    "priceComponentType" .

schema:PhysicalActivityCategory
        a                rdfs:Class ;
        rdfs:comment     "Categories of physical activity, organized by physiologic classification." ;
        rdfs:label       "PhysicalActivityCategory" ;
        rdfs:subClassOf  schema:Enumeration .

schema:Recommendation
        a                rdfs:Class ;
        rdfs:comment     "[[Recommendation]] is a type of [[Review]] that suggests or proposes something as the best option or best course of action. Recommendations may be for products or services, or other concrete things, as in the case of a ranked list or product guide. A [[Guide]] may list multiple recommendations for different categories. For example, in a [[Guide]] about which TVs to buy, the author may have several [[Recommendation]]s." ;
        rdfs:label       "Recommendation" ;
        rdfs:subClassOf  schema:Review .

schema:tickerSymbol  a  rdf:Property ;
        rdfs:comment  "The exchange traded instrument associated with a Corporation object. The tickerSymbol is expressed as an exchange and an instrument name separated by a space character. For the exchange component of the tickerSymbol attribute, we recommend using the controlled vocabulary of Market Identifier Codes (MIC) specified in ISO15022." ;
        rdfs:label    "tickerSymbol" .

schema:creditedTo  a  rdf:Property ;
        rdfs:comment  "The group the release is credited to if different than the byArtist. For example, Red and Blue is credited to \"Stefani Germanotta Band\", but by Lady Gaga." ;
        rdfs:label    "creditedTo" .

schema:MedicalDevice  a  rdfs:Class ;
        rdfs:comment     "Any object used in a medical capacity, such as to diagnose or treat a patient." ;
        rdfs:label       "MedicalDevice" ;
        rdfs:subClassOf  schema:MedicalEntity .

schema:publicTransportClosuresInfo
        a             rdf:Property ;
        rdfs:comment  "Information about public transport closures." ;
        rdfs:label    "publicTransportClosuresInfo" .

schema:earlyPrepaymentPenalty
        a             rdf:Property ;
        rdfs:comment  "The amount to be paid as a penalty in the event of early payment of the loan." ;
        rdfs:label    "earlyPrepaymentPenalty" .

schema:Demand  a         rdfs:Class ;
        rdfs:comment     "A demand entity represents the public, not necessarily binding, not necessarily exclusive, announcement by an organization or person to seek a certain type of goods or services. For describing demand using this type, the very same properties used for Offer apply." ;
        rdfs:label       "Demand" ;
        rdfs:subClassOf  schema:Intangible .

schema:SeekToAction  a   rdfs:Class ;
        rdfs:comment     "This is the [[Action]] of navigating to a specific [[startOffset]] timestamp within a [[VideoObject]], typically represented with a URL template structure." ;
        rdfs:label       "SeekToAction" ;
        rdfs:subClassOf  schema:Action .

schema:StadiumOrArena
        a                rdfs:Class ;
        rdfs:comment     "A stadium." ;
        rdfs:label       "StadiumOrArena" ;
        rdfs:subClassOf  schema:SportsActivityLocation , schema:CivicStructure .

schema:isBasedOn  a   rdf:Property ;
        rdfs:comment  "A resource from which this work is derived or from which it is a modification or adaption." ;
        rdfs:label    "isBasedOn" .

schema:TrackAction  a    rdfs:Class ;
        rdfs:comment     "An agent tracks an object for updates.\\n\\nRelated actions:\\n\\n* [[FollowAction]]: Unlike FollowAction, TrackAction refers to the interest on the location of innanimates objects.\\n* [[SubscribeAction]]: Unlike SubscribeAction, TrackAction refers to  the interest on the location of innanimate objects." ;
        rdfs:label       "TrackAction" ;
        rdfs:subClassOf  schema:FindAction .

schema:fiberContent  a  rdf:Property ;
        rdfs:comment  "The number of grams of fiber." ;
        rdfs:label    "fiberContent" .

schema:guidelineDate  a  rdf:Property ;
        rdfs:comment  "Date on which this guideline's recommendation was made." ;
        rdfs:label    "guidelineDate" .

schema:LinkRole  a       rdfs:Class ;
        rdfs:comment     "A Role that represents a Web link e.g. as expressed via the 'url' property. Its linkRelationship property can indicate URL-based and plain textual link types e.g. those in IANA link registry or others such as 'amphtml'. This structure provides a placeholder where details from HTML's link element can be represented outside of HTML, e.g. in JSON-LD feeds." ;
        rdfs:label       "LinkRole" ;
        rdfs:subClassOf  schema:Role .

schema:TVClip  a         rdfs:Class ;
        rdfs:comment     "A short TV program or a segment/part of a TV program." ;
        rdfs:label       "TVClip" ;
        rdfs:subClassOf  schema:Clip .

schema:ineligibleRegion
        a             rdf:Property ;
        rdfs:comment  "The ISO 3166-1 (ISO 3166-1 alpha-2) or ISO 3166-2 code, the place, or the GeoShape for the geo-political region(s) for which the offer or delivery charge specification is not valid, e.g. a region where the transaction is not allowed.\\n\\nSee also [[eligibleRegion]].\n      " ;
        rdfs:label    "ineligibleRegion" .

schema:Distillery  a     rdfs:Class ;
        rdfs:comment     "A distillery." ;
        rdfs:label       "Distillery" ;
        rdfs:subClassOf  schema:FoodEstablishment .

schema:PriceTypeEnumeration
        a                rdfs:Class ;
        rdfs:comment     "Enumerates different price types, for example list price, invoice price, and sale price." ;
        rdfs:label       "PriceTypeEnumeration" ;
        rdfs:subClassOf  schema:Enumeration .

schema:assesses  a    rdf:Property ;
        rdfs:comment  "The item being described is intended to assess the competency or learning outcome defined by the referenced term." ;
        rdfs:label    "assesses" .

schema:MedicalContraindication
        a                rdfs:Class ;
        rdfs:comment     "A condition or factor that serves as a reason to withhold a certain medical therapy. Contraindications can be absolute (there are no reasonable circumstances for undertaking a course of action) or relative (the patient is at higher risk of complications, but that these risks may be outweighed by other considerations or mitigated by other measures)." ;
        rdfs:label       "MedicalContraindication" ;
        rdfs:subClassOf  schema:MedicalEntity .

schema:numberOfEpisodes
        a             rdf:Property ;
        rdfs:comment  "The number of episodes in this season or series." ;
        rdfs:label    "numberOfEpisodes" .

dcmitype:Image  a  rdfs:Class .

schema:requirements  a  rdf:Property ;
        rdfs:comment  "Component dependency requirements for application. This includes runtime environments and shared libraries that are not included in the application distribution package, but required to run the application (Examples: DirectX, Java or .NET runtime)." ;
        rdfs:label    "requirements" .

schema:partOfOrder  a  rdf:Property ;
        rdfs:comment  "The overall order the items in this delivery were included in." ;
        rdfs:label    "partOfOrder" .

schema:RadioSeries  a    rdfs:Class ;
        rdfs:comment     "CreativeWorkSeries dedicated to radio broadcast and associated online delivery." ;
        rdfs:label       "RadioSeries" ;
        rdfs:subClassOf  schema:CreativeWorkSeries .

schema:seeks  a       rdf:Property ;
        rdfs:comment  "A pointer to products or services sought by the organization or person (demand)." ;
        rdfs:label    "seeks" .

schema:geoEquals  a   rdf:Property ;
        rdfs:comment  "Represents spatial relations in which two geometries (or the places they represent) are topologically equal, as defined in [DE-9IM](https://en.wikipedia.org/wiki/DE-9IM). \"Two geometries are topologically equal if their interiors intersect and no part of the interior or boundary of one geometry intersects the exterior of the other\" (a symmetric relationship)" ;
        rdfs:label    "geoEquals" .

schema:includesObject
        a             rdf:Property ;
        rdfs:comment  "This links to a node or nodes indicating the exact quantity of the products included in  an [[Offer]] or [[ProductCollection]]." ;
        rdfs:label    "includesObject" .

schema:FinancialProduct
        a                rdfs:Class ;
        rdfs:comment     "A product provided to consumers and businesses by financial institutions such as banks, insurance companies, brokerage firms, consumer finance companies, and investment companies which comprise the financial services industry." ;
        rdfs:label       "FinancialProduct" ;
        rdfs:subClassOf  schema:Service .

schema:RadioBroadcastService
        a                rdfs:Class ;
        rdfs:comment     "A delivery service through which radio content is provided via broadcast over the air or online." ;
        rdfs:label       "RadioBroadcastService" ;
        rdfs:subClassOf  schema:BroadcastService .

schema:cvdNumICUBedsOcc
        a             rdf:Property ;
        rdfs:comment  "numicubedsocc - ICU BED OCCUPANCY: Total number of staffed inpatient ICU beds that are occupied." ;
        rdfs:label    "cvdNumICUBedsOcc" .

schema:relevantSpecialty
        a             rdf:Property ;
        rdfs:comment  "If applicable, a medical specialty in which this entity is relevant." ;
        rdfs:label    "relevantSpecialty" .

schema:LegalForceStatus
        a                rdfs:Class ;
        rdfs:comment     "A list of possible statuses for the legal force of a legislation." ;
        rdfs:label       "LegalForceStatus" ;
        rdfs:subClassOf  schema:StatusEnumeration .

schema:AskAction  a      rdfs:Class ;
        rdfs:comment     "The act of posing a question / favor to someone.\\n\\nRelated actions:\\n\\n* [[ReplyAction]]: Appears generally as a response to AskAction." ;
        rdfs:label       "AskAction" ;
        rdfs:subClassOf  schema:CommunicateAction .

schema:doseValue  a   rdf:Property ;
        rdfs:comment  "The value of the dose, e.g. 500." ;
        rdfs:label    "doseValue" .

schema:PhysicalTherapy
        a                rdfs:Class ;
        rdfs:comment     "A process of progressive physical care and rehabilitation aimed at improving a health condition." ;
        rdfs:label       "PhysicalTherapy" ;
        rdfs:subClassOf  schema:MedicalTherapy .

schema:ApartmentComplex
        a                rdfs:Class ;
        rdfs:comment     "Residence type: Apartment complex." ;
        rdfs:label       "ApartmentComplex" ;
        rdfs:subClassOf  schema:Residence .

schema:possibleComplication
        a             rdf:Property ;
        rdfs:comment  "A possible unexpected and unfavorable evolution of a medical condition. Complications may include worsening of the signs or symptoms of the disease, extension of the condition to other organ systems, etc." ;
        rdfs:label    "possibleComplication" .

schema:ShareAction  a    rdfs:Class ;
        rdfs:comment     "The act of distributing content to people for their amusement or edification." ;
        rdfs:label       "ShareAction" ;
        rdfs:subClassOf  schema:CommunicateAction .

schema:gameServer  a  rdf:Property ;
        rdfs:comment  "The server on which  it is possible to play the game." ;
        rdfs:label    "gameServer" .

schema:cvdNumBedsOcc  a  rdf:Property ;
        rdfs:comment  "numbedsocc - HOSPITAL INPATIENT BED OCCUPANCY: Total number of staffed inpatient beds that are occupied." ;
        rdfs:label    "cvdNumBedsOcc" .

schema:releaseOf  a   rdf:Property ;
        rdfs:comment  "The album this is a release of." ;
        rdfs:label    "releaseOf" .

schema:EnergyConsumptionDetails
        a                rdfs:Class ;
        rdfs:comment     "EnergyConsumptionDetails represents information related to the energy efficiency of a product that consumes energy. The information that can be provided is based on international regulations such as for example [EU directive 2017/1369](https://eur-lex.europa.eu/eli/reg/2017/1369/oj) for energy labeling and the [Energy labeling rule](https://www.ftc.gov/enforcement/rules/rulemaking-regulatory-reform-proceedings/energy-water-use-labeling-consumer) under the Energy Policy and Conservation Act (EPCA) in the US." ;
        rdfs:label       "EnergyConsumptionDetails" ;
        rdfs:subClassOf  schema:Intangible .

schema:expectedPrognosis
        a             rdf:Property ;
        rdfs:comment  "The likely outcome in either the short term or long term of the medical condition." ;
        rdfs:label    "expectedPrognosis" .

schema:Table  a          rdfs:Class ;
        rdfs:comment     "A table on a Web page." ;
        rdfs:label       "Table" ;
        rdfs:subClassOf  schema:WebPageElement .

schema:Order  a          rdfs:Class ;
        rdfs:comment     "An order is a confirmation of a transaction (a receipt), which can contain multiple line items, each represented by an Offer that has been accepted by the customer." ;
        rdfs:label       "Order" ;
        rdfs:subClassOf  schema:Intangible .

schema:accessibilityControl
        a             rdf:Property ;
        rdfs:comment  "Identifies input methods that are sufficient to fully control the described resource ([WebSchemas wiki lists possible values](http://www.w3.org/wiki/WebSchemas/Accessibility))." ;
        rdfs:label    "accessibilityControl" .

schema:rsvpResponse  a  rdf:Property ;
        rdfs:comment  "The response (yes, no, maybe) to the RSVP." ;
        rdfs:label    "rsvpResponse" .

schema:scheduledTime  a  rdf:Property ;
        rdfs:comment  "The time the object is scheduled to." ;
        rdfs:label    "scheduledTime" .

schema:error  a       rdf:Property ;
        rdfs:comment  "For failed actions, more information on the cause of the failure." ;
        rdfs:label    "error" .

schema:eligibleCustomerType
        a             rdf:Property ;
        rdfs:comment  "The type(s) of customers for which the given offer is valid." ;
        rdfs:label    "eligibleCustomerType" .

schema:ReservationStatusType
        a                rdfs:Class ;
        rdfs:comment     "Enumerated status values for Reservation." ;
        rdfs:label       "ReservationStatusType" ;
        rdfs:subClassOf  schema:StatusEnumeration .

schema:measuredValue  a  rdf:Property ;
        rdfs:comment  "The measuredValue of an [[Observation]]." ;
        rdfs:label    "measuredValue" .

schema:totalPrice  a  rdf:Property ;
        rdfs:comment  "The total price for the reservation or ticket, including applicable taxes, shipping, etc.\\n\\nUsage guidelines:\\n\\n* Use values from 0123456789 (Unicode 'DIGIT ZERO' (U+0030) to 'DIGIT NINE' (U+0039)) rather than superficially similiar Unicode symbols.\\n* Use '.' (Unicode 'FULL STOP' (U+002E)) rather than ',' to indicate a decimal point. Avoid using these symbols as a readability separator." ;
        rdfs:label    "totalPrice" .

schema:GovernmentOrganization
        a                rdfs:Class ;
        rdfs:comment     "A governmental organization or agency." ;
        rdfs:label       "GovernmentOrganization" ;
        rdfs:subClassOf  schema:Organization .

schema:RecyclingCenter
        a                rdfs:Class ;
        rdfs:comment     "A recycling center." ;
        rdfs:label       "RecyclingCenter" ;
        rdfs:subClassOf  schema:LocalBusiness .

schema:isResizable  a  rdf:Property ;
        rdfs:comment  "Whether the 3DModel allows resizing. For example, room layout applications often do not allow 3DModel elements to be resized to reflect reality." ;
        rdfs:label    "isResizable" .

schema:tributary  a   rdf:Property ;
        rdfs:comment  "The anatomical or organ system that the vein flows into; a larger structure that the vein connects to." ;
        rdfs:label    "tributary" .

schema:deathDate  a   rdf:Property ;
        rdfs:comment  "Date of death." ;
        rdfs:label    "deathDate" .

schema:jobLocation  a  rdf:Property ;
        rdfs:comment  "A (typically single) geographic location associated with the job position." ;
        rdfs:label    "jobLocation" .

schema:PetStore  a       rdfs:Class ;
        rdfs:comment     "A pet store." ;
        rdfs:label       "PetStore" ;
        rdfs:subClassOf  schema:Store .

schema:BoardingPolicyType
        a                rdfs:Class ;
        rdfs:comment     "A type of boarding policy used by an airline." ;
        rdfs:label       "BoardingPolicyType" ;
        rdfs:subClassOf  schema:Enumeration .

schema:eligibleQuantity
        a             rdf:Property ;
        rdfs:comment  "The interval and unit of measurement of ordering quantities for which the offer or price specification is valid. This allows e.g. specifying that a certain freight charge is valid only for a certain quantity." ;
        rdfs:label    "eligibleQuantity" .

schema:DDxElement  a     rdfs:Class ;
        rdfs:comment     "An alternative, closely-related condition typically considered later in the differential diagnosis process along with the signs that are used to distinguish it." ;
        rdfs:label       "DDxElement" ;
        rdfs:subClassOf  schema:MedicalIntangible .

schema:MedicalProcedure
        a                rdfs:Class ;
        rdfs:comment     "A process of care used in either a diagnostic, therapeutic, preventive or palliative capacity that relies on invasive (surgical), non-invasive, or other techniques." ;
        rdfs:label       "MedicalProcedure" ;
        rdfs:subClassOf  schema:MedicalEntity .

schema:healthPlanCoinsuranceOption
        a             rdf:Property ;
        rdfs:comment  "Whether the coinsurance applies before or after deductible, etc. TODO: Is this a closed set?" ;
        rdfs:label    "healthPlanCoinsuranceOption" .

schema:nationality  a  rdf:Property ;
        rdfs:comment  "Nationality of the person." ;
        rdfs:label    "nationality" .

schema:printEdition  a  rdf:Property ;
        rdfs:comment  "The edition of the print product in which the NewsArticle appears." ;
        rdfs:label    "printEdition" .

schema:SheetMusic  a     rdfs:Class ;
        rdfs:comment     "Printed music, as opposed to performed or recorded music." ;
        rdfs:label       "SheetMusic" ;
        rdfs:subClassOf  schema:CreativeWork .

schema:alignmentType  a  rdf:Property ;
        rdfs:comment  "A category of alignment between the learning resource and the framework node. Recommended values include: 'requires', 'textComplexity', 'readingLevel', and 'educationalSubject'." ;
        rdfs:label    "alignmentType" .

schema:relevantOccupation
        a             rdf:Property ;
        rdfs:comment  "The Occupation for the JobPosting." ;
        rdfs:label    "relevantOccupation" .

schema:associatedPathophysiology
        a             rdf:Property ;
        rdfs:comment  "If applicable, a description of the pathophysiology associated with the anatomical system, including potential abnormal changes in the mechanical, physical, and biochemical functions of the system." ;
        rdfs:label    "associatedPathophysiology" .

schema:disambiguatingDescription
        a                   rdf:Property ;
        rdfs:comment        "A sub property of description. A short description of the item used to disambiguate from other, similar items. Information from other properties (in particular, name) may be necessary for the description to be useful for disambiguation." ;
        rdfs:label          "disambiguatingDescription" ;
        rdfs:subPropertyOf  schema:description .

schema:floorLevel  a  rdf:Property ;
        rdfs:comment  "The floor level for an [[Accommodation]] in a multi-storey building. Since counting\n  systems [vary internationally](https://en.wikipedia.org/wiki/Storey#Consecutive_number_floor_designations), the local system should be used where possible." ;
        rdfs:label    "floorLevel" .

schema:HomeGoodsStore
        a                rdfs:Class ;
        rdfs:comment     "A home goods store." ;
        rdfs:label       "HomeGoodsStore" ;
        rdfs:subClassOf  schema:Store .

schema:drugClass  a   rdf:Property ;
        rdfs:comment  "The class of drug this belongs to (e.g., statins)." ;
        rdfs:label    "drugClass" .

schema:Ticket  a         rdfs:Class ;
        rdfs:comment     "Used to describe a ticket to an event, a flight, a bus ride, etc." ;
        rdfs:label       "Ticket" ;
        rdfs:subClassOf  schema:Intangible .

schema:Code  a           rdfs:Class ;
        rdfs:comment     "Computer programming source code. Example: Full (compile ready) solutions, code snippet samples, scripts, templates." ;
        rdfs:label       "Code" ;
        rdfs:subClassOf  schema:CreativeWork .

schema:significance  a  rdf:Property ;
        rdfs:comment  "The significance associated with the superficial anatomy; as an example, how characteristics of the superficial anatomy can suggest underlying medical conditions or courses of treatment." ;
        rdfs:label    "significance" .

schema:ChildCare  a      rdfs:Class ;
        rdfs:comment     "A Childcare center." ;
        rdfs:label       "ChildCare" ;
        rdfs:subClassOf  schema:LocalBusiness .

schema:MediaObject  a    rdfs:Class ;
        rdfs:comment     "A media object, such as an image, video, or audio object embedded in a web page or a downloadable dataset i.e. DataDownload. Note that a creative work may have many media objects associated with it on the same web page. For example, a page about a single song (MusicRecording) may have a music video (VideoObject), and a high and low bandwidth audio stream (2 AudioObject's)." ;
        rdfs:label       "MediaObject" ;
        rdfs:subClassOf  schema:CreativeWork .

schema:FurnitureStore
        a                rdfs:Class ;
        rdfs:comment     "A furniture store." ;
        rdfs:label       "FurnitureStore" ;
        rdfs:subClassOf  schema:Store .

schema:doorTime  a    rdf:Property ;
        rdfs:comment  "The time admission will commence." ;
        rdfs:label    "doorTime" .

schema:scheduleTimezone
        a             rdf:Property ;
        rdfs:comment  "Indicates the timezone for which the time(s) indicated in the [[Schedule]] are given. The value provided should be among those listed in the IANA Time Zone Database." ;
        rdfs:label    "scheduleTimezone" .

schema:WPSideBar  a      rdfs:Class ;
        rdfs:comment     "A sidebar section of the page." ;
        rdfs:label       "WPSideBar" ;
        rdfs:subClassOf  schema:WebPageElement .

schema:MovingCompany  a  rdfs:Class ;
        rdfs:comment     "A moving company." ;
        rdfs:label       "MovingCompany" ;
        rdfs:subClassOf  schema:HomeAndConstructionBusiness .

schema:menu  a        rdf:Property ;
        rdfs:comment  "Either the actual menu as a structured representation, as text, or a URL of the menu." ;
        rdfs:label    "menu" .

schema:Enumeration  a    rdfs:Class ;
        rdfs:comment     "Lists or enumerations—for example, a list of cuisines or music genres, etc." ;
        rdfs:label       "Enumeration" ;
        rdfs:subClassOf  schema:Intangible .

schema:artist  a      rdf:Property ;
        rdfs:comment  "The primary artist for a work\n    \tin a medium other than pencils or digital line art--for example, if the\n    \tprimary artwork is done in watercolors or digital paints." ;
        rdfs:label    "artist" .

schema:EducationalAudience
        a                rdfs:Class ;
        rdfs:comment     "An EducationalAudience." ;
        rdfs:label       "EducationalAudience" ;
        rdfs:subClassOf  schema:Audience .

schema:ConfirmAction  a  rdfs:Class ;
        rdfs:comment     "The act of notifying someone that a future event/action is going to happen as expected.\\n\\nRelated actions:\\n\\n* [[CancelAction]]: The antonym of ConfirmAction." ;
        rdfs:label       "ConfirmAction" ;
        rdfs:subClassOf  schema:InformAction .

schema:variantCover  a  rdf:Property ;
        rdfs:comment  "A description of the variant cover\n    \tfor the issue, if the issue is a variant printing. For example, \"Bryan Hitch\n    \tVariant Cover\" or \"2nd Printing Variant\"." ;
        rdfs:label    "variantCover" .

schema:contraindication
        a             rdf:Property ;
        rdfs:comment  "A contraindication for this therapy." ;
        rdfs:label    "contraindication" .

schema:PropertyValue  a  rdfs:Class ;
        rdfs:comment     "A property-value pair, e.g. representing a feature of a product or place. Use the 'name' property for the name of the property. If there is an additional human-readable version of the value, put that into the 'description' property.\\n\\n Always use specific schema.org properties when a) they exist and b) you can populate them. Using PropertyValue as a substitute will typically not trigger the same effect as using the original, specific property.\n    " ;
        rdfs:label       "PropertyValue" ;
        rdfs:subClassOf  schema:StructuredValue .

schema:isRelatedTo  a  rdf:Property ;
        rdfs:comment  "A pointer to another, somehow related product (or multiple products)." ;
        rdfs:label    "isRelatedTo" .

schema:OrganizeAction
        a                rdfs:Class ;
        rdfs:comment     "The act of manipulating/administering/supervising/controlling one or more objects." ;
        rdfs:label       "OrganizeAction" ;
        rdfs:subClassOf  schema:Action .

schema:carrierRequirements
        a             rdf:Property ;
        rdfs:comment  "Specifies specific carrier(s) requirements for the application (e.g. an application may only work on a specific carrier network)." ;
        rdfs:label    "carrierRequirements" .

schema:aircraft  a    rdf:Property ;
        rdfs:comment  "The kind of aircraft (e.g., \"Boeing 747\")." ;
        rdfs:label    "aircraft" .

schema:BackgroundNewsArticle
        a                rdfs:Class ;
        rdfs:comment     "A [[NewsArticle]] providing historical context, definition and detail on a specific topic (aka \"explainer\" or \"backgrounder\"). For example, an in-depth article or frequently-asked-questions ([FAQ](https://en.wikipedia.org/wiki/FAQ)) document on topics such as Climate Change or the European Union. Other kinds of background material from a non-news setting are often described using [[Book]] or [[Article]], in particular [[ScholarlyArticle]]. See also [[NewsArticle]] for related vocabulary from a learning/education perspective." ;
        rdfs:label       "BackgroundNewsArticle" ;
        rdfs:subClassOf  schema:NewsArticle .

schema:domainIncludes
        a             rdf:Property ;
        rdfs:comment  "Relates a property to a class that is (one of) the type(s) the property is expected to be used on." ;
        rdfs:label    "domainIncludes" .

schema:ScholarlyArticle
        a                rdfs:Class ;
        rdfs:comment     "A scholarly article." ;
        rdfs:label       "ScholarlyArticle" ;
        rdfs:subClassOf  schema:Article .

schema:BankOrCreditUnion
        a                rdfs:Class ;
        rdfs:comment     "Bank or credit union." ;
        rdfs:label       "BankOrCreditUnion" ;
        rdfs:subClassOf  schema:FinancialService .

schema:MedicalSign  a    rdfs:Class ;
        rdfs:comment     "Any physical manifestation of a person's medical condition discoverable by objective diagnostic tests or physical examination." ;
        rdfs:label       "MedicalSign" ;
        rdfs:subClassOf  schema:MedicalSignOrSymptom .

schema:orderNumber  a       rdf:Property ;
        rdfs:comment        "The identifier of the transaction." ;
        rdfs:label          "orderNumber" ;
        rdfs:subPropertyOf  schema:identifier .

schema:screenshot  a  rdf:Property ;
        rdfs:comment  "A link to a screenshot image of the app." ;
        rdfs:label    "screenshot" .

schema:TVEpisode  a      rdfs:Class ;
        rdfs:comment     "A TV episode which can be part of a series or season." ;
        rdfs:label       "TVEpisode" ;
        rdfs:subClassOf  schema:Episode .

schema:EducationEvent
        a                rdfs:Class ;
        rdfs:comment     "Event type: Education event." ;
        rdfs:label       "EducationEvent" ;
        rdfs:subClassOf  schema:Event .

schema:refundType  a  rdf:Property ;
        rdfs:comment  "A refundType, from an enumerated list." ;
        rdfs:label    "refundType" .

schema:keywords  a    rdf:Property ;
        rdfs:comment  "Keywords or tags used to describe this content. Multiple entries in a keywords list are typically delimited by commas." ;
        rdfs:label    "keywords" .

schema:GeoCoordinates
        a                rdfs:Class ;
        rdfs:comment     "The geographic coordinates of a place or event." ;
        rdfs:label       "GeoCoordinates" ;
        rdfs:subClassOf  schema:StructuredValue .

schema:seasonNumber  a      rdf:Property ;
        rdfs:comment        "Position of the season within an ordered group of seasons." ;
        rdfs:label          "seasonNumber" ;
        rdfs:subPropertyOf  schema:position .

schema:accelerationTime
        a             rdf:Property ;
        rdfs:comment  "The time needed to accelerate the vehicle from a given start velocity to a given target velocity.\\n\\nTypical unit code(s): SEC for seconds\\n\\n* Note: There are unfortunately no standard unit codes for seconds/0..100 km/h or seconds/0..60 mph. Simply use \"SEC\" for seconds and indicate the velocities in the [[name]] of the [[QuantitativeValue]], or use [[valueReference]] with a [[QuantitativeValue]] of 0..60 mph or 0..100 km/h to specify the reference speeds." ;
        rdfs:label    "accelerationTime" .

schema:Quotation  a      rdfs:Class ;
        rdfs:comment     "A quotation. Often but not necessarily from some written work, attributable to a real world author and - if associated with a fictional character - to any fictional Person. Use [[isBasedOn]] to link to source/origin. The [[recordedIn]] property can be used to reference a Quotation from an [[Event]]." ;
        rdfs:label       "Quotation" ;
        rdfs:subClassOf  schema:CreativeWork .

schema:vehicleInteriorColor
        a             rdf:Property ;
        rdfs:comment  "The color or color combination of the interior of the vehicle." ;
        rdfs:label    "vehicleInteriorColor" .

schema:dependencies  a  rdf:Property ;
        rdfs:comment  "Prerequisites needed to fulfill steps in article." ;
        rdfs:label    "dependencies" .

schema:learningResourceType
        a             rdf:Property ;
        rdfs:comment  "The predominant type or kind characterizing the learning resource. For example, 'presentation', 'handout'." ;
        rdfs:label    "learningResourceType" .

schema:DayOfWeek  a      rdfs:Class ;
        rdfs:comment     "The day of the week, e.g. used to specify to which day the opening hours of an OpeningHoursSpecification refer.\n\nOriginally, URLs from [GoodRelations](http://purl.org/goodrelations/v1) were used (for [[Monday]], [[Tuesday]], [[Wednesday]], [[Thursday]], [[Friday]], [[Saturday]], [[Sunday]] plus a special entry for [[PublicHolidays]]); these have now been integrated directly into schema.org.\n      " ;
        rdfs:label       "DayOfWeek" ;
        rdfs:subClassOf  schema:Enumeration .

schema:accessCode  a  rdf:Property ;
        rdfs:comment  "Password, PIN, or access code needed for delivery (e.g. from a locker)." ;
        rdfs:label    "accessCode" .

schema:jobImmediateStart
        a             rdf:Property ;
        rdfs:comment  "An indicator as to whether a position is available for an immediate start." ;
        rdfs:label    "jobImmediateStart" .

schema:gtin14  a            rdf:Property ;
        rdfs:comment        "The GTIN-14 code of the product, or the product to which the offer refers. See [GS1 GTIN Summary](http://www.gs1.org/barcodes/technical/idkeys/gtin) for more details." ;
        rdfs:label          "gtin14" ;
        rdfs:subPropertyOf  schema:identifier , schema:gtin .

schema:medicalAudience
        a             rdf:Property ;
        rdfs:comment  "Medical audience for page." ;
        rdfs:label    "medicalAudience" .

schema:ActivateAction
        a                rdfs:Class ;
        rdfs:comment     "The act of starting or activating a device or application (e.g. starting a timer or turning on a flashlight)." ;
        rdfs:label       "ActivateAction" ;
        rdfs:subClassOf  schema:ControlAction .

schema:applicationStartDate
        a             rdf:Property ;
        rdfs:comment  "The date at which the program begins collecting applications for the next enrollment cycle." ;
        rdfs:label    "applicationStartDate" .

schema:Quantity  a       rdfs:Class ;
        rdfs:comment     "Quantities such as distance, time, mass, weight, etc. Particular instances of say Mass are entities like '3 Kg' or '4 milligrams'." ;
        rdfs:label       "Quantity" ;
        rdfs:subClassOf  schema:Intangible .

schema:appliesToPaymentMethod
        a             rdf:Property ;
        rdfs:comment  "The payment method(s) to which the payment charge specification applies." ;
        rdfs:label    "appliesToPaymentMethod" .

schema:workExample  a  rdf:Property ;
        rdfs:comment  "Example/instance/realization/derivation of the concept of this creative work. eg. The paperback edition, first edition, or eBook." ;
        rdfs:label    "workExample" .

schema:Poster  a         rdfs:Class ;
        rdfs:comment     "A large, usually printed placard, bill, or announcement, often illustrated, that is posted to advertise or publicize something." ;
        rdfs:label       "Poster" ;
        rdfs:subClassOf  schema:CreativeWork .

schema:loser  a             rdf:Property ;
        rdfs:comment        "A sub property of participant. The loser of the action." ;
        rdfs:label          "loser" ;
        rdfs:subPropertyOf  schema:participant .

schema:dissolutionDate
        a             rdf:Property ;
        rdfs:comment  "The date that this organization was dissolved." ;
        rdfs:label    "dissolutionDate" .

schema:performTime  a  rdf:Property ;
        rdfs:comment  "The length of time it takes to perform instructions or a direction (not including time to prepare the supplies), in [ISO 8601 duration format](http://en.wikipedia.org/wiki/ISO_8601)." ;
        rdfs:label    "performTime" .

schema:Optician  a       rdfs:Class ;
        rdfs:comment     "A store that sells reading glasses and similar devices for improving vision." ;
        rdfs:label       "Optician" ;
        rdfs:subClassOf  schema:MedicalBusiness .

schema:NutritionInformation
        a                rdfs:Class ;
        rdfs:comment     "Nutritional information about the recipe." ;
        rdfs:label       "NutritionInformation" ;
        rdfs:subClassOf  schema:StructuredValue .

schema:exifData  a    rdf:Property ;
        rdfs:comment  "exif data for this object." ;
        rdfs:label    "exifData" .

schema:DownloadAction
        a                rdfs:Class ;
        rdfs:comment     "The act of downloading an object." ;
        rdfs:label       "DownloadAction" ;
        rdfs:subClassOf  schema:TransferAction .

schema:hasCredential  a  rdf:Property ;
        rdfs:comment  "A credential awarded to the Person or Organization." ;
        rdfs:label    "hasCredential" .

schema:warranty  a    rdf:Property ;
        rdfs:comment  "The warranty promise(s) included in the offer." ;
        rdfs:label    "warranty" .

schema:vehicleIdentificationNumber
        a                   rdf:Property ;
        rdfs:comment        "The Vehicle Identification Number (VIN) is a unique serial number used by the automotive industry to identify individual motor vehicles." ;
        rdfs:label          "vehicleIdentificationNumber" ;
        rdfs:subPropertyOf  schema:serialNumber .

schema:Store  a          rdfs:Class ;
        rdfs:comment     "A retail good store." ;
        rdfs:label       "Store" ;
        rdfs:subClassOf  schema:LocalBusiness .

schema:industry  a    rdf:Property ;
        rdfs:comment  "The industry associated with the job position." ;
        rdfs:label    "industry" .

schema:OrderItem  a      rdfs:Class ;
        rdfs:comment     "An order item is a line of an order. It includes the quantity and shipping details of a bought offer." ;
        rdfs:label       "OrderItem" ;
        rdfs:subClassOf  schema:Intangible .

schema:eligibleDuration
        a             rdf:Property ;
        rdfs:comment  "The duration for which the given offer is valid." ;
        rdfs:label    "eligibleDuration" .

schema:MotorcycleRepair
        a                rdfs:Class ;
        rdfs:comment     "A motorcycle repair shop." ;
        rdfs:label       "MotorcycleRepair" ;
        rdfs:subClassOf  schema:AutomotiveBusiness .

schema:Playground  a     rdfs:Class ;
        rdfs:comment     "A playground." ;
        rdfs:label       "Playground" ;
        rdfs:subClassOf  schema:CivicStructure .

schema:LandmarksOrHistoricalBuildings
        a                rdfs:Class ;
        rdfs:comment     "An historical landmark or building." ;
        rdfs:label       "LandmarksOrHistoricalBuildings" ;
        rdfs:subClassOf  schema:Place .

schema:SpeakableSpecification
        a                rdfs:Class ;
        rdfs:comment     "A SpeakableSpecification indicates (typically via [[xpath]] or [[cssSelector]]) sections of a document that are highlighted as particularly [[speakable]]. Instances of this type are expected to be used primarily as values of the [[speakable]] property." ;
        rdfs:label       "SpeakableSpecification" ;
        rdfs:subClassOf  schema:Intangible .

schema:availableTest  a  rdf:Property ;
        rdfs:comment  "A diagnostic test or procedure offered by this lab." ;
        rdfs:label    "availableTest" .

schema:Mass  a           rdfs:Class ;
        rdfs:comment     "Properties that take Mass as values are of the form '&lt;Number&gt; &lt;Mass unit of measure&gt;'. E.g., '7 kg'." ;
        rdfs:label       "Mass" ;
        rdfs:subClassOf  schema:Quantity .

schema:Physician  a      rdfs:Class ;
        rdfs:comment     "A doctor's office." ;
        rdfs:label       "Physician" ;
        rdfs:subClassOf  schema:MedicalBusiness , schema:MedicalOrganization .

schema:maxValue  a    rdf:Property ;
        rdfs:comment  "The upper value of some characteristic or property." ;
        rdfs:label    "maxValue" .

schema:muscleAction  a  rdf:Property ;
        rdfs:comment  "The movement the muscle generates." ;
        rdfs:label    "muscleAction" .

schema:seasons  a     rdf:Property ;
        rdfs:comment  "A season in a media series." ;
        rdfs:label    "seasons" .

schema:alcoholWarning
        a             rdf:Property ;
        rdfs:comment  "Any precaution, guidance, contraindication, etc. related to consumption of alcohol while taking this drug." ;
        rdfs:label    "alcoholWarning" .

schema:incentiveCompensation
        a             rdf:Property ;
        rdfs:comment  "Description of bonus and commission compensation aspects of the job." ;
        rdfs:label    "incentiveCompensation" .

schema:MedicalGuidelineRecommendation
        a                rdfs:Class ;
        rdfs:comment     "A guideline recommendation that is regarded as efficacious and where quality of the data supporting the recommendation is sound." ;
        rdfs:label       "MedicalGuidelineRecommendation" ;
        rdfs:subClassOf  schema:MedicalGuideline .

schema:musicalKey  a  rdf:Property ;
        rdfs:comment  "The key, mode, or scale this composition uses." ;
        rdfs:label    "musicalKey" .

schema:naturalProgression
        a             rdf:Property ;
        rdfs:comment  "The expected progression of the condition if it is not treated and allowed to progress naturally." ;
        rdfs:label    "naturalProgression" .

schema:Hostel  a         rdfs:Class ;
        rdfs:comment     "A hostel - cheap accommodation, often in shared dormitories.\n<br /><br />\nSee also the <a href=\"/docs/hotels.html\">dedicated document on the use of schema.org for marking up hotels and other forms of accommodations</a>.\n" ;
        rdfs:label       "Hostel" ;
        rdfs:subClassOf  schema:LodgingBusiness .

schema:countryOfOrigin
        a             rdf:Property ;
        rdfs:comment  "The country of the principal offices of the production company or individual responsible for the movie or program." ;
        rdfs:label    "countryOfOrigin" .

schema:AddAction  a      rdfs:Class ;
        rdfs:comment     "The act of editing by adding an object to a collection." ;
        rdfs:label       "AddAction" ;
        rdfs:subClassOf  schema:UpdateAction .

schema:Message  a        rdfs:Class ;
        rdfs:comment     "A single message from a sender to one or more organizations or people." ;
        rdfs:label       "Message" ;
        rdfs:subClassOf  schema:CreativeWork .

schema:numberOfCredits
        a             rdf:Property ;
        rdfs:comment  "The number of credits or units awarded by a Course or required to complete an EducationalOccupationalProgram." ;
        rdfs:label    "numberOfCredits" .

schema:trailerWeight  a  rdf:Property ;
        rdfs:comment  "The permitted weight of a trailer attached to the vehicle.\\n\\nTypical unit code(s): KGM for kilogram, LBR for pound\\n* Note 1: You can indicate additional information in the [[name]] of the [[QuantitativeValue]] node.\\n* Note 2: You may also link to a [[QualitativeValue]] node that provides additional information using [[valueReference]].\\n* Note 3: Note that you can use [[minValue]] and [[maxValue]] to indicate ranges." ;
        rdfs:label    "trailerWeight" .

schema:correction  a  rdf:Property ;
        rdfs:comment  "Indicates a correction to a [[CreativeWork]], either via a [[CorrectionComment]], textually or in another document." ;
        rdfs:label    "correction" .

schema:RsvpResponseType
        a                rdfs:Class ;
        rdfs:comment     "RsvpResponseType is an enumeration type whose instances represent responding to an RSVP request." ;
        rdfs:label       "RsvpResponseType" ;
        rdfs:subClassOf  schema:Enumeration .

schema:DefinedTermSet
        a                rdfs:Class ;
        rdfs:comment     "A set of defined terms for example a set of categories or a classification scheme, a glossary, dictionary or enumeration." ;
        rdfs:label       "DefinedTermSet" ;
        rdfs:subClassOf  schema:CreativeWork .

schema:DefenceEstablishment
        a                rdfs:Class ;
        rdfs:comment     "A defence establishment, such as an army or navy base." ;
        rdfs:label       "DefenceEstablishment" ;
        rdfs:subClassOf  schema:GovernmentBuilding .

schema:schemaVersion  a  rdf:Property ;
        rdfs:comment  "Indicates (by URL or string) a particular version of a schema used in some CreativeWork. This property was created primarily to\n    indicate the use of a specific schema.org release, e.g. ```10.0``` as a simple string, or more explicitly via URL, ```http://schema.org/docs/releases.html#v10.0```. There may be situations in which other schemas might usefully be referenced this way, e.g. ```http://dublincore.org/specifications/dublin-core/dces/1999-07-02/``` but this has not been carefully explored in the community." ;
        rdfs:label    "schemaVersion" .

schema:surface  a           rdf:Property ;
        rdfs:comment        "A material used as a surface in some artwork, e.g. Canvas, Paper, Wood, Board, etc." ;
        rdfs:label          "surface" ;
        rdfs:subPropertyOf  schema:material .

schema:advanceBookingRequirement
        a             rdf:Property ;
        rdfs:comment  "The amount of time that is required between accepting the offer and the actual usage of the resource or service." ;
        rdfs:label    "advanceBookingRequirement" .

schema:hasBroadcastChannel
        a             rdf:Property ;
        rdfs:comment  "A broadcast channel of a broadcast service." ;
        rdfs:label    "hasBroadcastChannel" .

schema:includesHealthPlanNetwork
        a             rdf:Property ;
        rdfs:comment  "Networks covered by this plan." ;
        rdfs:label    "includesHealthPlanNetwork" .

schema:ItemListOrderType
        a                rdfs:Class ;
        rdfs:comment     "Enumerated for values for itemListOrder for indicating how an ordered ItemList is organized." ;
        rdfs:label       "ItemListOrderType" ;
        rdfs:subClassOf  schema:Enumeration .

schema:billingDuration
        a             rdf:Property ;
        rdfs:comment  "Specifies for how long this price (or price component) will be billed. Can be used, for example, to model the contractual duration of a subscription or payment plan. Type can be either a Duration or a Number (in which case the unit of measurement, for example month, is specified by the unitCode property)." ;
        rdfs:label    "billingDuration" .

schema:relatedLink  a  rdf:Property ;
        rdfs:comment  "A link related to this web page, for example to other related web pages." ;
        rdfs:label    "relatedLink" .

schema:discount  a    rdf:Property ;
        rdfs:comment  "Any discount applied (to an Order)." ;
        rdfs:label    "discount" .

schema:serviceLocation
        a             rdf:Property ;
        rdfs:comment  "The location (e.g. civic structure, local business, etc.) where a person can go to access the service." ;
        rdfs:label    "serviceLocation" .

schema:isAvailableGenerically
        a             rdf:Property ;
        rdfs:comment  "True if the drug is available in a generic form (regardless of name)." ;
        rdfs:label    "isAvailableGenerically" .

schema:employmentUnit
        a             rdf:Property ;
        rdfs:comment  "Indicates the department, unit and/or facility where the employee reports and/or in which the job is to be performed." ;
        rdfs:label    "employmentUnit" .

schema:applicableLocation
        a             rdf:Property ;
        rdfs:comment  "The location in which the status applies." ;
        rdfs:label    "applicableLocation" .

schema:Person  a         rdfs:Class ;
        rdfs:comment     "A person (alive, dead, undead, or fictional)." ;
        rdfs:label       "Person" ;
        rdfs:subClassOf  schema:Thing .

schema:TVSeason  a       rdfs:Class ;
        rdfs:comment     "Season dedicated to TV broadcast and associated online delivery." ;
        rdfs:label       "TVSeason" ;
        rdfs:subClassOf  schema:CreativeWorkSeason , schema:CreativeWork .

schema:PronounceableText
        a                rdfs:Class ;
        rdfs:comment     "Data type: PronounceableText." ;
        rdfs:label       "PronounceableText" ;
        rdfs:subClassOf  schema:Text .

schema:activityFrequency
        a             rdf:Property ;
        rdfs:comment  "How often one should engage in the activity." ;
        rdfs:label    "activityFrequency" .

schema:amenityFeature
        a             rdf:Property ;
        rdfs:comment  "An amenity feature (e.g. a characteristic or service) of the Accommodation. This generic property does not make a statement about whether the feature is included in an offer for the main accommodation or available at extra costs." ;
        rdfs:label    "amenityFeature" .

schema:maxPrice  a    rdf:Property ;
        rdfs:comment  "The highest price if the price is a range." ;
        rdfs:label    "maxPrice" .

schema:programMembershipUsed
        a             rdf:Property ;
        rdfs:comment  "Any membership in a frequent flyer, hotel loyalty program, etc. being applied to the reservation." ;
        rdfs:label    "programMembershipUsed" .

schema:serviceAudience
        a             rdf:Property ;
        rdfs:comment  "The audience eligible for this service." ;
        rdfs:label    "serviceAudience" .

schema:strengthUnit  a  rdf:Property ;
        rdfs:comment  "The units of an active ingredient's strength, e.g. mg." ;
        rdfs:label    "strengthUnit" .

dcat:Dataset  a  rdfs:Class .

schema:sponsor  a     rdf:Property ;
        rdfs:comment  "A person or organization that supports a thing through a pledge, promise, or financial contribution. e.g. a sponsor of a Medical Study or a corporate sponsor of an event." ;
        rdfs:label    "sponsor" .

schema:URL  a            rdfs:Class ;
        rdfs:comment     "Data type: URL." ;
        rdfs:label       "URL" ;
        rdfs:subClassOf  schema:Text .

schema:Apartment  a      rdfs:Class ;
        rdfs:comment     "An apartment (in American English) or flat (in British English) is a self-contained housing unit (a type of residential real estate) that occupies only part of a building (Source: Wikipedia, the free encyclopedia, see <a href=\"http://en.wikipedia.org/wiki/Apartment\">http://en.wikipedia.org/wiki/Apartment</a>)." ;
        rdfs:label       "Apartment" ;
        rdfs:subClassOf  schema:Accommodation .

schema:deliveryStatus
        a             rdf:Property ;
        rdfs:comment  "New entry added as the package passes through each leg of its journey (from shipment to final delivery)." ;
        rdfs:label    "deliveryStatus" .

schema:legislationConsolidates
        a             rdf:Property ;
        rdfs:comment  "Indicates another legislation taken into account in this consolidated legislation (which is usually the product of an editorial process that revises the legislation). This property should be used multiple times to refer to both the original version or the previous consolidated version, and to the legislations making the change." ;
        rdfs:label    "legislationConsolidates" .

schema:JobPosting  a     rdfs:Class ;
        rdfs:comment     "A listing that describes a job opening in a certain organization." ;
        rdfs:label       "JobPosting" ;
        rdfs:subClassOf  schema:Intangible .

schema:BusReservation
        a                rdfs:Class ;
        rdfs:comment     "A reservation for bus travel. \\n\\nNote: This type is for information about actual reservations, e.g. in confirmation emails or HTML pages with individual confirmations of reservations. For offers of tickets, use [[Offer]]." ;
        rdfs:label       "BusReservation" ;
        rdfs:subClassOf  schema:Reservation .

schema:physicalRequirement
        a             rdf:Property ;
        rdfs:comment  "A description of the types of physical activity associated with the job. Defined terms such as those in O*net may be used, but note that there is no way to specify the level of ability as well as its nature when using a defined term." ;
        rdfs:label    "physicalRequirement" .

schema:colleague  a   rdf:Property ;
        rdfs:comment  "A colleague of the person." ;
        rdfs:label    "colleague" .

schema:Duration  a       rdfs:Class ;
        rdfs:comment     "Quantity: Duration (use [ISO 8601 duration format](http://en.wikipedia.org/wiki/ISO_8601))." ;
        rdfs:label       "Duration" ;
        rdfs:subClassOf  schema:Quantity .

schema:numberOfRooms  a  rdf:Property ;
        rdfs:comment  "The number of rooms (excluding bathrooms and closets) of the accommodation or lodging business.\nTypical unit code(s): ROM for room or C62 for no unit. The type of room can be put in the unitText property of the QuantitativeValue." ;
        rdfs:label    "numberOfRooms" .

schema:TransferAction
        a                rdfs:Class ;
        rdfs:comment     "The act of transferring/moving (abstract or concrete) animate or inanimate objects from one place to another." ;
        rdfs:label       "TransferAction" ;
        rdfs:subClassOf  schema:Action .

schema:SizeSpecification
        a                rdfs:Class ;
        rdfs:comment     "Size related properties of a product, typically a size code ([[name]]) and optionally a [[sizeSystem]], [[sizeGroup]], and product measurements ([[hasMeasurement]]). In addition, the intended audience can be defined through [[suggestedAge]], [[suggestedGender]], and suggested body measurements ([[suggestedMeasurement]])." ;
        rdfs:label       "SizeSpecification" ;
        rdfs:subClassOf  schema:QualitativeValue .

schema:inCodeSet  a         rdf:Property ;
        rdfs:comment        "A [[CategoryCodeSet]] that contains this category code." ;
        rdfs:label          "inCodeSet" ;
        rdfs:subPropertyOf  schema:inDefinedTermSet .

schema:TheaterGroup  a   rdfs:Class ;
        rdfs:comment     "A theater group or company, for example, the Royal Shakespeare Company or Druid Theatre." ;
        rdfs:label       "TheaterGroup" ;
        rdfs:subClassOf  schema:PerformingGroup .

schema:pageStart  a   rdf:Property ;
        rdfs:comment  "The page on which the work starts; for example \"135\" or \"xiii\"." ;
        rdfs:label    "pageStart" .

schema:spatial  a     rdf:Property ;
        rdfs:comment  "The \"spatial\" property can be used in cases when more specific properties\n(e.g. [[locationCreated]], [[spatialCoverage]], [[contentLocation]]) are not known to be appropriate." ;
        rdfs:label    "spatial" .

schema:unnamedSourcesPolicy
        a                   rdf:Property ;
        rdfs:comment        "For an [[Organization]] (typically a [[NewsMediaOrganization]]), a statement about policy on use of unnamed sources and the decision process required." ;
        rdfs:label          "unnamedSourcesPolicy" ;
        rdfs:subPropertyOf  schema:publishingPrinciples .

schema:additionalNumberOfGuests
        a             rdf:Property ;
        rdfs:comment  "If responding yes, the number of guests who will attend in addition to the invitee." ;
        rdfs:label    "additionalNumberOfGuests" .

schema:foodEstablishment
        a                   rdf:Property ;
        rdfs:comment        "A sub property of location. The specific food establishment where the action occurred." ;
        rdfs:label          "foodEstablishment" ;
        rdfs:subPropertyOf  schema:location .

schema:fuelConsumption
        a             rdf:Property ;
        rdfs:comment  "The amount of fuel consumed for traveling a particular distance or temporal duration with the given vehicle (e.g. liters per 100 km).\\n\\n* Note 1: There are unfortunately no standard unit codes for liters per 100 km.  Use [[unitText]] to indicate the unit of measurement, e.g. L/100 km.\\n* Note 2: There are two ways of indicating the fuel consumption, [[fuelConsumption]] (e.g. 8 liters per 100 km) and [[fuelEfficiency]] (e.g. 30 miles per gallon). They are reciprocal.\\n* Note 3: Often, the absolute value is useful only when related to driving speed (\"at 80 km/h\") or usage pattern (\"city traffic\"). You can use [[valueReference]] to link the value for the fuel consumption to another value." ;
        rdfs:label    "fuelConsumption" .

schema:passengerSequenceNumber
        a             rdf:Property ;
        rdfs:comment  "The passenger's sequence number as assigned by the airline." ;
        rdfs:label    "passengerSequenceNumber" .

schema:IceCreamShop  a   rdfs:Class ;
        rdfs:comment     "An ice cream shop." ;
        rdfs:label       "IceCreamShop" ;
        rdfs:subClassOf  schema:FoodEstablishment .

schema:JoinAction  a     rdfs:Class ;
        rdfs:comment     "An agent joins an event/group with participants/friends at a location.\\n\\nRelated actions:\\n\\n* [[RegisterAction]]: Unlike RegisterAction, JoinAction refers to joining a group/team of people.\\n* [[SubscribeAction]]: Unlike SubscribeAction, JoinAction does not imply that you'll be receiving updates.\\n* [[FollowAction]]: Unlike FollowAction, JoinAction does not imply that you'll be polling for updates." ;
        rdfs:label       "JoinAction" ;
        rdfs:subClassOf  schema:InteractAction .

schema:commentTime  a  rdf:Property ;
        rdfs:comment  "The time at which the UserComment was made." ;
        rdfs:label    "commentTime" .

schema:WebPage  a        rdfs:Class ;
        rdfs:comment     "A web page. Every web page is implicitly assumed to be declared to be of type WebPage, so the various properties about that webpage, such as <code>breadcrumb</code> may be used. We recommend explicit declaration if these properties are specified, but if they are found outside of an itemscope, they will be assumed to be about the page." ;
        rdfs:label       "WebPage" ;
        rdfs:subClassOf  schema:CreativeWork .

schema:PrependAction  a  rdfs:Class ;
        rdfs:comment     "The act of inserting at the beginning if an ordered collection." ;
        rdfs:label       "PrependAction" ;
        rdfs:subClassOf  schema:InsertAction .

schema:busName  a     rdf:Property ;
        rdfs:comment  "The name of the bus (e.g. Bolt Express)." ;
        rdfs:label    "busName" .

schema:nonprofitStatus
        a             rdf:Property ;
        rdfs:comment  "nonprofit Status indicates the legal status of a non-profit organization in its primary place of business." ;
        rdfs:label    "nonprofitStatus" .

schema:deathPlace  a  rdf:Property ;
        rdfs:comment  "The place where the person died." ;
        rdfs:label    "deathPlace" .

schema:availableStrength
        a             rdf:Property ;
        rdfs:comment  "An available dosage strength for the drug." ;
        rdfs:label    "availableStrength" .

schema:isLiveBroadcast
        a             rdf:Property ;
        rdfs:comment  "True if the broadcast is of a live event." ;
        rdfs:label    "isLiveBroadcast" .

schema:studyLocation  a  rdf:Property ;
        rdfs:comment  "The location in which the study is taking/took place." ;
        rdfs:label    "studyLocation" .

schema:namedPosition  a  rdf:Property ;
        rdfs:comment  "A position played, performed or filled by a person or organization, as part of an organization. For example, an athlete in a SportsTeam might play in the position named 'Quarterback'." ;
        rdfs:label    "namedPosition" .

schema:NightClub  a      rdfs:Class ;
        rdfs:comment     "A nightclub or discotheque." ;
        rdfs:label       "NightClub" ;
        rdfs:subClassOf  schema:EntertainmentBusiness .

schema:HowToTool  a      rdfs:Class ;
        rdfs:comment     "A tool used (but not consumed) when performing instructions for how to achieve a result." ;
        rdfs:label       "HowToTool" ;
        rdfs:subClassOf  schema:HowToItem .

schema:productID  a         rdf:Property ;
        rdfs:comment        "The product identifier, such as ISBN. For example: ``` meta itemprop=\"productID\" content=\"isbn:123-456-789\" ```." ;
        rdfs:label          "productID" ;
        rdfs:subPropertyOf  schema:identifier .

schema:LikeAction  a     rdfs:Class ;
        rdfs:comment     "The act of expressing a positive sentiment about the object. An agent likes an object (a proposition, topic or theme) with participants." ;
        rdfs:label       "LikeAction" ;
        rdfs:subClassOf  schema:ReactAction .

schema:CreditCard  a     rdfs:Class ;
        rdfs:comment     "A card payment method of a particular brand or name.  Used to mark up a particular payment method and/or the financial product/service that supplies the card account.\\n\\nCommonly used values:\\n\\n* http://purl.org/goodrelations/v1#AmericanExpress\\n* http://purl.org/goodrelations/v1#DinersClub\\n* http://purl.org/goodrelations/v1#Discover\\n* http://purl.org/goodrelations/v1#JCB\\n* http://purl.org/goodrelations/v1#MasterCard\\n* http://purl.org/goodrelations/v1#VISA\n       " ;
        rdfs:label       "CreditCard" ;
        rdfs:subClassOf  schema:PaymentCard , schema:LoanOrCredit .

schema:predecessorOf  a  rdf:Property ;
        rdfs:comment  "A pointer from a previous, often discontinued variant of the product to its newer variant." ;
        rdfs:label    "predecessorOf" .

schema:offeredBy  a   rdf:Property ;
        rdfs:comment  "A pointer to the organization or person making the offer." ;
        rdfs:label    "offeredBy" .

schema:tongueWeight  a  rdf:Property ;
        rdfs:comment  "The permitted vertical load (TWR) of a trailer attached to the vehicle. Also referred to as Tongue Load Rating (TLR) or Vertical Load Rating (VLR)\\n\\nTypical unit code(s): KGM for kilogram, LBR for pound\\n\\n* Note 1: You can indicate additional information in the [[name]] of the [[QuantitativeValue]] node.\\n* Note 2: You may also link to a [[QualitativeValue]] node that provides additional information using [[valueReference]].\\n* Note 3: Note that you can use [[minValue]] and [[maxValue]] to indicate ranges." ;
        rdfs:label    "tongueWeight" .

schema:endorsers  a   rdf:Property ;
        rdfs:comment  "People or organizations that endorse the plan." ;
        rdfs:label    "endorsers" .

schema:PaymentChargeSpecification
        a                rdfs:Class ;
        rdfs:comment     "The costs of settling the payment using a particular payment method." ;
        rdfs:label       "PaymentChargeSpecification" ;
        rdfs:subClassOf  schema:PriceSpecification .

schema:timeRequired  a  rdf:Property ;
        rdfs:comment  "Approximate or typical time it takes to work with or through this learning resource for the typical intended target audience, e.g. 'PT30M', 'PT1H25M'." ;
        rdfs:label    "timeRequired" .

schema:availabilityStarts
        a             rdf:Property ;
        rdfs:comment  "The beginning of the availability of the product or service included in the offer." ;
        rdfs:label    "availabilityStarts" .

schema:PreOrderAction
        a                rdfs:Class ;
        rdfs:comment     "An agent orders a (not yet released) object/product/service to be delivered/sent." ;
        rdfs:label       "PreOrderAction" ;
        rdfs:subClassOf  schema:TradeAction .

schema:TireShop  a       rdfs:Class ;
        rdfs:comment     "A tire shop." ;
        rdfs:label       "TireShop" ;
        rdfs:subClassOf  schema:Store .

schema:APIReference  a   rdfs:Class ;
        rdfs:comment     "Reference documentation for application programming interfaces (APIs)." ;
        rdfs:label       "APIReference" ;
        rdfs:subClassOf  schema:TechArticle .

schema:ImagingTest  a    rdfs:Class ;
        rdfs:comment     "Any medical imaging modality typically used for diagnostic purposes." ;
        rdfs:label       "ImagingTest" ;
        rdfs:subClassOf  schema:MedicalTest .

schema:Clip  a           rdfs:Class ;
        rdfs:comment     "A short TV or radio program or a segment/part of a program." ;
        rdfs:label       "Clip" ;
        rdfs:subClassOf  schema:CreativeWork .

schema:DryCleaningOrLaundry
        a                rdfs:Class ;
        rdfs:comment     "A dry-cleaning business." ;
        rdfs:label       "DryCleaningOrLaundry" ;
        rdfs:subClassOf  schema:LocalBusiness .

schema:holdingArchive
        a             rdf:Property ;
        rdfs:comment  "[[ArchiveOrganization]] that holds, keeps or maintains the [[ArchiveComponent]]."@en ;
        rdfs:label    "holdingArchive"@en .

schema:jobLocationType
        a             rdf:Property ;
        rdfs:comment  "A description of the job location (e.g TELECOMMUTE for telecommute jobs)." ;
        rdfs:label    "jobLocationType" .

schema:DataDownload  a   rdfs:Class ;
        rdfs:comment     "A dataset in downloadable form." ;
        rdfs:label       "DataDownload" ;
        rdfs:subClassOf  schema:MediaObject .

schema:CriticReview  a   rdfs:Class ;
        rdfs:comment     "A [[CriticReview]] is a more specialized form of Review written or published by a source that is recognized for its reviewing activities. These can include online columns, travel and food guides, TV and radio shows, blogs and other independent Web sites. [[CriticReview]]s are typically more in-depth and professionally written. For simpler, casually written user/visitor/viewer/customer reviews, it is more appropriate to use the [[UserReview]] type. Review aggregator sites such as Metacritic already separate out the site's user reviews from selected critic reviews that originate from third-party sources." ;
        rdfs:label       "CriticReview" ;
        rdfs:subClassOf  schema:Review .

schema:RoofingContractor
        a                rdfs:Class ;
        rdfs:comment     "A roofing contractor." ;
        rdfs:label       "RoofingContractor" ;
        rdfs:subClassOf  schema:HomeAndConstructionBusiness .

schema:StatusEnumeration
        a                rdfs:Class ;
        rdfs:comment     "Lists or enumerations dealing with status types." ;
        rdfs:label       "StatusEnumeration" ;
        rdfs:subClassOf  schema:Enumeration .

schema:isFamilyFriendly
        a             rdf:Property ;
        rdfs:comment  "Indicates whether this content is family friendly." ;
        rdfs:label    "isFamilyFriendly" .

schema:workPerformed  a     rdf:Property ;
        rdfs:comment        "A work performed in some event, for example a play performed in a TheaterEvent." ;
        rdfs:label          "workPerformed" ;
        rdfs:subPropertyOf  schema:workFeatured .

schema:leaseLength  a  rdf:Property ;
        rdfs:comment  "Length of the lease for some [[Accommodation]], either particular to some [[Offer]] or in some cases intrinsic to the property." ;
        rdfs:label    "leaseLength" .

schema:repeatCount  a  rdf:Property ;
        rdfs:comment  "Defines the number of times a recurring [[Event]] will take place" ;
        rdfs:label    "repeatCount" .

schema:exceptDate  a  rdf:Property ;
        rdfs:comment  "Defines a [[Date]] or [[DateTime]] during which a scheduled [[Event]] will not take place. The property allows exceptions to\n      a [[Schedule]] to be specified. If an exception is specified as a [[DateTime]] then only the event that would have started at that specific date and time\n      should be excluded from the schedule. If an exception is specified as a [[Date]] then any event that is scheduled for that 24 hour period should be\n      excluded from the schedule. This allows a whole day to be excluded from the schedule without having to itemise every scheduled event." ;
        rdfs:label    "exceptDate" .

schema:estimatedFlightDuration
        a             rdf:Property ;
        rdfs:comment  "The estimated time the flight will take." ;
        rdfs:label    "estimatedFlightDuration" .

schema:preparation  a  rdf:Property ;
        rdfs:comment  "Typical preparation that a patient must undergo before having the procedure performed." ;
        rdfs:label    "preparation" .

schema:dropoffLocation
        a             rdf:Property ;
        rdfs:comment  "Where a rental car can be dropped off." ;
        rdfs:label    "dropoffLocation" .

schema:VoteAction  a     rdfs:Class ;
        rdfs:comment     "The act of expressing a preference from a fixed/finite/structured set of choices/options." ;
        rdfs:label       "VoteAction" ;
        rdfs:subClassOf  schema:ChooseAction .

schema:BedType  a        rdfs:Class ;
        rdfs:comment     "A type of bed. This is used for indicating the bed or beds available in an accommodation." ;
        rdfs:label       "BedType" ;
        rdfs:subClassOf  schema:QualitativeValue .

schema:cvdFacilityCounty
        a             rdf:Property ;
        rdfs:comment  "Name of the County of the NHSN facility that this data record applies to. Use [[cvdFacilityId]] to identify the facility. To provide other details, [[healthcareReportingData]] can be used on a [[Hospital]] entry." ;
        rdfs:label    "cvdFacilityCounty" .

schema:WriteAction  a    rdfs:Class ;
        rdfs:comment     "The act of authoring written creative content." ;
        rdfs:label       "WriteAction" ;
        rdfs:subClassOf  schema:CreateAction .

schema:MenuSection  a    rdfs:Class ;
        rdfs:comment     "A sub-grouping of food or drink items in a menu. E.g. courses (such as 'Dinner', 'Breakfast', etc.), specific type of dishes (such as 'Meat', 'Vegan', 'Drinks', etc.), or some other classification made by the menu provider." ;
        rdfs:label       "MenuSection" ;
        rdfs:subClassOf  schema:CreativeWork .

schema:ContactPage  a    rdfs:Class ;
        rdfs:comment     "Web page type: Contact page." ;
        rdfs:label       "ContactPage" ;
        rdfs:subClassOf  schema:WebPage .

schema:reviewCount  a  rdf:Property ;
        rdfs:comment  "The count of total number of reviews." ;
        rdfs:label    "reviewCount" .

schema:Photograph  a     rdfs:Class ;
        rdfs:comment     "A photograph." ;
        rdfs:label       "Photograph" ;
        rdfs:subClassOf  schema:CreativeWork .

schema:expectedArrivalFrom
        a             rdf:Property ;
        rdfs:comment  "The earliest date the package may arrive." ;
        rdfs:label    "expectedArrivalFrom" .

schema:recipe  a            rdf:Property ;
        rdfs:comment        "A sub property of instrument. The recipe/instructions used to perform the action." ;
        rdfs:label          "recipe" ;
        rdfs:subPropertyOf  schema:instrument .

schema:checkoutTime  a  rdf:Property ;
        rdfs:comment  "The latest someone may check out of a lodging establishment." ;
        rdfs:label    "checkoutTime" .

schema:InvestmentFund
        a                rdfs:Class ;
        rdfs:comment     "A company or fund that gathers capital from a number of investors to create a pool of money that is then re-invested into stocks, bonds and other assets." ;
        rdfs:label       "InvestmentFund" ;
        rdfs:subClassOf  schema:InvestmentOrDeposit .

schema:fuelEfficiency
        a             rdf:Property ;
        rdfs:comment  "The distance traveled per unit of fuel used; most commonly miles per gallon (mpg) or kilometers per liter (km/L).\\n\\n* Note 1: There are unfortunately no standard unit codes for miles per gallon or kilometers per liter. Use [[unitText]] to indicate the unit of measurement, e.g. mpg or km/L.\\n* Note 2: There are two ways of indicating the fuel consumption, [[fuelConsumption]] (e.g. 8 liters per 100 km) and [[fuelEfficiency]] (e.g. 30 miles per gallon). They are reciprocal.\\n* Note 3: Often, the absolute value is useful only when related to driving speed (\"at 80 km/h\") or usage pattern (\"city traffic\"). You can use [[valueReference]] to link the value for the fuel economy to another value." ;
        rdfs:label    "fuelEfficiency" .

schema:orderedItem  a  rdf:Property ;
        rdfs:comment  "The item ordered." ;
        rdfs:label    "orderedItem" .

schema:map  a         rdf:Property ;
        rdfs:comment  "A URL to a map of the place." ;
        rdfs:label    "map" .

schema:circle  a      rdf:Property ;
        rdfs:comment  "A circle is the circular region of a specified radius centered at a specified latitude and longitude. A circle is expressed as a pair followed by a radius in meters." ;
        rdfs:label    "circle" .

schema:materialExtent
        a             rdf:Property ;
        rdfs:comment  "The quantity of the materials being described or an expression of the physical space they occupy."@en ;
        rdfs:label    "materialExtent"@en .

schema:actors  a      rdf:Property ;
        rdfs:comment  "An actor, e.g. in tv, radio, movie, video games etc. Actors can be associated with individual items or with a series, episode, clip." ;
        rdfs:label    "actors" .

schema:PlayAction  a     rdfs:Class ;
        rdfs:comment     "The act of playing/exercising/training/performing for enjoyment, leisure, recreation, Competition or exercise.\\n\\nRelated actions:\\n\\n* [[ListenAction]]: Unlike ListenAction (which is under ConsumeAction), PlayAction refers to performing for an audience or at an event, rather than consuming music.\\n* [[WatchAction]]: Unlike WatchAction (which is under ConsumeAction), PlayAction refers to showing/displaying for an audience or at an event, rather than consuming visual content." ;
        rdfs:label       "PlayAction" ;
        rdfs:subClassOf  schema:Action .

schema:parents  a     rdf:Property ;
        rdfs:comment  "A parents of the person." ;
        rdfs:label    "parents" .

schema:Airline  a        rdfs:Class ;
        rdfs:comment     "An organization that provides flights for passengers." ;
        rdfs:label       "Airline" ;
        rdfs:subClassOf  schema:Organization .

schema:jobTitle  a    rdf:Property ;
        rdfs:comment  "The job title of the person (for example, Financial Manager)." ;
        rdfs:label    "jobTitle" .

schema:correctionsPolicy
        a                   rdf:Property ;
        rdfs:comment        "For an [[Organization]] (e.g. [[NewsMediaOrganization]]), a statement describing (in news media, the newsroom’s) disclosure and correction policy for errors." ;
        rdfs:label          "correctionsPolicy" ;
        rdfs:subPropertyOf  schema:publishingPrinciples .

schema:legislationPassedBy
        a                   rdf:Property ;
        rdfs:comment        "The person or organization that originally passed or made the law : typically parliament (for primary legislation) or government (for secondary legislation). This indicates the \"legal author\" of the law, as opposed to its physical author." ;
        rdfs:label          "legislationPassedBy" ;
        rdfs:subPropertyOf  schema:creator .

schema:BroadcastChannel
        a                rdfs:Class ;
        rdfs:comment     "A unique instance of a BroadcastService on a CableOrSatelliteService lineup." ;
        rdfs:label       "BroadcastChannel" ;
        rdfs:subClassOf  schema:Intangible .

schema:membershipPointsEarned
        a             rdf:Property ;
        rdfs:comment  "The number of membership points earned by the member. If necessary, the unitText can be used to express the units the points are issued in. (e.g. stars, miles, etc.)" ;
        rdfs:label    "membershipPointsEarned" .

schema:ConvenienceStore
        a                rdfs:Class ;
        rdfs:comment     "A convenience store." ;
        rdfs:label       "ConvenienceStore" ;
        rdfs:subClassOf  schema:Store .

schema:xpath  a       rdf:Property ;
        rdfs:comment  "An XPath, e.g. of a [[SpeakableSpecification]] or [[WebPageElement]]. In the latter case, multiple matches within a page can constitute a single conceptual \"Web page element\"." ;
        rdfs:label    "xpath" .

schema:CatholicChurch
        a                rdfs:Class ;
        rdfs:comment     "A Catholic church." ;
        rdfs:label       "CatholicChurch" ;
        rdfs:subClassOf  schema:Church .

schema:cookingMethod  a  rdf:Property ;
        rdfs:comment  "The method of cooking, such as Frying, Steaming, ..." ;
        rdfs:label    "cookingMethod" .

schema:executableLibraryName
        a             rdf:Property ;
        rdfs:comment  "Library file name e.g., mscorlib.dll, system.web.dll." ;
        rdfs:label    "executableLibraryName" .

schema:TrainTrip  a      rdfs:Class ;
        rdfs:comment     "A trip on a commercial train line." ;
        rdfs:label       "TrainTrip" ;
        rdfs:subClassOf  schema:Trip .

schema:BroadcastService
        a                rdfs:Class ;
        rdfs:comment     "A delivery service through which content is provided via broadcast over the air or online." ;
        rdfs:label       "BroadcastService" ;
        rdfs:subClassOf  schema:Service .

schema:numberOfPages  a  rdf:Property ;
        rdfs:comment  "The number of pages in the book." ;
        rdfs:label    "numberOfPages" .

schema:EmployeeRole  a   rdfs:Class ;
        rdfs:comment     "A subclass of OrganizationRole used to describe employee relationships." ;
        rdfs:label       "EmployeeRole" ;
        rdfs:subClassOf  schema:OrganizationRole .

schema:ImageObject  a    rdfs:Class ;
        rdfs:comment     "An image file." ;
        rdfs:label       "ImageObject" ;
        rdfs:subClassOf  schema:MediaObject .

schema:LegalService  a   rdfs:Class ;
        rdfs:comment     "A LegalService is a business that provides legally-oriented services, advice and representation, e.g. law firms.\\n\\nAs a [[LocalBusiness]] it can be described as a [[provider]] of one or more [[Service]]\\(s)." ;
        rdfs:label       "LegalService" ;
        rdfs:subClassOf  schema:LocalBusiness .

schema:UserCheckins  a   rdfs:Class ;
        rdfs:comment     "UserInteraction and its subtypes is an old way of talking about users interacting with pages. It is generally better to use [[Action]]-based vocabulary, alongside types such as [[Comment]]." ;
        rdfs:label       "UserCheckins" ;
        rdfs:subClassOf  schema:UserInteraction .

schema:bccRecipient  a      rdf:Property ;
        rdfs:comment        "A sub property of recipient. The recipient blind copied on a message." ;
        rdfs:label          "bccRecipient" ;
        rdfs:subPropertyOf  schema:recipient .

schema:AchieveAction  a  rdfs:Class ;
        rdfs:comment     "The act of accomplishing something via previous efforts. It is an instantaneous action rather than an ongoing process." ;
        rdfs:label       "AchieveAction" ;
        rdfs:subClassOf  schema:Action .

schema:collection  a        rdf:Property ;
        rdfs:comment        "A sub property of object. The collection target of the action." ;
        rdfs:label          "collection" ;
        rdfs:subPropertyOf  schema:object .

schema:occupancy  a   rdf:Property ;
        rdfs:comment  "The allowed total occupancy for the accommodation in persons (including infants etc). For individual accommodations, this is not necessarily the legal maximum but defines the permitted usage as per the contractual agreement (e.g. a double room used by a single person).\nTypical unit code(s): C62 for person" ;
        rdfs:label    "occupancy" .

schema:ReservationPackage
        a                rdfs:Class ;
        rdfs:comment     "A group of multiple reservations with common values for all sub-reservations." ;
        rdfs:label       "ReservationPackage" ;
        rdfs:subClassOf  schema:Reservation .

schema:faxNumber  a   rdf:Property ;
        rdfs:comment  "The fax number." ;
        rdfs:label    "faxNumber" .

schema:CheckAction  a    rdfs:Class ;
        rdfs:comment     "An agent inspects, determines, investigates, inquires, or examines an object's accuracy, quality, condition, or state." ;
        rdfs:label       "CheckAction" ;
        rdfs:subClassOf  schema:FindAction .

schema:cvdNumTotBeds  a  rdf:Property ;
        rdfs:comment  "numtotbeds - ALL HOSPITAL BEDS: Total number of all Inpatient and outpatient beds, including all staffed,ICU, licensed, and overflow (surge) beds used for inpatients or outpatients." ;
        rdfs:label    "cvdNumTotBeds" .

schema:previousItem  a  rdf:Property ;
        rdfs:comment  "A link to the ListItem that preceeds the current one." ;
        rdfs:label    "previousItem" .

schema:transmissionMethod
        a             rdf:Property ;
        rdfs:comment  "How the disease spreads, either as a route or vector, for example 'direct contact', 'Aedes aegypti', etc." ;
        rdfs:label    "transmissionMethod" .

schema:track  a       rdf:Property ;
        rdfs:comment  "A music recording (track)&#x2014;usually a single song. If an ItemList is given, the list should contain items of type MusicRecording." ;
        rdfs:label    "track" .

schema:MusicStore  a     rdfs:Class ;
        rdfs:comment     "A music store." ;
        rdfs:label       "MusicStore" ;
        rdfs:subClassOf  schema:Store .

schema:requiredCollateral
        a             rdf:Property ;
        rdfs:comment  "Assets required to secure loan or credit repayments. It may take form of third party pledge, goods, financial instruments (cash, securities, etc.)" ;
        rdfs:label    "requiredCollateral" .

schema:Casino  a         rdfs:Class ;
        rdfs:comment     "A casino." ;
        rdfs:label       "Casino" ;
        rdfs:subClassOf  schema:EntertainmentBusiness .

schema:Flight  a         rdfs:Class ;
        rdfs:comment     "An airline flight." ;
        rdfs:label       "Flight" ;
        rdfs:subClassOf  schema:Trip .

schema:Grant  a          rdfs:Class ;
        rdfs:comment     "A grant, typically financial or otherwise quantifiable, of resources. Typically a [[funder]] sponsors some [[MonetaryAmount]] to an [[Organization]] or [[Person]],\n    sometimes not necessarily via a dedicated or long-lived [[Project]], resulting in one or more outputs, or [[fundedItem]]s. For financial sponsorship, indicate the [[funder]] of a [[MonetaryGrant]]. For non-financial support, indicate [[sponsor]] of [[Grant]]s of resources (e.g. office space).\n\nGrants support  activities directed towards some agreed collective goals, often but not always organized as [[Project]]s. Long-lived projects are sometimes sponsored by a variety of grants over time, but it is also common for a project to be associated with a single grant.\n\nThe amount of a [[Grant]] is represented using [[amount]] as a [[MonetaryAmount]].\n    " ;
        rdfs:label       "Grant" ;
        rdfs:subClassOf  schema:Intangible .

schema:warrantyScope  a  rdf:Property ;
        rdfs:comment  "The scope of the warranty promise." ;
        rdfs:label    "warrantyScope" .

schema:SendAction  a     rdfs:Class ;
        rdfs:comment     "The act of physically/electronically dispatching an object for transfer from an origin to a destination.Related actions:\\n\\n* [[ReceiveAction]]: The reciprocal of SendAction.\\n* [[GiveAction]]: Unlike GiveAction, SendAction does not imply the transfer of ownership (e.g. I can send you my laptop, but I'm not necessarily giving it to you)." ;
        rdfs:label       "SendAction" ;
        rdfs:subClassOf  schema:TransferAction .

schema:ProfilePage  a    rdfs:Class ;
        rdfs:comment     "Web page type: Profile page." ;
        rdfs:label       "ProfilePage" ;
        rdfs:subClassOf  schema:WebPage .

schema:evidenceLevel  a  rdf:Property ;
        rdfs:comment  "Strength of evidence of the data used to formulate the guideline (enumerated)." ;
        rdfs:label    "evidenceLevel" .

schema:device  a      rdf:Property ;
        rdfs:comment  "Device required to run the application. Used in cases where a specific make/model is required to run the application." ;
        rdfs:label    "device" .

schema:subEvents  a   rdf:Property ;
        rdfs:comment  "Events that are a part of this event. For example, a conference event includes many presentations, each subEvents of the conference." ;
        rdfs:label    "subEvents" .

schema:schoolClosuresInfo
        a             rdf:Property ;
        rdfs:comment  "Information about school closures." ;
        rdfs:label    "schoolClosuresInfo" .

schema:utterances  a  rdf:Property ;
        rdfs:comment  "Text of an utterances (spoken words, lyrics etc.) that occurs at a certain section of a media object, represented as a [[HyperTocEntry]]." ;
        rdfs:label    "utterances" .

schema:publishedBy  a  rdf:Property ;
        rdfs:comment  "An agent associated with the publication event." ;
        rdfs:label    "publishedBy" .

schema:usedToDiagnose
        a             rdf:Property ;
        rdfs:comment  "A condition the test is used to diagnose." ;
        rdfs:label    "usedToDiagnose" .

schema:relatedAnatomy
        a             rdf:Property ;
        rdfs:comment  "Anatomical systems or structures that relate to the superficial anatomy." ;
        rdfs:label    "relatedAnatomy" .

schema:siblings  a    rdf:Property ;
        rdfs:comment  "A sibling of the person." ;
        rdfs:label    "siblings" .

schema:trackingNumber
        a             rdf:Property ;
        rdfs:comment  "Shipper tracking number." ;
        rdfs:label    "trackingNumber" .

schema:elevation  a   rdf:Property ;
        rdfs:comment  "The elevation of a location ([WGS 84](https://en.wikipedia.org/wiki/World_Geodetic_System)). Values may be of the form 'NUMBER UNIT_OF_MEASUREMENT' (e.g., '1,000 m', '3,200 ft') while numbers alone should be assumed to be a value in meters." ;
        rdfs:label    "elevation" .

schema:timeOfDay  a   rdf:Property ;
        rdfs:comment  "The time of day the program normally runs. For example, \"evenings\"." ;
        rdfs:label    "timeOfDay" .

schema:datePublished  a  rdf:Property ;
        rdfs:comment  "Date of first broadcast/publication." ;
        rdfs:label    "datePublished" .

schema:interactingDrug
        a             rdf:Property ;
        rdfs:comment  "Another drug that is known to interact with this drug in a way that impacts the effect of this drug or causes a risk to the patient. Note: disease interactions are typically captured as contraindications." ;
        rdfs:label    "interactingDrug" .

schema:gender  a      rdf:Property ;
        rdfs:comment  "Gender of something, typically a [[Person]], but possibly also fictional characters, animals, etc. While http://schema.org/Male and http://schema.org/Female may be used, text strings are also acceptable for people who do not identify as a binary gender. The [[gender]] property can also be used in an extended sense to cover e.g. the gender of sports teams. As with the gender of individuals, we do not try to enumerate all possibilities. A mixed-gender [[SportsTeam]] can be indicated with a text value of \"Mixed\"." ;
        rdfs:label    "gender" .

schema:offers  a      rdf:Property ;
        rdfs:comment  "An offer to provide this item&#x2014;for example, an offer to sell a product, rent the DVD of a movie, perform a service, or give away tickets to an event. Use [[businessFunction]] to indicate the kind of transaction offered, i.e. sell, lease, etc. This property can also be used to describe a [[Demand]]. While this property is listed as expected on a number of common types, it can be used in others. In that case, using a second type, such as Product or a subtype of Product, can clarify the nature of the offer.\n      " ;
        rdfs:label    "offers" .

schema:Bakery  a         rdfs:Class ;
        rdfs:comment     "A bakery." ;
        rdfs:label       "Bakery" ;
        rdfs:subClassOf  schema:FoodEstablishment .

schema:healthCondition
        a             rdf:Property ;
        rdfs:comment  "Specifying the health condition(s) of a patient, medical study, or other target audience." ;
        rdfs:label    "healthCondition" .

schema:isPlanForApartment
        a             rdf:Property ;
        rdfs:comment  "Indicates some accommodation that this floor plan describes." ;
        rdfs:label    "isPlanForApartment" .

schema:ExerciseGym  a    rdfs:Class ;
        rdfs:comment     "A gym." ;
        rdfs:label       "ExerciseGym" ;
        rdfs:subClassOf  schema:SportsActivityLocation .

schema:WebAPI  a         rdfs:Class ;
        rdfs:comment     "An application programming interface accessible over Web/Internet technologies." ;
        rdfs:label       "WebAPI" ;
        rdfs:subClassOf  schema:Service .

schema:genre  a       rdf:Property ;
        rdfs:comment  "Genre of the creative work, broadcast channel or group." ;
        rdfs:label    "genre" .

schema:Volcano  a        rdfs:Class ;
        rdfs:comment     "A volcano, like Fuji san." ;
        rdfs:label       "Volcano" ;
        rdfs:subClassOf  schema:Landform .

schema:geoTouches  a  rdf:Property ;
        rdfs:comment  "Represents spatial relations in which two geometries (or the places they represent) touch: they have at least one boundary point in common, but no interior points.\" (a symmetric relationship, as defined in [DE-9IM](https://en.wikipedia.org/wiki/DE-9IM) )" ;
        rdfs:label    "geoTouches" .

schema:MathSolver  a     rdfs:Class ;
        rdfs:comment     "A math solver which is capable of solving a subset of mathematical problems." ;
        rdfs:label       "MathSolver" ;
        rdfs:subClassOf  schema:CreativeWork .

schema:SizeGroupEnumeration
        a                rdfs:Class ;
        rdfs:comment     "Enumerates common size groups for various product categories." ;
        rdfs:label       "SizeGroupEnumeration" ;
        rdfs:subClassOf  schema:Enumeration .

schema:BroadcastFrequencySpecification
        a                rdfs:Class ;
        rdfs:comment     "The frequency in MHz and the modulation used for a particular BroadcastService." ;
        rdfs:label       "BroadcastFrequencySpecification" ;
        rdfs:subClassOf  schema:Intangible .

schema:Resort  a         rdfs:Class ;
        rdfs:comment     "A resort is a place used for relaxation or recreation, attracting visitors for holidays or vacations. Resorts are places, towns or sometimes commercial establishment operated by a single company (Source: Wikipedia, the free encyclopedia, see <a href=\"http://en.wikipedia.org/wiki/Resort\">http://en.wikipedia.org/wiki/Resort</a>).\n<br /><br />\nSee also the <a href=\"/docs/hotels.html\">dedicated document on the use of schema.org for marking up hotels and other forms of accommodations</a>.\n    " ;
        rdfs:label       "Resort" ;
        rdfs:subClassOf  schema:LodgingBusiness .

schema:ingredients  a       rdf:Property ;
        rdfs:comment        "A single ingredient used in the recipe, e.g. sugar, flour or garlic." ;
        rdfs:label          "ingredients" ;
        rdfs:subPropertyOf  schema:supply .

schema:maximumVirtualAttendeeCapacity
        a             rdf:Property ;
        rdfs:comment  "The maximum physical attendee capacity of an [[Event]] whose [[eventAttendanceMode]] is [[OnlineEventAttendanceMode]] (or the online aspects, in the case of a [[MixedEventAttendanceMode]]). " ;
        rdfs:label    "maximumVirtualAttendeeCapacity" .

schema:loanRepaymentForm
        a             rdf:Property ;
        rdfs:comment  "A form of paying back money previously borrowed from a lender. Repayment usually takes the form of periodic payments that normally include part principal plus interest in each payment." ;
        rdfs:label    "loanRepaymentForm" .

schema:MedicalTest  a    rdfs:Class ;
        rdfs:comment     "Any medical test, typically performed for diagnostic purposes." ;
        rdfs:label       "MedicalTest" ;
        rdfs:subClassOf  schema:MedicalEntity .

schema:PoliceStation  a  rdfs:Class ;
        rdfs:comment     "A police station." ;
        rdfs:label       "PoliceStation" ;
        rdfs:subClassOf  schema:CivicStructure , schema:EmergencyService .

schema:VisualArtsEvent
        a                rdfs:Class ;
        rdfs:comment     "Event type: Visual arts event." ;
        rdfs:label       "VisualArtsEvent" ;
        rdfs:subClassOf  schema:Event .

schema:currenciesAccepted
        a             rdf:Property ;
        rdfs:comment  "The currency accepted.\\n\\nUse standard formats: [ISO 4217 currency format](http://en.wikipedia.org/wiki/ISO_4217) e.g. \"USD\"; [Ticker symbol](https://en.wikipedia.org/wiki/List_of_cryptocurrencies) for cryptocurrencies e.g. \"BTC\"; well known names for [Local Exchange Tradings Systems](https://en.wikipedia.org/wiki/Local_exchange_trading_system) (LETS) and other currency types e.g. \"Ithaca HOUR\"." ;
        rdfs:label    "currenciesAccepted" .

schema:healthPlanCostSharing
        a             rdf:Property ;
        rdfs:comment  "Whether The costs to the patient for services under this network or formulary." ;
        rdfs:label    "healthPlanCostSharing" .

schema:DefinedTerm  a    rdfs:Class ;
        rdfs:comment     "A word, name, acronym, phrase, etc. with a formal definition. Often used in the context of category or subject classification, glossaries or dictionaries, product or creative work types, etc. Use the name property for the term being defined, use termCode if the term has an alpha-numeric code allocated, use description to provide the definition of the term." ;
        rdfs:label       "DefinedTerm" ;
        rdfs:subClassOf  schema:Intangible .

schema:administrationRoute
        a             rdf:Property ;
        rdfs:comment  "A route by which this drug may be administered, e.g. 'oral'." ;
        rdfs:label    "administrationRoute" .

schema:fileSize  a    rdf:Property ;
        rdfs:comment  "Size of the application / package (e.g. 18MB). In the absence of a unit (MB, KB etc.), KB will be assumed." ;
        rdfs:label    "fileSize" .

schema:applicationCategory
        a             rdf:Property ;
        rdfs:comment  "Type of software application, e.g. 'Game, Multimedia'." ;
        rdfs:label    "applicationCategory" .

schema:ConsumeAction  a  rdfs:Class ;
        rdfs:comment     "The act of ingesting information/resources/food." ;
        rdfs:label       "ConsumeAction" ;
        rdfs:subClassOf  schema:Action .

schema:paymentAccepted
        a             rdf:Property ;
        rdfs:comment  "Cash, Credit Card, Cryptocurrency, Local Exchange Tradings System, etc." ;
        rdfs:label    "paymentAccepted" .

schema:CompleteDataFeed
        a                rdfs:Class ;
        rdfs:comment     "A [[CompleteDataFeed]] is a [[DataFeed]] whose standard representation includes content for every item currently in the feed.\n\nThis is the equivalent of Atom's element as defined in Feed Paging and Archiving [RFC 5005](https://tools.ietf.org/html/rfc5005), For example (and as defined for Atom), when using data from a feed that represents a collection of items that varies over time (e.g. \"Top Twenty Records\") there is no need to have newer entries mixed in alongside older, obsolete entries. By marking this feed as a CompleteDataFeed, old entries can be safely discarded when the feed is refreshed, since we can assume the feed has provided descriptions for all current items." ;
        rdfs:label       "CompleteDataFeed" ;
        rdfs:subClassOf  schema:DataFeed .

schema:TouristAttraction
        a                rdfs:Class ;
        rdfs:comment     "A tourist attraction.  In principle any Thing can be a [[TouristAttraction]], from a [[Mountain]] and [[LandmarksOrHistoricalBuildings]] to a [[LocalBusiness]].  This Type can be used on its own to describe a general [[TouristAttraction]], or be used as an [[additionalType]] to add tourist attraction properties to any other type.  (See examples below)" ;
        rdfs:label       "TouristAttraction" ;
        rdfs:subClassOf  schema:Place .

schema:AudioObject  a    rdfs:Class ;
        rdfs:comment     "An audio file." ;
        rdfs:label       "AudioObject" ;
        rdfs:subClassOf  schema:MediaObject .

schema:geographicArea
        a             rdf:Property ;
        rdfs:comment  "The geographic area associated with the audience." ;
        rdfs:label    "geographicArea" .

schema:BusinessEvent  a  rdfs:Class ;
        rdfs:comment     "Event type: Business event." ;
        rdfs:label       "BusinessEvent" ;
        rdfs:subClassOf  schema:Event .

schema:noBylinesPolicy
        a                   rdf:Property ;
        rdfs:comment        "For a [[NewsMediaOrganization]] or other news-related [[Organization]], a statement explaining when authors of articles are not named in bylines." ;
        rdfs:label          "noBylinesPolicy" ;
        rdfs:subPropertyOf  schema:publishingPrinciples .

schema:actionAccessibilityRequirement
        a             rdf:Property ;
        rdfs:comment  "A set of requirements that a must be fulfilled in order to perform an Action. If more than one value is specied, fulfilling one set of requirements will allow the Action to be performed." ;
        rdfs:label    "actionAccessibilityRequirement" .

schema:customer  a    rdf:Property ;
        rdfs:comment  "Party placing the order or paying the invoice." ;
        rdfs:label    "customer" .

schema:awayTeam  a          rdf:Property ;
        rdfs:comment        "The away team in a sports event." ;
        rdfs:label          "awayTeam" ;
        rdfs:subPropertyOf  schema:competitor .

schema:Otolaryngologic
        a                rdfs:Class ;
        rdfs:comment     "A specific branch of medical science that is concerned with the ear, nose and throat and their respective disease states." ;
        rdfs:label       "Otolaryngologic" ;
        rdfs:subClassOf  schema:MedicalBusiness .

schema:significantLink
        a             rdf:Property ;
        rdfs:comment  "One of the more significant URLs on the page. Typically, these are the non-navigation links that are clicked on the most." ;
        rdfs:label    "significantLink" .

schema:CoverArt  a       rdfs:Class ;
        rdfs:comment     "The artwork on the outer surface of a CreativeWork." ;
        rdfs:label       "CoverArt" ;
        rdfs:subClassOf  schema:VisualArtwork .

schema:areaServed  a  rdf:Property ;
        rdfs:comment  "The geographic area where a service or offered item is provided." ;
        rdfs:label    "areaServed" .

schema:serialNumber  a      rdf:Property ;
        rdfs:comment        "The serial number or any alphanumeric identifier of a particular product. When attached to an offer, it is a shortcut for the serial number of the product included in the offer." ;
        rdfs:label          "serialNumber" ;
        rdfs:subPropertyOf  schema:identifier .

schema:specialOpeningHoursSpecification
        a             rdf:Property ;
        rdfs:comment  "The special opening hours of a certain place.\\n\\nUse this to explicitly override general opening hours brought in scope by [[openingHoursSpecification]] or [[openingHours]].\n      " ;
        rdfs:label    "specialOpeningHoursSpecification" .

schema:Zoo  a            rdfs:Class ;
        rdfs:comment     "A zoo." ;
        rdfs:label       "Zoo" ;
        rdfs:subClassOf  schema:CivicStructure .

schema:episode  a           rdf:Property ;
        rdfs:comment        "An episode of a tv, radio or game media within a series or season." ;
        rdfs:label          "episode" ;
        rdfs:subPropertyOf  schema:hasPart .

schema:jurisdiction  a  rdf:Property ;
        rdfs:comment  "Indicates a legal jurisdiction, e.g. of some legislation, or where some government service is based." ;
        rdfs:label    "jurisdiction" .

schema:MedicalClinic  a  rdfs:Class ;
        rdfs:comment     "A facility, often associated with a hospital or medical school, that is devoted to the specific diagnosis and/or healthcare. Previously limited to outpatients but with evolution it may be open to inpatients as well." ;
        rdfs:label       "MedicalClinic" ;
        rdfs:subClassOf  schema:MedicalBusiness , schema:MedicalOrganization .

schema:CategoryCode  a   rdfs:Class ;
        rdfs:comment     "A Category Code." ;
        rdfs:label       "CategoryCode" ;
        rdfs:subClassOf  schema:DefinedTerm .

schema:DataFeedItem  a   rdfs:Class ;
        rdfs:comment     "A single item within a larger data feed." ;
        rdfs:label       "DataFeedItem" ;
        rdfs:subClassOf  schema:Intangible .

schema:warrantyPromise
        a             rdf:Property ;
        rdfs:comment  "The warranty promise(s) included in the offer." ;
        rdfs:label    "warrantyPromise" .

schema:PodcastEpisode
        a                rdfs:Class ;
        rdfs:comment     "A single episode of a podcast series." ;
        rdfs:label       "PodcastEpisode" ;
        rdfs:subClassOf  schema:Episode .

schema:sodiumContent  a  rdf:Property ;
        rdfs:comment  "The number of milligrams of sodium." ;
        rdfs:label    "sodiumContent" .

schema:bookingTime  a  rdf:Property ;
        rdfs:comment  "The date and time the reservation was booked." ;
        rdfs:label    "bookingTime" .

schema:hasHealthAspect
        a             rdf:Property ;
        rdfs:comment  "Indicates the aspect or aspects specifically addressed in some [[HealthTopicContent]]. For example, that the content is an overview, or that it talks about treatment, self-care, treatments or their side-effects." ;
        rdfs:label    "hasHealthAspect" .

schema:gameItem  a    rdf:Property ;
        rdfs:comment  "An item is an object within the game world that can be collected by a player or, occasionally, a non-player character." ;
        rdfs:label    "gameItem" .

schema:supersededBy  a  rdf:Property ;
        rdfs:comment  "Relates a term (i.e. a property, class or enumeration) to one that supersedes it." ;
        rdfs:label    "supersededBy" .

schema:printColumn  a  rdf:Property ;
        rdfs:comment  "The number of the column in which the NewsArticle appears in the print edition." ;
        rdfs:label    "printColumn" .

schema:numberOfPlayers
        a             rdf:Property ;
        rdfs:comment  "Indicate how many people can play this game (minimum, maximum, or range)." ;
        rdfs:label    "numberOfPlayers" .

schema:comment  a     rdf:Property ;
        rdfs:comment  "Comments, typically from users." ;
        rdfs:label    "comment" .

schema:Place  a          rdfs:Class ;
        rdfs:comment     "Entities that have a somewhat fixed, physical extension." ;
        rdfs:label       "Place" ;
        rdfs:subClassOf  schema:Thing .

schema:letterer  a    rdf:Property ;
        rdfs:comment  "The individual who adds lettering, including speech balloons and sound effects, to artwork." ;
        rdfs:label    "letterer" .

schema:contactPoint  a  rdf:Property ;
        rdfs:comment  "A contact point for a person or organization." ;
        rdfs:label    "contactPoint" .

schema:broker  a      rdf:Property ;
        rdfs:comment  "An entity that arranges for an exchange between a buyer and a seller.  In most cases a broker never acquires or releases ownership of a product or service involved in an exchange.  If it is not clear whether an entity is a broker, seller, or buyer, the latter two terms are preferred." ;
        rdfs:label    "broker" .

schema:MedicalRiskCalculator
        a                rdfs:Class ;
        rdfs:comment     "A complex mathematical calculation requiring an online calculator, used to assess prognosis. Note: use the url property of Thing to record any URLs for online calculators." ;
        rdfs:label       "MedicalRiskCalculator" ;
        rdfs:subClassOf  schema:MedicalRiskEstimator .

schema:appliesToDeliveryMethod
        a             rdf:Property ;
        rdfs:comment  "The delivery method(s) to which the delivery charge or payment charge specification applies." ;
        rdfs:label    "appliesToDeliveryMethod" .

schema:suggestedMeasurement
        a             rdf:Property ;
        rdfs:comment  "A suggested range of body measurements for the intended audience or person, for example inseam between 32 and 34 inches or height between 170 and 190 cm. Typically found on a size chart for wearable products." ;
        rdfs:label    "suggestedMeasurement" .

schema:UserDownloads  a  rdfs:Class ;
        rdfs:comment     "UserInteraction and its subtypes is an old way of talking about users interacting with pages. It is generally better to use [[Action]]-based vocabulary, alongside types such as [[Comment]]." ;
        rdfs:label       "UserDownloads" ;
        rdfs:subClassOf  schema:UserInteraction .

schema:dateSent  a    rdf:Property ;
        rdfs:comment  "The date/time at which the message was sent." ;
        rdfs:label    "dateSent" .

schema:SuperficialAnatomy
        a                rdfs:Class ;
        rdfs:comment     "Anatomical features that can be observed by sight (without dissection), including the form and proportions of the human body as well as surface landmarks that correspond to deeper subcutaneous structures. Superficial anatomy plays an important role in sports medicine, phlebotomy, and other medical specialties as underlying anatomical structures can be identified through surface palpation. For example, during back surgery, superficial anatomy can be used to palpate and count vertebrae to find the site of incision. Or in phlebotomy, superficial anatomy can be used to locate an underlying vein; for example, the median cubital vein can be located by palpating the borders of the cubital fossa (such as the epicondyles of the humerus) and then looking for the superficial signs of the vein, such as size, prominence, ability to refill after depression, and feel of surrounding tissue support. As another example, in a subluxation (dislocation) of the glenohumeral joint, the bony structure becomes pronounced with the deltoid muscle failing to cover the glenohumeral joint allowing the edges of the scapula to be superficially visible. Here, the superficial anatomy is the visible edges of the scapula, implying the underlying dislocation of the joint (the related anatomical structure)." ;
        rdfs:label       "SuperficialAnatomy" ;
        rdfs:subClassOf  schema:MedicalEntity .

schema:supplyTo  a    rdf:Property ;
        rdfs:comment  "The area to which the artery supplies blood." ;
        rdfs:label    "supplyTo" .

schema:game  a        rdf:Property ;
        rdfs:comment  "Video game which is played on this server." ;
        rdfs:label    "game" .

schema:MotorcycleDealer
        a                rdfs:Class ;
        rdfs:comment     "A motorcycle dealer." ;
        rdfs:label       "MotorcycleDealer" ;
        rdfs:subClassOf  schema:AutomotiveBusiness .

schema:providerMobility
        a             rdf:Property ;
        rdfs:comment  "Indicates the mobility of a provided service (e.g. 'static', 'dynamic')." ;
        rdfs:label    "providerMobility" .

schema:boardingPolicy
        a             rdf:Property ;
        rdfs:comment  "The type of boarding policy used by the airline (e.g. zone-based or group-based)." ;
        rdfs:label    "boardingPolicy" .

schema:variableMeasured
        a             rdf:Property ;
        rdfs:comment  "The variableMeasured property can indicate (repeated as necessary) the  variables that are measured in some dataset, either described as text or as pairs of identifier and description using PropertyValue." ;
        rdfs:label    "variableMeasured" .

schema:DonateAction  a   rdfs:Class ;
        rdfs:comment     "The act of providing goods, services, or money without compensation, often for philanthropic reasons." ;
        rdfs:label       "DonateAction" ;
        rdfs:subClassOf  schema:TradeAction .

schema:ProductCollection
        a                rdfs:Class ;
        rdfs:comment     "A set of products (either [[ProductGroup]]s or specific variants) that are listed together e.g. in an [[Offer]]." ;
        rdfs:label       "ProductCollection" ;
        rdfs:subClassOf  schema:Product , schema:Collection .

schema:ActionAccessSpecification
        a                rdfs:Class ;
        rdfs:comment     "A set of requirements that a must be fulfilled in order to perform an Action." ;
        rdfs:label       "ActionAccessSpecification" ;
        rdfs:subClassOf  schema:Intangible .

schema:labelDetails  a  rdf:Property ;
        rdfs:comment  "Link to the drug's label details." ;
        rdfs:label    "labelDetails" .

schema:tocContinuation
        a             rdf:Property ;
        rdfs:comment  "A [[HyperTocEntry]] can have a [[tocContinuation]] indicated, which is another [[HyperTocEntry]] that would be the default next item to play or render." ;
        rdfs:label    "tocContinuation" .

schema:OrganizationRole
        a                rdfs:Class ;
        rdfs:comment     "A subclass of Role used to describe roles within organizations." ;
        rdfs:label       "OrganizationRole" ;
        rdfs:subClassOf  schema:Role .

schema:BodyMeasurementTypeEnumeration
        a                rdfs:Class ;
        rdfs:comment     "Enumerates types (or dimensions) of a person's body measurements, for example for fitting of clothes." ;
        rdfs:label       "BodyMeasurementTypeEnumeration" ;
        rdfs:subClassOf  schema:MeasurementTypeEnumeration .

schema:SkiResort  a      rdfs:Class ;
        rdfs:comment     "A ski resort." ;
        rdfs:label       "SkiResort" ;
        rdfs:subClassOf  schema:SportsActivityLocation , schema:Resort .

schema:itinerary  a   rdf:Property ;
        rdfs:comment  "Destination(s) ( [[Place]] ) that make up a trip. For a trip where destination order is important use [[ItemList]] to specify that order (see examples)." ;
        rdfs:label    "itinerary" .

void:Dataset  a  rdfs:Class .

schema:interactionService
        a             rdf:Property ;
        rdfs:comment  "The WebSite or SoftwareApplication where the interactions took place." ;
        rdfs:label    "interactionService" .

schema:floorSize  a   rdf:Property ;
        rdfs:comment  "The size of the accommodation, e.g. in square meter or squarefoot.\nTypical unit code(s): MTK for square meter, FTK for square foot, or YDK for square yard " ;
        rdfs:label    "floorSize" .

schema:warning  a     rdf:Property ;
        rdfs:comment  "Any FDA or other warnings about the drug (text or URL)." ;
        rdfs:label    "warning" .

schema:Quiz  a           rdfs:Class ;
        rdfs:comment     "Quiz: A test of knowledge, skills and abilities." ;
        rdfs:label       "Quiz" ;
        rdfs:subClassOf  schema:LearningResource .

schema:DrugClass  a      rdfs:Class ;
        rdfs:comment     "A class of medical drugs, e.g., statins. Classes can represent general pharmacological class, common mechanisms of action, common physiological effects, etc." ;
        rdfs:label       "DrugClass" ;
        rdfs:subClassOf  schema:MedicalEntity .

schema:includedComposition
        a             rdf:Property ;
        rdfs:comment  "Smaller compositions included in this work (e.g. a movement in a symphony)." ;
        rdfs:label    "includedComposition" .

schema:costCategory  a  rdf:Property ;
        rdfs:comment  "The category of cost, such as wholesale, retail, reimbursement cap, etc." ;
        rdfs:label    "costCategory" .

schema:WPHeader  a       rdfs:Class ;
        rdfs:comment     "The header section of the page." ;
        rdfs:label       "WPHeader" ;
        rdfs:subClassOf  schema:WebPageElement .

schema:EmployerReview
        a                rdfs:Class ;
        rdfs:comment     "An [[EmployerReview]] is a review of an [[Organization]] regarding its role as an employer, written by a current or former employee of that organization." ;
        rdfs:label       "EmployerReview" ;
        rdfs:subClassOf  schema:Review .

schema:backstory  a   rdf:Property ;
        rdfs:comment  "For an [[Article]], typically a [[NewsArticle]], the backstory property provides a textual summary giving a brief explanation of why and how an article was created. In a journalistic setting this could include information about reporting process, methods, interviews, data sources, etc." ;
        rdfs:label    "backstory" .

schema:reservationId  a  rdf:Property ;
        rdfs:comment  "A unique identifier for the reservation." ;
        rdfs:label    "reservationId" .

schema:followee  a          rdf:Property ;
        rdfs:comment        "A sub property of object. The person or organization being followed." ;
        rdfs:label          "followee" ;
        rdfs:subPropertyOf  schema:object .

schema:copyrightHolder
        a             rdf:Property ;
        rdfs:comment  "The party holding the legal copyright to the CreativeWork." ;
        rdfs:label    "copyrightHolder" .

schema:targetCollection
        a                   rdf:Property ;
        rdfs:comment        "A sub property of object. The collection target of the action." ;
        rdfs:label          "targetCollection" ;
        rdfs:subPropertyOf  schema:object .

schema:WorkersUnion  a   rdfs:Class ;
        rdfs:comment     "A Workers Union (also known as a Labor Union, Labour Union, or Trade Union) is an organization that promotes the interests of its worker members by collectively bargaining with management, organizing, and political lobbying." ;
        rdfs:label       "WorkersUnion" ;
        rdfs:subClassOf  schema:Organization .

schema:toLocation  a        rdf:Property ;
        rdfs:comment        "A sub property of location. The final location of the object or the agent after the action." ;
        rdfs:label          "toLocation" ;
        rdfs:subPropertyOf  schema:location .

schema:ItemPage  a       rdfs:Class ;
        rdfs:comment     "A page devoted to a single item, such as a particular product or hotel." ;
        rdfs:label       "ItemPage" ;
        rdfs:subClassOf  schema:WebPage .

schema:naics  a       rdf:Property ;
        rdfs:comment  "The North American Industry Classification System (NAICS) code for a particular organization or business person." ;
        rdfs:label    "naics" .

schema:partOfSystem  a  rdf:Property ;
        rdfs:comment  "The anatomical or organ system that this structure is part of." ;
        rdfs:label    "partOfSystem" .

schema:Notary  a         rdfs:Class ;
        rdfs:comment     "A notary." ;
        rdfs:label       "Notary" ;
        rdfs:subClassOf  schema:LegalService .

schema:birthPlace  a  rdf:Property ;
        rdfs:comment  "The place where the person was born." ;
        rdfs:label    "birthPlace" .

schema:returnFees  a  rdf:Property ;
        rdfs:comment  "Indicates (via enumerated options) the return fees policy for a MerchantReturnPolicy" ;
        rdfs:label    "returnFees" .

schema:estimatesRiskOf
        a             rdf:Property ;
        rdfs:comment  "The condition, complication, or symptom whose risk is being estimated." ;
        rdfs:label    "estimatesRiskOf" .

schema:depth  a       rdf:Property ;
        rdfs:comment  "The depth of the item." ;
        rdfs:label    "depth" .

schema:numAdults  a   rdf:Property ;
        rdfs:comment  "The number of adults staying in the unit." ;
        rdfs:label    "numAdults" .

schema:strengthValue  a  rdf:Property ;
        rdfs:comment  "The value of an active ingredient's strength, e.g. 325." ;
        rdfs:label    "strengthValue" .

schema:hasMap  a      rdf:Property ;
        rdfs:comment  "A URL to a map of the place." ;
        rdfs:label    "hasMap" .

schema:ratingExplanation
        a             rdf:Property ;
        rdfs:comment  "A short explanation (e.g. one to two sentences) providing background context and other information that led to the conclusion expressed in the rating. This is particularly applicable to ratings associated with \"fact check\" markup using [[ClaimReview]]." ;
        rdfs:label    "ratingExplanation" .

schema:eligibleRegion
        a                   rdf:Property ;
        rdfs:comment        "The ISO 3166-1 (ISO 3166-1 alpha-2) or ISO 3166-2 code, the place, or the GeoShape for the geo-political region(s) for which the offer or delivery charge specification is valid.\\n\\nSee also [[ineligibleRegion]].\n    " ;
        rdfs:label          "eligibleRegion" ;
        rdfs:subPropertyOf  schema:areaServed .

schema:dietFeatures  a  rdf:Property ;
        rdfs:comment  "Nutritional information specific to the dietary plan. May include dietary recommendations on what foods to avoid, what foods to consume, and specific alterations/deviations from the USDA or other regulatory body's approved dietary guidelines." ;
        rdfs:label    "dietFeatures" .

schema:courseCode  a  rdf:Property ;
        rdfs:comment  "The identifier for the [[Course]] used by the course [[provider]] (e.g. CS101 or 6.001)." ;
        rdfs:label    "courseCode" .

schema:cvdNumC19OverflowPats
        a             rdf:Property ;
        rdfs:comment  "numc19overflowpats - ED/OVERFLOW: Patients with suspected or confirmed COVID-19 who are in the ED or any overflow location awaiting an inpatient bed." ;
        rdfs:label    "cvdNumC19OverflowPats" .

schema:rxcui  a       rdf:Property ;
        rdfs:comment  "The RxCUI drug identifier from RXNORM." ;
        rdfs:label    "rxcui" .

schema:Seat  a           rdfs:Class ;
        rdfs:comment     "Used to describe a seat, such as a reserved seat in an event reservation." ;
        rdfs:label       "Seat" ;
        rdfs:subClassOf  schema:Intangible .

schema:serviceUrl  a  rdf:Property ;
        rdfs:comment  "The website to access the service." ;
        rdfs:label    "serviceUrl" .

schema:percentile90  a  rdf:Property ;
        rdfs:comment  "The 90th percentile value." ;
        rdfs:label    "percentile90" .

schema:MedicalEvidenceLevel
        a                rdfs:Class ;
        rdfs:comment     "Level of evidence for a medical guideline. Enumerated type." ;
        rdfs:label       "MedicalEvidenceLevel" ;
        rdfs:subClassOf  schema:MedicalEnumeration .

schema:isAcceptingNewPatients
        a             rdf:Property ;
        rdfs:comment  "Whether the provider is accepting new patients." ;
        rdfs:label    "isAcceptingNewPatients" .

schema:ReplyAction  a    rdfs:Class ;
        rdfs:comment     "The act of responding to a question/message asked/sent by the object. Related to [[AskAction]]\\n\\nRelated actions:\\n\\n* [[AskAction]]: Appears generally as an origin of a ReplyAction." ;
        rdfs:label       "ReplyAction" ;
        rdfs:subClassOf  schema:CommunicateAction .

schema:CableOrSatelliteService
        a                rdfs:Class ;
        rdfs:comment     "A service which provides access to media programming like TV or radio. Access may be via cable or satellite." ;
        rdfs:label       "CableOrSatelliteService" ;
        rdfs:subClassOf  schema:Service .

schema:DaySpa  a         rdfs:Class ;
        rdfs:comment     "A day spa." ;
        rdfs:label       "DaySpa" ;
        rdfs:subClassOf  schema:HealthAndBeautyBusiness .

schema:GovernmentBenefitsType
        a                rdfs:Class ;
        rdfs:comment     "GovernmentBenefitsType enumerates several kinds of government benefits to support the COVID-19 situation. Note that this structure may not capture all benefits offered." ;
        rdfs:label       "GovernmentBenefitsType" ;
        rdfs:subClassOf  schema:Enumeration .

schema:CheckInAction  a  rdfs:Class ;
        rdfs:comment     "The act of an agent communicating (service provider, social media, etc) their arrival by registering/confirming for a previously reserved service (e.g. flight check in) or at a place (e.g. hotel), possibly resulting in a result (boarding pass, etc).\\n\\nRelated actions:\\n\\n* [[CheckOutAction]]: The antonym of CheckInAction.\\n* [[ArriveAction]]: Unlike ArriveAction, CheckInAction implies that the agent is informing/confirming the start of a previously reserved service.\\n* [[ConfirmAction]]: Unlike ConfirmAction, CheckInAction implies that the agent is informing/confirming the *start* of a previously reserved service rather than its validity/existence." ;
        rdfs:label       "CheckInAction" ;
        rdfs:subClassOf  schema:CommunicateAction .

schema:Taxi  a           rdfs:Class ;
        rdfs:comment     "A taxi." ;
        rdfs:label       "Taxi" ;
        rdfs:subClassOf  schema:Service .

schema:downvoteCount  a  rdf:Property ;
        rdfs:comment  "The number of downvotes this question, answer or comment has received from the community." ;
        rdfs:label    "downvoteCount" .

schema:menuAddOn  a   rdf:Property ;
        rdfs:comment  "Additional menu item(s) such as a side dish of salad or side order of fries that can be added to this menu item. Additionally it can be a menu section containing allowed add-on menu items for this menu item." ;
        rdfs:label    "menuAddOn" .

schema:relatedDrug  a  rdf:Property ;
        rdfs:comment  "Any other drug related to this one, for example commonly-prescribed alternatives." ;
        rdfs:label    "relatedDrug" .

schema:dateReceived  a  rdf:Property ;
        rdfs:comment  "The date/time the message was received if a single recipient exists." ;
        rdfs:label    "dateReceived" .

schema:partOfSeason  a      rdf:Property ;
        rdfs:comment        "The season to which this episode belongs." ;
        rdfs:label          "partOfSeason" ;
        rdfs:subPropertyOf  schema:isPartOf .

schema:offersPrescriptionByMail
        a             rdf:Property ;
        rdfs:comment  "Whether prescriptions can be delivered by mail." ;
        rdfs:label    "offersPrescriptionByMail" .

schema:LiveBlogPosting
        a                rdfs:Class ;
        rdfs:comment     "A blog post intended to provide a rolling textual coverage of an ongoing event through continuous updates." ;
        rdfs:label       "LiveBlogPosting" ;
        rdfs:subClassOf  schema:BlogPosting .

schema:object  a      rdf:Property ;
        rdfs:comment  "The object upon which the action is carried out, whose state is kept intact or changed. Also known as the semantic roles patient, affected or undergoer (which change their state) or theme (which doesn't). e.g. John read *a book*." ;
        rdfs:label    "object" .

schema:DiscoverAction
        a                rdfs:Class ;
        rdfs:comment     "The act of discovering/finding an object." ;
        rdfs:label       "DiscoverAction" ;
        rdfs:subClassOf  schema:FindAction .

schema:Play  a           rdfs:Class ;
        rdfs:comment     "A play is a form of literature, usually consisting of dialogue between characters, intended for theatrical performance rather than just reading. Note the peformance of a Play would be a [[TheaterEvent]] - the *Play* being the [[workPerformed]]." ;
        rdfs:label       "Play" ;
        rdfs:subClassOf  schema:CreativeWork .

schema:CampingPitch  a   rdfs:Class ;
        rdfs:comment     "A [[CampingPitch]] is an individual place for overnight stay in the outdoors, typically being part of a larger camping site, or [[Campground]].\\n\\n\nIn British English a campsite, or campground, is an area, usually divided into a number of pitches, where people can camp overnight using tents or camper vans or caravans; this British English use of the word is synonymous with the American English expression campground. In American English the term campsite generally means an area where an individual, family, group, or military unit can pitch a tent or park a camper; a campground may contain many campsites.\n(Source: Wikipedia see [https://en.wikipedia.org/wiki/Campsite](https://en.wikipedia.org/wiki/Campsite)).\\n\\n\nSee also the dedicated [document on the use of schema.org for marking up hotels and other forms of accommodations](/docs/hotels.html).\n" ;
        rdfs:label       "CampingPitch" ;
        rdfs:subClassOf  schema:Accommodation .

schema:healthPlanCopay
        a             rdf:Property ;
        rdfs:comment  "Whether The copay amount." ;
        rdfs:label    "healthPlanCopay" .

schema:conditionsOfAccess
        a             rdf:Property ;
        rdfs:comment  "Conditions that affect the availability of, or method(s) of access to, an item. Typically used for real world items such as an [[ArchiveComponent]] held by an [[ArchiveOrganization]]. This property is not suitable for use as a general Web access control mechanism. It is expressed only in natural language.\\n\\nFor example \"Available by appointment from the Reading Room\" or \"Accessible only from logged-in accounts \". " ;
        rdfs:label    "conditionsOfAccess" .

schema:arrivalGate  a  rdf:Property ;
        rdfs:comment  "Identifier of the flight's arrival gate." ;
        rdfs:label    "arrivalGate" .

schema:occupationLocation
        a             rdf:Property ;
        rdfs:comment  " The region/country for which this occupational description is appropriate. Note that educational requirements and qualifications can vary between jurisdictions." ;
        rdfs:label    "occupationLocation" .

schema:hasEnergyConsumptionDetails
        a             rdf:Property ;
        rdfs:comment  "Defines the energy efficiency Category (also known as \"class\" or \"rating\") for a product according to an international energy efficiency standard." ;
        rdfs:label    "hasEnergyConsumptionDetails" .

schema:salaryUponCompletion
        a             rdf:Property ;
        rdfs:comment  "The expected salary upon completing the training." ;
        rdfs:label    "salaryUponCompletion" .

schema:SportsTeam  a     rdfs:Class ;
        rdfs:comment     "Organization: Sports team." ;
        rdfs:label       "SportsTeam" ;
        rdfs:subClassOf  schema:SportsOrganization .

schema:amount  a      rdf:Property ;
        rdfs:comment  "The amount of money." ;
        rdfs:label    "amount" .

schema:ApprovedIndication
        a                rdfs:Class ;
        rdfs:comment     "An indication for a medical therapy that has been formally specified or approved by a regulatory body that regulates use of the therapy; for example, the US FDA approves indications for most drugs in the US." ;
        rdfs:label       "ApprovedIndication" ;
        rdfs:subClassOf  schema:MedicalIndication .

schema:reportNumber  a  rdf:Property ;
        rdfs:comment  "The number or other unique designator assigned to a Report by the publishing organization." ;
        rdfs:label    "reportNumber" .

schema:medicineSystem
        a             rdf:Property ;
        rdfs:comment  "The system of medicine that includes this MedicalEntity, for example 'evidence-based', 'homeopathic', 'chiropractic', etc." ;
        rdfs:label    "medicineSystem" .

schema:PaintAction  a    rdfs:Class ;
        rdfs:comment     "The act of producing a painting, typically with paint and canvas as instruments." ;
        rdfs:label       "PaintAction" ;
        rdfs:subClassOf  schema:CreateAction .

schema:CityHall  a       rdfs:Class ;
        rdfs:comment     "A city hall." ;
        rdfs:label       "CityHall" ;
        rdfs:subClassOf  schema:GovernmentBuilding .

schema:seatSection  a  rdf:Property ;
        rdfs:comment  "The section location of the reserved seat (e.g. Orchestra)." ;
        rdfs:label    "seatSection" .

schema:releaseDate  a  rdf:Property ;
        rdfs:comment  "The release date of a product or product model. This can be used to distinguish the exact variant of a product." ;
        rdfs:label    "releaseDate" .

schema:ComicStory  a     rdfs:Class ;
        rdfs:comment     "The term \"story\" is any indivisible, re-printable\n    \tunit of a comic, including the interior stories, covers, and backmatter. Most\n    \tcomics have at least two stories: a cover (ComicCoverArt) and an interior story." ;
        rdfs:label       "ComicStory" ;
        rdfs:subClassOf  schema:CreativeWork .

schema:EnergyStarEnergyEfficiencyEnumeration
        a                rdfs:Class ;
        rdfs:comment     "Used to indicate whether a product is EnergyStar certified." ;
        rdfs:label       "EnergyStarEnergyEfficiencyEnumeration" ;
        rdfs:subClassOf  schema:EnergyEfficiencyEnumeration .

schema:EventVenue  a     rdfs:Class ;
        rdfs:comment     "An event venue." ;
        rdfs:label       "EventVenue" ;
        rdfs:subClassOf  schema:CivicStructure .

schema:jobStartDate  a  rdf:Property ;
        rdfs:comment  "The date on which a successful applicant for this job would be expected to start work. Choose a specific date in the future or use the jobImmediateStart property to indicate the position is to be filled as soon as possible." ;
        rdfs:label    "jobStartDate" .

schema:isPartOf  a    rdf:Property ;
        rdfs:comment  "Indicates an item or CreativeWork that this item, or CreativeWork (in some sense), is part of." ;
        rdfs:label    "isPartOf" .

schema:DriveWheelConfigurationValue
        a                rdfs:Class ;
        rdfs:comment     "A value indicating which roadwheels will receive torque." ;
        rdfs:label       "DriveWheelConfigurationValue" ;
        rdfs:subClassOf  schema:QualitativeValue .

schema:accessMode  a  rdf:Property ;
        rdfs:comment  "The human sensory perceptual system or cognitive faculty through which a person may process or perceive information. Expected values include: auditory, tactile, textual, visual, colorDependent, chartOnVisual, chemOnVisual, diagramOnVisual, mathOnVisual, musicOnVisual, textOnVisual.\n      " ;
        rdfs:label    "accessMode" .

schema:EngineSpecification
        a                rdfs:Class ;
        rdfs:comment     "Information about the engine of the vehicle. A vehicle can have multiple engines represented by multiple engine specification entities." ;
        rdfs:label       "EngineSpecification" ;
        rdfs:subClassOf  schema:StructuredValue .

schema:nonProprietaryName
        a             rdf:Property ;
        rdfs:comment  "The generic name of this drug or supplement." ;
        rdfs:label    "nonProprietaryName" .

schema:weight  a      rdf:Property ;
        rdfs:comment  "The weight of the product or person." ;
        rdfs:label    "weight" .

schema:VirtualLocation
        a                rdfs:Class ;
        rdfs:comment     "An online or virtual location for attending events. For example, one may attend an online seminar or educational event. While a virtual location may be used as the location of an event, virtual locations should not be confused with physical locations in the real world." ;
        rdfs:label       "VirtualLocation" ;
        rdfs:subClassOf  schema:Intangible .

schema:knownVehicleDamages
        a             rdf:Property ;
        rdfs:comment  "A textual description of known damages, both repaired and unrepaired." ;
        rdfs:label    "knownVehicleDamages" .

schema:characterAttribute
        a             rdf:Property ;
        rdfs:comment  "A piece of data that represents a particular aspect of a fictional character (skill, power, character points, advantage, disadvantage)." ;
        rdfs:label    "characterAttribute" .

schema:estimatedCost  a  rdf:Property ;
        rdfs:comment  "The estimated cost of the supply or supplies consumed when performing instructions." ;
        rdfs:label    "estimatedCost" .

schema:legalName  a   rdf:Property ;
        rdfs:comment  "The official name of the organization, e.g. the registered company name." ;
        rdfs:label    "legalName" .

schema:HighSchool  a     rdfs:Class ;
        rdfs:comment     "A high school." ;
        rdfs:label       "HighSchool" ;
        rdfs:subClassOf  schema:EducationalOrganization .

schema:CategoryCodeSet
        a                rdfs:Class ;
        rdfs:comment     "A set of Category Code values." ;
        rdfs:label       "CategoryCodeSet" ;
        rdfs:subClassOf  schema:DefinedTermSet .

schema:deliveryMethod
        a                   rdf:Property ;
        rdfs:comment        "A sub property of instrument. The method of delivery." ;
        rdfs:label          "deliveryMethod" ;
        rdfs:subPropertyOf  schema:instrument .

schema:PublicHealth  a   rdfs:Class ;
        rdfs:comment     "Branch of medicine that pertains to the health services to improve and protect community health, especially epidemiology, sanitation, immunization, and preventive medicine." ;
        rdfs:label       "PublicHealth" ;
        rdfs:subClassOf  schema:MedicalBusiness .

schema:infectiousAgentClass
        a             rdf:Property ;
        rdfs:comment  "The class of infectious agent (bacteria, prion, etc.) that causes the disease." ;
        rdfs:label    "infectiousAgentClass" .

schema:CancelAction  a   rdfs:Class ;
        rdfs:comment     "The act of asserting that a future event/action is no longer going to happen.\\n\\nRelated actions:\\n\\n* [[ConfirmAction]]: The antonym of CancelAction." ;
        rdfs:label       "CancelAction" ;
        rdfs:subClassOf  schema:PlanAction .

schema:audienceType  a  rdf:Property ;
        rdfs:comment  "The target group associated with a given audience (e.g. veterans, car owners, musicians, etc.)." ;
        rdfs:label    "audienceType" .

schema:MedicalStudyStatus
        a                rdfs:Class ;
        rdfs:comment     "The status of a medical study. Enumerated type." ;
        rdfs:label       "MedicalStudyStatus" ;
        rdfs:subClassOf  schema:MedicalEnumeration .

schema:citation  a    rdf:Property ;
        rdfs:comment  "A citation or reference to another creative work, such as another publication, web page, scholarly article, etc." ;
        rdfs:label    "citation" .

schema:hasMerchantReturnPolicy
        a             rdf:Property ;
        rdfs:comment  "Indicates a MerchantReturnPolicy that may be applicable." ;
        rdfs:label    "hasMerchantReturnPolicy" .

schema:primaryPrevention
        a             rdf:Property ;
        rdfs:comment  "A preventative therapy used to prevent an initial occurrence of the medical condition, such as vaccination." ;
        rdfs:label    "primaryPrevention" .

schema:PrimaryCare  a    rdfs:Class ;
        rdfs:comment     "The medical care by a physician, or other health-care professional, who is the patient's first contact with the health-care system and who may recommend a specialist if necessary." ;
        rdfs:label       "PrimaryCare" ;
        rdfs:subClassOf  schema:MedicalBusiness .

schema:ListenAction  a   rdfs:Class ;
        rdfs:comment     "The act of consuming audio content." ;
        rdfs:label       "ListenAction" ;
        rdfs:subClassOf  schema:ConsumeAction .

schema:servicePostalAddress
        a             rdf:Property ;
        rdfs:comment  "The address for accessing the service by mail." ;
        rdfs:label    "servicePostalAddress" .

schema:ClaimReview  a    rdfs:Class ;
        rdfs:comment     "A fact-checking review of claims made (or reported) in some creative work (referenced via itemReviewed)." ;
        rdfs:label       "ClaimReview" ;
        rdfs:subClassOf  schema:Review .

schema:MedicalConditionStage
        a                rdfs:Class ;
        rdfs:comment     "A stage of a medical condition, such as 'Stage IIIa'." ;
        rdfs:label       "MedicalConditionStage" ;
        rdfs:subClassOf  schema:MedicalIntangible .

schema:parentOrganization
        a             rdf:Property ;
        rdfs:comment  "The larger organization that this organization is a [[subOrganization]] of, if any." ;
        rdfs:label    "parentOrganization" .

schema:permittedUsage
        a             rdf:Property ;
        rdfs:comment  "Indications regarding the permitted usage of the accommodation." ;
        rdfs:label    "permittedUsage" .

schema:ServiceChannel
        a                rdfs:Class ;
        rdfs:comment     "A means for accessing a service, e.g. a government office location, web site, or phone number." ;
        rdfs:label       "ServiceChannel" ;
        rdfs:subClassOf  schema:Intangible .

schema:percentile10  a  rdf:Property ;
        rdfs:comment  "The 10th percentile value." ;
        rdfs:label    "percentile10" .

schema:endorsee  a          rdf:Property ;
        rdfs:comment        "A sub property of participant. The person/organization being supported." ;
        rdfs:label          "endorsee" ;
        rdfs:subPropertyOf  schema:participant .

schema:trainNumber  a  rdf:Property ;
        rdfs:comment  "The unique identifier for the train." ;
        rdfs:label    "trainNumber" .

schema:repeatFrequency
        a                   rdf:Property ;
        rdfs:comment        "Defines the frequency at which [[Event]]s will occur according to a schedule [[Schedule]]. The intervals between\n      events should be defined as a [[Duration]] of time." ;
        rdfs:label          "repeatFrequency" ;
        rdfs:subPropertyOf  schema:frequency .

schema:weightTotal  a  rdf:Property ;
        rdfs:comment  "The permitted total weight of the loaded vehicle, including passengers and cargo and the weight of the empty vehicle.\\n\\nTypical unit code(s): KGM for kilogram, LBR for pound\\n\\n* Note 1: You can indicate additional information in the [[name]] of the [[QuantitativeValue]] node.\\n* Note 2: You may also link to a [[QualitativeValue]] node that provides additional information using [[valueReference]].\\n* Note 3: Note that you can use [[minValue]] and [[maxValue]] to indicate ranges." ;
        rdfs:label    "weightTotal" .

schema:remainingAttendeeCapacity
        a             rdf:Property ;
        rdfs:comment  "The number of attendee places for an event that remain unallocated." ;
        rdfs:label    "remainingAttendeeCapacity" .

schema:Canal  a          rdfs:Class ;
        rdfs:comment     "A canal, like the Panama Canal." ;
        rdfs:label       "Canal" ;
        rdfs:subClassOf  schema:BodyOfWater .

schema:PodcastSeries  a  rdfs:Class ;
        rdfs:comment     "A podcast is an episodic series of digital audio or video files which a user can download and listen to." ;
        rdfs:label       "PodcastSeries" ;
        rdfs:subClassOf  schema:CreativeWorkSeries .

schema:legislationDateVersion
        a             rdf:Property ;
        rdfs:comment  "The point-in-time at which the provided description of the legislation is valid (e.g. : when looking at the law on the 2016-04-07 (= dateVersion), I get the consolidation of 2015-04-12 of the \"National Insurance Contributions Act 2015\")" ;
        rdfs:label    "legislationDateVersion" .

schema:QualitativeValue
        a                rdfs:Class ;
        rdfs:comment     "A predefined value for a product characteristic, e.g. the power cord plug type 'US' or the garment sizes 'S', 'M', 'L', and 'XL'." ;
        rdfs:label       "QualitativeValue" ;
        rdfs:subClassOf  schema:Enumeration .

schema:applicationSuite
        a             rdf:Property ;
        rdfs:comment  "The name of the application suite to which the application belongs (e.g. Excel belongs to Office)." ;
        rdfs:label    "applicationSuite" .

schema:version  a     rdf:Property ;
        rdfs:comment  "The version of the CreativeWork embodied by a specified resource." ;
        rdfs:label    "version" .

schema:relatedStructure
        a             rdf:Property ;
        rdfs:comment  "Related anatomical structure(s) that are not part of the system but relate or connect to it, such as vascular bundles associated with an organ system." ;
        rdfs:label    "relatedStructure" .

schema:floorLimit  a  rdf:Property ;
        rdfs:comment  "A floor limit is the amount of money above which credit card transactions must be authorized." ;
        rdfs:label    "floorLimit" .

schema:MedicalCondition
        a                rdfs:Class ;
        rdfs:comment     "Any condition of the human body that affects the normal functioning of a person, whether physically or mentally. Includes diseases, injuries, disabilities, disorders, syndromes, etc." ;
        rdfs:label       "MedicalCondition" ;
        rdfs:subClassOf  schema:MedicalEntity .

schema:HowToSupply  a    rdfs:Class ;
        rdfs:comment     "A supply consumed when performing the instructions for how to achieve a result." ;
        rdfs:label       "HowToSupply" ;
        rdfs:subClassOf  schema:HowToItem .

schema:HealthPlanNetwork
        a                rdfs:Class ;
        rdfs:comment     "A US-style health insurance plan network. " ;
        rdfs:label       "HealthPlanNetwork" ;
        rdfs:subClassOf  schema:Intangible .

schema:Physiotherapy  a  rdfs:Class ;
        rdfs:comment     "The practice of treatment of disease, injury, or deformity by physical methods such as massage, heat treatment, and exercise rather than by drugs or surgery.." ;
        rdfs:label       "Physiotherapy" ;
        rdfs:subClassOf  schema:MedicalBusiness .

schema:Time  a        rdfs:Class ;
        rdfs:comment  "A point in time recurring on multiple days in the form hh:mm:ss[Z|(+|-)hh:mm] (see [XML schema for details](http://www.w3.org/TR/xmlschema-2/#time))." ;
        rdfs:label    "Time" .

schema:isBasedOnUrl  a  rdf:Property ;
        rdfs:comment  "A resource that was used in the creation of this resource. This term can be repeated for multiple sources. For example, http://example.com/great-multiplication-intro.html." ;
        rdfs:label    "isBasedOnUrl" .

schema:MoveAction  a     rdfs:Class ;
        rdfs:comment     "The act of an agent relocating to a place.\\n\\nRelated actions:\\n\\n* [[TransferAction]]: Unlike TransferAction, the subject of the move is a living Person or Organization rather than an inanimate object." ;
        rdfs:label       "MoveAction" ;
        rdfs:subClassOf  schema:Action .

schema:EventReservation
        a                rdfs:Class ;
        rdfs:comment     "A reservation for an event like a concert, sporting event, or lecture.\\n\\nNote: This type is for information about actual reservations, e.g. in confirmation emails or HTML pages with individual confirmations of reservations. For offers of tickets, use [[Offer]]." ;
        rdfs:label       "EventReservation" ;
        rdfs:subClassOf  schema:Reservation .

schema:House  a          rdfs:Class ;
        rdfs:comment     "A house is a building or structure that has the ability to be occupied for habitation by humans or other creatures (Source: Wikipedia, the free encyclopedia, see <a href=\"http://en.wikipedia.org/wiki/House\">http://en.wikipedia.org/wiki/House</a>)." ;
        rdfs:label       "House" ;
        rdfs:subClassOf  schema:Accommodation .

schema:sportsActivityLocation
        a                   rdf:Property ;
        rdfs:comment        "A sub property of location. The sports activity location where this action occurred." ;
        rdfs:label          "sportsActivityLocation" ;
        rdfs:subPropertyOf  schema:location .

schema:SearchAction  a   rdfs:Class ;
        rdfs:comment     "The act of searching for an object.\\n\\nRelated actions:\\n\\n* [[FindAction]]: SearchAction generally leads to a FindAction, but not necessarily." ;
        rdfs:label       "SearchAction" ;
        rdfs:subClassOf  schema:Action .

schema:TravelAgency  a   rdfs:Class ;
        rdfs:comment     "A travel agency." ;
        rdfs:label       "TravelAgency" ;
        rdfs:subClassOf  schema:LocalBusiness .

schema:orderItemStatus
        a             rdf:Property ;
        rdfs:comment  "The current status of the order item." ;
        rdfs:label    "orderItemStatus" .

schema:netWorth  a    rdf:Property ;
        rdfs:comment  "The total financial value of the person as calculated by subtracting assets from liabilities." ;
        rdfs:label    "netWorth" .

schema:signOrSymptom  a  rdf:Property ;
        rdfs:comment  "A sign or symptom of this condition. Signs are objective or physically observable manifestations of the medical condition while symptoms are the subjective experience of the medical condition." ;
        rdfs:label    "signOrSymptom" .

schema:AccountingService
        a                rdfs:Class ;
        rdfs:comment     "Accountancy business.\\n\\nAs a [[LocalBusiness]] it can be described as a [[provider]] of one or more [[Service]]\\(s).\n      " ;
        rdfs:label       "AccountingService" ;
        rdfs:subClassOf  schema:FinancialService .

schema:serviceOperator
        a             rdf:Property ;
        rdfs:comment  "The operating organization, if different from the provider.  This enables the representation of services that are provided by an organization, but operated by another organization like a subcontractor." ;
        rdfs:label    "serviceOperator" .

schema:validFor  a    rdf:Property ;
        rdfs:comment  "The duration of validity of a permit or similar thing." ;
        rdfs:label    "validFor" .

schema:costCurrency  a  rdf:Property ;
        rdfs:comment  "The currency (in 3-letter of the drug cost. See: http://en.wikipedia.org/wiki/ISO_4217. " ;
        rdfs:label    "costCurrency" .

schema:partOfTrip  a  rdf:Property ;
        rdfs:comment  "Identifies that this [[Trip]] is a subTrip of another Trip.  For example Day 1, Day 2, etc. of a multi-day trip." ;
        rdfs:label    "partOfTrip" .

schema:slogan  a      rdf:Property ;
        rdfs:comment  "A slogan or motto associated with the item." ;
        rdfs:label    "slogan" .

schema:Review  a         rdfs:Class ;
        rdfs:comment     "A review of an item - for example, of a restaurant, movie, or store." ;
        rdfs:label       "Review" ;
        rdfs:subClassOf  schema:CreativeWork .

schema:SpreadsheetDigitalDocument
        a                rdfs:Class ;
        rdfs:comment     "A spreadsheet file." ;
        rdfs:label       "SpreadsheetDigitalDocument" ;
        rdfs:subClassOf  schema:DigitalDocument .

schema:albumReleaseType
        a             rdf:Property ;
        rdfs:comment  "The kind of release which this album is: single, EP or album." ;
        rdfs:label    "albumReleaseType" .

schema:calories  a    rdf:Property ;
        rdfs:comment  "The number of calories." ;
        rdfs:label    "calories" .

schema:Winery  a         rdfs:Class ;
        rdfs:comment     "A winery." ;
        rdfs:label       "Winery" ;
        rdfs:subClassOf  schema:FoodEstablishment .

schema:PlaceOfWorship
        a                rdfs:Class ;
        rdfs:comment     "Place of worship, such as a church, synagogue, or mosque." ;
        rdfs:label       "PlaceOfWorship" ;
        rdfs:subClassOf  schema:CivicStructure .

schema:distribution  a  rdf:Property ;
        rdfs:comment  "A downloadable form of this dataset, at a specific location, in a specific format." ;
        rdfs:label    "distribution" .

schema:alternateName  a  rdf:Property ;
        rdfs:comment  "An alias for the item." ;
        rdfs:label    "alternateName" .

schema:HVACBusiness  a   rdfs:Class ;
        rdfs:comment     "A business that provide Heating, Ventilation and Air Conditioning services." ;
        rdfs:label       "HVACBusiness" ;
        rdfs:subClassOf  schema:HomeAndConstructionBusiness .

schema:energyEfficiencyScaleMax
        a             rdf:Property ;
        rdfs:comment  "Specifies the most energy efficient class on the regulated EU energy consumption scale for the product category a product belongs to. For example, energy consumption for televisions placed on the market after January 1, 2020 is scaled from D to A+++." ;
        rdfs:label    "energyEfficiencyScaleMax" .

schema:hasMenuItem  a  rdf:Property ;
        rdfs:comment  "A food or drink item contained in a menu or menu section." ;
        rdfs:label    "hasMenuItem" .

schema:workFeatured  a  rdf:Property ;
        rdfs:comment  "A work featured in some event, e.g. exhibited in an ExhibitionEvent.\n       Specific subproperties are available for workPerformed (e.g. a play), or a workPresented (a Movie at a ScreeningEvent)." ;
        rdfs:label    "workFeatured" .

schema:TrainStation  a   rdfs:Class ;
        rdfs:comment     "A train station." ;
        rdfs:label       "TrainStation" ;
        rdfs:subClassOf  schema:CivicStructure .

schema:biomechnicalClass
        a             rdf:Property ;
        rdfs:comment  "The biomechanical properties of the bone." ;
        rdfs:label    "biomechnicalClass" .

schema:Property  a       rdfs:Class ;
        rdfs:comment     "A property, used to indicate attributes and relationships of some Thing; equivalent to rdf:Property." ;
        rdfs:label       "Property" ;
        rdfs:subClassOf  schema:Intangible .

schema:UserPageVisits
        a                rdfs:Class ;
        rdfs:comment     "UserInteraction and its subtypes is an old way of talking about users interacting with pages. It is generally better to use [[Action]]-based vocabulary, alongside types such as [[Comment]]." ;
        rdfs:label       "UserPageVisits" ;
        rdfs:subClassOf  schema:UserInteraction .

schema:howPerformed  a  rdf:Property ;
        rdfs:comment  "How the procedure is performed." ;
        rdfs:label    "howPerformed" .

schema:AdultEntertainment
        a                rdfs:Class ;
        rdfs:comment     "An adult entertainment establishment." ;
        rdfs:label       "AdultEntertainment" ;
        rdfs:subClassOf  schema:EntertainmentBusiness .

schema:priceCurrency  a  rdf:Property ;
        rdfs:comment  "The currency of the price, or a price component when attached to [[PriceSpecification]] and its subtypes.\\n\\nUse standard formats: [ISO 4217 currency format](http://en.wikipedia.org/wiki/ISO_4217) e.g. \"USD\"; [Ticker symbol](https://en.wikipedia.org/wiki/List_of_cryptocurrencies) for cryptocurrencies e.g. \"BTC\"; well known names for [Local Exchange Tradings Systems](https://en.wikipedia.org/wiki/Local_exchange_trading_system) (LETS) and other currency types e.g. \"Ithaca HOUR\"." ;
        rdfs:label    "priceCurrency" .

schema:Integer  a        rdfs:Class ;
        rdfs:comment     "Data type: Integer." ;
        rdfs:label       "Integer" ;
        rdfs:subClassOf  schema:Number .

schema:abridged  a    rdf:Property ;
        rdfs:comment  "Indicates whether the book is an abridged edition." ;
        rdfs:label    "abridged" .

schema:targetDescription
        a             rdf:Property ;
        rdfs:comment  "The description of a node in an established educational framework." ;
        rdfs:label    "targetDescription" .

schema:inPlaylist  a  rdf:Property ;
        rdfs:comment  "The playlist to which this recording belongs." ;
        rdfs:label    "inPlaylist" .

schema:InformAction  a   rdfs:Class ;
        rdfs:comment     "The act of notifying someone of information pertinent to them, with no expectation of a response." ;
        rdfs:label       "InformAction" ;
        rdfs:subClassOf  schema:CommunicateAction .

schema:replacer  a          rdf:Property ;
        rdfs:comment        "A sub property of object. The object that replaces." ;
        rdfs:label          "replacer" ;
        rdfs:subPropertyOf  schema:object .

schema:tracks  a      rdf:Property ;
        rdfs:comment  "A music recording (track)&#x2014;usually a single song." ;
        rdfs:label    "tracks" .

schema:NailSalon  a      rdfs:Class ;
        rdfs:comment     "A nail salon." ;
        rdfs:label       "NailSalon" ;
        rdfs:subClassOf  schema:HealthAndBeautyBusiness .

schema:recognizedBy  a  rdf:Property ;
        rdfs:comment  "An organization that acknowledges the validity, value or utility of a credential. Note: recognition may include a process of quality assurance or accreditation." ;
        rdfs:label    "recognizedBy" .

schema:item  a        rdf:Property ;
        rdfs:comment  "An entity represented by an entry in a list or data feed (e.g. an 'artist' in a list of 'artists')’." ;
        rdfs:label    "item" .

schema:OccupationalTherapy
        a                rdfs:Class ;
        rdfs:comment     "A treatment of people with physical, emotional, or social problems, using purposeful activity to help them overcome or learn to deal with their problems." ;
        rdfs:label       "OccupationalTherapy" ;
        rdfs:subClassOf  schema:MedicalTherapy .

schema:OwnershipInfo  a  rdfs:Class ;
        rdfs:comment     "A structured value providing information about when a certain organization or person owned a certain product." ;
        rdfs:label       "OwnershipInfo" ;
        rdfs:subClassOf  schema:StructuredValue .

schema:buyer  a             rdf:Property ;
        rdfs:comment        "A sub property of participant. The participant/person/organization that bought the object." ;
        rdfs:label          "buyer" ;
        rdfs:subPropertyOf  schema:participant .

schema:runtime  a     rdf:Property ;
        rdfs:comment  "Runtime platform or script interpreter dependencies (Example - Java v1, Python2.3, .Net Framework 3.0)." ;
        rdfs:label    "runtime" .

schema:query  a             rdf:Property ;
        rdfs:comment        "A sub property of instrument. The query used on this action." ;
        rdfs:label          "query" ;
        rdfs:subPropertyOf  schema:instrument .

schema:numberOfAccommodationUnits
        a             rdf:Property ;
        rdfs:comment  "Indicates the total (available plus unavailable) number of accommodation units in an [[ApartmentComplex]], or the number of accommodation units for a specific [[FloorPlan]] (within its specific [[ApartmentComplex]]). See also [[numberOfAvailableAccommodationUnits]]." ;
        rdfs:label    "numberOfAccommodationUnits" .

schema:encodesCreativeWork
        a             rdf:Property ;
        rdfs:comment  "The CreativeWork encoded by this media object." ;
        rdfs:label    "encodesCreativeWork" .

schema:gtin13  a            rdf:Property ;
        rdfs:comment        "The GTIN-13 code of the product, or the product to which the offer refers. This is equivalent to 13-digit ISBN codes and EAN UCC-13. Former 12-digit UPC codes can be converted into a GTIN-13 code by simply adding a preceding zero. See [GS1 GTIN Summary](http://www.gs1.org/barcodes/technical/idkeys/gtin) for more details." ;
        rdfs:label          "gtin13" ;
        rdfs:subPropertyOf  schema:identifier , schema:gtin .

schema:temporalCoverage
        a             rdf:Property ;
        rdfs:comment  "The temporalCoverage of a CreativeWork indicates the period that the content applies to, i.e. that it describes, either as a DateTime or as a textual string indicating a time period in [ISO 8601 time interval format](https://en.wikipedia.org/wiki/ISO_8601#Time_intervals). In\n      the case of a Dataset it will typically indicate the relevant time period in a precise notation (e.g. for a 2011 census dataset, the year 2011 would be written \"2011/2012\"). Other forms of content e.g. ScholarlyArticle, Book, TVSeries or TVEpisode may indicate their temporalCoverage in broader terms - textually or via well-known URL.\n      Written works such as books may sometimes have precise temporal coverage too, e.g. a work set in 1939 - 1945 can be indicated in ISO 8601 interval format format via \"1939/1945\".\n\nOpen-ended date ranges can be written with \"..\" in place of the end date. For example, \"2015-11/..\" indicates a range beginning in November 2015 and with no specified final date. This is tentative and might be updated in future when ISO 8601 is officially updated." ;
        rdfs:label    "temporalCoverage" .

schema:applicationContact
        a             rdf:Property ;
        rdfs:comment  "Contact details for further information relevant to this job posting." ;
        rdfs:label    "applicationContact" .

schema:median  a      rdf:Property ;
        rdfs:comment  "The median value." ;
        rdfs:label    "median" .

schema:3DModel  a        rdfs:Class ;
        rdfs:comment     "A 3D model represents some kind of 3D content, which may have [[encoding]]s in one or more [[MediaObject]]s. Many 3D formats are available (e.g. see [Wikipedia](https://en.wikipedia.org/wiki/Category:3D_graphics_file_formats)); specific encoding formats can be represented using the [[encodingFormat]] property applied to the relevant [[MediaObject]]. For the\ncase of a single file published after Zip compression, the convention of appending '+zip' to the [[encodingFormat]] can be used. Geospatial, AR/VR, artistic/animation, gaming, engineering and scientific content can all be represented using [[3DModel]]." ;
        rdfs:label       "3DModel" ;
        rdfs:subClassOf  schema:MediaObject .

schema:steeringPosition
        a             rdf:Property ;
        rdfs:comment  "The position of the steering wheel or similar device (mostly for cars)." ;
        rdfs:label    "steeringPosition" .

schema:postalCode  a  rdf:Property ;
        rdfs:comment  "The postal code. For example, 94043." ;
        rdfs:label    "postalCode" .

schema:healthPlanDrugOption
        a             rdf:Property ;
        rdfs:comment  "TODO." ;
        rdfs:label    "healthPlanDrugOption" .

schema:AnalysisNewsArticle
        a                rdfs:Class ;
        rdfs:comment     "An AnalysisNewsArticle is a [[NewsArticle]] that, while based on factual reporting, incorporates the expertise of the author/producer, offering interpretations and conclusions." ;
        rdfs:label       "AnalysisNewsArticle" ;
        rdfs:subClassOf  schema:NewsArticle .

schema:requiredMaxAge
        a             rdf:Property ;
        rdfs:comment  "Audiences defined by a person's maximum age." ;
        rdfs:label    "requiredMaxAge" .

schema:MedicalGuidelineContraindication
        a                rdfs:Class ;
        rdfs:comment     "A guideline contraindication that designates a process as harmful and where quality of the data supporting the contraindication is sound." ;
        rdfs:label       "MedicalGuidelineContraindication" ;
        rdfs:subClassOf  schema:MedicalGuideline .

schema:activityDuration
        a             rdf:Property ;
        rdfs:comment  "Length of time to engage in the activity." ;
        rdfs:label    "activityDuration" .

schema:hasOccupation  a  rdf:Property ;
        rdfs:comment  "The Person's occupation. For past professions, use Role for expressing dates." ;
        rdfs:label    "hasOccupation" .

schema:videoFormat  a  rdf:Property ;
        rdfs:comment  "The type of screening or video broadcast used (e.g. IMAX, 3D, SD, HD, etc.)." ;
        rdfs:label    "videoFormat" .

schema:dateVehicleFirstRegistered
        a             rdf:Property ;
        rdfs:comment  "The date of the first registration of the vehicle with the respective public authorities." ;
        rdfs:label    "dateVehicleFirstRegistered" .

schema:broadcaster  a  rdf:Property ;
        rdfs:comment  "The organization owning or operating the broadcast service." ;
        rdfs:label    "broadcaster" .

schema:members  a     rdf:Property ;
        rdfs:comment  "A member of this organization." ;
        rdfs:label    "members" .

schema:addressLocality
        a             rdf:Property ;
        rdfs:comment  "The locality in which the street address is, and which is in the region. For example, Mountain View." ;
        rdfs:label    "addressLocality" .

schema:reservationStatus
        a             rdf:Property ;
        rdfs:comment  "The current status of the reservation." ;
        rdfs:label    "reservationStatus" .

schema:license  a     rdf:Property ;
        rdfs:comment  "A license document that applies to this content, typically indicated by URL." ;
        rdfs:label    "license" .

schema:bed  a         rdf:Property ;
        rdfs:comment  "The type of bed or beds included in the accommodation. For the single case of just one bed of a certain type, you use bed directly with a text.\n      If you want to indicate the quantity of a certain kind of bed, use an instance of BedDetails. For more detailed information, use the amenityFeature property." ;
        rdfs:label    "bed" .

schema:Audiobook  a      rdfs:Class ;
        rdfs:comment     "An audiobook." ;
        rdfs:label       "Audiobook" ;
        rdfs:subClassOf  schema:Book , schema:AudioObject .

schema:recipeInstructions
        a                   rdf:Property ;
        rdfs:comment        "A step in making the recipe, in the form of a single item (document, video, etc.) or an ordered list with HowToStep and/or HowToSection items." ;
        rdfs:label          "recipeInstructions" ;
        rdfs:subPropertyOf  schema:step .

schema:replyToUrl  a  rdf:Property ;
        rdfs:comment  "The URL at which a reply may be posted to the specified UserComment." ;
        rdfs:label    "replyToUrl" .

schema:additionalType
        a                   rdf:Property ;
        rdfs:comment        "An additional type for the item, typically used for adding more specific types from external vocabularies in microdata syntax. This is a relationship between something and a class that the thing is in. In RDFa syntax, it is better to use the native RDFa syntax - the 'typeof' attribute - for multiple types. Schema.org tools may have only weaker understanding of extra types, in particular those defined externally." ;
        rdfs:label          "additionalType" ;
        rdfs:subPropertyOf  rdf:type .

schema:OrderAction  a    rdfs:Class ;
        rdfs:comment     "An agent orders an object/product/service to be delivered/sent." ;
        rdfs:label       "OrderAction" ;
        rdfs:subClassOf  schema:TradeAction .

schema:skills  a      rdf:Property ;
        rdfs:comment  "A statement of knowledge, skill, ability, task or any other assertion expressing a competency that is desired or required to fulfill this role or to work in this occupation." ;
        rdfs:label    "skills" .

schema:newsUpdatesAndGuidelines
        a             rdf:Property ;
        rdfs:comment  "Indicates a page with news updates and guidelines. This could often be (but is not required to be) the main page containing [[SpecialAnnouncement]] markup on a site." ;
        rdfs:label    "newsUpdatesAndGuidelines" .

schema:WorkBasedProgram
        a                rdfs:Class ;
        rdfs:comment     "A program with both an educational and employment component. Typically based at a workplace and structured around work-based learning, with the aim of instilling competencies related to an occupation. WorkBasedProgram is used to distinguish programs such as apprenticeships from school, college or other classroom based educational programs." ;
        rdfs:label       "WorkBasedProgram" ;
        rdfs:subClassOf  schema:EducationalOccupationalProgram .

schema:OfferForLease  a  rdfs:Class ;
        rdfs:comment     "An [[OfferForLease]] in Schema.org represents an [[Offer]] to lease out something, i.e. an [[Offer]] whose\n  [[businessFunction]] is [lease out](http://purl.org/goodrelations/v1#LeaseOut.). See [Good Relations](https://en.wikipedia.org/wiki/GoodRelations) for\n  background on the underlying concepts.\n  " ;
        rdfs:label       "OfferForLease" ;
        rdfs:subClassOf  schema:Offer .

schema:ScheduleAction
        a                rdfs:Class ;
        rdfs:comment     "Scheduling future actions, events, or tasks.\\n\\nRelated actions:\\n\\n* [[ReserveAction]]: Unlike ReserveAction, ScheduleAction allocates future actions (e.g. an event, a task, etc) towards a time slot / spatial allocation." ;
        rdfs:label       "ScheduleAction" ;
        rdfs:subClassOf  schema:PlanAction .

schema:boardingGroup  a  rdf:Property ;
        rdfs:comment  "The airline-specific indicator of boarding order / preference." ;
        rdfs:label    "boardingGroup" .

schema:energyEfficiencyScaleMin
        a             rdf:Property ;
        rdfs:comment  "Specifies the least energy efficient class on the regulated EU energy consumption scale for the product category a product belongs to. For example, energy consumption for televisions placed on the market after January 1, 2020 is scaled from D to A+++." ;
        rdfs:label    "energyEfficiencyScaleMin" .

schema:AnatomicalSystem
        a                rdfs:Class ;
        rdfs:comment     "An anatomical system is a group of anatomical structures that work together to perform a certain task. Anatomical systems, such as organ systems, are one organizing principle of anatomy, and can includes circulatory, digestive, endocrine, integumentary, immune, lymphatic, muscular, nervous, reproductive, respiratory, skeletal, urinary, vestibular, and other systems." ;
        rdfs:label       "AnatomicalSystem" ;
        rdfs:subClassOf  schema:MedicalEntity .

schema:assembly  a    rdf:Property ;
        rdfs:comment  "Library file name e.g., mscorlib.dll, system.web.dll." ;
        rdfs:label    "assembly" .

schema:TipAction  a      rdfs:Class ;
        rdfs:comment     "The act of giving money voluntarily to a beneficiary in recognition of services rendered." ;
        rdfs:label       "TipAction" ;
        rdfs:subClassOf  schema:TradeAction .

schema:MusicRecording
        a                rdfs:Class ;
        rdfs:comment     "A music recording (track), usually a single song." ;
        rdfs:label       "MusicRecording" ;
        rdfs:subClassOf  schema:CreativeWork .

schema:BeautySalon  a    rdfs:Class ;
        rdfs:comment     "Beauty salon." ;
        rdfs:label       "BeautySalon" ;
        rdfs:subClassOf  schema:HealthAndBeautyBusiness .

schema:hasCourseInstance
        a             rdf:Property ;
        rdfs:comment  "An offering of the course at a specific time and place or through specific media or mode of study or to a specific section of students." ;
        rdfs:label    "hasCourseInstance" .

schema:issuedBy  a    rdf:Property ;
        rdfs:comment  "The organization issuing the ticket or permit." ;
        rdfs:label    "issuedBy" .

schema:dataset  a     rdf:Property ;
        rdfs:comment  "A dataset contained in this catalog." ;
        rdfs:label    "dataset" .

schema:SatiricalArticle
        a                rdfs:Class ;
        rdfs:comment     "An [[Article]] whose content is primarily [[satirical]](https://en.wikipedia.org/wiki/Satire) in nature, i.e. unlikely to be literally true. A satirical article is sometimes but not necessarily also a [[NewsArticle]]. [[ScholarlyArticle]]s are also sometimes satirized." ;
        rdfs:label       "SatiricalArticle" ;
        rdfs:subClassOf  schema:Article .

schema:structuralClass
        a             rdf:Property ;
        rdfs:comment  "The name given to how bone physically connects to each other." ;
        rdfs:label    "structuralClass" .

schema:AutoDealer  a     rdfs:Class ;
        rdfs:comment     "An car dealership." ;
        rdfs:label       "AutoDealer" ;
        rdfs:subClassOf  schema:AutomotiveBusiness .

schema:medicalSpecialty
        a             rdf:Property ;
        rdfs:comment  "A medical specialty of the provider." ;
        rdfs:label    "medicalSpecialty" .

schema:MovieRentalStore
        a                rdfs:Class ;
        rdfs:comment     "A movie rental store." ;
        rdfs:label       "MovieRentalStore" ;
        rdfs:subClassOf  schema:Store .

schema:regionDrained  a  rdf:Property ;
        rdfs:comment  "The anatomical or organ system drained by this vessel; generally refers to a specific part of an organ." ;
        rdfs:label    "regionDrained" .

schema:postalCodeEnd  a  rdf:Property ;
        rdfs:comment  "Last postal code in the range (included). Needs to be after [[postalCodeBegin]]." ;
        rdfs:label    "postalCodeEnd" .

schema:teaches  a     rdf:Property ;
        rdfs:comment  "The item being described is intended to help a person learn the competency or learning outcome defined by the referenced term." ;
        rdfs:label    "teaches" .

schema:geo  a         rdf:Property ;
        rdfs:comment  "The geo coordinates of the place." ;
        rdfs:label    "geo" .

schema:PerformingGroup
        a                rdfs:Class ;
        rdfs:comment     "A performance group, such as a band, an orchestra, or a circus." ;
        rdfs:label       "PerformingGroup" ;
        rdfs:subClassOf  schema:Organization .

schema:SelfStorage  a    rdfs:Class ;
        rdfs:comment     "A self-storage facility." ;
        rdfs:label       "SelfStorage" ;
        rdfs:subClassOf  schema:LocalBusiness .

schema:SellAction  a     rdfs:Class ;
        rdfs:comment     "The act of taking money from a buyer in exchange for goods or services rendered. An agent sells an object, product, or service to a buyer for a price. Reciprocal of BuyAction." ;
        rdfs:label       "SellAction" ;
        rdfs:subClassOf  schema:TradeAction .

schema:tissueSample  a  rdf:Property ;
        rdfs:comment  "The type of tissue sample required for the test." ;
        rdfs:label    "tissueSample" .

schema:datasetTimeInterval
        a             rdf:Property ;
        rdfs:comment  "The range of temporal applicability of a dataset, e.g. for a 2011 census dataset, the year 2011 (in ISO 8601 time interval format)." ;
        rdfs:label    "datasetTimeInterval" .

schema:hasOfferCatalog
        a             rdf:Property ;
        rdfs:comment  "Indicates an OfferCatalog listing for this Organization, Person, or Service." ;
        rdfs:label    "hasOfferCatalog" .

schema:Locksmith  a      rdfs:Class ;
        rdfs:comment     "A locksmith." ;
        rdfs:label       "Locksmith" ;
        rdfs:subClassOf  schema:HomeAndConstructionBusiness .

schema:pregnancyCategory
        a             rdf:Property ;
        rdfs:comment  "Pregnancy category of this drug." ;
        rdfs:label    "pregnancyCategory" .

schema:Language  a       rdfs:Class ;
        rdfs:comment     "Natural languages such as Spanish, Tamil, Hindi, English, etc. Formal language code tags expressed in [BCP 47](https://en.wikipedia.org/wiki/IETF_language_tag) can be used via the [[alternateName]] property. The Language type previously also covered programming languages such as Scheme and Lisp, which are now best represented using [[ComputerLanguage]]." ;
        rdfs:label       "Language" ;
        rdfs:subClassOf  schema:Intangible .

schema:resultComment  a     rdf:Property ;
        rdfs:comment        "A sub property of result. The Comment created or sent as a result of this action." ;
        rdfs:label          "resultComment" ;
        rdfs:subPropertyOf  schema:result .

schema:FastFoodRestaurant
        a                rdfs:Class ;
        rdfs:comment     "A fast-food restaurant." ;
        rdfs:label       "FastFoodRestaurant" ;
        rdfs:subClassOf  schema:FoodEstablishment .

schema:incentives  a  rdf:Property ;
        rdfs:comment  "Description of bonus and commission compensation aspects of the job." ;
        rdfs:label    "incentives" .

schema:benefits  a    rdf:Property ;
        rdfs:comment  "Description of benefits associated with the job." ;
        rdfs:label    "benefits" .

schema:vehicleSeatingCapacity
        a             rdf:Property ;
        rdfs:comment  "The number of passengers that can be seated in the vehicle, both in terms of the physical space available, and in terms of limitations set by law.\\n\\nTypical unit code(s): C62 for persons." ;
        rdfs:label    "vehicleSeatingCapacity" .

schema:thumbnailUrl  a  rdf:Property ;
        rdfs:comment  "A thumbnail image relevant to the Thing." ;
        rdfs:label    "thumbnailUrl" .

schema:Event  a          rdfs:Class ;
        rdfs:comment     "An event happening at a certain time and location, such as a concert, lecture, or festival. Ticketing information may be added via the [[offers]] property. Repeated events may be structured as separate Event objects." ;
        rdfs:label       "Event" ;
        rdfs:subClassOf  schema:Thing .

schema:releaseNotes  a  rdf:Property ;
        rdfs:comment  "Description of what changed in this version." ;
        rdfs:label    "releaseNotes" .

schema:annualPercentageRate
        a             rdf:Property ;
        rdfs:comment  "The annual rate that is charged for borrowing (or made by investing), expressed as a single percentage number that represents the actual yearly cost of funds over the term of a loan. This includes any fees or additional costs associated with the transaction." ;
        rdfs:label    "annualPercentageRate" .

schema:IndividualProduct
        a                rdfs:Class ;
        rdfs:comment     "A single, identifiable product instance (e.g. a laptop with a particular serial number)." ;
        rdfs:label       "IndividualProduct" ;
        rdfs:subClassOf  schema:Product .

schema:gracePeriod  a  rdf:Property ;
        rdfs:comment  "The period of time after any due date that the borrower has to fulfil its obligations before a default (failure to pay) is deemed to have occurred." ;
        rdfs:label    "gracePeriod" .

schema:UserLikes  a      rdfs:Class ;
        rdfs:comment     "UserInteraction and its subtypes is an old way of talking about users interacting with pages. It is generally better to use [[Action]]-based vocabulary, alongside types such as [[Comment]]." ;
        rdfs:label       "UserLikes" ;
        rdfs:subClassOf  schema:UserInteraction .

schema:expectsAcceptanceOf
        a             rdf:Property ;
        rdfs:comment  "An Offer which must be accepted before the user can perform the Action. For example, the user may need to buy a movie before being able to watch it." ;
        rdfs:label    "expectsAcceptanceOf" .

schema:valuePattern  a  rdf:Property ;
        rdfs:comment  "Specifies a regular expression for testing literal values according to the HTML spec." ;
        rdfs:label    "valuePattern" .

schema:performerIn  a  rdf:Property ;
        rdfs:comment  "Event that this person is a performer or participant in." ;
        rdfs:label    "performerIn" .

schema:priceRange  a  rdf:Property ;
        rdfs:comment  "The price range of the business, for example ```$$$```." ;
        rdfs:label    "priceRange" .

schema:ShippingRateSettings
        a                rdfs:Class ;
        rdfs:comment     "A ShippingRateSettings represents re-usable pieces of shipping information. It is designed for publication on an URL that may be referenced via the [[shippingSettingsLink]] property of an [[OfferShippingDetails]]. Several occurrences can be published, distinguished and matched (i.e. identified/referenced) by their different values for [[shippingLabel]]." ;
        rdfs:label       "ShippingRateSettings" ;
        rdfs:subClassOf  schema:StructuredValue .

schema:WebApplication
        a                rdfs:Class ;
        rdfs:comment     "Web applications." ;
        rdfs:label       "WebApplication" ;
        rdfs:subClassOf  schema:SoftwareApplication .

schema:VideoObject  a    rdfs:Class ;
        rdfs:comment     "A video file." ;
        rdfs:label       "VideoObject" ;
        rdfs:subClassOf  schema:MediaObject .

schema:programmingLanguage
        a             rdf:Property ;
        rdfs:comment  "The computer programming language." ;
        rdfs:label    "programmingLanguage" .

schema:qualifications
        a             rdf:Property ;
        rdfs:comment  "Specific qualifications required for this role or Occupation." ;
        rdfs:label    "qualifications" .

schema:BankAccount  a    rdfs:Class ;
        rdfs:comment     "A product or service offered by a bank whereby one may deposit, withdraw or transfer money and in some cases be paid interest." ;
        rdfs:label       "BankAccount" ;
        rdfs:subClassOf  schema:FinancialProduct .

schema:postOfficeBoxNumber
        a             rdf:Property ;
        rdfs:comment  "The post office box number for PO box addresses." ;
        rdfs:label    "postOfficeBoxNumber" .

schema:Florist  a        rdfs:Class ;
        rdfs:comment     "A florist." ;
        rdfs:label       "Florist" ;
        rdfs:subClassOf  schema:Store .

schema:currentExchangeRate
        a             rdf:Property ;
        rdfs:comment  "The current price of a currency." ;
        rdfs:label    "currentExchangeRate" .

voc:Municipality  a  rdfs:Class .

schema:flightDistance
        a             rdf:Property ;
        rdfs:comment  "The distance of the flight." ;
        rdfs:label    "flightDistance" .

schema:DigitalDocumentPermissionType
        a                rdfs:Class ;
        rdfs:comment     "A type of permission which can be granted for accessing a digital document." ;
        rdfs:label       "DigitalDocumentPermissionType" ;
        rdfs:subClassOf  schema:Enumeration .

schema:discountCode  a  rdf:Property ;
        rdfs:comment  "Code used to redeem a discount." ;
        rdfs:label    "discountCode" .

schema:quarantineGuidelines
        a             rdf:Property ;
        rdfs:comment  "Guidelines about quarantine rules, e.g. in the context of a pandemic." ;
        rdfs:label    "quarantineGuidelines" .

schema:archiveHeld  a  rdf:Property ;
        rdfs:comment  "Collection, [fonds](https://en.wikipedia.org/wiki/Fonds), or item held, kept or maintained by an [[ArchiveOrganization]]."@en ;
        rdfs:label    "archiveHeld"@en .

schema:openingHoursSpecification
        a             rdf:Property ;
        rdfs:comment  "The opening hours of a certain place." ;
        rdfs:label    "openingHoursSpecification" .

schema:BedAndBreakfast
        a                rdfs:Class ;
        rdfs:comment     "Bed and breakfast.\n<br /><br />\nSee also the <a href=\"/docs/hotels.html\">dedicated document on the use of schema.org for marking up hotels and other forms of accommodations</a>.\n" ;
        rdfs:label       "BedAndBreakfast" ;
        rdfs:subClassOf  schema:LodgingBusiness .

schema:encodingFormat
        a             rdf:Property ;
        rdfs:comment  "Media type typically expressed using a MIME format (see [IANA site](http://www.iana.org/assignments/media-types/media-types.xhtml) and [MDN reference](https://developer.mozilla.org/en-US/docs/Web/HTTP/Basics_of_HTTP/MIME_types)) e.g. application/zip for a SoftwareApplication binary, audio/mpeg for .mp3 etc.).\n\nIn cases where a [[CreativeWork]] has several media type representations, [[encoding]] can be used to indicate each [[MediaObject]] alongside particular [[encodingFormat]] information.\n\nUnregistered or niche encoding and file formats can be indicated instead via the most appropriate URL, e.g. defining Web page or a Wikipedia/Wikidata entry." ;
        rdfs:label    "encodingFormat" .

schema:numberOfPreviousOwners
        a             rdf:Property ;
        rdfs:comment  "The number of owners of the vehicle, including the current one.\\n\\nTypical unit code(s): C62" ;
        rdfs:label    "numberOfPreviousOwners" .

schema:ArriveAction  a   rdfs:Class ;
        rdfs:comment     "The act of arriving at a place. An agent arrives at a destination from a fromLocation, optionally with participants." ;
        rdfs:label       "ArriveAction" ;
        rdfs:subClassOf  schema:MoveAction .

schema:Continent  a      rdfs:Class ;
        rdfs:comment     "One of the continents (for example, Europe or Africa)." ;
        rdfs:label       "Continent" ;
        rdfs:subClassOf  schema:Landform .

schema:wheelbase  a   rdf:Property ;
        rdfs:comment  "The distance between the centers of the front and rear wheels.\\n\\nTypical unit code(s): CMT for centimeters, MTR for meters, INH for inches, FOT for foot/feet" ;
        rdfs:label    "wheelbase" .

schema:GovernmentOffice
        a                rdfs:Class ;
        rdfs:comment     "A government office&#x2014;for example, an IRS or DMV office." ;
        rdfs:label       "GovernmentOffice" ;
        rdfs:subClassOf  schema:LocalBusiness .

schema:Class  a          rdfs:Class ;
        rdfs:comment     "A class, also often called a 'Type'; equivalent to rdfs:Class." ;
        rdfs:label       "Class" ;
        rdfs:subClassOf  schema:Intangible .

schema:source  a  rdf:Property .

schema:address  a     rdf:Property ;
        rdfs:comment  "Physical address of the item." ;
        rdfs:label    "address" .

schema:CreativeWorkSeries
        a                rdfs:Class ;
        rdfs:comment     "A CreativeWorkSeries in schema.org is a group of related items, typically but not necessarily of the same kind. CreativeWorkSeries are usually organized into some order, often chronological. Unlike [[ItemList]] which is a general purpose data structure for lists of things, the emphasis with CreativeWorkSeries is on published materials (written e.g. books and periodicals, or media such as tv, radio and games).\\n\\nSpecific subtypes are available for describing [[TVSeries]], [[RadioSeries]], [[MovieSeries]], [[BookSeries]], [[Periodical]] and [[VideoGameSeries]]. In each case, the [[hasPart]] / [[isPartOf]] properties can be used to relate the CreativeWorkSeries to its parts. The general CreativeWorkSeries type serves largely just to organize these more specific and practical subtypes.\\n\\nIt is common for properties applicable to an item from the series to be usefully applied to the containing group. Schema.org attempts to anticipate some of these cases, but publishers should be free to apply properties of the series parts to the series as a whole wherever they seem appropriate.\n\t  " ;
        rdfs:label       "CreativeWorkSeries" ;
        rdfs:subClassOf  schema:Series , schema:CreativeWork .

schema:vendor  a            rdf:Property ;
        rdfs:comment        "'vendor' is an earlier term for 'seller'." ;
        rdfs:label          "vendor" ;
        rdfs:subPropertyOf  schema:participant .

schema:evidenceOrigin
        a             rdf:Property ;
        rdfs:comment  "Source of the data used to formulate the guidance, e.g. RCT, consensus opinion, etc." ;
        rdfs:label    "evidenceOrigin" .

schema:broadcastTimezone
        a             rdf:Property ;
        rdfs:comment  "The timezone in [ISO 8601 format](http://en.wikipedia.org/wiki/ISO_8601) for which the service bases its broadcasts" ;
        rdfs:label    "broadcastTimezone" .

schema:estimatedSalary
        a             rdf:Property ;
        rdfs:comment  "An estimated salary for a job posting or occupation, based on a variety of variables including, but not limited to industry, job title, and location. Estimated salaries  are often computed by outside organizations rather than the hiring organization, who may not have committed to the estimated value." ;
        rdfs:label    "estimatedSalary" .

schema:SearchResultsPage
        a                rdfs:Class ;
        rdfs:comment     "Web page type: Search results page." ;
        rdfs:label       "SearchResultsPage" ;
        rdfs:subClassOf  schema:WebPage .

schema:WebContent  a     rdfs:Class ;
        rdfs:comment     "WebContent is a type representing all [[WebPage]], [[WebSite]] and [[WebPageElement]] content. It is sometimes the case that detailed distinctions between Web pages, sites and their parts is not always important or obvious. The  [[WebContent]] type makes it easier to describe Web-addressable content without requiring such distinctions to always be stated. (The intent is that the existing types [[WebPage]], [[WebSite]] and [[WebPageElement]] will eventually be declared as subtypes of [[WebContent]])." ;
        rdfs:label       "WebContent" ;
        rdfs:subClassOf  schema:CreativeWork .

schema:HardwareStore  a  rdfs:Class ;
        rdfs:comment     "A hardware store." ;
        rdfs:label       "HardwareStore" ;
        rdfs:subClassOf  schema:Store .

schema:nerveMotor  a  rdf:Property ;
        rdfs:comment  "The neurological pathway extension that involves muscle control." ;
        rdfs:label    "nerveMotor" .

schema:size  a        rdf:Property ;
        rdfs:comment  "A standardized size of a product or creative work, specified either through a simple textual string (for example 'XL', '32Wx34L'), a  QuantitativeValue with a unitCode, or a comprehensive and structured [[SizeSpecification]]; in other cases, the [[width]], [[height]], [[depth]] and [[weight]] properties may be more applicable. " ;
        rdfs:label    "size" .

schema:albumProductionType
        a             rdf:Property ;
        rdfs:comment  "Classification of the album by it's type of content: soundtrack, live album, studio album, etc." ;
        rdfs:label    "albumProductionType" .

schema:NewsMediaOrganization
        a                rdfs:Class ;
        rdfs:comment     "A News/Media organization such as a newspaper or TV station." ;
        rdfs:label       "NewsMediaOrganization" ;
        rdfs:subClassOf  schema:Organization .

schema:SchoolDistrict
        a                rdfs:Class ;
        rdfs:comment     "A School District is an administrative area for the administration of schools." ;
        rdfs:label       "SchoolDistrict" ;
        rdfs:subClassOf  schema:AdministrativeArea .

schema:competencyRequired
        a             rdf:Property ;
        rdfs:comment  "Knowledge, skill, ability or personal attribute that must be demonstrated by a person or other entity in order to do something such as earn an Educational Occupational Credential or understand a LearningResource." ;
        rdfs:label    "competencyRequired" .

schema:Date  a        rdfs:Class ;
        rdfs:comment  "A date value in [ISO 8601 date format](http://en.wikipedia.org/wiki/ISO_8601)." ;
        rdfs:label    "Date" .

schema:ExercisePlan  a   rdfs:Class ;
        rdfs:comment     "Fitness-related activity designed for a specific health-related purpose, including defined exercise routines as well as activity prescribed by a clinician." ;
        rdfs:label       "ExercisePlan" ;
        rdfs:subClassOf  schema:PhysicalActivity , schema:CreativeWork .

schema:numChildren  a  rdf:Property ;
        rdfs:comment  "The number of children staying in the unit." ;
        rdfs:label    "numChildren" .

schema:addressCountry
        a             rdf:Property ;
        rdfs:comment  "The country. For example, USA. You can also provide the two-letter [ISO 3166-1 alpha-2 country code](http://en.wikipedia.org/wiki/ISO_3166-1)." ;
        rdfs:label    "addressCountry" .

schema:thumbnail  a   rdf:Property ;
        rdfs:comment  "Thumbnail image for an image or video." ;
        rdfs:label    "thumbnail" .

schema:eventStatus  a  rdf:Property ;
        rdfs:comment  "An eventStatus of an event represents its status; particularly useful when an event is cancelled or rescheduled." ;
        rdfs:label    "eventStatus" .

schema:BedDetails  a     rdfs:Class ;
        rdfs:comment     "An entity holding detailed information about the available bed types, e.g. the quantity of twin beds for a hotel room. For the single case of just one bed of a certain type, you can use bed directly with a text. See also [[BedType]] (under development)." ;
        rdfs:label       "BedDetails" ;
        rdfs:subClassOf  schema:Intangible .

schema:supply  a            rdf:Property ;
        rdfs:comment        "A sub-property of instrument. A supply consumed when performing instructions or a direction." ;
        rdfs:label          "supply" ;
        rdfs:subPropertyOf  schema:instrument .

schema:isProprietary  a  rdf:Property ;
        rdfs:comment  "True if this item's name is a proprietary/brand name (vs. generic name)." ;
        rdfs:label    "isProprietary" .

schema:value  a       rdf:Property ;
        rdfs:comment  "The value of the quantitative value or property value node.\\n\\n* For [[QuantitativeValue]] and [[MonetaryAmount]], the recommended type for values is 'Number'.\\n* For [[PropertyValue]], it can be 'Text;', 'Number', 'Boolean', or 'StructuredValue'.\\n* Use values from 0123456789 (Unicode 'DIGIT ZERO' (U+0030) to 'DIGIT NINE' (U+0039)) rather than superficially similiar Unicode symbols.\\n* Use '.' (Unicode 'FULL STOP' (U+002E)) rather than ',' to indicate a decimal point. Avoid using these symbols as a readability separator." ;
        rdfs:label    "value" .

schema:MedicalOrganization
        a                rdfs:Class ;
        rdfs:comment     "A medical organization (physical or not), such as hospital, institution or clinic." ;
        rdfs:label       "MedicalOrganization" ;
        rdfs:subClassOf  schema:Organization .

schema:termCode  a    rdf:Property ;
        rdfs:comment  "A code that identifies this [[DefinedTerm]] within a [[DefinedTermSet]]" ;
        rdfs:label    "termCode" .

schema:area  a        rdf:Property ;
        rdfs:comment  "The area within which users can expect to reach the broadcast service." ;
        rdfs:label    "area" .

schema:NonprofitType  a  rdfs:Class ;
        rdfs:comment     "NonprofitType enumerates several kinds of official non-profit types of which a non-profit organization can be." ;
        rdfs:label       "NonprofitType" ;
        rdfs:subClassOf  schema:Enumeration .

schema:hasDefinedTerm
        a             rdf:Property ;
        rdfs:comment  "A Defined Term contained in this term set." ;
        rdfs:label    "hasDefinedTerm" .

schema:lender  a            rdf:Property ;
        rdfs:comment        "A sub property of participant. The person that lends the object being borrowed." ;
        rdfs:label          "lender" ;
        rdfs:subPropertyOf  schema:participant .

schema:stepValue  a   rdf:Property ;
        rdfs:comment  "The stepValue attribute indicates the granularity that is expected (and required) of the value in a PropertyValueSpecification." ;
        rdfs:label    "stepValue" .

schema:inDefinedTermSet
        a                   rdf:Property ;
        rdfs:comment        "A [[DefinedTermSet]] that contains this term." ;
        rdfs:label          "inDefinedTermSet" ;
        rdfs:subPropertyOf  schema:isPartOf .

schema:SocialMediaPosting
        a                rdfs:Class ;
        rdfs:comment     "A post to a social media platform, including blog posts, tweets, Facebook posts, etc." ;
        rdfs:label       "SocialMediaPosting" ;
        rdfs:subClassOf  schema:Article .

schema:itemOffered  a  rdf:Property ;
        rdfs:comment  "An item being offered (or demanded). The transactional nature of the offer or demand is documented using [[businessFunction]], e.g. sell, lease etc. While several common expected types are listed explicitly in this definition, others can be used. Using a second type, such as Product or a subtype of Product, can clarify the nature of the offer." ;
        rdfs:label    "itemOffered" .

schema:readBy  a            rdf:Property ;
        rdfs:comment        "A person who reads (performs) the audiobook." ;
        rdfs:label          "readBy" ;
        rdfs:subPropertyOf  schema:actor .

schema:City  a           rdfs:Class ;
        rdfs:comment     "A city or town." ;
        rdfs:label       "City" ;
        rdfs:subClassOf  schema:AdministrativeArea .

schema:courseWorkload
        a             rdf:Property ;
        rdfs:comment  "The amount of work expected of students taking the course, often provided as a figure per week or per month, and may be broken down by type. For example, \"2 hours of lectures, 1 hour of lab work and 3 hours of independent study per week\"." ;
        rdfs:label    "courseWorkload" .

rdf:type  a     rdf:Property .

schema:sizeSystem  a  rdf:Property ;
        rdfs:comment  "The size system used to identify a product's size. Typically either a standard (for example, \"GS1\" or \"ISO-EN13402\"), country code (for example \"US\" or \"JP\"), or a measuring system (for example \"Metric\" or \"Imperial\")." ;
        rdfs:label    "sizeSystem" .

schema:MedicalScholarlyArticle
        a                rdfs:Class ;
        rdfs:comment     "A scholarly article in the medical domain." ;
        rdfs:label       "MedicalScholarlyArticle" ;
        rdfs:subClassOf  schema:ScholarlyArticle .

schema:ArchiveComponent
        a                rdfs:Class ;
        rdfs:comment     "An intangible type to be applied to any archive content, carrying with it a set of properties required to describe archival items and collections."@en ;
        rdfs:label       "ArchiveComponent"@en ;
        rdfs:subClassOf  schema:CreativeWork .

schema:closes  a      rdf:Property ;
        rdfs:comment  "The closing hour of the place or service on the given day(s) of the week." ;
        rdfs:label    "closes" .

schema:albums  a      rdf:Property ;
        rdfs:comment  "A collection of music albums." ;
        rdfs:label    "albums" .

schema:highPrice  a   rdf:Property ;
        rdfs:comment  "The highest price of all offers available.\\n\\nUsage guidelines:\\n\\n* Use values from 0123456789 (Unicode 'DIGIT ZERO' (U+0030) to 'DIGIT NINE' (U+0039)) rather than superficially similiar Unicode symbols.\\n* Use '.' (Unicode 'FULL STOP' (U+002E)) rather than ',' to indicate a decimal point. Avoid using these symbols as a readability separator." ;
        rdfs:label    "highPrice" .

schema:Bone  a           rdfs:Class ;
        rdfs:comment     "Rigid connective tissue that comprises up the skeletal structure of the human body." ;
        rdfs:label       "Bone" ;
        rdfs:subClassOf  schema:AnatomicalStructure .

schema:Museum  a         rdfs:Class ;
        rdfs:comment     "A museum." ;
        rdfs:label       "Museum" ;
        rdfs:subClassOf  schema:CivicStructure .

schema:EndorsementRating
        a                rdfs:Class ;
        rdfs:comment     "An EndorsementRating is a rating that expresses some level of endorsement, for example inclusion in a \"critic's pick\" blog, a\n\"Like\" or \"+1\" on a social network. It can be considered the [[result]] of an [[EndorseAction]] in which the [[object]] of the action is rated positively by\nsome [[agent]]. As is common elsewhere in schema.org, it is sometimes more useful to describe the results of such an action without explicitly describing the [[Action]].\n\nAn [[EndorsementRating]] may be part of a numeric scale or organized system, but this is not required: having an explicit type for indicating a positive,\nendorsement rating is particularly useful in the absence of numeric scales as it helps consumers understand that the rating is broadly positive.\n" ;
        rdfs:label       "EndorsementRating" ;
        rdfs:subClassOf  schema:Rating .

schema:issueNumber  a       rdf:Property ;
        rdfs:comment        "Identifies the issue of publication; for example, \"iii\" or \"2\"." ;
        rdfs:label          "issueNumber" ;
        rdfs:subPropertyOf  schema:position .

schema:wordCount  a   rdf:Property ;
        rdfs:comment  "The number of words in the text of the Article." ;
        rdfs:label    "wordCount" .

schema:Claim  a          rdfs:Class ;
        rdfs:comment     "A [[Claim]] in Schema.org represents a specific, factually-oriented claim that could be the [[itemReviewed]] in a [[ClaimReview]]. The content of a claim can be summarized with the [[text]] property. Variations on well known claims can have their common identity indicated via [[sameAs]] links, and summarized with a [[name]]. Ideally, a [[Claim]] description includes enough contextual information to minimize the risk of ambiguity or inclarity. In practice, many claims are better understood in the context in which they appear or the interpretations provided by claim reviews.\n\n  Beyond [[ClaimReview]], the Claim type can be associated with related creative works - for example a [[ScholarlyArticle]] or [[Question]] might be [[about]] some [[Claim]].\n\n  At this time, Schema.org does not define any types of relationship between claims. This is a natural area for future exploration.\n  " ;
        rdfs:label       "Claim" ;
        rdfs:subClassOf  schema:CreativeWork .

schema:MiddleSchool  a   rdfs:Class ;
        rdfs:comment     "A middle school (typically for children aged around 11-14, although this varies somewhat)." ;
        rdfs:label       "MiddleSchool" ;
        rdfs:subClassOf  schema:EducationalOrganization .

schema:validIn  a     rdf:Property ;
        rdfs:comment  "The geographic area where a permit or similar thing is valid." ;
        rdfs:label    "validIn" .

schema:AgreeAction  a    rdfs:Class ;
        rdfs:comment     "The act of expressing a consistency of opinion with the object. An agent agrees to/about an object (a proposition, topic or theme) with participants." ;
        rdfs:label       "AgreeAction" ;
        rdfs:subClassOf  schema:ReactAction .

schema:vehicleConfiguration
        a             rdf:Property ;
        rdfs:comment  "A short text indicating the configuration of the vehicle, e.g. '5dr hatchback ST 2.5 MT 225 hp' or 'limited edition'." ;
        rdfs:label    "vehicleConfiguration" .

schema:artEdition  a  rdf:Property ;
        rdfs:comment  "The number of copies when multiple copies of a piece of artwork are produced - e.g. for a limited edition of 20 prints, 'artEdition' refers to the total number of copies (in this example \"20\")." ;
        rdfs:label    "artEdition" .

schema:diagnosis  a   rdf:Property ;
        rdfs:comment  "One or more alternative conditions considered in the differential diagnosis process as output of a diagnosis process." ;
        rdfs:label    "diagnosis" .

schema:duration  a    rdf:Property ;
        rdfs:comment  "The duration of the item (movie, audio recording, event, etc.) in [ISO 8601 date format](http://en.wikipedia.org/wiki/ISO_8601)." ;
        rdfs:label    "duration" .

schema:guidelineSubject
        a             rdf:Property ;
        rdfs:comment  "The medical conditions, treatments, etc. that are the subject of the guideline." ;
        rdfs:label    "guidelineSubject" .

schema:TrainReservation
        a                rdfs:Class ;
        rdfs:comment     "A reservation for train travel.\\n\\nNote: This type is for information about actual reservations, e.g. in confirmation emails or HTML pages with individual confirmations of reservations. For offers of tickets, use [[Offer]]." ;
        rdfs:label       "TrainReservation" ;
        rdfs:subClassOf  schema:Reservation .

schema:actionOption  a      rdf:Property ;
        rdfs:comment        "A sub property of object. The options subject to this action." ;
        rdfs:label          "actionOption" ;
        rdfs:subPropertyOf  schema:object .

schema:MedicalProcedureType
        a                rdfs:Class ;
        rdfs:comment     "An enumeration that describes different types of medical procedures." ;
        rdfs:label       "MedicalProcedureType" ;
        rdfs:subClassOf  schema:MedicalEnumeration .

schema:price  a       rdf:Property ;
        rdfs:comment  "The offer price of a product, or of a price component when attached to PriceSpecification and its subtypes.\\n\\nUsage guidelines:\\n\\n* Use the [[priceCurrency]] property (with standard formats: [ISO 4217 currency format](http://en.wikipedia.org/wiki/ISO_4217) e.g. \"USD\"; [Ticker symbol](https://en.wikipedia.org/wiki/List_of_cryptocurrencies) for cryptocurrencies e.g. \"BTC\"; well known names for [Local Exchange Tradings Systems](https://en.wikipedia.org/wiki/Local_exchange_trading_system) (LETS) and other currency types e.g. \"Ithaca HOUR\") instead of including [ambiguous symbols](http://en.wikipedia.org/wiki/Dollar_sign#Currencies_that_use_the_dollar_or_peso_sign) such as '$' in the value.\\n* Use '.' (Unicode 'FULL STOP' (U+002E)) rather than ',' to indicate a decimal point. Avoid using these symbols as a readability separator.\\n* Note that both [RDFa](http://www.w3.org/TR/xhtml-rdfa-primer/#using-the-content-attribute) and Microdata syntax allow the use of a \"content=\" attribute for publishing simple machine-readable values alongside more human-friendly formatting.\\n* Use values from 0123456789 (Unicode 'DIGIT ZERO' (U+0030) to 'DIGIT NINE' (U+0039)) rather than superficially similiar Unicode symbols.\n      " ;
        rdfs:label    "price" .

schema:servicePhone  a  rdf:Property ;
        rdfs:comment  "The phone number to use to access the service." ;
        rdfs:label    "servicePhone" .

schema:flightNumber  a      rdf:Property ;
        rdfs:comment        "The unique identifier for a flight including the airline IATA code. For example, if describing United flight 110, where the IATA code for United is 'UA', the flightNumber is 'UA110'." ;
        rdfs:label          "flightNumber" ;
        rdfs:subPropertyOf  schema:identifier .

schema:recognizingAuthority
        a             rdf:Property ;
        rdfs:comment  "If applicable, the organization that officially recognizes this entity as part of its endorsed system of medicine." ;
        rdfs:label    "recognizingAuthority" .

schema:availableOnDevice
        a             rdf:Property ;
        rdfs:comment  "Device required to run the application. Used in cases where a specific make/model is required to run the application." ;
        rdfs:label    "availableOnDevice" .

schema:MedicalCode  a    rdfs:Class ;
        rdfs:comment     "A code for a medical entity." ;
        rdfs:label       "MedicalCode" ;
        rdfs:subClassOf  schema:CategoryCode , schema:MedicalIntangible .

schema:duringMedia  a  rdf:Property ;
        rdfs:comment  "A media object representing the circumstances while performing this direction." ;
        rdfs:label    "duringMedia" .

schema:sugarContent  a  rdf:Property ;
        rdfs:comment  "The number of grams of sugar." ;
        rdfs:label    "sugarContent" .

schema:Waterfall  a      rdfs:Class ;
        rdfs:comment     "A waterfall, like Niagara." ;
        rdfs:label       "Waterfall" ;
        rdfs:subClassOf  schema:BodyOfWater .

schema:inBroadcastLineup
        a             rdf:Property ;
        rdfs:comment  "The CableOrSatelliteService offering the channel." ;
        rdfs:label    "inBroadcastLineup" .

schema:WarrantyScope  a  rdfs:Class ;
        rdfs:comment     "A range of of services that will be provided to a customer free of charge in case of a defect or malfunction of a product.\\n\\nCommonly used values:\\n\\n* http://purl.org/goodrelations/v1#Labor-BringIn\\n* http://purl.org/goodrelations/v1#PartsAndLabor-BringIn\\n* http://purl.org/goodrelations/v1#PartsAndLabor-PickUp\n      " ;
        rdfs:label       "WarrantyScope" ;
        rdfs:subClassOf  schema:Enumeration .

schema:loanMortgageMandateAmount
        a             rdf:Property ;
        rdfs:comment  "Amount of mortgage mandate that can be converted into a proper mortgage at a later stage." ;
        rdfs:label    "loanMortgageMandateAmount" .

schema:inventoryLevel
        a             rdf:Property ;
        rdfs:comment  "The current approximate inventory level for the item or items." ;
        rdfs:label    "inventoryLevel" .

schema:Crematorium  a    rdfs:Class ;
        rdfs:comment     "A crematorium." ;
        rdfs:label       "Crematorium" ;
        rdfs:subClassOf  schema:CivicStructure .

schema:httpMethod  a  rdf:Property ;
        rdfs:comment  "An HTTP method that specifies the appropriate HTTP method for a request to an HTTP EntryPoint. Values are capitalized strings as used in HTTP." ;
        rdfs:label    "httpMethod" .

schema:LiquorStore  a    rdfs:Class ;
        rdfs:comment     "A shop that sells alcoholic drinks such as wine, beer, whisky and other spirits." ;
        rdfs:label       "LiquorStore" ;
        rdfs:subClassOf  schema:Store .

schema:yearBuilt  a   rdf:Property ;
        rdfs:comment  "The year an [[Accommodation]] was constructed. This corresponds to the [YearBuilt field in RESO](https://ddwiki.reso.org/display/DDW17/YearBuilt+Field). " ;
        rdfs:label    "yearBuilt" .

schema:seatingCapacity
        a             rdf:Property ;
        rdfs:comment  "The number of persons that can be seated (e.g. in a vehicle), both in terms of the physical space available, and in terms of limitations set by law.\\n\\nTypical unit code(s): C62 for persons " ;
        rdfs:label    "seatingCapacity" .

schema:event  a       rdf:Property ;
        rdfs:comment  "Upcoming or past event associated with this place, organization, or action." ;
        rdfs:label    "event" .

schema:tourBookingPage
        a             rdf:Property ;
        rdfs:comment  "A page providing information on how to book a tour of some [[Place]], such as an [[Accommodation]] or [[ApartmentComplex]] in a real estate setting, as well as other kinds of tours as appropriate." ;
        rdfs:label    "tourBookingPage" .

schema:exchangeRateSpread
        a             rdf:Property ;
        rdfs:comment  "The difference between the price at which a broker or other intermediary buys and sells foreign currency." ;
        rdfs:label    "exchangeRateSpread" .

schema:openingHours  a  rdf:Property ;
        rdfs:comment  "The general opening hours for a business. Opening hours can be specified as a weekly time range, starting with days, then times per day. Multiple days can be listed with commas ',' separating each day. Day or time ranges are specified using a hyphen '-'.\\n\\n* Days are specified using the following two-letter combinations: ```Mo```, ```Tu```, ```We```, ```Th```, ```Fr```, ```Sa```, ```Su```.\\n* Times are specified using 24:00 format. For example, 3pm is specified as ```15:00```, 10am as ```10:00```. \\n* Here is an example: <code>&lt;time itemprop=\"openingHours\" datetime=&quot;Tu,Th 16:00-20:00&quot;&gt;Tuesdays and Thursdays 4-8pm&lt;/time&gt;</code>.\\n* If a business is open 7 days a week, then it can be specified as <code>&lt;time itemprop=&quot;openingHours&quot; datetime=&quot;Mo-Su&quot;&gt;Monday through Sunday, all day&lt;/time&gt;</code>." ;
        rdfs:label    "openingHours" .

schema:HealthPlanCostSharingSpecification
        a                rdfs:Class ;
        rdfs:comment     "A description of costs to the patient under a given network or formulary." ;
        rdfs:label       "HealthPlanCostSharingSpecification" ;
        rdfs:subClassOf  schema:Intangible .

schema:GeospatialGeometry
        a                rdfs:Class ;
        rdfs:comment     "(Eventually to be defined as) a supertype of GeoShape designed to accommodate definitions from Geo-Spatial best practices." ;
        rdfs:label       "GeospatialGeometry" ;
        rdfs:subClassOf  schema:Intangible .

schema:accessibilitySummary
        a             rdf:Property ;
        rdfs:comment  "A human-readable summary of specific accessibility features or deficiencies, consistent with the other accessibility metadata but expressing subtleties such as \"short descriptions are present but long descriptions will be needed for non-visual users\" or \"short descriptions are present and no long descriptions are needed.\"" ;
        rdfs:label    "accessibilitySummary" .

schema:DateTime  a    rdfs:Class ;
        rdfs:comment  "A combination of date and time of day in the form [-]CCYY-MM-DDThh:mm:ss[Z|(+|-)hh:mm] (see Chapter 5.4 of ISO 8601)." ;
        rdfs:label    "DateTime" .

schema:spokenByCharacter
        a             rdf:Property ;
        rdfs:comment  "The (e.g. fictional) character, Person or Organization to whom the quotation is attributed within the containing CreativeWork." ;
        rdfs:label    "spokenByCharacter" .

schema:Festival  a       rdfs:Class ;
        rdfs:comment     "Event type: Festival." ;
        rdfs:label       "Festival" ;
        rdfs:subClassOf  schema:Event .

schema:OfferItemCondition
        a                rdfs:Class ;
        rdfs:comment     "A list of possible conditions for the item." ;
        rdfs:label       "OfferItemCondition" ;
        rdfs:subClassOf  schema:Enumeration .

schema:CompoundPriceSpecification
        a                rdfs:Class ;
        rdfs:comment     "A compound price specification is one that bundles multiple prices that all apply in combination for different dimensions of consumption. Use the name property of the attached unit price specification for indicating the dimension of a price component (e.g. \"electricity\" or \"final cleaning\")." ;
        rdfs:label       "CompoundPriceSpecification" ;
        rdfs:subClassOf  schema:PriceSpecification .

schema:sdLicense  a   rdf:Property ;
        rdfs:comment  "A license document that applies to this structured data, typically indicated by URL." ;
        rdfs:label    "sdLicense" .

schema:hasCourse  a   rdf:Property ;
        rdfs:comment  "A course or class that is one of the learning opportunities that constitute an educational / occupational program. No information is implied about whether the course is mandatory or optional; no guarantee is implied about whether the course will be available to everyone on the program." ;
        rdfs:label    "hasCourse" .

schema:hoursAvailable
        a             rdf:Property ;
        rdfs:comment  "The hours during which this service or contact is available." ;
        rdfs:label    "hoursAvailable" .

schema:GenderType  a     rdfs:Class ;
        rdfs:comment     "An enumeration of genders." ;
        rdfs:label       "GenderType" ;
        rdfs:subClassOf  schema:Enumeration .

schema:Service  a        rdfs:Class ;
        rdfs:comment     "A service provided by an organization, e.g. delivery service, print services, etc." ;
        rdfs:label       "Service" ;
        rdfs:subClassOf  schema:Intangible .

schema:interactivityType
        a             rdf:Property ;
        rdfs:comment  "The predominant mode of learning supported by the learning resource. Acceptable values are 'active', 'expositive', or 'mixed'." ;
        rdfs:label    "interactivityType" .

schema:addOn  a       rdf:Property ;
        rdfs:comment  "An additional offer that can only be obtained in combination with the first base offer (e.g. supplements and extensions that are available for a surcharge)." ;
        rdfs:label    "addOn" .

schema:streetAddress  a  rdf:Property ;
        rdfs:comment  "The street address. For example, 1600 Amphitheatre Pkwy." ;
        rdfs:label    "streetAddress" .

schema:sportsEvent  a       rdf:Property ;
        rdfs:comment        "A sub property of location. The sports event where this action occurred." ;
        rdfs:label          "sportsEvent" ;
        rdfs:subPropertyOf  schema:location .

schema:MedicalGuideline
        a                rdfs:Class ;
        rdfs:comment     "Any recommendation made by a standard society (e.g. ACC/AHA) or consensus statement that denotes how to diagnose and treat a particular condition. Note: this type should be used to tag the actual guideline recommendation; if the guideline recommendation occurs in a larger scholarly article, use MedicalScholarlyArticle to tag the overall article, not this type. Note also: the organization making the recommendation should be captured in the recognizingAuthority base property of MedicalEntity." ;
        rdfs:label       "MedicalGuideline" ;
        rdfs:subClassOf  schema:MedicalEntity .

schema:AggregateOffer
        a                rdfs:Class ;
        rdfs:comment     "When a single product is associated with multiple offers (for example, the same pair of shoes is offered by different merchants), then AggregateOffer can be used.\\n\\nNote: AggregateOffers are normally expected to associate multiple offers that all share the same defined [[businessFunction]] value, or default to http://purl.org/goodrelations/v1#Sell if businessFunction is not explicitly defined." ;
        rdfs:label       "AggregateOffer" ;
        rdfs:subClassOf  schema:Offer .

schema:fatContent  a  rdf:Property ;
        rdfs:comment  "The number of grams of fat." ;
        rdfs:label    "fatContent" .

schema:connectedTo  a  rdf:Property ;
        rdfs:comment  "Other anatomical structures to which this structure is connected." ;
        rdfs:label    "connectedTo" .

schema:yearsInOperation
        a             rdf:Property ;
        rdfs:comment  "The age of the business." ;
        rdfs:label    "yearsInOperation" .

schema:attendee  a    rdf:Property ;
        rdfs:comment  "A person or organization attending the event." ;
        rdfs:label    "attendee" .

schema:discountCurrency
        a             rdf:Property ;
        rdfs:comment  "The currency of the discount.\\n\\nUse standard formats: [ISO 4217 currency format](http://en.wikipedia.org/wiki/ISO_4217) e.g. \"USD\"; [Ticker symbol](https://en.wikipedia.org/wiki/List_of_cryptocurrencies) for cryptocurrencies e.g. \"BTC\"; well known names for [Local Exchange Tradings Systems](https://en.wikipedia.org/wiki/Local_exchange_trading_system) (LETS) and other currency types e.g. \"Ithaca HOUR\"." ;
        rdfs:label    "discountCurrency" .

schema:GameServerStatus
        a                rdfs:Class ;
        rdfs:comment     "Status of a game server." ;
        rdfs:label       "GameServerStatus" ;
        rdfs:subClassOf  schema:StatusEnumeration .

schema:benefitsSummaryUrl
        a             rdf:Property ;
        rdfs:comment  "The URL that goes directly to the summary of benefits and coverage for the specific standard plan or plan variation." ;
        rdfs:label    "benefitsSummaryUrl" .

schema:hasDriveThroughService
        a             rdf:Property ;
        rdfs:comment  "Indicates whether some facility (e.g. [[FoodEstablishment]], [[CovidTestingFacility]]) offers a service that can be used by driving through in a car. In the case of [[CovidTestingFacility]] such facilities could potentially help with social distancing from other potentially-infected users." ;
        rdfs:label    "hasDriveThroughService" .

schema:TravelAction  a   rdfs:Class ;
        rdfs:comment     "The act of traveling from an fromLocation to a destination by a specified mode of transport, optionally with participants." ;
        rdfs:label       "TravelAction" ;
        rdfs:subClassOf  schema:MoveAction .

schema:sport  a       rdf:Property ;
        rdfs:comment  "A type of sport (e.g. Baseball)." ;
        rdfs:label    "sport" .

schema:serviceSmsNumber
        a             rdf:Property ;
        rdfs:comment  "The number to access the service by text message." ;
        rdfs:label    "serviceSmsNumber" .

dcat:Catalog  a  rdfs:Class .

schema:hospitalAffiliation
        a             rdf:Property ;
        rdfs:comment  "A hospital with which the physician or office is affiliated." ;
        rdfs:label    "hospitalAffiliation" .

schema:VideoGame  a      rdfs:Class ;
        rdfs:comment     "A video game is an electronic game that involves human interaction with a user interface to generate visual feedback on a video device." ;
        rdfs:label       "VideoGame" ;
        rdfs:subClassOf  schema:Game , schema:SoftwareApplication .

schema:category  a    rdf:Property ;
        rdfs:comment  "A category for the item. Greater signs or slashes can be used to informally indicate a category hierarchy." ;
        rdfs:label    "category" .

schema:regionsAllowed
        a             rdf:Property ;
        rdfs:comment  "The regions where the media is allowed. If not specified, then it's assumed to be allowed everywhere. Specify the countries in [ISO 3166 format](http://en.wikipedia.org/wiki/ISO_3166)." ;
        rdfs:label    "regionsAllowed" .

schema:RentalCarReservation
        a                rdfs:Class ;
        rdfs:comment     "A reservation for a rental car.\\n\\nNote: This type is for information about actual reservations, e.g. in confirmation emails or HTML pages with individual confirmations of reservations." ;
        rdfs:label       "RentalCarReservation" ;
        rdfs:subClassOf  schema:Reservation .

schema:MedicalRiskScore
        a                rdfs:Class ;
        rdfs:comment     "A simple system that adds up the number of risk factors to yield a score that is associated with prognosis, e.g. CHAD score, TIMI risk score." ;
        rdfs:label       "MedicalRiskScore" ;
        rdfs:subClassOf  schema:MedicalRiskEstimator .

schema:occupationalCategory
        a             rdf:Property ;
        rdfs:comment  "A category describing the job, preferably using a term from a taxonomy such as [BLS O*NET-SOC](http://www.onetcenter.org/taxonomy.html), [ISCO-08](https://www.ilo.org/public/english/bureau/stat/isco/isco08/) or similar, with the property repeated for each applicable value. Ideally the taxonomy should be identified, and both the textual label and formal code for the category should be provided.\\n\nNote: for historical reasons, any textual label and formal code provided as a literal may be assumed to be from O*NET-SOC." ;
        rdfs:label    "occupationalCategory" .

schema:publicAccess  a  rdf:Property ;
        rdfs:comment  "A flag to signal that the [[Place]] is open to public visitors.  If this property is omitted there is no assumed default boolean value" ;
        rdfs:label    "publicAccess" .

schema:announcementLocation
        a                   rdf:Property ;
        rdfs:comment        "Indicates a specific [[CivicStructure]] or [[LocalBusiness]] associated with the SpecialAnnouncement. For example, a specific testing facility or business with special opening hours. For a larger geographic region like a quarantine of an entire region, use [[spatialCoverage]]." ;
        rdfs:label          "announcementLocation" ;
        rdfs:subPropertyOf  schema:spatialCoverage .

schema:signDetected  a  rdf:Property ;
        rdfs:comment  "A sign detected by the test." ;
        rdfs:label    "signDetected" .

schema:upvoteCount  a  rdf:Property ;
        rdfs:comment  "The number of upvotes this question, answer or comment has received from the community." ;
        rdfs:label    "upvoteCount" .

schema:CDCPMDRecord  a   rdfs:Class ;
        rdfs:comment     "A CDCPMDRecord is a data structure representing a record in a CDC tabular data format\n      used for hospital data reporting. See [documentation](/docs/cdc-covid.html) for details, and the linked CDC materials for authoritative\n      definitions used as the source here.\n      " ;
        rdfs:label       "CDCPMDRecord" ;
        rdfs:subClassOf  schema:StructuredValue .

schema:branch  a      rdf:Property ;
        rdfs:comment  "The branches that delineate from the nerve bundle. Not to be confused with [[branchOf]]." ;
        rdfs:label    "branch" .

schema:clincalPharmacology
        a             rdf:Property ;
        rdfs:comment  "Description of the absorption and elimination of drugs, including their concentration (pharmacokinetics, pK) and biological effects (pharmacodynamics, pD)." ;
        rdfs:label    "clincalPharmacology" .

schema:MusicAlbumReleaseType
        a                rdfs:Class ;
        rdfs:comment     "The kind of release which this album is: single, EP or album." ;
        rdfs:label       "MusicAlbumReleaseType" ;
        rdfs:subClassOf  schema:Enumeration .

schema:MedicalObservationalStudyDesign
        a                rdfs:Class ;
        rdfs:comment     "Design models for observational medical studies. Enumerated type." ;
        rdfs:label       "MedicalObservationalStudyDesign" ;
        rdfs:subClassOf  schema:MedicalEnumeration .

schema:LymphaticVessel
        a                rdfs:Class ;
        rdfs:comment     "A type of blood vessel that specifically carries lymph fluid unidirectionally toward the heart." ;
        rdfs:label       "LymphaticVessel" ;
        rdfs:subClassOf  schema:Vessel .

schema:serverStatus  a  rdf:Property ;
        rdfs:comment  "Status of a game server." ;
        rdfs:label    "serverStatus" .

schema:offerCount  a  rdf:Property ;
        rdfs:comment  "The number of offers for the product." ;
        rdfs:label    "offerCount" .

schema:box  a         rdf:Property ;
        rdfs:comment  "A box is the area enclosed by the rectangle formed by two points. The first point is the lower corner, the second point is the upper corner. A box is expressed as two points separated by a space character." ;
        rdfs:label    "box" .

schema:vehicleEngine  a  rdf:Property ;
        rdfs:comment  "Information about the engine or engines of the vehicle." ;
        rdfs:label    "vehicleEngine" .

schema:acceptedAnswer
        a                   rdf:Property ;
        rdfs:comment        "The answer(s) that has been accepted as best, typically on a Question/Answer site. Sites vary in their selection mechanisms, e.g. drawing on community opinion and/or the view of the Question author." ;
        rdfs:label          "acceptedAnswer" ;
        rdfs:subPropertyOf  schema:suggestedAnswer .

schema:Organization  a   rdfs:Class ;
        rdfs:comment     "An organization such as a school, NGO, corporation, club, etc." ;
        rdfs:label       "Organization" ;
        rdfs:subClassOf  schema:Thing .

schema:award  a       rdf:Property ;
        rdfs:comment  "An award won by or for this item." ;
        rdfs:label    "award" .

schema:actionPlatform
        a             rdf:Property ;
        rdfs:comment  "The high level platform(s) where the Action can be performed for the given URL. To specify a specific application or operating system instance, use actionApplication." ;
        rdfs:label    "actionPlatform" .

schema:specialty  a   rdf:Property ;
        rdfs:comment  "One of the domain specialities to which this web page's content applies." ;
        rdfs:label    "specialty" .

schema:WearAction  a     rdfs:Class ;
        rdfs:comment     "The act of dressing oneself in clothing." ;
        rdfs:label       "WearAction" ;
        rdfs:subClassOf  schema:UseAction .

schema:MusicEvent  a     rdfs:Class ;
        rdfs:comment     "Event type: Music event." ;
        rdfs:label       "MusicEvent" ;
        rdfs:subClassOf  schema:Event .

schema:freeShippingThreshold
        a             rdf:Property ;
        rdfs:comment  "A monetary value above which (or equal to) the shipping rate becomes free. Intended to be used via an [[OfferShippingDetails]] with [[shippingSettingsLink]] matching this [[ShippingRateSettings]]." ;
        rdfs:label    "freeShippingThreshold" .

rdfs:Class  a   rdfs:Class .

schema:merchant  a    rdf:Property ;
        rdfs:comment  "'merchant' is an out-dated term for 'seller'." ;
        rdfs:label    "merchant" .

schema:accountOverdraftLimit
        a             rdf:Property ;
        rdfs:comment  "An overdraft is an extension of credit from a lending institution when an account reaches zero. An overdraft allows the individual to continue withdrawing money even if the account has no funds in it. Basically the bank allows people to borrow a set amount of money." ;
        rdfs:label    "accountOverdraftLimit" .

schema:Pond  a           rdfs:Class ;
        rdfs:comment     "A pond." ;
        rdfs:label       "Pond" ;
        rdfs:subClassOf  schema:BodyOfWater .

schema:MaximumDoseSchedule
        a                rdfs:Class ;
        rdfs:comment     "The maximum dosing schedule considered safe for a drug or supplement as recommended by an authority or by the drug/supplement's manufacturer. Capture the recommending authority in the recognizingAuthority property of MedicalEntity." ;
        rdfs:label       "MaximumDoseSchedule" ;
        rdfs:subClassOf  schema:DoseSchedule .

schema:homeTeam  a          rdf:Property ;
        rdfs:comment        "The home team in a sports event." ;
        rdfs:label          "homeTeam" ;
        rdfs:subPropertyOf  schema:competitor .

schema:legislationIdentifier
        a                   rdf:Property ;
        rdfs:comment        "An identifier for the legislation. This can be either a string-based identifier, like the CELEX at EU level or the NOR in France, or a web-based, URL/URI identifier, like an ELI (European Legislation Identifier) or an URN-Lex." ;
        rdfs:label          "legislationIdentifier" ;
        rdfs:subPropertyOf  schema:identifier .

schema:printPage  a   rdf:Property ;
        rdfs:comment  "If this NewsArticle appears in print, this field indicates the name of the page on which the article is found. Please note that this field is intended for the exact page name (e.g. A5, B18)." ;
        rdfs:label    "printPage" .

schema:byMonthDay  a  rdf:Property ;
        rdfs:comment  "Defines the day(s) of the month on which a recurring [[Event]] takes place. Specified as an [[Integer]] between 1-31." ;
        rdfs:label    "byMonthDay" .

schema:seatRow  a     rdf:Property ;
        rdfs:comment  "The row location of the reserved seat (e.g., B)." ;
        rdfs:label    "seatRow" .

schema:engineDisplacement
        a             rdf:Property ;
        rdfs:comment  "The volume swept by all of the pistons inside the cylinders of an internal combustion engine in a single movement. \\n\\nTypical unit code(s): CMQ for cubic centimeter, LTR for liters, INQ for cubic inches\\n* Note 1: You can link to information about how the given value has been determined using the [[valueReference]] property.\\n* Note 2: You can use [[minValue]] and [[maxValue]] to indicate ranges." ;
        rdfs:label    "engineDisplacement" .

schema:courseMode  a  rdf:Property ;
        rdfs:comment  "The medium or means of delivery of the course instance or the mode of study, either as a text label (e.g. \"online\", \"onsite\" or \"blended\"; \"synchronous\" or \"asynchronous\"; \"full-time\" or \"part-time\") or as a URL reference to a term from a controlled vocabulary (e.g. https://ceds.ed.gov/element/001311#Asynchronous )." ;
        rdfs:label    "courseMode" .

schema:artform  a     rdf:Property ;
        rdfs:comment  "e.g. Painting, Drawing, Sculpture, Print, Photograph, Assemblage, Collage, etc." ;
        rdfs:label    "artform" .

schema:financialAidEligible
        a             rdf:Property ;
        rdfs:comment  "A financial aid type or program which students may use to pay for tuition or fees associated with the program." ;
        rdfs:label    "financialAidEligible" .

schema:EnergyEfficiencyEnumeration
        a                rdfs:Class ;
        rdfs:comment     "Enumerates energy efficiency levels (also known as \"classes\" or \"ratings\") and certifications that are part of several international energy efficiency standards." ;
        rdfs:label       "EnergyEfficiencyEnumeration" ;
        rdfs:subClassOf  schema:Enumeration .

schema:bookEdition  a  rdf:Property ;
        rdfs:comment  "The edition of the book." ;
        rdfs:label    "bookEdition" .

schema:BarOrPub  a       rdfs:Class ;
        rdfs:comment     "A bar or pub." ;
        rdfs:label       "BarOrPub" ;
        rdfs:subClassOf  schema:FoodEstablishment .

schema:isVariantOf  a  rdf:Property ;
        rdfs:comment  "Indicates the kind of product that this is a variant of. In the case of [[ProductModel]], this is a pointer (from a ProductModel) to a base product from which this product is a variant. It is safe to infer that the variant inherits all product features from the base model, unless defined locally. This is not transitive. In the case of a [[ProductGroup]], the group description also serves as a template, representing a set of Products that vary on explicitly defined, specific dimensions only (so it defines both a set of variants, as well as which values distinguish amongst those variants). When used with [[ProductGroup]], this property can apply to any [[Product]] included in the group." ;
        rdfs:label    "isVariantOf" .

schema:masthead  a          rdf:Property ;
        rdfs:comment        "For a [[NewsMediaOrganization]], a link to the masthead page or a page listing top editorial management." ;
        rdfs:label          "masthead" ;
        rdfs:subPropertyOf  schema:publishingPrinciples .

schema:availabilityEnds
        a             rdf:Property ;
        rdfs:comment  "The end of the availability of the product or service included in the offer." ;
        rdfs:label    "availabilityEnds" .

schema:AmusementPark  a  rdfs:Class ;
        rdfs:comment     "An amusement park." ;
        rdfs:label       "AmusementPark" ;
        rdfs:subClassOf  schema:EntertainmentBusiness .

schema:recourseLoan  a  rdf:Property ;
        rdfs:comment  "The only way you get the money back in the event of default is the security. Recourse is where you still have the opportunity to go back to the borrower for the rest of the money." ;
        rdfs:label    "recourseLoan" .

schema:alumniOf  a    rdf:Property ;
        rdfs:comment  "An organization that the person is an alumni of." ;
        rdfs:label    "alumniOf" .

schema:reviewRating  a  rdf:Property ;
        rdfs:comment  "The rating given in this review. Note that reviews can themselves be rated. The ```reviewRating``` applies to rating given by the review. The [[aggregateRating]] property applies to the review itself, as a creative work." ;
        rdfs:label    "reviewRating" .

schema:educationalFramework
        a             rdf:Property ;
        rdfs:comment  "The framework to which the resource being described is aligned." ;
        rdfs:label    "educationalFramework" .

dcat:Distribution  a  rdfs:Class .

schema:playersOnline  a  rdf:Property ;
        rdfs:comment  "Number of players on the server." ;
        rdfs:label    "playersOnline" .

schema:HobbyShop  a      rdfs:Class ;
        rdfs:comment     "A store that sells materials useful or necessary for various hobbies." ;
        rdfs:label       "HobbyShop" ;
        rdfs:subClassOf  schema:Store .

schema:MedicalBusiness
        a                rdfs:Class ;
        rdfs:comment     "A particular physical or virtual business of an organization for medical purposes. Examples of MedicalBusiness include differents business run by health professionals." ;
        rdfs:label       "MedicalBusiness" ;
        rdfs:subClassOf  schema:LocalBusiness .

schema:PostalCodeRangeSpecification
        a                rdfs:Class ;
        rdfs:comment     "Indicates a range of postalcodes, usually defined as the set of valid codes between [[postalCodeBegin]] and [[postalCodeEnd]], inclusively." ;
        rdfs:label       "PostalCodeRangeSpecification" ;
        rdfs:subClassOf  schema:StructuredValue .

schema:BlogPosting  a    rdfs:Class ;
        rdfs:comment     "A blog post." ;
        rdfs:label       "BlogPosting" ;
        rdfs:subClassOf  schema:SocialMediaPosting .

schema:BuddhistTemple
        a                rdfs:Class ;
        rdfs:comment     "A Buddhist temple." ;
        rdfs:label       "BuddhistTemple" ;
        rdfs:subClassOf  schema:PlaceOfWorship .

schema:billingPeriod  a  rdf:Property ;
        rdfs:comment  "The time interval used to compute the invoice." ;
        rdfs:label    "billingPeriod" .

schema:RecommendedDoseSchedule
        a                rdfs:Class ;
        rdfs:comment     "A recommended dosing schedule for a drug or supplement as prescribed or recommended by an authority or by the drug/supplement's manufacturer. Capture the recommending authority in the recognizingAuthority property of MedicalEntity." ;
        rdfs:label       "RecommendedDoseSchedule" ;
        rdfs:subClassOf  schema:DoseSchedule .

schema:broadcastServiceTier
        a             rdf:Property ;
        rdfs:comment  "The type of service required to have access to the channel (e.g. Standard or Premium)." ;
        rdfs:label    "broadcastServiceTier" .

schema:fundedItem  a  rdf:Property ;
        rdfs:comment  "Indicates an item funded or sponsored through a [[Grant]]." ;
        rdfs:label    "fundedItem" .

schema:suggestedMinAge
        a             rdf:Property ;
        rdfs:comment  "Minimum recommended age in years for the audience or user." ;
        rdfs:label    "suggestedMinAge" .

schema:bookingAgent  a  rdf:Property ;
        rdfs:comment  "'bookingAgent' is an out-dated term indicating a 'broker' that serves as a booking agent." ;
        rdfs:label    "bookingAgent" .

schema:paymentMethod  a  rdf:Property ;
        rdfs:comment  "The name of the credit card or other method of payment for the order." ;
        rdfs:label    "paymentMethod" .

schema:postalCodePrefix
        a             rdf:Property ;
        rdfs:comment  "A defined range of postal codes indicated by a common textual prefix. Used for non-numeric systems such as UK." ;
        rdfs:label    "postalCodePrefix" .

schema:arrivalTime  a  rdf:Property ;
        rdfs:comment  "The expected arrival time." ;
        rdfs:label    "arrivalTime" .

schema:observationDate
        a             rdf:Property ;
        rdfs:comment  "The observationDate of an [[Observation]]." ;
        rdfs:label    "observationDate" .

schema:member  a      rdf:Property ;
        rdfs:comment  "A member of an Organization or a ProgramMembership. Organizations can be members of organizations; ProgramMembership is typically for individuals." ;
        rdfs:label    "member" .

schema:recipeCategory
        a             rdf:Property ;
        rdfs:comment  "The category of the recipe—for example, appetizer, entree, etc." ;
        rdfs:label    "recipeCategory" .

schema:loanTerm  a          rdf:Property ;
        rdfs:comment        "The duration of the loan or credit agreement." ;
        rdfs:label          "loanTerm" ;
        rdfs:subPropertyOf  schema:duration .

schema:checkinTime  a  rdf:Property ;
        rdfs:comment  "The earliest someone may check into a lodging establishment." ;
        rdfs:label    "checkinTime" .

schema:encodingType  a  rdf:Property ;
        rdfs:comment  "The supported encoding type(s) for an EntryPoint request." ;
        rdfs:label    "encodingType" .

schema:shippingSettingsLink
        a             rdf:Property ;
        rdfs:comment  "Link to a page containing [[ShippingRateSettings]] and [[DeliveryTimeSettings]] details." ;
        rdfs:label    "shippingSettingsLink" .

schema:athlete  a     rdf:Property ;
        rdfs:comment  "A person that acts as performing member of a sports team; a player as opposed to a coach." ;
        rdfs:label    "athlete" .

schema:recipeIngredient
        a                   rdf:Property ;
        rdfs:comment        "A single ingredient used in the recipe, e.g. sugar, flour or garlic." ;
        rdfs:label          "recipeIngredient" ;
        rdfs:subPropertyOf  schema:supply .

schema:StatisticalPopulation
        a                rdfs:Class ;
        rdfs:comment     "A StatisticalPopulation is a set of instances of a certain given type that satisfy some set of constraints. The property [[populationType]] is used to specify the type. Any property that can be used on instances of that type can appear on the statistical population. For example, a [[StatisticalPopulation]] representing all [[Person]]s with a [[homeLocation]] of East Podunk California, would be described by applying the appropriate [[homeLocation]] and [[populationType]] properties to a [[StatisticalPopulation]] item that stands for that set of people.\nThe properties [[numConstraints]] and [[constrainingProperty]] are used to specify which of the populations properties are used to specify the population. Note that the sense of \"population\" used here is the general sense of a statistical\npopulation, and does not imply that the population consists of people. For example, a [[populationType]] of [[Event]] or [[NewsArticle]] could be used. See also [[Observation]], and the [data and datasets](/docs/data-and-datasets.html) overview for more details.\n  " ;
        rdfs:label       "StatisticalPopulation" ;
        rdfs:subClassOf  schema:Intangible .

schema:confirmationNumber
        a                   rdf:Property ;
        rdfs:comment        "A number that confirms the given order or payment has been received." ;
        rdfs:label          "confirmationNumber" ;
        rdfs:subPropertyOf  schema:identifier .

schema:MedicalCause  a   rdfs:Class ;
        rdfs:comment     "The causative agent(s) that are responsible for the pathophysiologic process that eventually results in a medical condition, symptom or sign. In this schema, unless otherwise specified this is meant to be the proximate cause of the medical condition, symptom or sign. The proximate cause is defined as the causative agent that most directly results in the medical condition, symptom or sign. For example, the HIV virus could be considered a cause of AIDS. Or in a diagnostic context, if a patient fell and sustained a hip fracture and two days later sustained a pulmonary embolism which eventuated in a cardiac arrest, the cause of the cardiac arrest (the proximate cause) would be the pulmonary embolism and not the fall. Medical causes can include cardiovascular, chemical, dermatologic, endocrine, environmental, gastroenterologic, genetic, hematologic, gynecologic, iatrogenic, infectious, musculoskeletal, neurologic, nutritional, obstetric, oncologic, otolaryngologic, pharmacologic, psychiatric, pulmonary, renal, rheumatologic, toxic, traumatic, or urologic causes; medical conditions can be causes as well." ;
        rdfs:label       "MedicalCause" ;
        rdfs:subClassOf  schema:MedicalEntity .

schema:dropoffTime  a  rdf:Property ;
        rdfs:comment  "When a rental car can be dropped off." ;
        rdfs:label    "dropoffTime" .

schema:TennisComplex  a  rdfs:Class ;
        rdfs:comment     "A tennis complex." ;
        rdfs:label       "TennisComplex" ;
        rdfs:subClassOf  schema:SportsActivityLocation .

schema:MediaReview  a    rdfs:Class ;
        rdfs:comment     "A [[MediaReview]] is a more specialized form of Review dedicated to the evaluation of media content online, typically in the context of fact-checking and misinformation.\n    For more general reviews of media in the broader sense, use [[UserReview]], [[CriticReview]] or other [[Review]] types. This definition is\n    a work in progress. While the [[MediaManipulationRatingEnumeration]] list reflects significant community review amongst fact-checkers and others working\n    to combat misinformation, the specific structures for representing media objects, their versions and publication context, is still evolving. Similarly, best practices for the relationship between [[MediaReview]] and [[ClaimReview]] markup has not yet been finalized." ;
        rdfs:label       "MediaReview" ;
        rdfs:subClassOf  schema:Review .

schema:urlTemplate  a  rdf:Property ;
        rdfs:comment  "An url template (RFC6570) that will be used to construct the target of the execution of the action." ;
        rdfs:label    "urlTemplate" .

schema:videoFrameSize
        a             rdf:Property ;
        rdfs:comment  "The frame size of the video." ;
        rdfs:label    "videoFrameSize" .

schema:ReceiveAction  a  rdfs:Class ;
        rdfs:comment     "The act of physically/electronically taking delivery of an object that has been transferred from an origin to a destination. Reciprocal of SendAction.\\n\\nRelated actions:\\n\\n* [[SendAction]]: The reciprocal of ReceiveAction.\\n* [[TakeAction]]: Unlike TakeAction, ReceiveAction does not imply that the ownership has been transfered (e.g. I can receive a package, but it does not mean the package is now mine)." ;
        rdfs:label       "ReceiveAction" ;
        rdfs:subClassOf  schema:TransferAction .

schema:AboutPage  a      rdfs:Class ;
        rdfs:comment     "Web page type: About page." ;
        rdfs:label       "AboutPage" ;
        rdfs:subClassOf  schema:WebPage .

schema:trailer  a     rdf:Property ;
        rdfs:comment  "The trailer of a movie or tv/radio series, season, episode, etc." ;
        rdfs:label    "trailer" .

schema:constrainingProperty
        a             rdf:Property ;
        rdfs:comment  "Indicates a property used as a constraint to define a [[StatisticalPopulation]] with respect to the set of entities\n  corresponding to an indicated type (via [[populationType]])." ;
        rdfs:label    "constrainingProperty" .

schema:opponent  a          rdf:Property ;
        rdfs:comment        "A sub property of participant. The opponent on this action." ;
        rdfs:label          "opponent" ;
        rdfs:subPropertyOf  schema:participant .

schema:TreatmentIndication
        a                rdfs:Class ;
        rdfs:comment     "An indication for treating an underlying condition, symptom, etc." ;
        rdfs:label       "TreatmentIndication" ;
        rdfs:subClassOf  schema:MedicalIndication .

schema:grantee  a     rdf:Property ;
        rdfs:comment  "The person, organization, contact point, or audience that has been granted this permission." ;
        rdfs:label    "grantee" .

schema:applicationDeadline
        a             rdf:Property ;
        rdfs:comment  "The date at which the program stops collecting applications for the next enrollment cycle." ;
        rdfs:label    "applicationDeadline" .

schema:transFatContent
        a             rdf:Property ;
        rdfs:comment  "The number of grams of trans fat." ;
        rdfs:label    "transFatContent" .

schema:aspect  a      rdf:Property ;
        rdfs:comment  "An aspect of medical practice that is considered on the page, such as 'diagnosis', 'treatment', 'causes', 'prognosis', 'etiology', 'epidemiology', etc." ;
        rdfs:label    "aspect" .

schema:PaymentStatusType
        a                rdfs:Class ;
        rdfs:comment     "A specific payment status. For example, PaymentDue, PaymentComplete, etc." ;
        rdfs:label       "PaymentStatusType" ;
        rdfs:subClassOf  schema:StatusEnumeration .

schema:hasDeliveryMethod
        a             rdf:Property ;
        rdfs:comment  "Method used for delivery or shipping." ;
        rdfs:label    "hasDeliveryMethod" .

schema:FoodEvent  a      rdfs:Class ;
        rdfs:comment     "Event type: Food event." ;
        rdfs:label       "FoodEvent" ;
        rdfs:subClassOf  schema:Event .

schema:DeleteAction  a   rdfs:Class ;
        rdfs:comment     "The act of editing a recipient by removing one of its objects." ;
        rdfs:label       "DeleteAction" ;
        rdfs:subClassOf  schema:UpdateAction .

schema:StructuredValue
        a                rdfs:Class ;
        rdfs:comment     "Structured values are used when the value of a property has a more complex structure than simply being a textual value or a reference to another thing." ;
        rdfs:label       "StructuredValue" ;
        rdfs:subClassOf  schema:Intangible .

schema:employmentType
        a             rdf:Property ;
        rdfs:comment  "Type of employment (e.g. full-time, part-time, contract, temporary, seasonal, internship)." ;
        rdfs:label    "employmentType" .

schema:byMonth  a     rdf:Property ;
        rdfs:comment  "Defines the month(s) of the year on which a recurring [[Event]] takes place. Specified as an [[Integer]] between 1-12. January is 1." ;
        rdfs:label    "byMonth" .

schema:deliveryLeadTime
        a             rdf:Property ;
        rdfs:comment  "The typical delay between the receipt of the order and the goods either leaving the warehouse or being prepared for pickup, in case the delivery method is on site pickup." ;
        rdfs:label    "deliveryLeadTime" .

schema:Report  a         rdfs:Class ;
        rdfs:comment     "A Report generated by governmental or non-governmental organization." ;
        rdfs:label       "Report" ;
        rdfs:subClassOf  schema:Article .

schema:equal  a       rdf:Property ;
        rdfs:comment  "This ordering relation for qualitative values indicates that the subject is equal to the object." ;
        rdfs:label    "equal" .

schema:Consortium  a     rdfs:Class ;
        rdfs:comment     "A Consortium is a membership [[Organization]] whose members are typically Organizations." ;
        rdfs:label       "Consortium" ;
        rdfs:subClassOf  schema:Organization .

schema:paymentMethodId
        a             rdf:Property ;
        rdfs:comment  "An identifier for the method of payment used (e.g. the last 4 digits of the credit card)." ;
        rdfs:label    "paymentMethodId" .

schema:currency  a    rdf:Property ;
        rdfs:comment  "The currency in which the monetary amount is expressed.\\n\\nUse standard formats: [ISO 4217 currency format](http://en.wikipedia.org/wiki/ISO_4217) e.g. \"USD\"; [Ticker symbol](https://en.wikipedia.org/wiki/List_of_cryptocurrencies) for cryptocurrencies e.g. \"BTC\"; well known names for [Local Exchange Tradings Systems](https://en.wikipedia.org/wiki/Local_exchange_trading_system) (LETS) and other currency types e.g. \"Ithaca HOUR\"." ;
        rdfs:label    "currency" .

schema:Collection  a     rdfs:Class ;
        rdfs:comment     "A collection of items e.g. creative works or products." ;
        rdfs:label       "Collection" ;
        rdfs:subClassOf  schema:CreativeWork .

schema:CollegeOrUniversity
        a                rdfs:Class ;
        rdfs:comment     "A college, university, or other third-level educational institution." ;
        rdfs:label       "CollegeOrUniversity" ;
        rdfs:subClassOf  schema:EducationalOrganization .

schema:itemShipped  a  rdf:Property ;
        rdfs:comment  "Item(s) being shipped." ;
        rdfs:label    "itemShipped" .

schema:PriceSpecification
        a                rdfs:Class ;
        rdfs:comment     "A structured value representing a price or price range. Typically, only the subclasses of this type are used for markup. It is recommended to use [[MonetaryAmount]] to describe independent amounts of money such as a salary, credit card limits, etc." ;
        rdfs:label       "PriceSpecification" ;
        rdfs:subClassOf  schema:StructuredValue .

schema:dataFeedElement
        a             rdf:Property ;
        rdfs:comment  "An item within in a data feed. Data feeds may have many elements." ;
        rdfs:label    "dataFeedElement" .

schema:FoodEstablishmentReservation
        a                rdfs:Class ;
        rdfs:comment     "A reservation to dine at a food-related business.\\n\\nNote: This type is for information about actual reservations, e.g. in confirmation emails or HTML pages with individual confirmations of reservations." ;
        rdfs:label       "FoodEstablishmentReservation" ;
        rdfs:subClassOf  schema:Reservation .

schema:PostOffice  a     rdfs:Class ;
        rdfs:comment     "A post office." ;
        rdfs:label       "PostOffice" ;
        rdfs:subClassOf  schema:GovernmentOffice .

schema:gtin8  a             rdf:Property ;
        rdfs:comment        "The GTIN-8 code of the product, or the product to which the offer refers. This code is also known as EAN/UCC-8 or 8-digit EAN. See [GS1 GTIN Summary](http://www.gs1.org/barcodes/technical/idkeys/gtin) for more details." ;
        rdfs:label          "gtin8" ;
        rdfs:subPropertyOf  schema:identifier , schema:gtin .

schema:drugUnit  a    rdf:Property ;
        rdfs:comment  "The unit in which the drug is measured, e.g. '5 mg tablet'." ;
        rdfs:label    "drugUnit" .

schema:episodeNumber  a     rdf:Property ;
        rdfs:comment        "Position of the episode within an ordered group of episodes." ;
        rdfs:label          "episodeNumber" ;
        rdfs:subPropertyOf  schema:position .

schema:healthPlanDrugTier
        a             rdf:Property ;
        rdfs:comment  "The tier(s) of drugs offered by this formulary or insurance plan." ;
        rdfs:label    "healthPlanDrugTier" .

schema:lowPrice  a    rdf:Property ;
        rdfs:comment  "The lowest price of all offers available.\\n\\nUsage guidelines:\\n\\n* Use values from 0123456789 (Unicode 'DIGIT ZERO' (U+0030) to 'DIGIT NINE' (U+0039)) rather than superficially similiar Unicode symbols.\\n* Use '.' (Unicode 'FULL STOP' (U+002E)) rather than ',' to indicate a decimal point. Avoid using these symbols as a readability separator." ;
        rdfs:label    "lowPrice" .

schema:DatedMoneySpecification
        a                rdfs:Class ;
        rdfs:comment     "A DatedMoneySpecification represents monetary values with optional start and end dates. For example, this could represent an employee's salary over a specific period of time. __Note:__ This type has been superseded by [[MonetaryAmount]] use of that type is recommended" ;
        rdfs:label       "DatedMoneySpecification" ;
        rdfs:subClassOf  schema:StructuredValue .

schema:inStoreReturnsOffered
        a             rdf:Property ;
        rdfs:comment  "Are in-store returns offered?" ;
        rdfs:label    "inStoreReturnsOffered" .

schema:bodyType  a    rdf:Property ;
        rdfs:comment  "Indicates the design and body style of the vehicle (e.g. station wagon, hatchback, etc.)." ;
        rdfs:label    "bodyType" .

schema:acquiredFrom  a  rdf:Property ;
        rdfs:comment  "The organization or person from which the product was acquired." ;
        rdfs:label    "acquiredFrom" .

schema:supportingData
        a             rdf:Property ;
        rdfs:comment  "Supporting data for a SoftwareApplication." ;
        rdfs:label    "supportingData" .

schema:childMinAge  a  rdf:Property ;
        rdfs:comment  "Minimal age of the child." ;
        rdfs:label    "childMinAge" .

schema:Article  a        rdfs:Class ;
        rdfs:comment     "An article, such as a news article or piece of investigative report. Newspapers and magazines have articles of many different types and this is intended to cover them all.\\n\\nSee also [blog post](http://blog.schema.org/2014/09/schemaorg-support-for-bibliographic_2.html)." ;
        rdfs:label       "Article" ;
        rdfs:subClassOf  schema:CreativeWork .

schema:translationOfWork
        a             rdf:Property ;
        rdfs:comment  "The work that this work has been translated from. e.g. 物种起源 is a translationOf “On the Origin of Species”" ;
        rdfs:label    "translationOfWork" .

schema:monthlyMinimumRepaymentAmount
        a             rdf:Property ;
        rdfs:comment  "The minimum payment is the lowest amount of money that one is required to pay on a credit card statement each month." ;
        rdfs:label    "monthlyMinimumRepaymentAmount" .

schema:superEvent  a  rdf:Property ;
        rdfs:comment  "An event that this event is a part of. For example, a collection of individual music performances might each have a music festival as their superEvent." ;
        rdfs:label    "superEvent" .

schema:AuthorizeAction
        a                rdfs:Class ;
        rdfs:comment     "The act of granting permission to an object." ;
        rdfs:label       "AuthorizeAction" ;
        rdfs:subClassOf  schema:AllocateAction .

schema:accessibilityFeature
        a             rdf:Property ;
        rdfs:comment  "Content features of the resource, such as accessible media, alternatives and supported enhancements for accessibility ([WebSchemas wiki lists possible values](http://www.w3.org/wiki/WebSchemas/Accessibility))." ;
        rdfs:label    "accessibilityFeature" .

schema:Electrician  a    rdfs:Class ;
        rdfs:comment     "An electrician." ;
        rdfs:label       "Electrician" ;
        rdfs:subClassOf  schema:HomeAndConstructionBusiness .

schema:DanceGroup  a     rdfs:Class ;
        rdfs:comment     "A dance group&#x2014;for example, the Alvin Ailey Dance Theater or Riverdance." ;
        rdfs:label       "DanceGroup" ;
        rdfs:subClassOf  schema:PerformingGroup .

schema:requiredQuantity
        a             rdf:Property ;
        rdfs:comment  "The required quantity of the item(s)." ;
        rdfs:label    "requiredQuantity" .

schema:securityScreening
        a             rdf:Property ;
        rdfs:comment  "The type of security screening the passenger is subject to." ;
        rdfs:label    "securityScreening" .

schema:AdvertiserContentArticle
        a                rdfs:Class ;
        rdfs:comment     "An [[Article]] that an external entity has paid to place or to produce to its specifications. Includes [advertorials](https://en.wikipedia.org/wiki/Advertorial), sponsored content, native advertising and other paid content." ;
        rdfs:label       "AdvertiserContentArticle" ;
        rdfs:subClassOf  schema:Article .

schema:eventAttendanceMode
        a             rdf:Property ;
        rdfs:comment  "The eventAttendanceMode of an event indicates whether it occurs online, offline, or a mix." ;
        rdfs:label    "eventAttendanceMode" .

schema:DisagreeAction
        a                rdfs:Class ;
        rdfs:comment     "The act of expressing a difference of opinion with the object. An agent disagrees to/about an object (a proposition, topic or theme) with participants." ;
        rdfs:label       "DisagreeAction" ;
        rdfs:subClassOf  schema:ReactAction .

schema:minimumPaymentDue
        a             rdf:Property ;
        rdfs:comment  "The minimum payment required at this time." ;
        rdfs:label    "minimumPaymentDue" .

schema:QAPage  a         rdfs:Class ;
        rdfs:comment     "A QAPage is a WebPage focussed on a specific Question and its Answer(s), e.g. in a question answering site or documenting Frequently Asked Questions (FAQs)." ;
        rdfs:label       "QAPage" ;
        rdfs:subClassOf  schema:WebPage .

schema:orderDate  a   rdf:Property ;
        rdfs:comment  "Date order was placed." ;
        rdfs:label    "orderDate" .

schema:maximumPhysicalAttendeeCapacity
        a             rdf:Property ;
        rdfs:comment  "The maximum physical attendee capacity of an [[Event]] whose [[eventAttendanceMode]] is [[OfflineEventAttendanceMode]] (or the offline aspects, in the case of a [[MixedEventAttendanceMode]]). " ;
        rdfs:label    "maximumPhysicalAttendeeCapacity" .

schema:Painting  a       rdfs:Class ;
        rdfs:comment     "A painting." ;
        rdfs:label       "Painting" ;
        rdfs:subClassOf  schema:CreativeWork .

schema:orderStatus  a  rdf:Property ;
        rdfs:comment  "The current status of the order." ;
        rdfs:label    "orderStatus" .

schema:HowToStep  a      rdfs:Class ;
        rdfs:comment     "A step in the instructions for how to achieve a result. It is an ordered list with HowToDirection and/or HowToTip items." ;
        rdfs:label       "HowToStep" ;
        rdfs:subClassOf  schema:ListItem , schema:ItemList , schema:CreativeWork .

schema:memberOf  a    rdf:Property ;
        rdfs:comment  "An Organization (or ProgramMembership) to which this Person or Organization belongs." ;
        rdfs:label    "memberOf" .

schema:HotelRoom  a      rdfs:Class ;
        rdfs:comment     "A hotel room is a single room in a hotel.\n<br /><br />\nSee also the <a href=\"/docs/hotels.html\">dedicated document on the use of schema.org for marking up hotels and other forms of accommodations</a>.\n" ;
        rdfs:label       "HotelRoom" ;
        rdfs:subClassOf  schema:Room .

schema:PsychologicalTreatment
        a                rdfs:Class ;
        rdfs:comment     "A process of care relying upon counseling, dialogue and communication  aimed at improving a mental health condition without use of drugs." ;
        rdfs:label       "PsychologicalTreatment" ;
        rdfs:subClassOf  schema:TherapeuticProcedure .

schema:blogPosts  a   rdf:Property ;
        rdfs:comment  "The postings that are part of this blog." ;
        rdfs:label    "blogPosts" .

schema:telephone  a   rdf:Property ;
        rdfs:comment  "The telephone number." ;
        rdfs:label    "telephone" .

ns1:exactMatch  a  rdf:Property .

schema:founder  a     rdf:Property ;
        rdfs:comment  "A person who founded this organization." ;
        rdfs:label    "founder" .

schema:produces  a    rdf:Property ;
        rdfs:comment  "The tangible thing generated by the service, e.g. a passport, permit, etc." ;
        rdfs:label    "produces" .

schema:coach  a       rdf:Property ;
        rdfs:comment  "A person that acts in a coaching role for a sports team." ;
        rdfs:label    "coach" .

schema:QuantitativeValueDistribution
        a                rdfs:Class ;
        rdfs:comment     "A statistical distribution of values." ;
        rdfs:label       "QuantitativeValueDistribution" ;
        rdfs:subClassOf  schema:StructuredValue .

schema:UnitPriceSpecification
        a                rdfs:Class ;
        rdfs:comment     "The price asked for a given offer by the respective organization or person." ;
        rdfs:label       "UnitPriceSpecification" ;
        rdfs:subClassOf  schema:PriceSpecification .

schema:composer  a    rdf:Property ;
        rdfs:comment  "The person or organization who wrote a composition, or who is the composer of a work performed at some event." ;
        rdfs:label    "composer" .

schema:Action  a         rdfs:Class ;
        rdfs:comment     "An action performed by a direct agent and indirect participants upon a direct object. Optionally happens at a location with the help of an inanimate instrument. The execution of the action may produce a result. Specific action sub-type documentation specifies the exact expectation of each argument/role.\\n\\nSee also [blog post](http://blog.schema.org/2014/04/announcing-schemaorg-actions.html) and [Actions overview document](http://schema.org/docs/actions.html)." ;
        rdfs:label       "Action" ;
        rdfs:subClassOf  schema:Thing .

schema:missionCoveragePrioritiesPolicy
        a                   rdf:Property ;
        rdfs:comment        "For a [[NewsMediaOrganization]], a statement on coverage priorities, including any public agenda or stance on issues." ;
        rdfs:label          "missionCoveragePrioritiesPolicy" ;
        rdfs:subPropertyOf  schema:publishingPrinciples .

schema:imagingTechnique
        a             rdf:Property ;
        rdfs:comment  "Imaging technique used." ;
        rdfs:label    "imagingTechnique" .

schema:steps  a       rdf:Property ;
        rdfs:comment  "A single step item (as HowToStep, text, document, video, etc.) or a HowToSection (originally misnamed 'steps'; 'step' is preferred)." ;
        rdfs:label    "steps" .

schema:line  a        rdf:Property ;
        rdfs:comment  "A line is a point-to-point path consisting of two or more points. A line is expressed as a series of two or more point objects separated by space." ;
        rdfs:label    "line" .

schema:jobBenefits  a  rdf:Property ;
        rdfs:comment  "Description of benefits associated with the job." ;
        rdfs:label    "jobBenefits" .

schema:spatialCoverage
        a                   rdf:Property ;
        rdfs:comment        "The spatialCoverage of a CreativeWork indicates the place(s) which are the focus of the content. It is a subproperty of\n      contentLocation intended primarily for more technical and detailed materials. For example with a Dataset, it indicates\n      areas that the dataset describes: a dataset of New York weather would have spatialCoverage which was the place: the state of New York." ;
        rdfs:label          "spatialCoverage" ;
        rdfs:subPropertyOf  schema:contentLocation .

schema:DiagnosticProcedure
        a                rdfs:Class ;
        rdfs:comment     "A medical procedure intended primarily for diagnostic, as opposed to therapeutic, purposes." ;
        rdfs:label       "DiagnosticProcedure" ;
        rdfs:subClassOf  schema:MedicalProcedure .

schema:ProductModel  a   rdfs:Class ;
        rdfs:comment     "A datasheet or vendor specification of a product (in the sense of a prototypical description)." ;
        rdfs:label       "ProductModel" ;
        rdfs:subClassOf  schema:Product .

schema:location  a    rdf:Property ;
        rdfs:comment  "The location of, for example, where an event is happening, where an organization is located, or where an action takes place." ;
        rdfs:label    "location" .

schema:creditText  a  rdf:Property ;
        rdfs:comment  "Text that can be used to credit person(s) and/or organization(s) associated with a published Creative Work." ;
        rdfs:label    "creditText" .

schema:EntertainmentBusiness
        a                rdfs:Class ;
        rdfs:comment     "A business providing entertainment." ;
        rdfs:label       "EntertainmentBusiness" ;
        rdfs:subClassOf  schema:LocalBusiness .

schema:PodcastSeason  a  rdfs:Class ;
        rdfs:comment     "A single season of a podcast. Many podcasts do not break down into separate seasons. In that case, PodcastSeries should be used." ;
        rdfs:label       "PodcastSeason" ;
        rdfs:subClassOf  schema:CreativeWorkSeason .

schema:TVSeries  a       rdfs:Class ;
        rdfs:comment     "CreativeWorkSeries dedicated to TV broadcast and associated online delivery." ;
        rdfs:label       "TVSeries" ;
        rdfs:subClassOf  schema:CreativeWorkSeries , schema:CreativeWork .

schema:WPAdBlock  a      rdfs:Class ;
        rdfs:comment     "An advertising section of the page." ;
        rdfs:label       "WPAdBlock" ;
        rdfs:subClassOf  schema:WebPageElement .

schema:proprietaryName
        a             rdf:Property ;
        rdfs:comment  "Proprietary name given to the diet plan, typically by its originator or creator." ;
        rdfs:label    "proprietaryName" .

voc:numberOfUnits  a  rdf:Property .

schema:epidemiology  a  rdf:Property ;
        rdfs:comment  "The characteristics of associated patients, such as age, gender, race etc." ;
        rdfs:label    "epidemiology" .

rdf:Property  a  rdfs:Class .

schema:HowTo  a          rdfs:Class ;
        rdfs:comment     "Instructions that explain how to achieve a result by performing a sequence of steps." ;
        rdfs:label       "HowTo" ;
        rdfs:subClassOf  schema:CreativeWork .

schema:fuelCapacity  a  rdf:Property ;
        rdfs:comment  "The capacity of the fuel tank or in the case of electric cars, the battery. If there are multiple components for storage, this should indicate the total of all storage of the same type.\\n\\nTypical unit code(s): LTR for liters, GLL of US gallons, GLI for UK / imperial gallons, AMH for ampere-hours (for electrical vehicles)." ;
        rdfs:label    "fuelCapacity" .

schema:starRating  a  rdf:Property ;
        rdfs:comment  "An official rating for a lodging business or food establishment, e.g. from national associations or standards bodies. Use the author property to indicate the rating organization, e.g. as an Organization with name such as (e.g. HOTREC, DEHOGA, WHR, or Hotelstars)." ;
        rdfs:label    "starRating" .

schema:InternetCafe  a   rdfs:Class ;
        rdfs:comment     "An internet cafe." ;
        rdfs:label       "InternetCafe" ;
        rdfs:subClassOf  schema:LocalBusiness .

schema:LodgingBusiness
        a                rdfs:Class ;
        rdfs:comment     "A lodging business, such as a motel, hotel, or inn." ;
        rdfs:label       "LodgingBusiness" ;
        rdfs:subClassOf  schema:LocalBusiness .

schema:BookFormatType
        a                rdfs:Class ;
        rdfs:comment     "The publication format of the book." ;
        rdfs:label       "BookFormatType" ;
        rdfs:subClassOf  schema:Enumeration .

schema:branchCode  a  rdf:Property ;
        rdfs:comment  "A short textual code (also called \"store code\") that uniquely identifies a place of business. The code is typically assigned by the parentOrganization and used in structured URLs.\\n\\nFor example, in the URL http://www.starbucks.co.uk/store-locator/etc/detail/3047 the code \"3047\" is a branchCode for a particular branch.\n      " ;
        rdfs:label    "branchCode" .

schema:participant  a  rdf:Property ;
        rdfs:comment  "Other co-agents that participated in the action indirectly. e.g. John wrote a book with *Steve*." ;
        rdfs:label    "participant" .

schema:discussionUrl  a  rdf:Property ;
        rdfs:comment  "A link to the page containing the comments of the CreativeWork." ;
        rdfs:label    "discussionUrl" .

schema:PawnShop  a       rdfs:Class ;
        rdfs:comment     "A shop that will buy, or lend money against the security of, personal possessions." ;
        rdfs:label       "PawnShop" ;
        rdfs:subClassOf  schema:Store .

schema:isUnlabelledFallback
        a             rdf:Property ;
        rdfs:comment  "This can be marked 'true' to indicate that some published [[DeliveryTimeSettings]] or [[ShippingRateSettings]] are intended to apply to all [[OfferShippingDetails]] published by the same merchant, when referenced by a [[shippingSettingsLink]] in those settings. It is not meaningful to use a 'true' value for this property alongside a transitTimeLabel (for [[DeliveryTimeSettings]]) or shippingLabel (for [[ShippingRateSettings]]), since this property is for use with unlabelled settings." ;
        rdfs:label    "isUnlabelledFallback" .

schema:DigitalDocument
        a                rdfs:Class ;
        rdfs:comment     "An electronic file or document." ;
        rdfs:label       "DigitalDocument" ;
        rdfs:subClassOf  schema:CreativeWork .

schema:inker  a       rdf:Property ;
        rdfs:comment  "The individual who traces over the pencil drawings in ink after pencils are complete." ;
        rdfs:label    "inker" .

schema:antagonist  a  rdf:Property ;
        rdfs:comment  "The muscle whose action counteracts the specified muscle." ;
        rdfs:label    "antagonist" .

schema:BodyOfWater  a    rdfs:Class ;
        rdfs:comment     "A body of water, such as a sea, ocean, or lake." ;
        rdfs:label       "BodyOfWater" ;
        rdfs:subClassOf  schema:Landform .

schema:AppendAction  a   rdfs:Class ;
        rdfs:comment     "The act of inserting at the end if an ordered collection." ;
        rdfs:label       "AppendAction" ;
        rdfs:subClassOf  schema:InsertAction .

schema:GamePlayMode  a   rdfs:Class ;
        rdfs:comment     "Indicates whether this game is multi-player, co-op or single-player." ;
        rdfs:label       "GamePlayMode" ;
        rdfs:subClassOf  schema:Enumeration .

schema:audio  a       rdf:Property ;
        rdfs:comment  "An embedded audio object." ;
        rdfs:label    "audio" .

schema:accountId  a         rdf:Property ;
        rdfs:comment        "The identifier for the account the payment will be applied to." ;
        rdfs:label          "accountId" ;
        rdfs:subPropertyOf  schema:identifier .

schema:SolveMathAction
        a                rdfs:Class ;
        rdfs:comment     "The action that takes in a math expression and directs users to a page potentially capable of solving/simplifying that expression." ;
        rdfs:label       "SolveMathAction" ;
        rdfs:subClassOf  schema:Action .

schema:ticketedSeat  a  rdf:Property ;
        rdfs:comment  "The seat associated with the ticket." ;
        rdfs:label    "ticketedSeat" .

schema:creativeWorkStatus
        a             rdf:Property ;
        rdfs:comment  "The status of a creative work in terms of its stage in a lifecycle. Example terms include Incomplete, Draft, Published, Obsolete. Some organizations define a set of terms for the stages of their publication lifecycle." ;
        rdfs:label    "creativeWorkStatus" .

schema:messageAttachment
        a             rdf:Property ;
        rdfs:comment  "A CreativeWork attached to the message." ;
        rdfs:label    "messageAttachment" .

schema:unitText  a    rdf:Property ;
        rdfs:comment  "A string or text indicating the unit of measurement. Useful if you cannot provide a standard unit code for\n<a href='unitCode'>unitCode</a>." ;
        rdfs:label    "unitText" .

schema:underName  a   rdf:Property ;
        rdfs:comment  "The person or organization the reservation or ticket is for." ;
        rdfs:label    "underName" .

schema:NoteDigitalDocument
        a                rdfs:Class ;
        rdfs:comment     "A file containing a note, primarily for the author." ;
        rdfs:label       "NoteDigitalDocument" ;
        rdfs:subClassOf  schema:DigitalDocument .

schema:cargoVolume  a  rdf:Property ;
        rdfs:comment  "The available volume for cargo or luggage. For automobiles, this is usually the trunk volume.\\n\\nTypical unit code(s): LTR for liters, FTQ for cubic foot/feet\\n\\nNote: You can use [[minValue]] and [[maxValue]] to indicate ranges." ;
        rdfs:label    "cargoVolume" .

schema:CheckoutPage  a   rdfs:Class ;
        rdfs:comment     "Web page type: Checkout page." ;
        rdfs:label       "CheckoutPage" ;
        rdfs:subClassOf  schema:WebPage .

schema:ChooseAction  a   rdfs:Class ;
        rdfs:comment     "The act of expressing a preference from a set of options or a large or unbounded set of choices/options." ;
        rdfs:label       "ChooseAction" ;
        rdfs:subClassOf  schema:AssessAction .

schema:postalCodeRange
        a             rdf:Property ;
        rdfs:comment  "A defined range of postal codes." ;
        rdfs:label    "postalCodeRange" .

schema:fuelType  a    rdf:Property ;
        rdfs:comment  "The type of fuel suitable for the engine or engines of the vehicle. If the vehicle has only one engine, this property can be attached directly to the vehicle." ;
        rdfs:label    "fuelType" .

schema:MedicalObservationalStudy
        a                rdfs:Class ;
        rdfs:comment     "An observational study is a type of medical study that attempts to infer the possible effect of a treatment through observation of a cohort of subjects over a period of time. In an observational study, the assignment of subjects into treatment groups versus control groups is outside the control of the investigator. This is in contrast with controlled studies, such as the randomized controlled trials represented by MedicalTrial, where each subject is randomly assigned to a treatment group or a control group before the start of the treatment." ;
        rdfs:label       "MedicalObservationalStudy" ;
        rdfs:subClassOf  schema:MedicalStudy .

schema:totalPaymentDue
        a             rdf:Property ;
        rdfs:comment  "The total amount due." ;
        rdfs:label    "totalPaymentDue" .

schema:LibrarySystem  a  rdfs:Class ;
        rdfs:comment     "A [[LibrarySystem]] is a collaborative system amongst several libraries." ;
        rdfs:label       "LibrarySystem" ;
        rdfs:subClassOf  schema:Organization .

schema:model  a       rdf:Property ;
        rdfs:comment  "The model of the product. Use with the URL of a ProductModel or a textual representation of the model identifier. The URL of the ProductModel can be from an external source. It is recommended to additionally provide strong product identifiers via the gtin8/gtin13/gtin14 and mpn properties." ;
        rdfs:label    "model" .

schema:InsertAction  a   rdfs:Class ;
        rdfs:comment     "The act of adding at a specific location in an ordered collection." ;
        rdfs:label       "InsertAction" ;
        rdfs:subClassOf  schema:AddAction .

schema:subjectOf  a   rdf:Property ;
        rdfs:comment  "A CreativeWork or Event about this Thing." ;
        rdfs:label    "subjectOf" .

schema:provider  a    rdf:Property ;
        rdfs:comment  "The service provider, service operator, or service performer; the goods producer. Another party (a seller) may offer those services or goods on behalf of the provider. A provider may also serve as the seller." ;
        rdfs:label    "provider" .

schema:MedicalWebPage
        a                rdfs:Class ;
        rdfs:comment     "A web page that provides medical information." ;
        rdfs:label       "MedicalWebPage" ;
        rdfs:subClassOf  schema:WebPage .

schema:lodgingUnitType
        a             rdf:Property ;
        rdfs:comment  "Textual description of the unit type (including suite vs. room, size of bed, etc.)." ;
        rdfs:label    "lodgingUnitType" .

schema:Motorcycle  a     rdfs:Class ;
        rdfs:comment     "A motorcycle or motorbike is a single-track, two-wheeled motor vehicle." ;
        rdfs:label       "Motorcycle" ;
        rdfs:subClassOf  schema:Vehicle .

schema:priceType  a   rdf:Property ;
        rdfs:comment  "Defines the type of a price specified for an offered product, for example a list price, a (temporary) sale price or a manufacturer suggested retail price. If multiple prices are specified for an offer the [[priceType]] property can be used to identify the type of each such specified price. The value of priceType can be specified as a value from enumeration PriceTypeEnumeration or as a free form text string for price types that are not already predefined in PriceTypeEnumeration." ;
        rdfs:label    "priceType" .

schema:answerCount  a  rdf:Property ;
        rdfs:comment  "The number of answers this question has received." ;
        rdfs:label    "answerCount" .

schema:DepartmentStore
        a                rdfs:Class ;
        rdfs:comment     "A department store." ;
        rdfs:label       "DepartmentStore" ;
        rdfs:subClassOf  schema:Store .

schema:SubscribeAction
        a                rdfs:Class ;
        rdfs:comment     "The act of forming a personal connection with someone/something (object) unidirectionally/asymmetrically to get updates pushed to.\\n\\nRelated actions:\\n\\n* [[FollowAction]]: Unlike FollowAction, SubscribeAction implies that the subscriber acts as a passive agent being constantly/actively pushed for updates.\\n* [[RegisterAction]]: Unlike RegisterAction, SubscribeAction implies that the agent is interested in continuing receiving updates from the object.\\n* [[JoinAction]]: Unlike JoinAction, SubscribeAction implies that the agent is interested in continuing receiving updates from the object." ;
        rdfs:label       "SubscribeAction" ;
        rdfs:subClassOf  schema:InteractAction .

schema:proficiencyLevel
        a             rdf:Property ;
        rdfs:comment  "Proficiency needed for this content; expected values: 'Beginner', 'Expert'." ;
        rdfs:label    "proficiencyLevel" .

schema:UpdateAction  a   rdfs:Class ;
        rdfs:comment     "The act of managing by changing/editing the state of the object." ;
        rdfs:label       "UpdateAction" ;
        rdfs:subClassOf  schema:Action .

dcmitype:Event  a  rdfs:Class .

schema:geoCrosses  a  rdf:Property ;
        rdfs:comment  "Represents a relationship between two geometries (or the places they represent), relating a geometry to another that crosses it: \"a crosses b: they have some but not all interior points in common, and the dimension of the intersection is less than that of at least one of them\". As defined in [DE-9IM](https://en.wikipedia.org/wiki/DE-9IM)." ;
        rdfs:label    "geoCrosses" .

schema:musicCompositionForm
        a             rdf:Property ;
        rdfs:comment  "The type of composition (e.g. overture, sonata, symphony, etc.)." ;
        rdfs:label    "musicCompositionForm" .

schema:entertainmentBusiness
        a                   rdf:Property ;
        rdfs:comment        "A sub property of location. The entertainment business where the action occurred." ;
        rdfs:label          "entertainmentBusiness" ;
        rdfs:subPropertyOf  schema:location .

schema:speed  a       rdf:Property ;
        rdfs:comment  "The speed range of the vehicle. If the vehicle is powered by an engine, the upper limit of the speed range (indicated by [[maxValue]] should be the maximum speed achievable under regular conditions.\\n\\nTypical unit code(s): KMH for km/h, HM for mile per hour (0.447 04 m/s), KNT for knot\\n\\n*Note 1: Use [[minValue]] and [[maxValue]] to indicate the range. Typically, the minimal value is zero.\\n* Note 2: There are many different ways of measuring the speed range. You can link to information about how the given value has been determined using the [[valueReference]] property." ;
        rdfs:label    "speed" .

schema:minValue  a    rdf:Property ;
        rdfs:comment  "The lower value of some characteristic or property." ;
        rdfs:label    "minValue" .

schema:interactionStatistic
        a             rdf:Property ;
        rdfs:comment  "The number of interactions for the CreativeWork using the WebSite or SoftwareApplication. The most specific child type of InteractionCounter should be used." ;
        rdfs:label    "interactionStatistic" .

schema:RadioEpisode  a   rdfs:Class ;
        rdfs:comment     "A radio episode which can be part of a series or season." ;
        rdfs:label       "RadioEpisode" ;
        rdfs:subClassOf  schema:Episode .

schema:makesOffer  a  rdf:Property ;
        rdfs:comment  "A pointer to products or services offered by the organization or person." ;
        rdfs:label    "makesOffer" .

schema:arrivalAirport
        a             rdf:Property ;
        rdfs:comment  "The airport where the flight terminates." ;
        rdfs:label    "arrivalAirport" .

schema:gtin12  a            rdf:Property ;
        rdfs:comment        "The GTIN-12 code of the product, or the product to which the offer refers. The GTIN-12 is the 12-digit GS1 Identification Key composed of a U.P.C. Company Prefix, Item Reference, and Check Digit used to identify trade items. See [GS1 GTIN Summary](http://www.gs1.org/barcodes/technical/idkeys/gtin) for more details." ;
        rdfs:label          "gtin12" ;
        rdfs:subPropertyOf  schema:identifier , schema:gtin .

schema:FireStation  a    rdfs:Class ;
        rdfs:comment     "A fire station. With firemen." ;
        rdfs:label       "FireStation" ;
        rdfs:subClassOf  schema:CivicStructure , schema:EmergencyService .

schema:byDay  a       rdf:Property ;
        rdfs:comment  "Defines the day(s) of the week on which a recurring [[Event]] takes place. May be specified using either [[DayOfWeek]], or alternatively [[Text]] conforming to iCal's syntax for byDay recurrence rules." ;
        rdfs:label    "byDay" .

schema:printSection  a  rdf:Property ;
        rdfs:comment  "If this NewsArticle appears in print, this field indicates the print section in which the article appeared." ;
        rdfs:label    "printSection" .

schema:liveBlogUpdate
        a             rdf:Property ;
        rdfs:comment  "An update to the LiveBlog." ;
        rdfs:label    "liveBlogUpdate" .

schema:alternativeHeadline
        a             rdf:Property ;
        rdfs:comment  "A secondary title of the CreativeWork." ;
        rdfs:label    "alternativeHeadline" .

schema:PublicationVolume
        a                rdfs:Class ;
        rdfs:comment     "A part of a successively published publication such as a periodical or multi-volume work, often numbered. It may represent a time span, such as a year.\\n\\nSee also [blog post](http://blog.schema.org/2014/09/schemaorg-support-for-bibliographic_2.html)." ;
        rdfs:label       "PublicationVolume" ;
        rdfs:subClassOf  schema:CreativeWork .

schema:amountOfThisGood
        a             rdf:Property ;
        rdfs:comment  "The quantity of the goods included in the offer." ;
        rdfs:label    "amountOfThisGood" .

schema:OpinionNewsArticle
        a                rdfs:Class ;
        rdfs:comment     "An [[OpinionNewsArticle]] is a [[NewsArticle]] that primarily expresses opinions rather than journalistic reporting of news and events. For example, a [[NewsArticle]] consisting of a column or [[Blog]]/[[BlogPosting]] entry in the Opinions section of a news publication. " ;
        rdfs:label       "OpinionNewsArticle" ;
        rdfs:subClassOf  schema:NewsArticle .

schema:containsPlace  a  owl:ObjectProperty ;
        rdfs:comment   "The basic containment relation between a place and another that it contains." ;
        rdfs:label     "containsPlace" ;
        owl:inverseOf  schema:containedInPlace .

schema:fileFormat  a  rdf:Property ;
        rdfs:comment  "Media type, typically MIME format (see [IANA site](http://www.iana.org/assignments/media-types/media-types.xhtml)) of the content e.g. application/zip of a SoftwareApplication binary. In cases where a CreativeWork has several media type representations, 'encoding' can be used to indicate each MediaObject alongside particular fileFormat information. Unregistered or niche file formats can be indicated instead via the most appropriate URL, e.g. defining Web page or a Wikipedia entry." ;
        rdfs:label    "fileFormat" .

schema:mealService  a  rdf:Property ;
        rdfs:comment  "Description of the meals that will be provided or available for purchase." ;
        rdfs:label    "mealService" .

schema:pathophysiology
        a             rdf:Property ;
        rdfs:comment  "Changes in the normal mechanical, physical, and biochemical functions that are associated with this activity or condition." ;
        rdfs:label    "pathophysiology" .

schema:Invoice  a        rdfs:Class ;
        rdfs:comment     "A statement of the money due for goods or services; a bill." ;
        rdfs:label       "Invoice" ;
        rdfs:subClassOf  schema:Intangible .

schema:mediaAuthenticityCategory
        a             rdf:Property ;
        rdfs:comment  "Indicates a MediaManipulationRatingEnumeration classification of a media object (in the context of how it was published or shared)." ;
        rdfs:label    "mediaAuthenticityCategory" .

schema:ApplyAction  a    rdfs:Class ;
        rdfs:comment     "The act of registering to an organization/service without the guarantee to receive it.\\n\\nRelated actions:\\n\\n* [[RegisterAction]]: Unlike RegisterAction, ApplyAction has no guarantees that the application will be accepted." ;
        rdfs:label       "ApplyAction" ;
        rdfs:subClassOf  schema:OrganizeAction .

schema:ComicIssue  a     rdfs:Class ;
        rdfs:comment     "Individual comic issues are serially published as\n    \tpart of a larger series. For the sake of consistency, even one-shot issues\n    \tbelong to a series comprised of a single issue. All comic issues can be\n    \tuniquely identified by: the combination of the name and volume number of the\n    \tseries to which the issue belongs; the issue number; and the variant\n    \tdescription of the issue (if any)." ;
        rdfs:label       "ComicIssue" ;
        rdfs:subClassOf  schema:PublicationIssue .

schema:breadcrumb  a  rdf:Property ;
        rdfs:comment  "A set of links that can help a user understand and navigate a website hierarchy." ;
        rdfs:label    "breadcrumb" .

schema:Geriatric  a      rdfs:Class ;
        rdfs:comment     "A specific branch of medical science that is concerned with the diagnosis and treatment of diseases, debilities and provision of care to the aged." ;
        rdfs:label       "Geriatric" ;
        rdfs:subClassOf  schema:MedicalBusiness .

schema:priceComponent
        a             rdf:Property ;
        rdfs:comment  "This property links to all [[UnitPriceSpecification]] nodes that apply in parallel for the [[CompoundPriceSpecification]] node." ;
        rdfs:label    "priceComponent" .

schema:contentSize  a  rdf:Property ;
        rdfs:comment  "File size in (mega/kilo) bytes." ;
        rdfs:label    "contentSize" .

schema:attendees  a   rdf:Property ;
        rdfs:comment  "A person attending the event." ;
        rdfs:label    "attendees" .

schema:webFeed  a     rdf:Property ;
        rdfs:comment  "The URL for a feed, e.g. associated with a podcast series, blog, or series of date-stamped updates. This is usually RSS or Atom." ;
        rdfs:label    "webFeed" .

schema:pattern  a     rdf:Property ;
        rdfs:comment  "A pattern that something has, for example 'polka dot', 'striped', 'Canadian flag'. Values are typically expressed as text, although links to controlled value schemes are also supported." ;
        rdfs:label    "pattern" .

schema:availableService
        a             rdf:Property ;
        rdfs:comment  "A medical service available from this provider." ;
        rdfs:label    "availableService" .

schema:MovieTheater  a   rdfs:Class ;
        rdfs:comment     "A movie theater." ;
        rdfs:label       "MovieTheater" ;
        rdfs:subClassOf  schema:EntertainmentBusiness , schema:CivicStructure .

schema:lyricist  a    rdf:Property ;
        rdfs:comment  "The person who wrote the words." ;
        rdfs:label    "lyricist" .

schema:PlanAction  a     rdfs:Class ;
        rdfs:comment     "The act of planning the execution of an event/task/action/reservation/plan to a future date." ;
        rdfs:label       "PlanAction" ;
        rdfs:subClassOf  schema:OrganizeAction .

schema:minPrice  a    rdf:Property ;
        rdfs:comment  "The lowest price if the price is a range." ;
        rdfs:label    "minPrice" .

schema:cvdNumVentUse  a  rdf:Property ;
        rdfs:comment  "numventuse - MECHANICAL VENTILATORS IN USE: Total number of ventilators in use." ;
        rdfs:label    "cvdNumVentUse" .

schema:UserComments  a   rdfs:Class ;
        rdfs:comment     "UserInteraction and its subtypes is an old way of talking about users interacting with pages. It is generally better to use [[Action]]-based vocabulary, alongside types such as [[Comment]]." ;
        rdfs:label       "UserComments" ;
        rdfs:subClassOf  schema:UserInteraction .

schema:PublicationIssue
        a                rdfs:Class ;
        rdfs:comment     "A part of a successively published publication such as a periodical or publication volume, often numbered, usually containing a grouping of works such as articles.\\n\\nSee also [blog post](http://blog.schema.org/2014/09/schemaorg-support-for-bibliographic_2.html)." ;
        rdfs:label       "PublicationIssue" ;
        rdfs:subClassOf  schema:CreativeWork .

schema:XPathType  a      rdfs:Class ;
        rdfs:comment     "Text representing an XPath (typically but not necessarily version 1.0)." ;
        rdfs:label       "XPathType" ;
        rdfs:subClassOf  schema:Text .

schema:Distance  a       rdfs:Class ;
        rdfs:comment     "Properties that take Distances as values are of the form '&lt;Number&gt; &lt;Length unit of measure&gt;'. E.g., '7 ft'." ;
        rdfs:label       "Distance" ;
        rdfs:subClassOf  schema:Quantity .

schema:valueRequired  a  rdf:Property ;
        rdfs:comment  "Whether the property must be filled in to complete the action.  Default is false." ;
        rdfs:label    "valueRequired" .

schema:studyDesign  a  rdf:Property ;
        rdfs:comment  "Specifics about the observational study design (enumerated)." ;
        rdfs:label    "studyDesign" .

schema:publishingPrinciples
        a             rdf:Property ;
        rdfs:comment  "The publishingPrinciples property indicates (typically via [[URL]]) a document describing the editorial principles of an [[Organization]] (or individual e.g. a [[Person]] writing a blog) that relate to their activities as a publisher, e.g. ethics or diversity policies. When applied to a [[CreativeWork]] (e.g. [[NewsArticle]]) the principles are those of the party primarily responsible for the creation of the [[CreativeWork]].\n\nWhile such policies are most typically expressed in natural language, sometimes related information (e.g. indicating a [[funder]]) can be expressed using schema.org terminology.\n" ;
        rdfs:label    "publishingPrinciples" .

schema:HousePainter  a   rdfs:Class ;
        rdfs:comment     "A house painting service." ;
        rdfs:label       "HousePainter" ;
        rdfs:subClassOf  schema:HomeAndConstructionBusiness .

schema:GovernmentPermit
        a                rdfs:Class ;
        rdfs:comment     "A permit issued by a government agency." ;
        rdfs:label       "GovernmentPermit" ;
        rdfs:subClassOf  schema:Permit .

schema:mileageFromOdometer
        a             rdf:Property ;
        rdfs:comment  "The total distance travelled by the particular vehicle since its initial production, as read from its odometer.\\n\\nTypical unit code(s): KMT for kilometers, SMI for statute miles" ;
        rdfs:label    "mileageFromOdometer" .

schema:vehicleInteriorType
        a             rdf:Property ;
        rdfs:comment  "The type or material of the interior of the vehicle (e.g. synthetic fabric, leather, wood, etc.). While most interior types are characterized by the material used, an interior type can also be based on vehicle usage or target audience." ;
        rdfs:label    "vehicleInteriorType" .

schema:AcceptAction  a   rdfs:Class ;
        rdfs:comment     "The act of committing to/adopting an object.\\n\\nRelated actions:\\n\\n* [[RejectAction]]: The antonym of AcceptAction." ;
        rdfs:label       "AcceptAction" ;
        rdfs:subClassOf  schema:AllocateAction .

schema:geoIntersects  a  rdf:Property ;
        rdfs:comment  "Represents spatial relations in which two geometries (or the places they represent) have at least one point in common. As defined in [DE-9IM](https://en.wikipedia.org/wiki/DE-9IM)." ;
        rdfs:label    "geoIntersects" .

schema:dateRead  a    rdf:Property ;
        rdfs:comment  "The date/time at which the message has been read by the recipient if a single recipient exists." ;
        rdfs:label    "dateRead" .

schema:Podiatric  a      rdfs:Class ;
        rdfs:comment     "Podiatry is the care of the human foot, especially the diagnosis and treatment of foot disorders." ;
        rdfs:label       "Podiatric" ;
        rdfs:subClassOf  schema:MedicalBusiness .

schema:sender  a            rdf:Property ;
        rdfs:comment        "A sub property of participant. The participant who is at the sending end of the action." ;
        rdfs:label          "sender" ;
        rdfs:subPropertyOf  schema:participant .

schema:Hospital  a       rdfs:Class ;
        rdfs:comment     "A hospital." ;
        rdfs:label       "Hospital" ;
        rdfs:subClassOf  schema:CivicStructure , schema:MedicalOrganization , schema:EmergencyService .

schema:comprisedOf  a  rdf:Property ;
        rdfs:comment  "Specifying something physically contained by something else. Typically used here for the underlying anatomical structures, such as organs, that comprise the anatomical system." ;
        rdfs:label    "comprisedOf" .

schema:priceSpecification
        a             rdf:Property ;
        rdfs:comment  "One or more detailed price specifications, indicating the unit price and delivery or payment charges." ;
        rdfs:label    "priceSpecification" .

schema:Artery  a         rdfs:Class ;
        rdfs:comment     "A type of blood vessel that specifically carries blood away from the heart." ;
        rdfs:label       "Artery" ;
        rdfs:subClassOf  schema:Vessel .

schema:MonetaryAmountDistribution
        a                rdfs:Class ;
        rdfs:comment     "A statistical distribution of monetary amounts." ;
        rdfs:label       "MonetaryAmountDistribution" ;
        rdfs:subClassOf  schema:QuantitativeValueDistribution .

schema:UserPlusOnes  a   rdfs:Class ;
        rdfs:comment     "UserInteraction and its subtypes is an old way of talking about users interacting with pages. It is generally better to use [[Action]]-based vocabulary, alongside types such as [[Comment]]." ;
        rdfs:label       "UserPlusOnes" ;
        rdfs:subClassOf  schema:UserInteraction .

schema:tool  a              rdf:Property ;
        rdfs:comment        "A sub property of instrument. An object used (but not consumed) when performing instructions or a direction." ;
        rdfs:label          "tool" ;
        rdfs:subPropertyOf  schema:instrument .

schema:answerExplanation
        a             rdf:Property ;
        rdfs:comment  "A step-by-step or full explanation about Answer. Can outline how this Answer was achieved or contain more broad clarification or statement about it. " ;
        rdfs:label    "answerExplanation" .

schema:publishedOn  a  rdf:Property ;
        rdfs:comment  "A broadcast service associated with the publication event." ;
        rdfs:label    "publishedOn" .

schema:numberOfBeds  a  rdf:Property ;
        rdfs:comment  "The quantity of the given bed type available in the HotelRoom, Suite, House, or Apartment." ;
        rdfs:label    "numberOfBeds" .

schema:endTime  a     rdf:Property ;
        rdfs:comment  "The endTime of something. For a reserved event or service (e.g. FoodEstablishmentReservation), the time that it is expected to end. For actions that span a period of time, when the action was performed. e.g. John wrote a book from January to *December*. For media, including audio and video, it's the time offset of the end of a clip within a larger file.\\n\\nNote that Event uses startDate/endDate instead of startTime/endTime, even when describing dates with times. This situation may be clarified in future revisions." ;
        rdfs:label    "endTime" .

schema:lyrics  a      rdf:Property ;
        rdfs:comment  "The words in the song." ;
        rdfs:label    "lyrics" .

schema:RejectAction  a   rdfs:Class ;
        rdfs:comment     "The act of rejecting to/adopting an object.\\n\\nRelated actions:\\n\\n* [[AcceptAction]]: The antonym of RejectAction." ;
        rdfs:label       "RejectAction" ;
        rdfs:subClassOf  schema:AllocateAction .

schema:Motel  a          rdfs:Class ;
        rdfs:comment     "A motel.\n<br /><br />\nSee also the <a href=\"/docs/hotels.html\">dedicated document on the use of schema.org for marking up hotels and other forms of accommodations</a>.\n" ;
        rdfs:label       "Motel" ;
        rdfs:subClassOf  schema:LodgingBusiness .

schema:BookSeries  a     rdfs:Class ;
        rdfs:comment     "A series of books. Included books can be indicated with the hasPart property." ;
        rdfs:label       "BookSeries" ;
        rdfs:subClassOf  schema:CreativeWorkSeries .

schema:issn  a              rdf:Property ;
        rdfs:comment        "The International Standard Serial Number (ISSN) that identifies this serial publication. You can repeat this property to identify different formats of, or the linking ISSN (ISSN-L) for, this serial publication." ;
        rdfs:label          "issn" ;
        rdfs:subPropertyOf  schema:identifier .

schema:expectedArrivalUntil
        a             rdf:Property ;
        rdfs:comment  "The latest date the package may arrive." ;
        rdfs:label    "expectedArrivalUntil" .

schema:measuredProperty
        a             rdf:Property ;
        rdfs:comment  "The measuredProperty of an [[Observation]], either a schema.org property, a property from other RDF-compatible systems e.g. W3C RDF Data Cube, or schema.org extensions such as [GS1's](https://www.gs1.org/voc/?show=properties)." ;
        rdfs:label    "measuredProperty" .

schema:educationalAlignment
        a             rdf:Property ;
        rdfs:comment  "An alignment to an established educational framework.\n\nThis property should not be used where the nature of the alignment can be described using a simple property, for example to express that a resource [[teaches]] or [[assesses]] a competency." ;
        rdfs:label    "educationalAlignment" .

schema:resultReview  a      rdf:Property ;
        rdfs:comment        "A sub property of result. The review that resulted in the performing of the action." ;
        rdfs:label          "resultReview" ;
        rdfs:subPropertyOf  schema:result .

schema:arrivalTerminal
        a             rdf:Property ;
        rdfs:comment  "Identifier of the flight's arrival terminal." ;
        rdfs:label    "arrivalTerminal" .

schema:providesService
        a             rdf:Property ;
        rdfs:comment  "The service provided by this channel." ;
        rdfs:label    "providesService" .

schema:eventSchedule  a  rdf:Property ;
        rdfs:comment  "Associates an [[Event]] with a [[Schedule]]. There are circumstances where it is preferable to share a schedule for a series of\n      repeating events rather than data on the individual events themselves. For example, a website or application might prefer to publish a schedule for a weekly\n      gym class rather than provide data on every event. A schedule could be processed by applications to add forthcoming events to a calendar. An [[Event]] that\n      is associated with a [[Schedule]] using this property should not have [[startDate]] or [[endDate]] properties. These are instead defined within the associated\n      [[Schedule]], this avoids any ambiguity for clients using the data. The property might have repeated values to specify different schedules, e.g. for different months\n      or seasons." ;
        rdfs:label    "eventSchedule" .

schema:assemblyVersion
        a             rdf:Property ;
        rdfs:comment  "Associated product/technology version. e.g., .NET Framework 4.5." ;
        rdfs:label    "assemblyVersion" .

schema:videoQuality  a  rdf:Property ;
        rdfs:comment  "The quality of the video." ;
        rdfs:label    "videoQuality" .

schema:worstRating  a  rdf:Property ;
        rdfs:comment  "The lowest value allowed in this rating system. If worstRating is omitted, 1 is assumed." ;
        rdfs:label    "worstRating" .

schema:PaymentCard  a    rdfs:Class ;
        rdfs:comment     "A payment method using a credit, debit, store or other card to associate the payment with an account." ;
        rdfs:label       "PaymentCard" ;
        rdfs:subClassOf  schema:PaymentMethod , schema:FinancialProduct .

foaf:Person  a  rdfs:Class .

schema:ChildrensEvent
        a                rdfs:Class ;
        rdfs:comment     "Event type: Children's event." ;
        rdfs:label       "ChildrensEvent" ;
        rdfs:subClassOf  schema:Event .

schema:hasMenu  a     rdf:Property ;
        rdfs:comment  "Either the actual menu as a structured representation, as text, or a URL of the menu." ;
        rdfs:label    "hasMenu" .

schema:HyperToc  a       rdfs:Class ;
        rdfs:comment     "A HyperToc represents a hypertext table of contents for complex media objects, such as [[VideoObject]], [[AudioObject]]. Items in the table of contents are indicated using the [[tocEntry]] property, and typed [[HyperTocEntry]]. For cases where the same larger work is split into multiple files, [[associatedMedia]] can be used on individual [[HyperTocEntry]] items." ;
        rdfs:label       "HyperToc" ;
        rdfs:subClassOf  schema:CreativeWork .

schema:recordedAt  a  rdf:Property ;
        rdfs:comment  "The Event where the CreativeWork was recorded. The CreativeWork may capture all or part of the event." ;
        rdfs:label    "recordedAt" .

schema:arrivalBoatTerminal
        a             rdf:Property ;
        rdfs:comment  "The terminal or port from which the boat arrives." ;
        rdfs:label    "arrivalBoatTerminal" .

schema:mainContentOfPage
        a             rdf:Property ;
        rdfs:comment  "Indicates if this web page element is the main subject of the page." ;
        rdfs:label    "mainContentOfPage" .

schema:Attorney  a       rdfs:Class ;
        rdfs:comment     "Professional service: Attorney. \\n\\nThis type is deprecated - [[LegalService]] is more inclusive and less ambiguous." ;
        rdfs:label       "Attorney" ;
        rdfs:subClassOf  schema:LegalService .

schema:spouse  a      rdf:Property ;
        rdfs:comment  "The person's spouse." ;
        rdfs:label    "spouse" .

schema:recordLabel  a  rdf:Property ;
        rdfs:comment  "The label that issued the release." ;
        rdfs:label    "recordLabel" .

schema:numberOfSeasons
        a             rdf:Property ;
        rdfs:comment  "The number of seasons in this series." ;
        rdfs:label    "numberOfSeasons" .

schema:MobileApplication
        a                rdfs:Class ;
        rdfs:comment     "A software application designed specifically to work well on a mobile device such as a telephone." ;
        rdfs:label       "MobileApplication" ;
        rdfs:subClassOf  schema:SoftwareApplication .

schema:ContactPoint  a   rdfs:Class ;
        rdfs:comment     "A contact point&#x2014;for example, a Customer Complaints department." ;
        rdfs:label       "ContactPoint" ;
        rdfs:subClassOf  schema:StructuredValue .

schema:nextItem  a    rdf:Property ;
        rdfs:comment  "A link to the ListItem that follows the current one." ;
        rdfs:label    "nextItem" .

schema:InteractAction
        a                rdfs:Class ;
        rdfs:comment     "The act of interacting with another person or organization." ;
        rdfs:label       "InteractAction" ;
        rdfs:subClassOf  schema:Action .

schema:costOrigin  a  rdf:Property ;
        rdfs:comment  "Additional details to capture the origin of the cost data. For example, 'Medicare Part B'." ;
        rdfs:label    "costOrigin" .

schema:cutoffTime  a  rdf:Property ;
        rdfs:comment  "Order cutoff time allows merchants to describe the time after which they will no longer process orders received on that day. For orders processed after cutoff time, one day gets added to the delivery time estimate. This property is expected to be most typically used via the [[ShippingRateSettings]] publication pattern. The time is indicated using the ISO-8601 Time format, e.g. \"23:30:00-05:00\" would represent 6:30 pm Eastern Standard Time (EST) which is 5 hours behind Coordinated Universal Time (UTC)." ;
        rdfs:label    "cutoffTime" .

schema:deliveryAddress
        a             rdf:Property ;
        rdfs:comment  "Destination address." ;
        rdfs:label    "deliveryAddress" .

schema:MedicalAudienceType
        a                rdfs:Class ;
        rdfs:comment     "Target audiences types for medical web pages. Enumerated type." ;
        rdfs:label       "MedicalAudienceType" ;
        rdfs:subClassOf  schema:MedicalEnumeration .

schema:DrugLegalStatus
        a                rdfs:Class ;
        rdfs:comment     "The legal availability status of a medical drug." ;
        rdfs:label       "DrugLegalStatus" ;
        rdfs:subClassOf  schema:MedicalIntangible .

schema:softwareHelp  a  rdf:Property ;
        rdfs:comment  "Software application help." ;
        rdfs:label    "softwareHelp" .

schema:SubwayStation  a  rdfs:Class ;
        rdfs:comment     "A subway station." ;
        rdfs:label       "SubwayStation" ;
        rdfs:subClassOf  schema:CivicStructure .

schema:valueMinLength
        a             rdf:Property ;
        rdfs:comment  "Specifies the minimum allowed range for number of characters in a literal value." ;
        rdfs:label    "valueMinLength" .

schema:FollowAction  a   rdfs:Class ;
        rdfs:comment     "The act of forming a personal connection with someone/something (object) unidirectionally/asymmetrically to get updates polled from.\\n\\nRelated actions:\\n\\n* [[BefriendAction]]: Unlike BefriendAction, FollowAction implies that the connection is *not* necessarily reciprocal.\\n* [[SubscribeAction]]: Unlike SubscribeAction, FollowAction implies that the follower acts as an active agent constantly/actively polling for updates.\\n* [[RegisterAction]]: Unlike RegisterAction, FollowAction implies that the agent is interested in continuing receiving updates from the object.\\n* [[JoinAction]]: Unlike JoinAction, FollowAction implies that the agent is interested in getting updates from the object.\\n* [[TrackAction]]: Unlike TrackAction, FollowAction refers to the polling of updates of all aspects of animate objects rather than the location of inanimate objects (e.g. you track a package, but you don't follow it)." ;
        rdfs:label       "FollowAction" ;
        rdfs:subClassOf  schema:InteractAction .

schema:speakable  a   rdf:Property ;
        rdfs:comment  "Indicates sections of a Web page that are particularly 'speakable' in the sense of being highlighted as being especially appropriate for text-to-speech conversion. Other sections of a page may also be usefully spoken in particular circumstances; the 'speakable' property serves to indicate the parts most likely to be generally useful for speech.\n\nThe *speakable* property can be repeated an arbitrary number of times, with three kinds of possible 'content-locator' values:\n\n1.) *id-value* URL references - uses *id-value* of an element in the page being annotated. The simplest use of *speakable* has (potentially relative) URL values, referencing identified sections of the document concerned.\n\n2.) CSS Selectors - addresses content in the annotated page, eg. via class attribute. Use the [[cssSelector]] property.\n\n3.)  XPaths - addresses content via XPaths (assuming an XML view of the content). Use the [[xpath]] property.\n\n\nFor more sophisticated markup of speakable sections beyond simple ID references, either CSS selectors or XPath expressions to pick out document section(s) as speakable. For this\nwe define a supporting type, [[SpeakableSpecification]]  which is defined to be a possible value of the *speakable* property.\n         " ;
        rdfs:label    "speakable" .

schema:includedRiskFactor
        a             rdf:Property ;
        rdfs:comment  "A modifiable or non-modifiable risk factor included in the calculation, e.g. age, coexisting condition." ;
        rdfs:label    "includedRiskFactor" .

schema:typicalTest  a  rdf:Property ;
        rdfs:comment  "A medical test typically performed given this condition." ;
        rdfs:label    "typicalTest" .

schema:material  a    rdf:Property ;
        rdfs:comment  "A material that something is made from, e.g. leather, wool, cotton, paper." ;
        rdfs:label    "material" .

schema:editEIDR  a          rdf:Property ;
        rdfs:comment        "An [EIDR](https://eidr.org/) (Entertainment Identifier Registry) [[identifier]] representing a specific edit / edition for a work of film or television.\n\nFor example, the motion picture known as \"Ghostbusters\" whose [[titleEIDR]] is \"10.5240/7EC7-228A-510A-053E-CBB8-J\", has several edits e.g. \"10.5240/1F2A-E1C5-680A-14C6-E76B-I\" and \"10.5240/8A35-3BEE-6497-5D12-9E4F-3\".\n\nSince schema.org types like [[Movie]] and [[TVEpisode]] can be used for both works and their multiple expressions, it is possible to use [[titleEIDR]] alone (for a general description), or alongside [[editEIDR]] for a more edit-specific description.\n" ;
        rdfs:label          "editEIDR" ;
        rdfs:subPropertyOf  schema:identifier .

schema:Oncologic  a      rdfs:Class ;
        rdfs:comment     "A specific branch of medical science that deals with benign and malignant tumors, including the study of their development, diagnosis, treatment and prevention." ;
        rdfs:label       "Oncologic" ;
        rdfs:subClassOf  schema:MedicalBusiness .

schema:Product  a        rdfs:Class ;
        rdfs:comment     "Any offered product or service. For example: a pair of shoes; a concert ticket; the rental of a car; a haircut; or an episode of a TV show streamed online." ;
        rdfs:label       "Product" ;
        rdfs:subClassOf  schema:Thing .

schema:unitCode  a    rdf:Property ;
        rdfs:comment  "The unit of measurement given using the UN/CEFACT Common Code (3 characters) or a URL. Other codes than the UN/CEFACT Common Code may be used with a prefix followed by a colon." ;
        rdfs:label    "unitCode" .

schema:subStageSuffix
        a             rdf:Property ;
        rdfs:comment  "The substage, e.g. 'a' for Stage IIIa." ;
        rdfs:label    "subStageSuffix" .

schema:isConsumableFor
        a             rdf:Property ;
        rdfs:comment  "A pointer to another product (or multiple products) for which this product is a consumable." ;
        rdfs:label    "isConsumableFor" .

schema:DataFeed  a       rdfs:Class ;
        rdfs:comment     "A single feed providing structured information about one or more entities or topics." ;
        rdfs:label       "DataFeed" ;
        rdfs:subClassOf  schema:Dataset .

schema:productSupported
        a             rdf:Property ;
        rdfs:comment  "The product or service this support contact point is related to (such as product support for a particular product line). This can be a specific product or product line (e.g. \"iPhone\") or a general category of products or services (e.g. \"smartphones\")." ;
        rdfs:label    "productSupported" .

schema:exerciseRelatedDiet
        a                   rdf:Property ;
        rdfs:comment        "A sub property of instrument. The diet used in this action." ;
        rdfs:label          "exerciseRelatedDiet" ;
        rdfs:subPropertyOf  schema:instrument .

schema:RealEstateListing
        a                rdfs:Class ;
        rdfs:comment     "A [[RealEstateListing]] is a listing that describes one or more real-estate [[Offer]]s (whose [[businessFunction]] is typically to lease out, or to sell).\n  The [[RealEstateListing]] type itself represents the overall listing, as manifested in some [[WebPage]].\n  " ;
        rdfs:label       "RealEstateListing" ;
        rdfs:subClassOf  schema:WebPage .

schema:DietarySupplement
        a                rdfs:Class ;
        rdfs:comment     "A product taken by mouth that contains a dietary ingredient intended to supplement the diet. Dietary ingredients may include vitamins, minerals, herbs or other botanicals, amino acids, and substances such as enzymes, organ tissues, glandulars and metabolites." ;
        rdfs:label       "DietarySupplement" ;
        rdfs:subClassOf  schema:Substance .

schema:instrument  a  rdf:Property ;
        rdfs:comment  "The object that helped the agent perform the action. e.g. John wrote a book with *a pen*." ;
        rdfs:label    "instrument" .

schema:PeopleAudience
        a                rdfs:Class ;
        rdfs:comment     "A set of characteristics belonging to people, e.g. who compose an item's target audience." ;
        rdfs:label       "PeopleAudience" ;
        rdfs:subClassOf  schema:Audience .

schema:ccRecipient  a       rdf:Property ;
        rdfs:comment        "A sub property of recipient. The recipient copied on a message." ;
        rdfs:label          "ccRecipient" ;
        rdfs:subPropertyOf  schema:recipient .

schema:MedicalIndication
        a                rdfs:Class ;
        rdfs:comment     "A condition or factor that indicates use of a medical therapy, including signs, symptoms, risk factors, anatomical states, etc." ;
        rdfs:label       "MedicalIndication" ;
        rdfs:subClassOf  schema:MedicalEntity .

schema:UserTweets  a     rdfs:Class ;
        rdfs:comment     "UserInteraction and its subtypes is an old way of talking about users interacting with pages. It is generally better to use [[Action]]-based vocabulary, alongside types such as [[Comment]]." ;
        rdfs:label       "UserTweets" ;
        rdfs:subClassOf  schema:UserInteraction .

schema:Question  a       rdfs:Class ;
        rdfs:comment     "A specific question - e.g. from a user seeking answers online, or collected in a Frequently Asked Questions (FAQ) document." ;
        rdfs:label       "Question" ;
        rdfs:subClassOf  schema:Comment .

schema:ownedThrough  a  rdf:Property ;
        rdfs:comment  "The date and time of giving up ownership on the product." ;
        rdfs:label    "ownedThrough" .

schema:acceptsReservations
        a             rdf:Property ;
        rdfs:comment  "Indicates whether a FoodEstablishment accepts reservations. Values can be Boolean, an URL at which reservations can be made or (for backwards compatibility) the strings ```Yes``` or ```No```." ;
        rdfs:label    "acceptsReservations" .

schema:MusicReleaseFormatType
        a                rdfs:Class ;
        rdfs:comment     "Format of this release (the type of recording media used, ie. compact disc, digital media, LP, etc.)." ;
        rdfs:label       "MusicReleaseFormatType" ;
        rdfs:subClassOf  schema:Enumeration .

schema:SingleFamilyResidence
        a                rdfs:Class ;
        rdfs:comment     "Residence type: Single-family home." ;
        rdfs:label       "SingleFamilyResidence" ;
        rdfs:subClassOf  schema:House .

schema:gettingTestedInfo
        a             rdf:Property ;
        rdfs:comment  "Information about getting tested (for a [[MedicalCondition]]), e.g. in the context of a pandemic." ;
        rdfs:label    "gettingTestedInfo" .

schema:acrissCode  a  rdf:Property ;
        rdfs:comment  "The ACRISS Car Classification Code is a code used by many car rental companies, for classifying vehicles. ACRISS stands for Association of Car Rental Industry Systems and Standards." ;
        rdfs:label    "acrissCode" .

schema:duplicateTherapy
        a             rdf:Property ;
        rdfs:comment  "A therapy that duplicates or overlaps this one." ;
        rdfs:label    "duplicateTherapy" .

schema:MedicalSpecialty
        a                rdfs:Class ;
        rdfs:comment     "Any specific branch of medical science or practice. Medical specialities include clinical specialties that pertain to particular organ systems and their respective disease states, as well as allied health specialties. Enumerated type." ;
        rdfs:label       "MedicalSpecialty" ;
        rdfs:subClassOf  schema:MedicalEnumeration , schema:Specialty .

schema:healthPlanId  a  rdf:Property ;
        rdfs:comment  "The 14-character, HIOS-generated Plan ID number. (Plan IDs must be unique, even across different markets.)" ;
        rdfs:label    "healthPlanId" .

schema:releasedEvent  a  rdf:Property ;
        rdfs:comment  "The place and time the release was issued, expressed as a PublicationEvent." ;
        rdfs:label    "releasedEvent" .

schema:Intangible  a     rdfs:Class ;
        rdfs:comment     "A utility class that serves as the umbrella for a number of 'intangible' things such as quantities, structured values, etc." ;
        rdfs:label       "Intangible" ;
        rdfs:subClassOf  schema:Thing .

schema:cvdFacilityId  a  rdf:Property ;
        rdfs:comment  "Identifier of the NHSN facility that this data record applies to. Use [[cvdFacilityCounty]] to indicate the county. To provide other details, [[healthcareReportingData]] can be used on a [[Hospital]] entry." ;
        rdfs:label    "cvdFacilityId" .

schema:Reservoir  a      rdfs:Class ;
        rdfs:comment     "A reservoir of water, typically an artificially created lake, like the Lake Kariba reservoir." ;
        rdfs:label       "Reservoir" ;
        rdfs:subClassOf  schema:BodyOfWater .

schema:InstallAction  a  rdfs:Class ;
        rdfs:comment     "The act of installing an application." ;
        rdfs:label       "InstallAction" ;
        rdfs:subClassOf  schema:ConsumeAction .

schema:adverseOutcome
        a             rdf:Property ;
        rdfs:comment  "A possible complication and/or side effect of this therapy. If it is known that an adverse outcome is serious (resulting in death, disability, or permanent damage; requiring hospitalization; or is otherwise life-threatening or requires immediate medical attention), tag it as a seriouseAdverseOutcome instead." ;
        rdfs:label    "adverseOutcome" .

schema:language  a          rdf:Property ;
        rdfs:comment        "A sub property of instrument. The language used on this action." ;
        rdfs:label          "language" ;
        rdfs:subPropertyOf  schema:instrument .

schema:ComputerStore  a  rdfs:Class ;
        rdfs:comment     "A computer store." ;
        rdfs:label       "ComputerStore" ;
        rdfs:subClassOf  schema:Store .

schema:MusicVenue  a     rdfs:Class ;
        rdfs:comment     "A music venue." ;
        rdfs:label       "MusicVenue" ;
        rdfs:subClassOf  schema:CivicStructure .

schema:layoutImage  a       rdf:Property ;
        rdfs:comment        "A schematic image showing the floorplan layout." ;
        rdfs:label          "layoutImage" ;
        rdfs:subPropertyOf  schema:image .

schema:BoatTrip  a       rdfs:Class ;
        rdfs:comment     "A trip on a commercial ferry line." ;
        rdfs:label       "BoatTrip" ;
        rdfs:subClassOf  schema:Trip .

schema:Specialty  a      rdfs:Class ;
        rdfs:comment     "Any branch of a field in which people typically develop specific expertise, usually after significant study, time, and effort." ;
        rdfs:label       "Specialty" ;
        rdfs:subClassOf  schema:Enumeration .

schema:Joint  a          rdfs:Class ;
        rdfs:comment     "The anatomical location at which two or more bones make contact." ;
        rdfs:label       "Joint" ;
        rdfs:subClassOf  schema:AnatomicalStructure .

schema:sdDatePublished
        a             rdf:Property ;
        rdfs:comment  "Indicates the date on which the current structured data was generated / published. Typically used alongside [[sdPublisher]]" ;
        rdfs:label    "sdDatePublished" .

schema:DislikeAction  a  rdfs:Class ;
        rdfs:comment     "The act of expressing a negative sentiment about the object. An agent dislikes an object (a proposition, topic or theme) with participants." ;
        rdfs:label       "DislikeAction" ;
        rdfs:subClassOf  schema:ReactAction .

schema:broadcastDisplayName
        a             rdf:Property ;
        rdfs:comment  "The name displayed in the channel guide. For many US affiliates, it is the network name." ;
        rdfs:label    "broadcastDisplayName" .

schema:Mountain  a       rdfs:Class ;
        rdfs:comment     "A mountain, like Mount Whitney or Mount Everest." ;
        rdfs:label       "Mountain" ;
        rdfs:subClassOf  schema:Landform .

schema:OfficeEquipmentStore
        a                rdfs:Class ;
        rdfs:comment     "An office equipment store." ;
        rdfs:label       "OfficeEquipmentStore" ;
        rdfs:subClassOf  schema:Store .

schema:TattooParlor  a   rdfs:Class ;
        rdfs:comment     "A tattoo parlor." ;
        rdfs:label       "TattooParlor" ;
        rdfs:subClassOf  schema:HealthAndBeautyBusiness .

schema:ownershipFundingInfo
        a                   rdf:Property ;
        rdfs:comment        "For an [[Organization]] (often but not necessarily a [[NewsMediaOrganization]]), a description of organizational ownership structure; funding and grants. In a news/media setting, this is with particular reference to editorial independence.   Note that the [[funder]] is also available and can be used to make basic funder information machine-readable." ;
        rdfs:label          "ownershipFundingInfo" ;
        rdfs:subPropertyOf  schema:publishingPrinciples .

schema:encodings  a   rdf:Property ;
        rdfs:comment  "A media object that encodes this CreativeWork." ;
        rdfs:label    "encodings" .

schema:photos  a      rdf:Property ;
        rdfs:comment  "Photographs of this place." ;
        rdfs:label    "photos" .

schema:requiredGender
        a             rdf:Property ;
        rdfs:comment  "Audiences defined by a person's gender." ;
        rdfs:label    "requiredGender" .

schema:cvdNumC19HOPats
        a             rdf:Property ;
        rdfs:comment  "numc19hopats - HOSPITAL ONSET: Patients hospitalized in an NHSN inpatient care location with onset of suspected or confirmed COVID-19 14 or more days after hospitalization." ;
        rdfs:label    "cvdNumC19HOPats" .

schema:SurgicalProcedure
        a                rdfs:Class ;
        rdfs:comment     "A medical procedure involving an incision with instruments; performed for diagnose, or therapeutic purposes." ;
        rdfs:label       "SurgicalProcedure" ;
        rdfs:subClassOf  schema:MedicalProcedure .

schema:SpecialAnnouncement
        a                rdfs:Class ;
        rdfs:comment     "A SpecialAnnouncement combines a simple date-stamped textual information update\n      with contextualized Web links and other structured data.  It represents an information update made by a\n      locally-oriented organization, for example schools, pharmacies, healthcare providers,  community groups, police,\n      local government.\n\nFor work in progress guidelines on Coronavirus-related markup see [this doc](https://docs.google.com/document/d/14ikaGCKxo50rRM7nvKSlbUpjyIk2WMQd3IkB1lItlrM/edit#).\n\nThe motivating scenario for SpecialAnnouncement is the [Coronavirus pandemic](https://en.wikipedia.org/wiki/2019%E2%80%9320_coronavirus_pandemic), and the initial vocabulary is oriented to this urgent situation. Schema.org\nexpect to improve the markup iteratively as it is deployed and as feedback emerges from use. In addition to our\nusual [Github entry](https://github.com/schemaorg/schemaorg/issues/2490), feedback comments can also be provided in [this document](https://docs.google.com/document/d/1fpdFFxk8s87CWwACs53SGkYv3aafSxz_DTtOQxMrBJQ/edit#).\n\n\nWhile this schema is designed to communicate urgent crisis-related information, it is not the same as an emergency warning technology like [CAP](https://en.wikipedia.org/wiki/Common_Alerting_Protocol), although there may be overlaps. The intent is to cover\nthe kinds of everyday practical information being posted to existing websites during an emergency situation.\n\nSeveral kinds of information can be provided:\n\nWe encourage the provision of \"name\", \"text\", \"datePosted\", \"expires\" (if appropriate), \"category\" and\n\"url\" as a simple baseline. It is important to provide a value for \"category\" where possible, most ideally as a well known\nURL from Wikipedia or Wikidata. In the case of the 2019-2020 Coronavirus pandemic, this should be \"https://en.wikipedia.org/w/index.php?title=2019-20\\_coronavirus\\_pandemic\" or \"https://www.wikidata.org/wiki/Q81068910\".\n\nFor many of the possible properties, values can either be simple links or an inline description, depending on whether a summary is available. For a link, provide just the URL of the appropriate page as the property's value. For an inline description, use a [[WebContent]] type, and provide the url as a property of that, alongside at least a simple \"[[text]]\" summary of the page. It is\nunlikely that a single SpecialAnnouncement will need all of the possible properties simultaneously.\n\nWe expect that in many cases the page referenced might contain more specialized structured data, e.g. contact info, [[openingHours]], [[Event]], [[FAQPage]] etc. By linking to those pages from a [[SpecialAnnouncement]] you can help make it clearer that the events are related to the situation (e.g. Coronavirus) indicated by the [[category]] property of the [[SpecialAnnouncement]].\n\nMany [[SpecialAnnouncement]]s will relate to particular regions and to identifiable local organizations. Use [[spatialCoverage]] for the region, and [[announcementLocation]] to indicate specific [[LocalBusiness]]es and [[CivicStructure]]s. If the announcement affects both a particular region and a specific location (for example, a library closure that serves an entire region), use both [[spatialCoverage]] and [[announcementLocation]].\n\nThe [[about]] property can be used to indicate entities that are the focus of the announcement. We now recommend using [[about]] only\nfor representing non-location entities (e.g. a [[Course]] or a [[RadioStation]]). For places, use [[announcementLocation]] and [[spatialCoverage]]. Consumers of this markup should be aware that the initial design encouraged the use of /about for locations too.\n\nThe basic content of [[SpecialAnnouncement]] is similar to that of an [RSS](https://en.wikipedia.org/wiki/RSS) or [Atom](https://en.wikipedia.org/wiki/Atom_(Web_standard)) feed. For publishers without such feeds, basic feed-like information can be shared by posting\n[[SpecialAnnouncement]] updates in a page, e.g. using JSON-LD. For sites with Atom/RSS functionality, you can point to a feed\nwith the [[webFeed]] property. This can be a simple URL, or an inline [[DataFeed]] object, with [[encodingFormat]] providing\nmedia type information e.g. \"application/rss+xml\" or \"application/atom+xml\".\n" ;
        rdfs:label       "SpecialAnnouncement" ;
        rdfs:subClassOf  schema:CreativeWork .

schema:TouristInformationCenter
        a                rdfs:Class ;
        rdfs:comment     "A tourist information center." ;
        rdfs:label       "TouristInformationCenter" ;
        rdfs:subClassOf  schema:LocalBusiness .

schema:mentions  a    rdf:Property ;
        rdfs:comment  "Indicates that the CreativeWork contains a reference to, but is not necessarily about a concept." ;
        rdfs:label    "mentions" .

schema:stageAsNumber  a  rdf:Property ;
        rdfs:comment  "The stage represented as a number, e.g. 3." ;
        rdfs:label    "stageAsNumber" .

schema:ExchangeRateSpecification
        a                rdfs:Class ;
        rdfs:comment     "A structured value representing exchange rate." ;
        rdfs:label       "ExchangeRateSpecification" ;
        rdfs:subClassOf  schema:StructuredValue .

schema:SportsClub  a     rdfs:Class ;
        rdfs:comment     "A sports club." ;
        rdfs:label       "SportsClub" ;
        rdfs:subClassOf  schema:SportsActivityLocation .

schema:accountablePerson
        a             rdf:Property ;
        rdfs:comment  "Specifies the Person that is legally accountable for the CreativeWork." ;
        rdfs:label    "accountablePerson" .

schema:DepartAction  a   rdfs:Class ;
        rdfs:comment     "The act of  departing from a place. An agent departs from an fromLocation for a destination, optionally with participants." ;
        rdfs:label       "DepartAction" ;
        rdfs:subClassOf  schema:MoveAction .

schema:follows  a     rdf:Property ;
        rdfs:comment  "The most generic uni-directional social relation." ;
        rdfs:label    "follows" .

schema:cholesterolContent
        a             rdf:Property ;
        rdfs:comment  "The number of milligrams of cholesterol." ;
        rdfs:label    "cholesterolContent" .

schema:Hackathon  a      rdfs:Class ;
        rdfs:comment     "A [hackathon](https://en.wikipedia.org/wiki/Hackathon) event." ;
        rdfs:label       "Hackathon" ;
        rdfs:subClassOf  schema:Event .

schema:knows  a       rdf:Property ;
        rdfs:comment  "The most generic bi-directional social/work relation." ;
        rdfs:label    "knows" .

schema:acceptedPaymentMethod
        a             rdf:Property ;
        rdfs:comment  "The payment method(s) accepted by seller for this offer." ;
        rdfs:label    "acceptedPaymentMethod" .

schema:BrainStructure
        a                rdfs:Class ;
        rdfs:comment     "Any anatomical structure which pertains to the soft nervous tissue functioning as the coordinating center of sensation and intellectual and nervous activity." ;
        rdfs:label       "BrainStructure" ;
        rdfs:subClassOf  schema:AnatomicalStructure .

schema:webCheckinTime
        a             rdf:Property ;
        rdfs:comment  "The time when a passenger can check into the flight online." ;
        rdfs:label    "webCheckinTime" .

schema:Season  a         rdfs:Class ;
        rdfs:comment     "A media season e.g. tv, radio, video game etc." ;
        rdfs:label       "Season" ;
        rdfs:subClassOf  schema:CreativeWork .

schema:validThrough  a  rdf:Property ;
        rdfs:comment  "The date after when the item is not valid. For example the end of an offer, salary period, or a period of opening hours." ;
        rdfs:label    "validThrough" .

schema:headline  a    rdf:Property ;
        rdfs:comment  "Headline of the article." ;
        rdfs:label    "headline" .

schema:BowlingAlley  a   rdfs:Class ;
        rdfs:comment     "A bowling alley." ;
        rdfs:label       "BowlingAlley" ;
        rdfs:subClassOf  schema:SportsActivityLocation .

schema:petsAllowed  a  rdf:Property ;
        rdfs:comment  "Indicates whether pets are allowed to enter the accommodation or lodging business. More detailed information can be put in a text value." ;
        rdfs:label    "petsAllowed" .

schema:readonlyValue  a  rdf:Property ;
        rdfs:comment  "Whether or not a property is mutable.  Default is false. Specifying this for a property that also has a value makes it act similar to a \"hidden\" input in an HTML form." ;
        rdfs:label    "readonlyValue" .

schema:album  a       rdf:Property ;
        rdfs:comment  "A music album." ;
        rdfs:label    "album" .

schema:volumeNumber  a      rdf:Property ;
        rdfs:comment        "Identifies the volume of publication or multi-part work; for example, \"iii\" or \"2\"." ;
        rdfs:label          "volumeNumber" ;
        rdfs:subPropertyOf  schema:position .

schema:Patient  a        rdfs:Class ;
        rdfs:comment     "A patient is any person recipient of health care services." ;
        rdfs:label       "Patient" ;
        rdfs:subClassOf  schema:MedicalAudience , schema:Person .

schema:DeliveryChargeSpecification
        a                rdfs:Class ;
        rdfs:comment     "The price for the delivery of an offer using a particular delivery method." ;
        rdfs:label       "DeliveryChargeSpecification" ;
        rdfs:subClassOf  schema:PriceSpecification .

schema:hiringOrganization
        a             rdf:Property ;
        rdfs:comment  "Organization offering the job position." ;
        rdfs:label    "hiringOrganization" .

schema:RefundTypeEnumeration
        a                rdfs:Class ;
        rdfs:comment     "RefundTypeEnumeration enumerates several kinds of product return refund types." ;
        rdfs:label       "RefundTypeEnumeration" ;
        rdfs:subClassOf  schema:Enumeration .

schema:Campground  a     rdfs:Class ;
        rdfs:comment     "A camping site, campsite, or [[Campground]] is a place used for overnight stay in the outdoors, typically containing individual [[CampingPitch]] locations. \\n\\n\nIn British English a campsite is an area, usually divided into a number of pitches, where people can camp overnight using tents or camper vans or caravans; this British English use of the word is synonymous with the American English expression campground. In American English the term campsite generally means an area where an individual, family, group, or military unit can pitch a tent or park a camper; a campground may contain many campsites (Source: Wikipedia see [https://en.wikipedia.org/wiki/Campsite](https://en.wikipedia.org/wiki/Campsite)).\\n\\n\n\nSee also the dedicated [document on the use of schema.org for marking up hotels and other forms of accommodations](/docs/hotels.html).\n" ;
        rdfs:label       "Campground" ;
        rdfs:subClassOf  schema:CivicStructure , schema:LodgingBusiness .

schema:exercisePlan  a      rdf:Property ;
        rdfs:comment        "A sub property of instrument. The exercise plan used on this action." ;
        rdfs:label          "exercisePlan" ;
        rdfs:subPropertyOf  schema:instrument .

schema:educationalLevel
        a             rdf:Property ;
        rdfs:comment  "The level in terms of progression through an educational or training context. Examples of educational levels include 'beginner', 'intermediate' or 'advanced', and formal sets of level indicators." ;
        rdfs:label    "educationalLevel" .

schema:firstAppearance
        a                   rdf:Property ;
        rdfs:comment        "Indicates the first known occurence of a [[Claim]] in some [[CreativeWork]]." ;
        rdfs:label          "firstAppearance" ;
        rdfs:subPropertyOf  schema:workExample .

schema:availableLanguage
        a             rdf:Property ;
        rdfs:comment  "A language someone may use with or at the item, service or place. Please use one of the language codes from the [IETF BCP 47 standard](http://tools.ietf.org/html/bcp47). See also [[inLanguage]]" ;
        rdfs:label    "availableLanguage" .

schema:Restaurant  a     rdfs:Class ;
        rdfs:comment     "A restaurant." ;
        rdfs:label       "Restaurant" ;
        rdfs:subClassOf  schema:FoodEstablishment .

schema:accessibilityAPI
        a             rdf:Property ;
        rdfs:comment  "Indicates that the resource is compatible with the referenced accessibility API ([WebSchemas wiki lists possible values](http://www.w3.org/wiki/WebSchemas/Accessibility))." ;
        rdfs:label    "accessibilityAPI" .

schema:LocationFeatureSpecification
        a                rdfs:Class ;
        rdfs:comment     "Specifies a location feature by providing a structured value representing a feature of an accommodation as a property-value pair of varying degrees of formality." ;
        rdfs:label       "LocationFeatureSpecification" ;
        rdfs:subClassOf  schema:PropertyValue .

schema:url  a         rdf:Property ;
        rdfs:comment  "URL of the item." ;
        rdfs:label    "url" .

schema:catalog  a     rdf:Property ;
        rdfs:comment  "A data catalog which contains this dataset." ;
        rdfs:label    "catalog" .

schema:bookFormat  a  rdf:Property ;
        rdfs:comment  "The format of the book." ;
        rdfs:label    "bookFormat" .

schema:usesDevice  a  rdf:Property ;
        rdfs:comment  "Device used to perform the test." ;
        rdfs:label    "usesDevice" .

schema:Country  a        rdfs:Class ;
        rdfs:comment     "A country." ;
        rdfs:label       "Country" ;
        rdfs:subClassOf  schema:AdministrativeArea .

schema:FilmAction  a     rdfs:Class ;
        rdfs:comment     "The act of capturing sound and moving images on film, video, or digitally." ;
        rdfs:label       "FilmAction" ;
        rdfs:subClassOf  schema:CreateAction .

schema:InviteAction  a   rdfs:Class ;
        rdfs:comment     "The act of asking someone to attend an event. Reciprocal of RsvpAction." ;
        rdfs:label       "InviteAction" ;
        rdfs:subClassOf  schema:CommunicateAction .

schema:serviceType  a  rdf:Property ;
        rdfs:comment  "The type of service being offered, e.g. veterans' benefits, emergency relief, etc." ;
        rdfs:label    "serviceType" .

schema:programPrerequisites
        a             rdf:Property ;
        rdfs:comment  "Prerequisites for enrolling in the program." ;
        rdfs:label    "programPrerequisites" .

schema:position  a    rdf:Property ;
        rdfs:comment  "The position of an item in a series or sequence of items." ;
        rdfs:label    "position" .

schema:vehicleTransmission
        a             rdf:Property ;
        rdfs:comment  "The type of component used for transmitting the power from a rotating power source to the wheels or other relevant component(s) (\"gearbox\" for cars)." ;
        rdfs:label    "vehicleTransmission" .

schema:cookTime  a          rdf:Property ;
        rdfs:comment        "The time it takes to actually cook the dish, in [ISO 8601 duration format](http://en.wikipedia.org/wiki/ISO_8601)." ;
        rdfs:label          "cookTime" ;
        rdfs:subPropertyOf  schema:performTime .

schema:endDate  a     rdf:Property ;
        rdfs:comment  "The end date and time of the item (in [ISO 8601 date format](http://en.wikipedia.org/wiki/ISO_8601))." ;
        rdfs:label    "endDate" .

schema:codeValue  a         rdf:Property ;
        rdfs:comment        "A short textual code that uniquely identifies the value." ;
        rdfs:label          "codeValue" ;
        rdfs:subPropertyOf  schema:termCode .

schema:LeaveAction  a    rdfs:Class ;
        rdfs:comment     "An agent leaves an event / group with participants/friends at a location.\\n\\nRelated actions:\\n\\n* [[JoinAction]]: The antonym of LeaveAction.\\n* [[UnRegisterAction]]: Unlike UnRegisterAction, LeaveAction implies leaving a group/team of people rather than a service." ;
        rdfs:label       "LeaveAction" ;
        rdfs:subClassOf  schema:InteractAction .

schema:Pediatric  a      rdfs:Class ;
        rdfs:comment     "A specific branch of medical science that specializes in the care of infants, children and adolescents." ;
        rdfs:label       "Pediatric" ;
        rdfs:subClassOf  schema:MedicalBusiness .

schema:userInteractionCount
        a             rdf:Property ;
        rdfs:comment  "The number of interactions for the CreativeWork using the WebSite or SoftwareApplication." ;
        rdfs:label    "userInteractionCount" .

schema:programmingModel
        a             rdf:Property ;
        rdfs:comment  "Indicates whether API is managed or unmanaged." ;
        rdfs:label    "programmingModel" .

schema:TelevisionChannel
        a                rdfs:Class ;
        rdfs:comment     "A unique instance of a television BroadcastService on a CableOrSatelliteService lineup." ;
        rdfs:label       "TelevisionChannel" ;
        rdfs:subClassOf  schema:BroadcastChannel .

schema:PlasticSurgery
        a                rdfs:Class ;
        rdfs:comment     "A specific branch of medical science that pertains to therapeutic or cosmetic repair or re-formation of missing, injured or malformed tissues or body parts by manual and instrumental means." ;
        rdfs:label       "PlasticSurgery" ;
        rdfs:subClassOf  schema:MedicalBusiness .

schema:UserPlays  a      rdfs:Class ;
        rdfs:comment     "UserInteraction and its subtypes is an old way of talking about users interacting with pages. It is generally better to use [[Action]]-based vocabulary, alongside types such as [[Comment]]." ;
        rdfs:label       "UserPlays" ;
        rdfs:subClassOf  schema:UserInteraction .

schema:UnRegisterAction
        a                rdfs:Class ;
        rdfs:comment     "The act of un-registering from a service.\\n\\nRelated actions:\\n\\n* [[RegisterAction]]: antonym of UnRegisterAction.\\n* [[LeaveAction]]: Unlike LeaveAction, UnRegisterAction implies that you are unregistering from a service you werer previously registered, rather than leaving a team/group of people." ;
        rdfs:label       "UnRegisterAction" ;
        rdfs:subClassOf  schema:InteractAction .

schema:iswcCode  a    rdf:Property ;
        rdfs:comment  "The International Standard Musical Work Code for the composition." ;
        rdfs:label    "iswcCode" .

schema:mainEntityOfPage
        a             rdf:Property ;
        rdfs:comment  "Indicates a page (or other CreativeWork) for which this thing is the main entity being described. See [background notes](/docs/datamodel.html#mainEntityBackground) for details." ;
        rdfs:label    "mainEntityOfPage" .

schema:requiresSubscription
        a             rdf:Property ;
        rdfs:comment  "Indicates if use of the media require a subscription  (either paid or free). Allowed values are ```true``` or ```false``` (note that an earlier version had 'yes', 'no')." ;
        rdfs:label    "requiresSubscription" .

schema:logo  a              rdf:Property ;
        rdfs:comment        "An associated logo." ;
        rdfs:label          "logo" ;
        rdfs:subPropertyOf  schema:image .

schema:pickupLocation
        a             rdf:Property ;
        rdfs:comment  "Where a taxi will pick up a passenger or a rental car can be picked up." ;
        rdfs:label    "pickupLocation" .

schema:transcript  a  rdf:Property ;
        rdfs:comment  "If this MediaObject is an AudioObject or VideoObject, the transcript of that object." ;
        rdfs:label    "transcript" .

schema:returnPolicyCategory
        a             rdf:Property ;
        rdfs:comment  "A returnPolicyCategory expresses at most one of several enumerated kinds of return." ;
        rdfs:label    "returnPolicyCategory" .

schema:vehicleModelDate
        a             rdf:Property ;
        rdfs:comment  "The release date of a vehicle model (often used to differentiate versions of the same make and model)." ;
        rdfs:label    "vehicleModelDate" .

schema:successorOf  a  rdf:Property ;
        rdfs:comment  "A pointer from a newer variant of a product  to its previous, often discontinued predecessor." ;
        rdfs:label    "successorOf" .

schema:physiologicalBenefits
        a             rdf:Property ;
        rdfs:comment  "Specific physiologic benefits associated to the plan." ;
        rdfs:label    "physiologicalBenefits" .

schema:title  a       rdf:Property ;
        rdfs:comment  "The title of the job." ;
        rdfs:label    "title" .

schema:GasStation  a     rdfs:Class ;
        rdfs:comment     "A gas station." ;
        rdfs:label       "GasStation" ;
        rdfs:subClassOf  schema:AutomotiveBusiness .

schema:DrinkAction  a    rdfs:Class ;
        rdfs:comment     "The act of swallowing liquids." ;
        rdfs:label       "DrinkAction" ;
        rdfs:subClassOf  schema:ConsumeAction .

schema:CarUsageType  a   rdfs:Class ;
        rdfs:comment     "A value indicating a special usage of a car, e.g. commercial rental, driving school, or as a taxi." ;
        rdfs:label       "CarUsageType" ;
        rdfs:subClassOf  schema:Enumeration .

schema:VideoGallery  a   rdfs:Class ;
        rdfs:comment     "Web page type: Video gallery page." ;
        rdfs:label       "VideoGallery" ;
        rdfs:subClassOf  schema:MediaGallery .

schema:primaryImageOfPage
        a             rdf:Property ;
        rdfs:comment  "Indicates the main image on the page." ;
        rdfs:label    "primaryImageOfPage" .

schema:businessFunction
        a             rdf:Property ;
        rdfs:comment  "The business function (e.g. sell, lease, repair, dispose) of the offer or component of a bundle (TypeAndQuantityNode). The default is http://purl.org/goodrelations/v1#Sell." ;
        rdfs:label    "businessFunction" .

schema:FoodEstablishment
        a                rdfs:Class ;
        rdfs:comment     "A food-related business." ;
        rdfs:label       "FoodEstablishment" ;
        rdfs:subClassOf  schema:LocalBusiness .

schema:LakeBodyOfWater
        a                rdfs:Class ;
        rdfs:comment     "A lake (for example, Lake Pontrachain)." ;
        rdfs:label       "LakeBodyOfWater" ;
        rdfs:subClassOf  schema:BodyOfWater .

schema:employees  a   rdf:Property ;
        rdfs:comment  "People working for this organization." ;
        rdfs:label    "employees" .

schema:partOfSeries  a      rdf:Property ;
        rdfs:comment        "The series to which this episode or season belongs." ;
        rdfs:label          "partOfSeries" ;
        rdfs:subPropertyOf  schema:isPartOf .

schema:ShortStory  a     rdfs:Class ;
        rdfs:comment     "Short story or tale. A brief work of literature, usually written in narrative prose." ;
        rdfs:label       "ShortStory" ;
        rdfs:subClassOf  schema:CreativeWork .

schema:Vehicle  a        rdfs:Class ;
        rdfs:comment     "A vehicle is a device that is designed or used to transport people or cargo over land, water, air, or through space." ;
        rdfs:label       "Vehicle" ;
        rdfs:subClassOf  schema:Product .

schema:educationalRole
        a             rdf:Property ;
        rdfs:comment  "An educationalRole of an EducationalAudience." ;
        rdfs:label    "educationalRole" .

schema:trainingSalary
        a             rdf:Property ;
        rdfs:comment  "The estimated salary earned while in the program." ;
        rdfs:label    "trainingSalary" .

schema:Menu  a           rdfs:Class ;
        rdfs:comment     "A structured representation of food or drink items available from a FoodEstablishment." ;
        rdfs:label       "Menu" ;
        rdfs:subClassOf  schema:CreativeWork .

schema:birthDate  a   rdf:Property ;
        rdfs:comment  "Date of birth." ;
        rdfs:label    "birthDate" .

schema:dateDeleted  a  rdf:Property ;
        rdfs:comment  "The datetime the item was removed from the DataFeed." ;
        rdfs:label    "dateDeleted" .

schema:significantLinks
        a             rdf:Property ;
        rdfs:comment  "The most significant URLs on the page. Typically, these are the non-navigation links that are clicked on the most." ;
        rdfs:label    "significantLinks" .

schema:review  a      rdf:Property ;
        rdfs:comment  "A review of the item." ;
        rdfs:label    "review" .

schema:loanPaymentAmount
        a             rdf:Property ;
        rdfs:comment  "The amount of money to pay in a single payment." ;
        rdfs:label    "loanPaymentAmount" .

schema:DepositAccount
        a                rdfs:Class ;
        rdfs:comment     "A type of Bank Account with a main purpose of depositing funds to gain interest or other benefits." ;
        rdfs:label       "DepositAccount" ;
        rdfs:subClassOf  schema:InvestmentOrDeposit , schema:BankAccount .

schema:actor  a       rdf:Property ;
        rdfs:comment  "An actor, e.g. in tv, radio, movie, video games etc., or in an event. Actors can be associated with individual items or with a series, episode, clip." ;
        rdfs:label    "actor" .

schema:carbohydrateContent
        a             rdf:Property ;
        rdfs:comment  "The number of grams of carbohydrates." ;
        rdfs:label    "carbohydrateContent" .

schema:downloadUrl  a  rdf:Property ;
        rdfs:comment  "If the file can be downloaded, URL to download the binary." ;
        rdfs:label    "downloadUrl" .

schema:documentation  a  rdf:Property ;
        rdfs:comment  "Further documentation describing the Web API in more detail." ;
        rdfs:label    "documentation" .

schema:PreventionIndication
        a                rdfs:Class ;
        rdfs:comment     "An indication for preventing an underlying condition, symptom, etc." ;
        rdfs:label       "PreventionIndication" ;
        rdfs:subClassOf  schema:MedicalIndication .

schema:DrugCost  a       rdfs:Class ;
        rdfs:comment     "The cost per unit of a medical drug. Note that this type is not meant to represent the price in an offer of a drug for sale; see the Offer type for that. This type will typically be used to tag wholesale or average retail cost of a drug, or maximum reimbursable cost. Costs of medical drugs vary widely depending on how and where they are paid for, so while this type captures some of the variables, costs should be used with caution by consumers of this schema's markup." ;
        rdfs:label       "DrugCost" ;
        rdfs:subClassOf  schema:MedicalEntity .

schema:propertyID  a  rdf:Property ;
        rdfs:comment  "A commonly used identifier for the characteristic represented by the property, e.g. a manufacturer or a standard code for a property. propertyID can be\n(1) a prefixed string, mainly meant to be used with standards for product properties; (2) a site-specific, non-prefixed string (e.g. the primary key of the property or the vendor-specific id of the property), or (3)\na URL indicating the type of the property, either pointing to an external vocabulary, or a Web resource that describes the property (e.g. a glossary entry).\nStandards bodies should promote a standard prefix for the identifiers of properties from their standards." ;
        rdfs:label    "propertyID" .

schema:option  a            rdf:Property ;
        rdfs:comment        "A sub property of object. The options subject to this action." ;
        rdfs:label          "option" ;
        rdfs:subPropertyOf  schema:object .

schema:PublicationEvent
        a                rdfs:Class ;
        rdfs:comment     "A PublicationEvent corresponds indifferently to the event of publication for a CreativeWork of any type e.g. a broadcast event, an on-demand event, a book/journal publication via a variety of delivery media." ;
        rdfs:label       "PublicationEvent" ;
        rdfs:subClassOf  schema:Event .

schema:MusicAlbum  a     rdfs:Class ;
        rdfs:comment     "A collection of music tracks." ;
        rdfs:label       "MusicAlbum" ;
        rdfs:subClassOf  schema:MusicPlaylist .

schema:Boolean  a     rdfs:Class ;
        rdfs:comment  "Boolean: True or False." ;
        rdfs:label    "Boolean" .

schema:transitTimeLabel
        a             rdf:Property ;
        rdfs:comment  "Label to match an [[OfferShippingDetails]] with a [[DeliveryTimeSettings]] (within the context of a [[shippingSettingsLink]] cross-reference)." ;
        rdfs:label    "transitTimeLabel" .

schema:contactlessPayment
        a             rdf:Property ;
        rdfs:comment  "A secure method for consumers to purchase products or services via debit, credit or smartcards by using RFID or NFC technology." ;
        rdfs:label    "contactlessPayment" .

schema:greaterOrEqual
        a             rdf:Property ;
        rdfs:comment  "This ordering relation for qualitative values indicates that the subject is greater than or equal to the object." ;
        rdfs:label    "greaterOrEqual" .

schema:softwareRequirements
        a             rdf:Property ;
        rdfs:comment  "Component dependency requirements for application. This includes runtime environments and shared libraries that are not included in the application distribution package, but required to run the application (Examples: DirectX, Java or .NET runtime)." ;
        rdfs:label    "softwareRequirements" .

schema:valueAddedTaxIncluded
        a             rdf:Property ;
        rdfs:comment  "Specifies whether the applicable value-added tax (VAT) is included in the price specification or not." ;
        rdfs:label    "valueAddedTaxIncluded" .

schema:associatedMedia
        a             rdf:Property ;
        rdfs:comment  "A media object that encodes this CreativeWork. This property is a synonym for encoding." ;
        rdfs:label    "associatedMedia" .

schema:hostingOrganization
        a             rdf:Property ;
        rdfs:comment  "The organization (airline, travelers' club, etc.) the membership is made with." ;
        rdfs:label    "hostingOrganization" .

schema:interestRate  a  rdf:Property ;
        rdfs:comment  "The interest rate, charged or paid, applicable to the financial product. Note: This is different from the calculated annualPercentageRate." ;
        rdfs:label    "interestRate" .

schema:penciler  a    rdf:Property ;
        rdfs:comment  "The individual who draws the primary narrative artwork." ;
        rdfs:label    "penciler" .

schema:yield  a       rdf:Property ;
        rdfs:comment  "The quantity that results by performing instructions. For example, a paper airplane, 10 personalized candles." ;
        rdfs:label    "yield" .

schema:geoCovers  a   rdf:Property ;
        rdfs:comment  "Represents a relationship between two geometries (or the places they represent), relating a covering geometry to a covered geometry. \"Every point of b is a point of (the interior or boundary of) a\". As defined in [DE-9IM](https://en.wikipedia.org/wiki/DE-9IM)." ;
        rdfs:label    "geoCovers" .

schema:potentialAction
        a             rdf:Property ;
        rdfs:comment  "Indicates a potential Action, which describes an idealized action in which this thing would play an 'object' role." ;
        rdfs:label    "potentialAction" .

schema:WantAction  a     rdfs:Class ;
        rdfs:comment     "The act of expressing a desire about the object. An agent wants an object." ;
        rdfs:label       "WantAction" ;
        rdfs:subClassOf  schema:ReactAction .

schema:gamePlatform  a  rdf:Property ;
        rdfs:comment  "The electronic systems used to play <a href=\"http://en.wikipedia.org/wiki/Category:Video_game_platforms\">video games</a>." ;
        rdfs:label    "gamePlatform" .

schema:discusses  a   rdf:Property ;
        rdfs:comment  "Specifies the CreativeWork associated with the UserComment." ;
        rdfs:label    "discusses" .

schema:artworkSurface
        a             rdf:Property ;
        rdfs:comment  "The supporting materials for the artwork, e.g. Canvas, Paper, Wood, Board, etc." ;
        rdfs:label    "artworkSurface" .

schema:targetUrl  a   rdf:Property ;
        rdfs:comment  "The URL of a node in an established educational framework." ;
        rdfs:label    "targetUrl" .

schema:diseaseSpreadStatistics
        a             rdf:Property ;
        rdfs:comment  "Statistical information about the spread of a disease, either as [[WebContent]], or\n  described directly as a [[Dataset]], or the specific [[Observation]]s in the dataset. When a [[WebContent]] URL is\n  provided, the page indicated might also contain more such markup." ;
        rdfs:label    "diseaseSpreadStatistics" .

schema:Library  a        rdfs:Class ;
        rdfs:comment     "A library." ;
        rdfs:label       "Library" ;
        rdfs:subClassOf  schema:LocalBusiness .

schema:credentialCategory
        a             rdf:Property ;
        rdfs:comment  "The category or type of credential being described, for example \"degree”, “certificate”, “badge”, or more specific term." ;
        rdfs:label    "credentialCategory" .

schema:accessModeSufficient
        a             rdf:Property ;
        rdfs:comment  "A list of single or combined accessModes that are sufficient to understand all the intellectual content of a resource. Expected values include:  auditory, tactile, textual, visual.\n      " ;
        rdfs:label    "accessModeSufficient" .

schema:PaymentMethod  a  rdfs:Class ;
        rdfs:comment     "A payment method is a standardized procedure for transferring the monetary amount for a purchase. Payment methods are characterized by the legal and technical structures used, and by the organization or group carrying out the transaction.\\n\\nCommonly used values:\\n\\n* http://purl.org/goodrelations/v1#ByBankTransferInAdvance\\n* http://purl.org/goodrelations/v1#ByInvoice\\n* http://purl.org/goodrelations/v1#Cash\\n* http://purl.org/goodrelations/v1#CheckInAdvance\\n* http://purl.org/goodrelations/v1#COD\\n* http://purl.org/goodrelations/v1#DirectDebit\\n* http://purl.org/goodrelations/v1#GoogleCheckout\\n* http://purl.org/goodrelations/v1#PayPal\\n* http://purl.org/goodrelations/v1#PaySwarm\n        " ;
        rdfs:label       "PaymentMethod" ;
        rdfs:subClassOf  schema:Enumeration .

schema:servingSize  a  rdf:Property ;
        rdfs:comment  "The serving size, in terms of the number of volume or mass." ;
        rdfs:label    "servingSize" .

schema:availability  a  rdf:Property ;
        rdfs:comment  "The availability of this item&#x2014;for example In stock, Out of stock, Pre-order, etc." ;
        rdfs:label    "availability" .

schema:MovieSeries  a    rdfs:Class ;
        rdfs:comment     "A series of movies. Included movies can be indicated with the hasPart property." ;
        rdfs:label       "MovieSeries" ;
        rdfs:subClassOf  schema:CreativeWorkSeries .

schema:events  a      rdf:Property ;
        rdfs:comment  "Upcoming or past events associated with this place or organization." ;
        rdfs:label    "events" .

schema:MensClothingStore
        a                rdfs:Class ;
        rdfs:comment     "A men's clothing store." ;
        rdfs:label       "MensClothingStore" ;
        rdfs:subClassOf  schema:Store .

schema:exerciseCourse
        a                   rdf:Property ;
        rdfs:comment        "A sub property of location. The course where this action was taken." ;
        rdfs:label          "exerciseCourse" ;
        rdfs:subPropertyOf  schema:location .

schema:LodgingReservation
        a                rdfs:Class ;
        rdfs:comment     "A reservation for lodging at a hotel, motel, inn, etc.\\n\\nNote: This type is for information about actual reservations, e.g. in confirmation emails or HTML pages with individual confirmations of reservations." ;
        rdfs:label       "LodgingReservation" ;
        rdfs:subClassOf  schema:Reservation .

schema:diagram  a     rdf:Property ;
        rdfs:comment  "An image containing a diagram that illustrates the structure and/or its component substructures and/or connections with other structures." ;
        rdfs:label    "diagram" .

schema:WearableSizeSystemEnumeration
        a                rdfs:Class ;
        rdfs:comment     "Enumerates common size systems specific for wearable products" ;
        rdfs:label       "WearableSizeSystemEnumeration" ;
        rdfs:subClassOf  schema:SizeSystemEnumeration .

geo:defaultGeometry  a  rdf:Property .

schema:MedicalEnumeration
        a                rdfs:Class ;
        rdfs:comment     "Enumerations related to health and the practice of medicine: A concept that is used to attribute a quality to another concept, as a qualifier, a collection of items or a listing of all of the elements of a set in medicine practice." ;
        rdfs:label       "MedicalEnumeration" ;
        rdfs:subClassOf  schema:Enumeration .

schema:DefinedRegion  a  rdfs:Class ;
        rdfs:comment     "A DefinedRegion is a geographic area defined by potentially arbitrary (rather than political, administrative or natural geographical) criteria. Properties are provided for defining a region by reference to sets of postal codes.\n\nExamples: a delivery destination when shopping. Region where regional pricing is configured.\n\nRequirement 1:\nCountry: US\nStates: \"NY\", \"CA\"\n\nRequirement 2:\nCountry: US\nPostalCode Set: { [94000-94585], [97000, 97999], [13000, 13599]}\n{ [12345, 12345], [78945, 78945], }\nRegion = state, canton, prefecture, autonomous community...\n" ;
        rdfs:label       "DefinedRegion" ;
        rdfs:subClassOf  schema:StructuredValue .

schema:legislationApplies
        a             rdf:Property ;
        rdfs:comment  "Indicates that this legislation (or part of a legislation) somehow transfers another legislation in a different legislative context. This is an informative link, and it has no legal value. For legally-binding links of transposition, use the <a href=\"/legislationTransposes\">legislationTransposes</a> property. For example an informative consolidated law of a European Union's member state \"applies\" the consolidated version of the European Directive implemented in it." ;
        rdfs:label    "legislationApplies" .

schema:FindAction  a     rdfs:Class ;
        rdfs:comment     "The act of finding an object.\\n\\nRelated actions:\\n\\n* [[SearchAction]]: FindAction is generally lead by a SearchAction, but not necessarily." ;
        rdfs:label       "FindAction" ;
        rdfs:subClassOf  schema:Action .

schema:NewsArticle  a    rdfs:Class ;
        rdfs:comment     "A NewsArticle is an article whose content reports news, or provides background context and supporting materials for understanding the news.\n\nA more detailed overview of [schema.org News markup](/docs/news.html) is also available.\n" ;
        rdfs:label       "NewsArticle" ;
        rdfs:subClassOf  schema:Article .

schema:productionDate
        a             rdf:Property ;
        rdfs:comment  "The date of production of the item, e.g. vehicle." ;
        rdfs:label    "productionDate" .

schema:Permit  a         rdfs:Class ;
        rdfs:comment     "A permit issued by an organization, e.g. a parking pass." ;
        rdfs:label       "Permit" ;
        rdfs:subClassOf  schema:Intangible .

schema:PhysicalActivity
        a                rdfs:Class ;
        rdfs:comment     "Any bodily activity that enhances or maintains physical fitness and overall health and wellness. Includes activity that is part of daily living and routine, structured exercise, and exercise prescribed as part of a medical treatment or recovery plan." ;
        rdfs:label       "PhysicalActivity" ;
        rdfs:subClassOf  schema:LifestyleModification .

schema:RsvpAction  a     rdfs:Class ;
        rdfs:comment     "The act of notifying an event organizer as to whether you expect to attend the event." ;
        rdfs:label       "RsvpAction" ;
        rdfs:subClassOf  schema:InformAction .

schema:uploadDate  a  rdf:Property ;
        rdfs:comment  "Date when this media object was uploaded to this site." ;
        rdfs:label    "uploadDate" .

schema:Number  a      rdfs:Class ;
        rdfs:comment  "Data type: Number.\\n\\nUsage guidelines:\\n\\n* Use values from 0123456789 (Unicode 'DIGIT ZERO' (U+0030) to 'DIGIT NINE' (U+0039)) rather than superficially similiar Unicode symbols.\\n* Use '.' (Unicode 'FULL STOP' (U+002E)) rather than ',' to indicate a decimal point. Avoid using these symbols as a readability separator." ;
        rdfs:label    "Number" .

schema:claimReviewed  a  rdf:Property ;
        rdfs:comment  "A short summary of the specific claims reviewed in a ClaimReview." ;
        rdfs:label    "claimReviewed" .

schema:Float  a          rdfs:Class ;
        rdfs:comment     "Data type: Floating number." ;
        rdfs:label       "Float" ;
        rdfs:subClassOf  schema:Number .

schema:specialCommitments
        a             rdf:Property ;
        rdfs:comment  "Any special commitments associated with this job posting. Valid entries include VeteranCommit, MilitarySpouseCommit, etc." ;
        rdfs:label    "specialCommitments" .

schema:legislationTransposes
        a                   rdf:Property ;
        rdfs:comment        "Indicates that this legislation (or part of legislation) fulfills the objectives set by another legislation, by passing appropriate implementation measures. Typically, some legislations of European Union's member states or regions transpose European Directives. This indicates a legally binding link between the 2 legislations." ;
        rdfs:label          "legislationTransposes" ;
        rdfs:subPropertyOf  schema:legislationApplies .

schema:prepTime  a    rdf:Property ;
        rdfs:comment  "The length of time it takes to prepare the items to be used in instructions or a direction, in [ISO 8601 duration format](http://en.wikipedia.org/wiki/ISO_8601)." ;
        rdfs:label    "prepTime" .

schema:availableAtOrFrom
        a                   rdf:Property ;
        rdfs:comment        "The place(s) from which the offer can be obtained (e.g. store locations)." ;
        rdfs:label          "availableAtOrFrom" ;
        rdfs:subPropertyOf  schema:areaServed .

schema:textValue  a   rdf:Property ;
        rdfs:comment  "Text value being annotated." ;
        rdfs:label    "textValue" .

schema:CommentAction  a  rdfs:Class ;
        rdfs:comment     "The act of generating a comment about a subject." ;
        rdfs:label       "CommentAction" ;
        rdfs:subClassOf  schema:CommunicateAction .

schema:verificationFactCheckingPolicy
        a                   rdf:Property ;
        rdfs:comment        "Disclosure about verification and fact-checking processes for a [[NewsMediaOrganization]] or other fact-checking [[Organization]]." ;
        rdfs:label          "verificationFactCheckingPolicy" ;
        rdfs:subPropertyOf  schema:publishingPrinciples .

schema:RentAction  a     rdfs:Class ;
        rdfs:comment     "The act of giving money in return for temporary use, but not ownership, of an object such as a vehicle or property. For example, an agent rents a property from a landlord in exchange for a periodic payment." ;
        rdfs:label       "RentAction" ;
        rdfs:subClassOf  schema:TradeAction .

schema:sensoryRequirement
        a             rdf:Property ;
        rdfs:comment  "A description of any sensory requirements and levels necessary to function on the job, including hearing and vision. Defined terms such as those in O*net may be used, but note that there is no way to specify the level of ability as well as its nature when using a defined term." ;
        rdfs:label    "sensoryRequirement" .

schema:numberOfAxles  a  rdf:Property ;
        rdfs:comment  "The number of axles.\\n\\nTypical unit code(s): C62" ;
        rdfs:label    "numberOfAxles" .

schema:embedUrl  a    rdf:Property ;
        rdfs:comment  "A URL pointing to a player for a specific video. In general, this is the information in the ```src``` element of an ```embed``` tag and should not be the same as the content of the ```loc``` tag." ;
        rdfs:label    "embedUrl" .

schema:permissions  a  rdf:Property ;
        rdfs:comment  "Permission(s) required to run the app (for example, a mobile app may require full internet access or may run only on wifi)." ;
        rdfs:label    "permissions" .

schema:parentItem  a  rdf:Property ;
        rdfs:comment  "The parent of a question, answer or item in general." ;
        rdfs:label    "parentItem" .

schema:Manuscript  a     rdfs:Class ;
        rdfs:comment     "A book, document, or piece of music written by hand rather than typed or printed." ;
        rdfs:label       "Manuscript" ;
        rdfs:subClassOf  schema:CreativeWork .

schema:riskFactor  a  rdf:Property ;
        rdfs:comment  "A modifiable or non-modifiable factor that increases the risk of a patient contracting this condition, e.g. age,  coexisting condition." ;
        rdfs:label    "riskFactor" .

schema:observedNode  a  rdf:Property ;
        rdfs:comment  "The observedNode of an [[Observation]], often a [[StatisticalPopulation]]." ;
        rdfs:label    "observedNode" .

schema:PublicSwimmingPool
        a                rdfs:Class ;
        rdfs:comment     "A public swimming pool." ;
        rdfs:label       "PublicSwimmingPool" ;
        rdfs:subClassOf  schema:SportsActivityLocation .

schema:authenticator  a  rdf:Property ;
        rdfs:comment  "The Organization responsible for authenticating the user's subscription. For example, many media apps require a cable/satellite provider to authenticate your subscription before playing media." ;
        rdfs:label    "authenticator" .

schema:OutletStore  a    rdfs:Class ;
        rdfs:comment     "An outlet store." ;
        rdfs:label       "OutletStore" ;
        rdfs:subClassOf  schema:Store .

schema:screenCount  a  rdf:Property ;
        rdfs:comment  "The number of screens in the movie theater." ;
        rdfs:label    "screenCount" .

schema:organizer  a   rdf:Property ;
        rdfs:comment  "An organizer of an Event." ;
        rdfs:label    "organizer" .

schema:ExerciseAction
        a                rdfs:Class ;
        rdfs:comment     "The act of participating in exertive activity for the purposes of improving health and fitness." ;
        rdfs:label       "ExerciseAction" ;
        rdfs:subClassOf  schema:PlayAction .

schema:Psychiatric  a    rdfs:Class ;
        rdfs:comment     "A specific branch of medical science that is concerned with the study, treatment, and prevention of mental illness, using both medical and psychological therapies." ;
        rdfs:label       "Psychiatric" ;
        rdfs:subClassOf  schema:MedicalBusiness .

schema:Accommodation  a  rdfs:Class ;
        rdfs:comment     "An accommodation is a place that can accommodate human beings, e.g. a hotel room, a camping pitch, or a meeting room. Many accommodations are for overnight stays, but this is not a mandatory requirement.\nFor more specific types of accommodations not defined in schema.org, one can use additionalType with external vocabularies.\n<br /><br />\nSee also the <a href=\"/docs/hotels.html\">dedicated document on the use of schema.org for marking up hotels and other forms of accommodations</a>.\n" ;
        rdfs:label       "Accommodation" ;
        rdfs:subClassOf  schema:Place .

schema:mapType  a     rdf:Property ;
        rdfs:comment  "Indicates the kind of Map, from the MapCategoryType Enumeration." ;
        rdfs:label    "mapType" .

schema:departureAirport
        a             rdf:Property ;
        rdfs:comment  "The airport where the flight originates." ;
        rdfs:label    "departureAirport" .

schema:bloodSupply  a  rdf:Property ;
        rdfs:comment  "The blood vessel that carries blood from the heart to the muscle." ;
        rdfs:label    "bloodSupply" .

schema:numberOfAvailableAccommodationUnits
        a             rdf:Property ;
        rdfs:comment  "Indicates the number of available accommodation units in an [[ApartmentComplex]], or the number of accommodation units for a specific [[FloorPlan]] (within its specific [[ApartmentComplex]]). See also [[numberOfAccommodationUnits]]." ;
        rdfs:label    "numberOfAvailableAccommodationUnits" .

schema:AutoRepair  a     rdfs:Class ;
        rdfs:comment     "Car repair business." ;
        rdfs:label       "AutoRepair" ;
        rdfs:subClassOf  schema:AutomotiveBusiness .

schema:unsaturatedFatContent
        a             rdf:Property ;
        rdfs:comment  "The number of grams of unsaturated fat." ;
        rdfs:label    "unsaturatedFatContent" .

schema:durationOfWarranty
        a             rdf:Property ;
        rdfs:comment  "The duration of the warranty promise. Common unitCode values are ANN for year, MON for months, or DAY for days." ;
        rdfs:label    "durationOfWarranty" .

schema:department  a  rdf:Property ;
        rdfs:comment  "A relationship between an organization and a department of that organization, also described as an organization (allowing different urls, logos, opening hours). For example: a store with a pharmacy, or a bakery with a cafe." ;
        rdfs:label    "department" .

schema:CourseInstance
        a                rdfs:Class ;
        rdfs:comment     "An instance of a [[Course]] which is distinct from other instances because it is offered at a different time or location or through different media or modes of study or to a specific section of students." ;
        rdfs:label       "CourseInstance" ;
        rdfs:subClassOf  schema:Event .

schema:email  a       rdf:Property ;
        rdfs:comment  "Email address." ;
        rdfs:label    "email" .

schema:copyrightYear  a  rdf:Property ;
        rdfs:comment  "The year during which the claimed copyright for the CreativeWork was first asserted." ;
        rdfs:label    "copyrightYear" .

schema:contactOption  a  rdf:Property ;
        rdfs:comment  "An option available on this contact point (e.g. a toll-free number or support for hearing-impaired callers)." ;
        rdfs:label    "contactOption" .

schema:representativeOfPage
        a             rdf:Property ;
        rdfs:comment  "Indicates whether this image is representative of the content of the page." ;
        rdfs:label    "representativeOfPage" .

schema:MedicalRiskEstimator
        a                rdfs:Class ;
        rdfs:comment     "Any rule set or interactive tool for estimating the risk of developing a complication or condition." ;
        rdfs:label       "MedicalRiskEstimator" ;
        rdfs:subClassOf  schema:MedicalEntity .

schema:name  a              rdf:Property ;
        rdfs:comment        "The name of the item." ;
        rdfs:label          "name" ;
        rdfs:subPropertyOf  rdfs:label .

schema:usageInfo  a   rdf:Property ;
        rdfs:comment  "The schema.org [[usageInfo]] property indicates further information about a [[CreativeWork]]. This property is applicable both to works that are freely available and to those that require payment or other transactions. It can reference additional information e.g. community expectations on preferred linking and citation conventions, as well as purchasing details. For something that can be commercially licensed, usageInfo can provide detailed, resource-specific information about licensing options.\n\nThis property can be used alongside the license property which indicates license(s) applicable to some piece of content. The usageInfo property can provide information about other licensing options, e.g. acquiring commercial usage rights for an image that is also available under non-commercial creative commons licenses." ;
        rdfs:label    "usageInfo" .

schema:subEvent  a    rdf:Property ;
        rdfs:comment  "An Event that is part of this event. For example, a conference event includes many presentations, each of which is a subEvent of the conference." ;
        rdfs:label    "subEvent" .

schema:Thesis  a         rdfs:Class ;
        rdfs:comment     "A thesis or dissertation document submitted in support of candidature for an academic degree or professional qualification." ;
        rdfs:label       "Thesis" ;
        rdfs:subClassOf  schema:CreativeWork .

schema:MedicalRiskFactor
        a                rdfs:Class ;
        rdfs:comment     "A risk factor is anything that increases a person's likelihood of developing or contracting a disease, medical condition, or complication." ;
        rdfs:label       "MedicalRiskFactor" ;
        rdfs:subClassOf  schema:MedicalEntity .

schema:diversityStaffingReport
        a                   rdf:Property ;
        rdfs:comment        "For an [[Organization]] (often but not necessarily a [[NewsMediaOrganization]]), a report on staffing diversity issues. In a news context this might be for example ASNE or RTDNA (US) reports, or self-reported." ;
        rdfs:label          "diversityStaffingReport" ;
        rdfs:subPropertyOf  schema:publishingPrinciples .

schema:healthcareReportingData
        a             rdf:Property ;
        rdfs:comment  "Indicates data describing a hospital, e.g. a CDC [[CDCPMDRecord]] or as some kind of [[Dataset]]." ;
        rdfs:label    "healthcareReportingData" .

schema:HomeAndConstructionBusiness
        a                rdfs:Class ;
        rdfs:comment     "A construction business.\\n\\nA HomeAndConstructionBusiness is a [[LocalBusiness]] that provides services around homes and buildings.\\n\\nAs a [[LocalBusiness]] it can be described as a [[provider]] of one or more [[Service]]\\(s)." ;
        rdfs:label       "HomeAndConstructionBusiness" ;
        rdfs:subClassOf  schema:LocalBusiness .

schema:icaoCode  a    rdf:Property ;
        rdfs:comment  "ICAO identifier for an airport." ;
        rdfs:label    "icaoCode" .

schema:actionStatus  a  rdf:Property ;
        rdfs:comment  "Indicates the current disposition of the Action." ;
        rdfs:label    "actionStatus" .

schema:itemCondition  a  rdf:Property ;
        rdfs:comment  "A predefined value from OfferItemCondition or a textual description of the condition of the product or service, or the products or services included in the offer." ;
        rdfs:label    "itemCondition" .

schema:sameAs  a      rdf:Property ;
        rdfs:comment  "URL of a reference Web page that unambiguously indicates the item's identity. E.g. the URL of the item's Wikipedia page, Wikidata entry, or official website." ;
        rdfs:label    "sameAs" .

schema:AlignmentObject
        a                rdfs:Class ;
        rdfs:comment     "An intangible item that describes an alignment between a learning resource and a node in an educational framework.\n\nShould not be used where the nature of the alignment can be described using a simple property, for example to express that a resource [[teaches]] or [[assesses]] a competency." ;
        rdfs:label       "AlignmentObject" ;
        rdfs:subClassOf  schema:Intangible .

schema:VideoGameSeries
        a                rdfs:Class ;
        rdfs:comment     "A video game series." ;
        rdfs:label       "VideoGameSeries" ;
        rdfs:subClassOf  schema:CreativeWorkSeries .

schema:safetyConsideration
        a             rdf:Property ;
        rdfs:comment  "Any potential safety concern associated with the supplement. May include interactions with other drugs and foods, pregnancy, breastfeeding, known adverse reactions, and documented efficacy of the supplement." ;
        rdfs:label    "safetyConsideration" .

schema:permissionType
        a             rdf:Property ;
        rdfs:comment  "The type of permission granted the person, organization, or audience." ;
        rdfs:label    "permissionType" .

schema:associatedAnatomy
        a             rdf:Property ;
        rdfs:comment  "The anatomy of the underlying organ system or structures associated with this entity." ;
        rdfs:label    "associatedAnatomy" .

schema:RadiationTherapy
        a                rdfs:Class ;
        rdfs:comment     "A process of care using radiation aimed at improving a health condition." ;
        rdfs:label       "RadiationTherapy" ;
        rdfs:subClassOf  schema:MedicalTherapy .

schema:legislationType
        a                   rdf:Property ;
        rdfs:comment        "The type of the legislation. Examples of values are \"law\", \"act\", \"directive\", \"decree\", \"regulation\", \"statutory instrument\", \"loi organique\", \"règlement grand-ducal\", etc., depending on the country." ;
        rdfs:label          "legislationType" ;
        rdfs:subPropertyOf  schema:genre .

schema:Episode  a        rdfs:Class ;
        rdfs:comment     "A media episode (e.g. TV, radio, video game) which can be part of a series or season." ;
        rdfs:label       "Episode" ;
        rdfs:subClassOf  schema:CreativeWork .

schema:Reservation  a    rdfs:Class ;
        rdfs:comment     "Describes a reservation for travel, dining or an event. Some reservations require tickets. \\n\\nNote: This type is for information about actual reservations, e.g. in confirmation emails or HTML pages with individual confirmations of reservations. For offers of tickets, restaurant reservations, flights, or rental cars, use [[Offer]]." ;
        rdfs:label       "Reservation" ;
        rdfs:subClassOf  schema:Intangible .

schema:SiteNavigationElement
        a                rdfs:Class ;
        rdfs:comment     "A navigation element of the page." ;
        rdfs:label       "SiteNavigationElement" ;
        rdfs:subClassOf  schema:WebPageElement .

schema:legislationResponsible
        a             rdf:Property ;
        rdfs:comment  "An individual or organization that has some kind of responsibility for the legislation. Typically the ministry who is/was in charge of elaborating the legislation, or the adressee for potential questions about the legislation once it is published." ;
        rdfs:label    "legislationResponsible" .

schema:UseAction  a      rdfs:Class ;
        rdfs:comment     "The act of applying an object to its intended purpose." ;
        rdfs:label       "UseAction" ;
        rdfs:subClassOf  schema:ConsumeAction .

schema:workPresented  a     rdf:Property ;
        rdfs:comment        "The movie presented during this event." ;
        rdfs:label          "workPresented" ;
        rdfs:subPropertyOf  schema:workFeatured .

schema:originatesFrom
        a             rdf:Property ;
        rdfs:comment  "The vasculature the lymphatic structure originates, or afferents, from." ;
        rdfs:label    "originatesFrom" .

schema:WearableSizeGroupEnumeration
        a                rdfs:Class ;
        rdfs:comment     "Enumerates common size groups (also known as \"size types\") for wearable products." ;
        rdfs:label       "WearableSizeGroupEnumeration" ;
        rdfs:subClassOf  schema:SizeGroupEnumeration .

schema:Comment  a        rdfs:Class ;
        rdfs:comment     "A comment on an item - for example, a comment on a blog post. The comment's content is expressed via the [[text]] property, and its topic via [[about]], properties shared with all CreativeWorks." ;
        rdfs:label       "Comment" ;
        rdfs:subClassOf  schema:CreativeWork .

schema:video  a       rdf:Property ;
        rdfs:comment  "An embedded video object." ;
        rdfs:label    "video" .

schema:MedicalSymptom
        a                rdfs:Class ;
        rdfs:comment     "Any complaint sensed and expressed by the patient (therefore defined as subjective)  like stomachache, lower-back pain, or fatigue." ;
        rdfs:label       "MedicalSymptom" ;
        rdfs:subClassOf  schema:MedicalSignOrSymptom .

schema:PaymentService
        a                rdfs:Class ;
        rdfs:comment     "A Service to transfer funds from a person or organization to a beneficiary person or organization." ;
        rdfs:label       "PaymentService" ;
        rdfs:subClassOf  schema:FinancialProduct .

schema:legalStatus  a  rdf:Property ;
        rdfs:comment  "The drug or supplement's legal status, including any controlled substance schedules that apply." ;
        rdfs:label    "legalStatus" .

schema:Thing  a       rdfs:Class ;
        rdfs:comment  "The most generic type of item." ;
        rdfs:label    "Thing" .

schema:affiliation  a       rdf:Property ;
        rdfs:comment        "An organization that this person is affiliated with. For example, a school/university, a club, or a team." ;
        rdfs:label          "affiliation" ;
        rdfs:subPropertyOf  schema:memberOf .

schema:recommendationStrength
        a             rdf:Property ;
        rdfs:comment  "Strength of the guideline's recommendation (e.g. 'class I')." ;
        rdfs:label    "recommendationStrength" .

schema:ItemAvailability
        a                rdfs:Class ;
        rdfs:comment     "A list of possible product availability options." ;
        rdfs:label       "ItemAvailability" ;
        rdfs:subClassOf  schema:Enumeration .

schema:numberOfLoanPayments
        a             rdf:Property ;
        rdfs:comment  "The number of payments contractually required at origination to repay the loan. For monthly paying loans this is the number of months from the contractual first payment date to the maturity date." ;
        rdfs:label    "numberOfLoanPayments" .

schema:HowToDirection
        a                rdfs:Class ;
        rdfs:comment     "A direction indicating a single action to do in the instructions for how to achieve a result." ;
        rdfs:label       "HowToDirection" ;
        rdfs:subClassOf  schema:ListItem , schema:CreativeWork .

schema:MobilePhoneStore
        a                rdfs:Class ;
        rdfs:comment     "A store that sells mobile phones and related accessories." ;
        rdfs:label       "MobilePhoneStore" ;
        rdfs:subClassOf  schema:Store .

schema:PhysicalExam  a   rdfs:Class ;
        rdfs:comment     "A type of physical examination of a patient performed by a physician. " ;
        rdfs:label       "PhysicalExam" ;
        rdfs:subClassOf  schema:MedicalEnumeration , schema:MedicalProcedure .

schema:associatedArticle
        a             rdf:Property ;
        rdfs:comment  "A NewsArticle associated with the Media Object." ;
        rdfs:label    "associatedArticle" .

schema:PerformingArtsTheater
        a                rdfs:Class ;
        rdfs:comment     "A theater or other performing art center." ;
        rdfs:label       "PerformingArtsTheater" ;
        rdfs:subClassOf  schema:CivicStructure .

schema:SteeringPositionValue
        a                rdfs:Class ;
        rdfs:comment     "A value indicating a steering position." ;
        rdfs:label       "SteeringPositionValue" ;
        rdfs:subClassOf  schema:QualitativeValue .

schema:securityClearanceRequirement
        a             rdf:Property ;
        rdfs:comment  "A description of any security clearance requirements of the job." ;
        rdfs:label    "securityClearanceRequirement" .

schema:latitude  a    rdf:Property ;
        rdfs:comment  "The latitude of a location. For example ```37.42242``` ([WGS 84](https://en.wikipedia.org/wiki/World_Geodetic_System))." ;
        rdfs:label    "latitude" .

schema:WebPageElement
        a                rdfs:Class ;
        rdfs:comment     "A web page element, like a table or an image." ;
        rdfs:label       "WebPageElement" ;
        rdfs:subClassOf  schema:CreativeWork .

schema:Church  a         rdfs:Class ;
        rdfs:comment     "A church." ;
        rdfs:label       "Church" ;
        rdfs:subClassOf  schema:PlaceOfWorship .

schema:preOp  a       rdf:Property ;
        rdfs:comment  "A description of the workup, testing, and other preparations required before implanting this device." ;
        rdfs:label    "preOp" .

schema:EventSeries  a    rdfs:Class ;
        rdfs:comment     "A series of [[Event]]s. Included events can relate with the series using the [[superEvent]] property.\n\nAn EventSeries is a collection of events that share some unifying characteristic. For example, \"The Olympic Games\" is a series, which\nis repeated regularly. The \"2012 London Olympics\" can be presented both as an [[Event]] in the series \"Olympic Games\", and as an\n[[EventSeries]] that included a number of sporting competitions as Events.\n\nThe nature of the association between the events in an [[EventSeries]] can vary, but typical examples could\ninclude a thematic event series (e.g. topical meetups or classes), or a series of regular events that share a location, attendee group and/or organizers.\n\nEventSeries has been defined as a kind of Event to make it easy for publishers to use it in an Event context without\nworrying about which kinds of series are really event-like enough to call an Event. In general an EventSeries\nmay seem more Event-like when the period of time is compact and when aspects such as location are fixed, but\nit may also sometimes prove useful to describe a longer-term series as an Event.\n   " ;
        rdfs:label       "EventSeries" ;
        rdfs:subClassOf  schema:Event , schema:Series .

schema:Substance  a      rdfs:Class ;
        rdfs:comment     "Any matter of defined composition that has discrete existence, whose origin may be biological, mineral or chemical." ;
        rdfs:label       "Substance" ;
        rdfs:subClassOf  schema:MedicalEntity .

schema:TieAction  a      rdfs:Class ;
        rdfs:comment     "The act of reaching a draw in a competitive activity." ;
        rdfs:label       "TieAction" ;
        rdfs:subClassOf  schema:AchieveAction .

schema:pageEnd  a     rdf:Property ;
        rdfs:comment  "The page on which the work ends; for example \"138\" or \"xvi\"." ;
        rdfs:label    "pageEnd" .

schema:intensity  a   rdf:Property ;
        rdfs:comment  "Quantitative measure gauging the degree of force involved in the exercise, for example, heartbeats per minute. May include the velocity of the movement." ;
        rdfs:label    "intensity" .

schema:healthPlanNetworkId
        a             rdf:Property ;
        rdfs:comment  "Name or unique ID of network. (Networks are often reused across different insurance plans)." ;
        rdfs:label    "healthPlanNetworkId" .

schema:Cemetery  a       rdfs:Class ;
        rdfs:comment     "A graveyard." ;
        rdfs:label       "Cemetery" ;
        rdfs:subClassOf  schema:CivicStructure .

schema:relatedTo  a   rdf:Property ;
        rdfs:comment  "The most generic familial relation." ;
        rdfs:label    "relatedTo" .

schema:HyperTocEntry  a  rdfs:Class ;
        rdfs:comment     "A HyperToEntry is an item within a [[HyperToc]], which represents a hypertext table of contents for complex media objects, such as [[VideoObject]], [[AudioObject]]. The media object itself is indicated using [[associatedMedia]]. Each section of interest within that content can be described with a [[HyperTocEntry]], with associated [[startOffset]] and [[endOffset]]. When several entries are all from the same file, [[associatedMedia]] is used on the overarching [[HyperTocEntry]]; if the content has been split into multiple files, they can be referenced using [[associatedMedia]] on each [[HyperTocEntry]]." ;
        rdfs:label       "HyperTocEntry" ;
        rdfs:subClassOf  schema:CreativeWork .

schema:Periodical  a     rdfs:Class ;
        rdfs:comment     "A publication in any medium issued in successive parts bearing numerical or chronological designations and intended, such as a magazine, scholarly journal, or newspaper to continue indefinitely.\\n\\nSee also [blog post](http://blog.schema.org/2014/09/schemaorg-support-for-bibliographic_2.html)." ;
        rdfs:label       "Periodical" ;
        rdfs:subClassOf  schema:CreativeWorkSeries .

schema:toRecipient  a       rdf:Property ;
        rdfs:comment        "A sub property of recipient. The recipient who was directly sent the message." ;
        rdfs:label          "toRecipient" ;
        rdfs:subPropertyOf  schema:recipient .

schema:pickupTime  a  rdf:Property ;
        rdfs:comment  "When a taxi will pickup a passenger or a rental car can be picked up." ;
        rdfs:label    "pickupTime" .

schema:bestRating  a  rdf:Property ;
        rdfs:comment  "The highest value allowed in this rating system. If bestRating is omitted, 5 is assumed." ;
        rdfs:label    "bestRating" .

schema:FundingAgency  a  rdfs:Class ;
        rdfs:comment     "A FundingAgency is an organization that implements one or more [[FundingScheme]]s and manages\n    the granting process (via [[Grant]]s, typically [[MonetaryGrant]]s).\n    A funding agency is not always required for grant funding, e.g. philanthropic giving, corporate sponsorship etc.\n    \nExamples of funding agencies include ERC, REA, NIH, Bill and Melinda Gates Foundation...\n    " ;
        rdfs:label       "FundingAgency" ;
        rdfs:subClassOf  schema:Project .

schema:OfferCatalog  a   rdfs:Class ;
        rdfs:comment     "An OfferCatalog is an ItemList that contains related Offers and/or further OfferCatalogs that are offeredBy the same provider." ;
        rdfs:label       "OfferCatalog" ;
        rdfs:subClassOf  schema:ItemList .

schema:WholesaleStore
        a                rdfs:Class ;
        rdfs:comment     "A wholesale store." ;
        rdfs:label       "WholesaleStore" ;
        rdfs:subClassOf  schema:Store .

schema:BreadcrumbList
        a                rdfs:Class ;
        rdfs:comment     "A BreadcrumbList is an ItemList consisting of a chain of linked Web pages, typically described using at least their URL and their name, and typically ending with the current page.\\n\\nThe [[position]] property is used to reconstruct the order of the items in a BreadcrumbList The convention is that a breadcrumb list has an [[itemListOrder]] of [[ItemListOrderAscending]] (lower values listed first), and that the first items in this list correspond to the \"top\" or beginning of the breadcrumb trail, e.g. with a site or section homepage. The specific values of 'position' are not assigned meaning for a BreadcrumbList, but they should be integers, e.g. beginning with '1' for the first item in the list.\n      " ;
        rdfs:label       "BreadcrumbList" ;
        rdfs:subClassOf  schema:ItemList .

schema:BusTrip  a        rdfs:Class ;
        rdfs:comment     "A trip on a commercial bus line." ;
        rdfs:label       "BusTrip" ;
        rdfs:subClassOf  schema:Trip .

schema:gameTip  a     rdf:Property ;
        rdfs:comment  "Links to tips, tactics, etc." ;
        rdfs:label    "gameTip" .

schema:worksFor  a    rdf:Property ;
        rdfs:comment  "Organizations that the person works for." ;
        rdfs:label    "worksFor" .

schema:emissionsCO2  a  rdf:Property ;
        rdfs:comment  "The CO2 emissions in g/km. When used in combination with a QuantitativeValue, put \"g/km\" into the unitText property of that value, since there is no UN/CEFACT Common Code for \"g/km\"." ;
        rdfs:label    "emissionsCO2" .

schema:photo  a             rdf:Property ;
        rdfs:comment        "A photograph of this place." ;
        rdfs:label          "photo" ;
        rdfs:subPropertyOf  schema:image .

schema:RadioChannel  a   rdfs:Class ;
        rdfs:comment     "A unique instance of a radio BroadcastService on a CableOrSatelliteService lineup." ;
        rdfs:label       "RadioChannel" ;
        rdfs:subClassOf  schema:BroadcastChannel .

schema:partySize  a   rdf:Property ;
        rdfs:comment  "Number of people the reservation should accommodate." ;
        rdfs:label    "partySize" .

schema:EmailMessage  a   rdfs:Class ;
        rdfs:comment     "An email message." ;
        rdfs:label       "EmailMessage" ;
        rdfs:subClassOf  schema:Message .

schema:CollectionPage
        a                rdfs:Class ;
        rdfs:comment     "Web page type: Collection page." ;
        rdfs:label       "CollectionPage" ;
        rdfs:subClassOf  schema:WebPage .

schema:EmploymentAgency
        a                rdfs:Class ;
        rdfs:comment     "An employment agency." ;
        rdfs:label       "EmploymentAgency" ;
        rdfs:subClassOf  schema:LocalBusiness .

schema:Pharmacy  a       rdfs:Class ;
        rdfs:comment     "A pharmacy or drugstore." ;
        rdfs:label       "Pharmacy" ;
        rdfs:subClassOf  schema:MedicalBusiness , schema:MedicalOrganization .

schema:color  a       rdf:Property ;
        rdfs:comment  "The color of the product." ;
        rdfs:label    "color" .

schema:producer  a    rdf:Property ;
        rdfs:comment  "The person or organization who produced the work (e.g. music album, movie, tv/radio series etc.)." ;
        rdfs:label    "producer" .

schema:Landform  a       rdfs:Class ;
        rdfs:comment     "A landform or physical feature.  Landform elements include mountains, plains, lakes, rivers, seascape and oceanic waterbody interface features such as bays, peninsulas, seas and so forth, including sub-aqueous terrain features such as submersed mountain ranges, volcanoes, and the great ocean basins." ;
        rdfs:label       "Landform" ;
        rdfs:subClassOf  schema:Place .

schema:hasVariant  a  rdf:Property ;
        rdfs:comment  "Indicates a [[Product]] that is a member of this [[ProductGroup]] (or [[ProductModel]])." ;
        rdfs:label    "hasVariant" .

schema:free  a        rdf:Property ;
        rdfs:comment  "A flag to signal that the item, event, or place is accessible for free." ;
        rdfs:label    "free" .

schema:acquireLicensePage
        a                   rdf:Property ;
        rdfs:comment        "Indicates a page documenting how licenses can be purchased or otherwise acquired, for the current item." ;
        rdfs:label          "acquireLicensePage" ;
        rdfs:subPropertyOf  schema:usageInfo .

schema:MoneyTransfer  a  rdfs:Class ;
        rdfs:comment     "The act of transferring money from one place to another place. This may occur electronically or physically." ;
        rdfs:label       "MoneyTransfer" ;
        rdfs:subClassOf  schema:TransferAction .

schema:startOffset  a  rdf:Property ;
        rdfs:comment  "The start time of the clip expressed as the number of seconds from the beginning of the work." ;
        rdfs:label    "startOffset" .

schema:cheatCode  a   rdf:Property ;
        rdfs:comment  "Cheat codes to the game." ;
        rdfs:label    "cheatCode" .

schema:GardenStore  a    rdfs:Class ;
        rdfs:comment     "A garden store." ;
        rdfs:label       "GardenStore" ;
        rdfs:subClassOf  schema:Store .

schema:MediaGallery  a   rdfs:Class ;
        rdfs:comment     "Web page type: Media gallery page. A mixed-media page that can contains media such as images, videos, and other multimedia." ;
        rdfs:label       "MediaGallery" ;
        rdfs:subClassOf  schema:CollectionPage .

schema:GiveAction  a     rdfs:Class ;
        rdfs:comment     "The act of transferring ownership of an object to a destination. Reciprocal of TakeAction.\\n\\nRelated actions:\\n\\n* [[TakeAction]]: Reciprocal of GiveAction.\\n* [[SendAction]]: Unlike SendAction, GiveAction implies that ownership is being transferred (e.g. I may send my laptop to you, but that doesn't mean I'm giving it to you)." ;
        rdfs:label       "GiveAction" ;
        rdfs:subClassOf  schema:TransferAction .

schema:blogPost  a    rdf:Property ;
        rdfs:comment  "A posting that is part of this blog." ;
        rdfs:label    "blogPost" .

schema:USNonprofitType
        a                rdfs:Class ;
        rdfs:comment     "USNonprofitType: Non-profit organization type originating from the United States." ;
        rdfs:label       "USNonprofitType" ;
        rdfs:subClassOf  schema:NonprofitType .

schema:Audience  a       rdfs:Class ;
        rdfs:comment     "Intended audience for an item, i.e. the group for whom the item was created." ;
        rdfs:label       "Audience" ;
        rdfs:subClassOf  schema:Intangible .

schema:contributor  a  rdf:Property ;
        rdfs:comment  "A secondary contributor to the CreativeWork or Event." ;
        rdfs:label    "contributor" .

schema:application  a  rdf:Property ;
        rdfs:comment  "An application that can complete the request." ;
        rdfs:label    "application" .

schema:educationRequirements
        a             rdf:Property ;
        rdfs:comment  "Educational background needed for the position or Occupation." ;
        rdfs:label    "educationRequirements" .

schema:DataType  a       rdfs:Class ;
        rdfs:comment     "The basic data types such as Integers, Strings, etc." ;
        rdfs:label       "DataType" ;
        rdfs:subClassOf  rdfs:Class .

schema:Rating  a         rdfs:Class ;
        rdfs:comment     "A rating is an evaluation on a numeric scale, such as 1 to 5 stars." ;
        rdfs:label       "Rating" ;
        rdfs:subClassOf  schema:Intangible .

schema:instructor  a  rdf:Property ;
        rdfs:comment  "A person assigned to instruct or provide instructional assistance for the [[CourseInstance]]." ;
        rdfs:label    "instructor" .

schema:experienceRequirements
        a             rdf:Property ;
        rdfs:comment  "Description of skills and experience needed for the position or Occupation." ;
        rdfs:label    "experienceRequirements" .

schema:Plumber  a        rdfs:Class ;
        rdfs:comment     "A plumbing service." ;
        rdfs:label       "Plumber" ;
        rdfs:subClassOf  schema:HomeAndConstructionBusiness .

schema:TouristTrip  a    rdfs:Class ;
        rdfs:comment     "A tourist trip. A created itinerary of visits to one or more places of interest ([[TouristAttraction]]/[[TouristDestination]]) often linked by a similar theme, geographic area, or interest to a particular [[touristType]]. The [UNWTO](http://www2.unwto.org/) defines tourism trip as the Trip taken by visitors.\n  (See examples below)." ;
        rdfs:label       "TouristTrip" ;
        rdfs:subClassOf  schema:Trip .

schema:paymentDueDate
        a             rdf:Property ;
        rdfs:comment  "The date that payment is due." ;
        rdfs:label    "paymentDueDate" .

schema:shippingLabel  a  rdf:Property ;
        rdfs:comment  "Label to match an [[OfferShippingDetails]] with a [[ShippingRateSettings]] (within the context of a [[shippingSettingsLink]] cross-reference)." ;
        rdfs:label    "shippingLabel" .

schema:competitor  a  rdf:Property ;
        rdfs:comment  "A competitor in a sports event." ;
        rdfs:label    "competitor" .

schema:increasesRiskOf
        a             rdf:Property ;
        rdfs:comment  "The condition, complication, etc. influenced by this factor." ;
        rdfs:label    "increasesRiskOf" .

schema:RadioSeason  a    rdfs:Class ;
        rdfs:comment     "Season dedicated to radio broadcast and associated online delivery." ;
        rdfs:label       "RadioSeason" ;
        rdfs:subClassOf  schema:CreativeWorkSeason .

schema:performers  a  rdf:Property ;
        rdfs:comment  "The main performer or performers of the event&#x2014;for example, a presenter, musician, or actor." ;
        rdfs:label    "performers" .

schema:numberOfEmployees
        a             rdf:Property ;
        rdfs:comment  "The number of employees in an organization e.g. business." ;
        rdfs:label    "numberOfEmployees" .

schema:endOffset  a   rdf:Property ;
        rdfs:comment  "The end time of the clip expressed as the number of seconds from the beginning of the work." ;
        rdfs:label    "endOffset" .

schema:suggestedGender
        a             rdf:Property ;
        rdfs:comment  "The suggested gender of the intended person or audience, for example \"male\", \"female\", or \"unisex\"." ;
        rdfs:label    "suggestedGender" .

schema:LearningResource
        a                rdfs:Class ;
        rdfs:comment     "The LearningResource type can be used to indicate [[CreativeWork]]s (whether physical or digital) that have a particular and explicit orientation towards learning, education, skill acquisition, and other educational purposes.\n\n[[LearningResource]] is expected to be used as an addition to a primary type such as [[Book]], [[VideoObject]], [[Product]] etc.\n\n[[EducationEvent]] serves a similar purpose for event-like things (e.g. a [[Trip]]). A [[LearningResource]] may be created as a result of an [[EducationEvent]], for example by recording one." ;
        rdfs:label       "LearningResource" ;
        rdfs:subClassOf  schema:CreativeWork .

schema:AutoPartsStore
        a                rdfs:Class ;
        rdfs:comment     "An auto parts store." ;
        rdfs:label       "AutoPartsStore" ;
        rdfs:subClassOf  schema:Store , schema:AutomotiveBusiness .

schema:UKNonprofitType
        a                rdfs:Class ;
        rdfs:comment     "UKNonprofitType: Non-profit organization type originating from the United Kingdom." ;
        rdfs:label       "UKNonprofitType" ;
        rdfs:subClassOf  schema:NonprofitType .

schema:MusicComposition
        a                rdfs:Class ;
        rdfs:comment     "A musical composition." ;
        rdfs:label       "MusicComposition" ;
        rdfs:subClassOf  schema:CreativeWork .

schema:DrugCostCategory
        a                rdfs:Class ;
        rdfs:comment     "Enumerated categories of medical drug costs." ;
        rdfs:label       "DrugCostCategory" ;
        rdfs:subClassOf  schema:MedicalEnumeration .

schema:algorithm  a   rdf:Property ;
        rdfs:comment  "The algorithm or rules to follow to compute the score." ;
        rdfs:label    "algorithm" .

schema:Beach  a          rdfs:Class ;
        rdfs:comment     "Beach." ;
        rdfs:label       "Beach" ;
        rdfs:subClassOf  schema:CivicStructure .

schema:hasEnergyEfficiencyCategory
        a             rdf:Property ;
        rdfs:comment  "Defines the energy efficiency Category (which could be either a rating out of range of values or a yes/no certification) for a product according to an international energy efficiency standard." ;
        rdfs:label    "hasEnergyEfficiencyCategory" .

schema:locationCreated
        a             rdf:Property ;
        rdfs:comment  "The location where the CreativeWork was created, which may not be the same as the location depicted in the CreativeWork." ;
        rdfs:label    "locationCreated" .

schema:CivicStructure
        a                rdfs:Class ;
        rdfs:comment     "A public structure, such as a town hall or concert hall." ;
        rdfs:label       "CivicStructure" ;
        rdfs:subClassOf  schema:Place .

schema:targetName  a  rdf:Property ;
        rdfs:comment  "The name of a node in an established educational framework." ;
        rdfs:label    "targetName" .

schema:validFrom  a   rdf:Property ;
        rdfs:comment  "The date when the item becomes valid." ;
        rdfs:label    "validFrom" .

schema:DoseSchedule  a   rdfs:Class ;
        rdfs:comment     "A specific dosing schedule for a drug or supplement." ;
        rdfs:label       "DoseSchedule" ;
        rdfs:subClassOf  schema:MedicalIntangible .

schema:PostalAddress  a  rdfs:Class ;
        rdfs:comment     "The mailing address." ;
        rdfs:label       "PostalAddress" ;
        rdfs:subClassOf  schema:ContactPoint .

schema:arrivalStation
        a             rdf:Property ;
        rdfs:comment  "The station where the train trip ends." ;
        rdfs:label    "arrivalStation" .

schema:MovieClip  a      rdfs:Class ;
        rdfs:comment     "A short segment/part of a movie." ;
        rdfs:label       "MovieClip" ;
        rdfs:subClassOf  schema:Clip .

schema:ParcelDelivery
        a                rdfs:Class ;
        rdfs:comment     "The delivery of a parcel either via the postal service or a commercial service." ;
        rdfs:label       "ParcelDelivery" ;
        rdfs:subClassOf  schema:Intangible .

schema:MerchantReturnEnumeration
        a                rdfs:Class ;
        rdfs:comment     "MerchantReturnEnumeration enumerates several kinds of product return policy. Note that this structure may not capture all aspects of the policy." ;
        rdfs:label       "MerchantReturnEnumeration" ;
        rdfs:subClassOf  schema:Enumeration .

schema:VeterinaryCare
        a                rdfs:Class ;
        rdfs:comment     "A vet's office." ;
        rdfs:label       "VeterinaryCare" ;
        rdfs:subClassOf  schema:MedicalOrganization .

schema:ReportageNewsArticle
        a                rdfs:Class ;
        rdfs:comment     "The [[ReportageNewsArticle]] type is a subtype of [[NewsArticle]] representing\n news articles which are the result of journalistic news reporting conventions.\n\nIn practice many news publishers produce a wide variety of article types, many of which might be considered a [[NewsArticle]] but not a [[ReportageNewsArticle]]. For example, opinion pieces, reviews, analysis, sponsored or satirical articles, or articles that combine several of these elements.\n\nThe [[ReportageNewsArticle]] type is based on a stricter ideal for \"news\" as a work of journalism, with articles based on factual information either observed or verified by the author, or reported and verified from knowledgeable sources.  This often includes perspectives from multiple viewpoints on a particular issue (distinguishing news reports from public relations or propaganda).  News reports in the [[ReportageNewsArticle]] sense de-emphasize the opinion of the author, with commentary and value judgements typically expressed elsewhere.\n\nA [[ReportageNewsArticle]] which goes deeper into analysis can also be marked with an additional type of [[AnalysisNewsArticle]].\n" ;
        rdfs:label       "ReportageNewsArticle" ;
        rdfs:subClassOf  schema:NewsArticle .

schema:HowToTip  a       rdfs:Class ;
        rdfs:comment     "An explanation in the instructions for how to achieve a result. It provides supplementary information about a technique, supply, author's preference, etc. It can explain what could be done, or what should not be done, but doesn't specify what should be done (see HowToDirection)." ;
        rdfs:label       "HowToTip" ;
        rdfs:subClassOf  schema:ListItem , schema:CreativeWork .

schema:employerOverview
        a             rdf:Property ;
        rdfs:comment  "A description of the employer, career opportunities and work environment for this position." ;
        rdfs:label    "employerOverview" .

schema:maps  a        rdf:Property ;
        rdfs:comment  "A URL to a map of the place." ;
        rdfs:label    "maps" .

schema:CommunicateAction
        a                rdfs:Class ;
        rdfs:comment     "The act of conveying information to another person via a communication medium (instrument) such as speech, email, or telephone conversation." ;
        rdfs:label       "CommunicateAction" ;
        rdfs:subClassOf  schema:InteractAction .

schema:ImageGallery  a   rdfs:Class ;
        rdfs:comment     "Web page type: Image gallery page." ;
        rdfs:label       "ImageGallery" ;
        rdfs:subClassOf  schema:MediaGallery .

schema:touristType  a  rdf:Property ;
        rdfs:comment  "Attraction suitable for type(s) of tourist. eg. Children, visitors from a particular country, etc. " ;
        rdfs:label    "touristType" .

schema:breastfeedingWarning
        a             rdf:Property ;
        rdfs:comment  "Any precaution, guidance, contraindication, etc. related to this drug's use by breastfeeding mothers." ;
        rdfs:label    "breastfeedingWarning" .

schema:GatedResidenceCommunity
        a                rdfs:Class ;
        rdfs:comment     "Residence type: Gated community." ;
        rdfs:label       "GatedResidenceCommunity" ;
        rdfs:subClassOf  schema:Residence .

schema:subOrganization
        a             rdf:Property ;
        rdfs:comment  "A relationship between two organizations where the first includes the second, e.g., as a subsidiary. See also: the more specific 'department' property." ;
        rdfs:label    "subOrganization" .

schema:ClothingStore  a  rdfs:Class ;
        rdfs:comment     "A clothing store." ;
        rdfs:label       "ClothingStore" ;
        rdfs:subClassOf  schema:Store .

schema:CssSelectorType
        a                rdfs:Class ;
        rdfs:comment     "Text representing a CSS selector." ;
        rdfs:label       "CssSelectorType" ;
        rdfs:subClassOf  schema:Text .

schema:accommodationCategory
        a                   rdf:Property ;
        rdfs:comment        "Category of an [[Accommodation]], following real estate conventions e.g. RESO (see [PropertySubType](https://ddwiki.reso.org/display/DDW17/PropertySubType+Field), and [PropertyType](https://ddwiki.reso.org/display/DDW17/PropertyType+Field) fields  for suggested values)." ;
        rdfs:label          "accommodationCategory" ;
        rdfs:subPropertyOf  schema:category .

schema:actionApplication
        a             rdf:Property ;
        rdfs:comment  "An application that can complete the request." ;
        rdfs:label    "actionApplication" .

schema:termsOfService
        a             rdf:Property ;
        rdfs:comment  "Human-readable terms of service documentation." ;
        rdfs:label    "termsOfService" .

schema:billingIncrement
        a             rdf:Property ;
        rdfs:comment  "This property specifies the minimal quantity and rounding increment that will be the basis for the billing. The unit of measurement is specified by the unitCode property." ;
        rdfs:label    "billingIncrement" .

bibo:Periodical  a  rdfs:Class .

schema:seatNumber  a  rdf:Property ;
        rdfs:comment  "The location of the reserved seat (e.g., 27)." ;
        rdfs:label    "seatNumber" .

schema:mathExpression
        a             rdf:Property ;
        rdfs:comment  "A mathematical expression (e.g. 'x^2-3x=0') that may be solved for a specific variable, simplified, or transformed. This can take many formats, e.g. LaTeX, Ascii-Math, or math as you would write with a keyboard." ;
        rdfs:label    "mathExpression" .

schema:PriceComponentTypeEnumeration
        a                rdfs:Class ;
        rdfs:comment     "Enumerates different price components that together make up the total price for an offered product." ;
        rdfs:label       "PriceComponentTypeEnumeration" ;
        rdfs:subClassOf  schema:Enumeration .

schema:numberOfAirbags
        a             rdf:Property ;
        rdfs:comment  "The number or type of airbags in the vehicle." ;
        rdfs:label    "numberOfAirbags" .

schema:ReadAction  a     rdfs:Class ;
        rdfs:comment     "The act of consuming written content." ;
        rdfs:label       "ReadAction" ;
        rdfs:subClassOf  schema:ConsumeAction .

schema:numberOfPartialBathrooms
        a             rdf:Property ;
        rdfs:comment  "Number of partial bathrooms - The total number of half and ¼ bathrooms in an [[Accommodation]]. This corresponds to the [BathroomsPartial field in RESO](https://ddwiki.reso.org/display/DDW17/BathroomsPartial+Field). " ;
        rdfs:label    "numberOfPartialBathrooms" .

schema:Energy  a         rdfs:Class ;
        rdfs:comment     "Properties that take Energy as values are of the form '&lt;Number&gt; &lt;Energy unit of measure&gt;'." ;
        rdfs:label       "Energy" ;
        rdfs:subClassOf  schema:Quantity .

schema:funder  a            rdf:Property ;
        rdfs:comment        "A person or organization that supports (sponsors) something through some kind of financial contribution." ;
        rdfs:label          "funder" ;
        rdfs:subPropertyOf  schema:sponsor .

schema:legislationLegalForce
        a             rdf:Property ;
        rdfs:comment  "Whether the legislation is currently in force, not in force, or partially in force." ;
        rdfs:label    "legislationLegalForce" .

schema:episodes  a    rdf:Property ;
        rdfs:comment  "An episode of a TV/radio series or season." ;
        rdfs:label    "episodes" .

schema:reviewBody  a  rdf:Property ;
        rdfs:comment  "The actual body of the review." ;
        rdfs:label    "reviewBody" .

schema:AutoBodyShop  a   rdfs:Class ;
        rdfs:comment     "Auto body shop." ;
        rdfs:label       "AutoBodyShop" ;
        rdfs:subClassOf  schema:AutomotiveBusiness .

schema:typeOfGood  a  rdf:Property ;
        rdfs:comment  "The product that this structured value is referring to." ;
        rdfs:label    "typeOfGood" .

schema:billingAddress
        a             rdf:Property ;
        rdfs:comment  "The billing address for the order." ;
        rdfs:label    "billingAddress" .

schema:BuyAction  a      rdfs:Class ;
        rdfs:comment     "The act of giving money to a seller in exchange for goods or services rendered. An agent buys an object, product, or service from a seller for a price. Reciprocal of SellAction." ;
        rdfs:label       "BuyAction" ;
        rdfs:subClassOf  schema:TradeAction .

schema:DataCatalog  a    rdfs:Class ;
        rdfs:comment     "A collection of datasets." ;
        rdfs:label       "DataCatalog" ;
        rdfs:subClassOf  schema:CreativeWork .

schema:postOp  a      rdf:Property ;
        rdfs:comment  "A description of the postoperative procedures, care, and/or followups for this device." ;
        rdfs:label    "postOp" .

schema:lastReviewed  a  rdf:Property ;
        rdfs:comment  "Date on which the content on this web page was last reviewed for accuracy and/or completeness." ;
        rdfs:label    "lastReviewed" .

schema:contentReferenceTime
        a             rdf:Property ;
        rdfs:comment  "The specific time described by a creative work, for works (e.g. articles, video objects etc.) that emphasise a particular moment within an Event." ;
        rdfs:label    "contentReferenceTime" .

schema:parentService  a  rdf:Property ;
        rdfs:comment  "A broadcast service to which the broadcast service may belong to such as regional variations of a national channel." ;
        rdfs:label    "parentService" .

schema:caption  a     rdf:Property ;
        rdfs:comment  "The caption for this object. For downloadable machine formats (closed caption, subtitles etc.) use MediaObject and indicate the [[encodingFormat]]." ;
        rdfs:label    "caption" .

schema:possibleTreatment
        a             rdf:Property ;
        rdfs:comment  "A possible treatment to address this condition, sign or symptom." ;
        rdfs:label    "possibleTreatment" .

schema:contactType  a  rdf:Property ;
        rdfs:comment  "A person or organization can have different contact points, for different purposes. For example, a sales contact point, a PR contact point and so on. This property is used to specify the kind of contact point." ;
        rdfs:label    "contactType" .

schema:sourceOrganization
        a             rdf:Property ;
        rdfs:comment  "The Organization on whose behalf the creator was working." ;
        rdfs:label    "sourceOrganization" .

schema:musicReleaseFormat
        a             rdf:Property ;
        rdfs:comment  "Format of this release (the type of recording media used, ie. compact disc, digital media, LP, etc.)." ;
        rdfs:label    "musicReleaseFormat" .

schema:cvdCollectionDate
        a             rdf:Property ;
        rdfs:comment  "collectiondate - Date for which patient counts are reported." ;
        rdfs:label    "cvdCollectionDate" .

schema:sibling  a     rdf:Property ;
        rdfs:comment  "A sibling of the person." ;
        rdfs:label    "sibling" .

schema:PresentationDigitalDocument
        a                rdfs:Class ;
        rdfs:comment     "A file containing slides or used for a presentation." ;
        rdfs:label       "PresentationDigitalDocument" ;
        rdfs:subClassOf  schema:DigitalDocument .

schema:nutrition  a   rdf:Property ;
        rdfs:comment  "Nutrition information about the recipe or menu item." ;
        rdfs:label    "nutrition" .

schema:Suite  a          rdfs:Class ;
        rdfs:comment     "A suite in a hotel or other public accommodation, denotes a class of luxury accommodations, the key feature of which is multiple rooms (Source: Wikipedia, the free encyclopedia, see <a href=\"http://en.wikipedia.org/wiki/Suite_(hotel)\">http://en.wikipedia.org/wiki/Suite_(hotel)</a>).\n<br /><br />\nSee also the <a href=\"/docs/hotels.html\">dedicated document on the use of schema.org for marking up hotels and other forms of accommodations</a>.\n" ;
        rdfs:label       "Suite" ;
        rdfs:subClassOf  schema:Accommodation .

schema:ControlAction  a  rdfs:Class ;
        rdfs:comment     "An agent controls a device or application." ;
        rdfs:label       "ControlAction" ;
        rdfs:subClassOf  schema:Action .

schema:InteractionCounter
        a                rdfs:Class ;
        rdfs:comment     "A summary of how users have interacted with this CreativeWork. In most cases, authors will use a subtype to specify the specific type of interaction." ;
        rdfs:label       "InteractionCounter" ;
        rdfs:subClassOf  schema:StructuredValue .

schema:CheckOutAction
        a                rdfs:Class ;
        rdfs:comment     "The act of an agent communicating (service provider, social media, etc) their departure of a previously reserved service (e.g. flight check in) or place (e.g. hotel).\\n\\nRelated actions:\\n\\n* [[CheckInAction]]: The antonym of CheckOutAction.\\n* [[DepartAction]]: Unlike DepartAction, CheckOutAction implies that the agent is informing/confirming the end of a previously reserved service.\\n* [[CancelAction]]: Unlike CancelAction, CheckOutAction implies that the agent is informing/confirming the end of a previously reserved service." ;
        rdfs:label       "CheckOutAction" ;
        rdfs:subClassOf  schema:CommunicateAction .

schema:PayAction  a      rdfs:Class ;
        rdfs:comment     "An agent pays a price to a participant." ;
        rdfs:label       "PayAction" ;
        rdfs:subClassOf  schema:TradeAction .

schema:MedicalAudience
        a                rdfs:Class ;
        rdfs:comment     "Target audiences for medical web pages." ;
        rdfs:label       "MedicalAudience" ;
        rdfs:subClassOf  schema:PeopleAudience , schema:Audience .

schema:workTranslation
        a             rdf:Property ;
        rdfs:comment  "A work that is a translation of the content of this work. e.g. 西遊記 has an English workTranslation “Journey to the West”,a German workTranslation “Monkeys Pilgerfahrt” and a Vietnamese  translation Tây du ký bình khảo." ;
        rdfs:label    "workTranslation" .

schema:subtitleLanguage
        a             rdf:Property ;
        rdfs:comment  "Languages in which subtitles/captions are available, in [IETF BCP 47 standard format](http://tools.ietf.org/html/bcp47)." ;
        rdfs:label    "subtitleLanguage" .

schema:ProfessionalService
        a                rdfs:Class ;
        rdfs:comment     "Original definition: \"provider of professional services.\"\\n\\nThe general [[ProfessionalService]] type for local businesses was deprecated due to confusion with [[Service]]. For reference, the types that it included were: [[Dentist]],\n        [[AccountingService]], [[Attorney]], [[Notary]], as well as types for several kinds of [[HomeAndConstructionBusiness]]: [[Electrician]], [[GeneralContractor]],\n        [[HousePainter]], [[Locksmith]], [[Plumber]], [[RoofingContractor]]. [[LegalService]] was introduced as a more inclusive supertype of [[Attorney]]." ;
        rdfs:label       "ProfessionalService" ;
        rdfs:subClassOf  schema:LocalBusiness .

schema:artMedium  a         rdf:Property ;
        rdfs:comment        "The material used. (e.g. Oil, Watercolour, Acrylic, Linoprint, Marble, Cyanotype, Digital, Lithograph, DryPoint, Intaglio, Pastel, Woodcut, Pencil, Mixed Media, etc.)" ;
        rdfs:label          "artMedium" ;
        rdfs:subPropertyOf  schema:material .

schema:purchaseDate  a  rdf:Property ;
        rdfs:comment  "The date the item e.g. vehicle was purchased by the current owner." ;
        rdfs:label    "purchaseDate" .

schema:seller  a            rdf:Property ;
        rdfs:comment        "An entity which offers (sells / leases / lends / loans) the services / goods.  A seller may also be a provider." ;
        rdfs:label          "seller" ;
        rdfs:subPropertyOf  schema:participant .

schema:arrivalBusStop
        a             rdf:Property ;
        rdfs:comment  "The stop or station from which the bus arrives." ;
        rdfs:label    "arrivalBusStop" .

schema:about  a       rdf:Property ;
        rdfs:comment  "The subject matter of the content." ;
        rdfs:label    "about" .

schema:eduQuestionType
        a             rdf:Property ;
        rdfs:comment  "For questions that are part of learning resources (e.g. Quiz), eduQuestionType indicates the format of question being given. Example: \"Multiple choice\", \"Open ended\", \"Flashcard\"." ;
        rdfs:label    "eduQuestionType" .

schema:inSupportOf  a  rdf:Property ;
        rdfs:comment  "Qualification, candidature, degree, application that Thesis supports." ;
        rdfs:label    "inSupportOf" .

schema:typicalAgeRange
        a             rdf:Property ;
        rdfs:comment  "The typical expected age range, e.g. '7-9', '11-'." ;
        rdfs:label    "typicalAgeRange" .

schema:shippingRate  a  rdf:Property ;
        rdfs:comment  "The shipping rate is the cost of shipping to the specified destination. Typically, the maxValue and currency values (of the [[MonetaryAmount]]) are most appropriate." ;
        rdfs:label    "shippingRate" .

schema:SoftwareSourceCode
        a                rdfs:Class ;
        rdfs:comment     "Computer programming source code. Example: Full (compile ready) solutions, code snippet samples, scripts, templates." ;
        rdfs:label       "SoftwareSourceCode" ;
        rdfs:subClassOf  schema:CreativeWork .

schema:WinAction  a      rdfs:Class ;
        rdfs:comment     "The act of achieving victory in a competitive activity." ;
        rdfs:label       "WinAction" ;
        rdfs:subClassOf  schema:AchieveAction .

schema:sharedContent  a  rdf:Property ;
        rdfs:comment  "A CreativeWork such as an image, video, or audio clip shared as part of this posting." ;
        rdfs:label    "sharedContent" .

schema:providesBroadcastService
        a             rdf:Property ;
        rdfs:comment  "The BroadcastService offered on this channel." ;
        rdfs:label    "providesBroadcastService" .

schema:LoseAction  a     rdfs:Class ;
        rdfs:comment     "The act of being defeated in a competitive activity." ;
        rdfs:label       "LoseAction" ;
        rdfs:subClassOf  schema:AchieveAction .

schema:IgnoreAction  a   rdfs:Class ;
        rdfs:comment     "The act of intentionally disregarding the object. An agent ignores an object." ;
        rdfs:label       "IgnoreAction" ;
        rdfs:subClassOf  schema:AssessAction .

schema:fromLocation  a      rdf:Property ;
        rdfs:comment        "A sub property of location. The original location of the object or the agent before the action." ;
        rdfs:label          "fromLocation" ;
        rdfs:subPropertyOf  schema:location .

schema:postalCodeBegin
        a             rdf:Property ;
        rdfs:comment  "First postal code in a range (included)." ;
        rdfs:label    "postalCodeBegin" .

schema:BroadcastEvent
        a                rdfs:Class ;
        rdfs:comment     "An over the air or online broadcast event." ;
        rdfs:label       "BroadcastEvent" ;
        rdfs:subClassOf  schema:PublicationEvent .

schema:inProductGroupWithID
        a             rdf:Property ;
        rdfs:comment  "Indicates the [[productGroupID]] for a [[ProductGroup]] that this product [[isVariantOf]]. " ;
        rdfs:label    "inProductGroupWithID" .

schema:Residence  a      rdfs:Class ;
        rdfs:comment     "The place where a person lives." ;
        rdfs:label       "Residence" ;
        rdfs:subClassOf  schema:Place .

schema:TelevisionStation
        a                rdfs:Class ;
        rdfs:comment     "A television station." ;
        rdfs:label       "TelevisionStation" ;
        rdfs:subClassOf  schema:LocalBusiness .

schema:ShippingDeliveryTime
        a                rdfs:Class ;
        rdfs:comment     "ShippingDeliveryTime provides various pieces of information about delivery times for shipping." ;
        rdfs:label       "ShippingDeliveryTime" ;
        rdfs:subClassOf  schema:StructuredValue .

schema:gtin  a              rdf:Property ;
        rdfs:comment        "A Global Trade Item Number ([GTIN](https://www.gs1.org/standards/id-keys/gtin)). GTINs identify trade items, including products and services, using numeric identification codes. The [[gtin]] property generalizes the earlier [[gtin8]], [[gtin12]], [[gtin13]], and [[gtin14]] properties. The GS1 [digital link specifications](https://www.gs1.org/standards/Digital-Link/) express GTINs as URLs. A correct [[gtin]] value should be a valid GTIN, which means that it should be an all-numeric string of either 8, 12, 13 or 14 digits, or a \"GS1 Digital Link\" URL based on such a string. The numeric component should also have a [valid GS1 check digit](https://www.gs1.org/services/check-digit-calculator) and meet the other rules for valid GTINs. See also [GS1's GTIN Summary](http://www.gs1.org/barcodes/technical/idkeys/gtin) and [Wikipedia](https://en.wikipedia.org/wiki/Global_Trade_Item_Number) for more details. Left-padding of the gtin values is not required or encouraged.\n   " ;
        rdfs:label          "gtin" ;
        rdfs:subPropertyOf  schema:identifier .

schema:QuoteAction  a    rdfs:Class ;
        rdfs:comment     "An agent quotes/estimates/appraises an object/product/service with a price at a location/store." ;
        rdfs:label       "QuoteAction" ;
        rdfs:subClassOf  schema:TradeAction .

schema:recordedIn  a  rdf:Property ;
        rdfs:comment  "The CreativeWork that captured all or part of this Event." ;
        rdfs:label    "recordedIn" .

schema:givenName  a   rdf:Property ;
        rdfs:comment  "Given name. In the U.S., the first name of a Person." ;
        rdfs:label    "givenName" .

schema:affectedBy  a  rdf:Property ;
        rdfs:comment  "Drugs that affect the test's results." ;
        rdfs:label    "affectedBy" .

schema:stage  a       rdf:Property ;
        rdfs:comment  "The stage of the condition, if applicable." ;
        rdfs:label    "stage" .

schema:recordedAs  a  rdf:Property ;
        rdfs:comment  "An audio recording of the work." ;
        rdfs:label    "recordedAs" .

schema:arterialBranch
        a             rdf:Property ;
        rdfs:comment  "The branches that comprise the arterial structure." ;
        rdfs:label    "arterialBranch" .

schema:meetsEmissionStandard
        a             rdf:Property ;
        rdfs:comment  "Indicates that the vehicle meets the respective emission standard." ;
        rdfs:label    "meetsEmissionStandard" .

schema:ComicCoverArt  a  rdfs:Class ;
        rdfs:comment     "The artwork on the cover of a comic." ;
        rdfs:label       "ComicCoverArt" ;
        rdfs:subClassOf  schema:CoverArt , schema:ComicStory .

schema:seriousAdverseOutcome
        a             rdf:Property ;
        rdfs:comment  "A possible serious complication and/or serious side effect of this therapy. Serious adverse outcomes include those that are life-threatening; result in death, disability, or permanent damage; require hospitalization or prolong existing hospitalization; cause congenital anomalies or birth defects; or jeopardize the patient and may require medical or surgical intervention to prevent one of the outcomes in this definition." ;
        rdfs:label    "seriousAdverseOutcome" .

schema:studySubject  a  rdf:Property ;
        rdfs:comment  "A subject of the study, i.e. one of the medical conditions, therapies, devices, drugs, etc. investigated by the study." ;
        rdfs:label    "studySubject" .

schema:secondaryPrevention
        a             rdf:Property ;
        rdfs:comment  "A preventative therapy used to prevent reoccurrence of the medical condition after an initial episode of the condition." ;
        rdfs:label    "secondaryPrevention" .

schema:issuedThrough  a  rdf:Property ;
        rdfs:comment  "The service through with the permit was granted." ;
        rdfs:label    "issuedThrough" .

schema:NLNonprofitType
        a                rdfs:Class ;
        rdfs:comment     "NLNonprofitType: Non-profit organization type originating from the Netherlands." ;
        rdfs:label       "NLNonprofitType" ;
        rdfs:subClassOf  schema:NonprofitType .

schema:risks  a       rdf:Property ;
        rdfs:comment  "Specific physiologic risks associated to the diet plan." ;
        rdfs:label    "risks" .

schema:ScreeningEvent
        a                rdfs:Class ;
        rdfs:comment     "A screening of a movie or other video." ;
        rdfs:label       "ScreeningEvent" ;
        rdfs:subClassOf  schema:Event .

schema:exerciseType  a  rdf:Property ;
        rdfs:comment  "Type(s) of exercise or activity, such as strength training, flexibility training, aerobics, cardiac rehabilitation, etc." ;
        rdfs:label    "exerciseType" .

schema:aggregateRating
        a             rdf:Property ;
        rdfs:comment  "The overall rating, based on a collection of reviews or ratings, of the item." ;
        rdfs:label    "aggregateRating" .

schema:orderDelivery  a  rdf:Property ;
        rdfs:comment  "The delivery of the parcel related to this order or order item." ;
        rdfs:label    "orderDelivery" .

schema:totalTime  a   rdf:Property ;
        rdfs:comment  "The total time required to perform instructions or a direction (including time to prepare the supplies), in [ISO 8601 duration format](http://en.wikipedia.org/wiki/ISO_8601)." ;
        rdfs:label    "totalTime" .

schema:MeetingRoom  a    rdfs:Class ;
        rdfs:comment     "A meeting room, conference room, or conference hall is a room provided for singular events such as business conferences and meetings (Source: Wikipedia, the free encyclopedia, see <a href=\"http://en.wikipedia.org/wiki/Conference_hall\">http://en.wikipedia.org/wiki/Conference_hall</a>).\n<br /><br />\nSee also the <a href=\"/docs/hotels.html\">dedicated document on the use of schema.org for marking up hotels and other forms of accommodations</a>.\n" ;
        rdfs:label       "MeetingRoom" ;
        rdfs:subClassOf  schema:Room .

schema:AnimalShelter  a  rdfs:Class ;
        rdfs:comment     "Animal shelter." ;
        rdfs:label       "AnimalShelter" ;
        rdfs:subClassOf  schema:LocalBusiness .

schema:directors  a   rdf:Property ;
        rdfs:comment  "A director of e.g. tv, radio, movie, video games etc. content. Directors can be associated with individual items or with a series, episode, clip." ;
        rdfs:label    "directors" .

schema:EventAttendanceModeEnumeration
        a                rdfs:Class ;
        rdfs:comment     "An EventAttendanceModeEnumeration value is one of potentially several modes of organising an event, relating to whether it is online or offline." ;
        rdfs:label       "EventAttendanceModeEnumeration" ;
        rdfs:subClassOf  schema:Enumeration .

schema:includedInDataCatalog
        a             rdf:Property ;
        rdfs:comment  "A data catalog which contains this dataset." ;
        rdfs:label    "includedInDataCatalog" .

schema:valueReference
        a             rdf:Property ;
        rdfs:comment  "A secondary value that provides additional information on the original value, e.g. a reference temperature or a type of measurement." ;
        rdfs:label    "valueReference" .

schema:DeliveryTimeSettings
        a                rdfs:Class ;
        rdfs:comment     "A DeliveryTimeSettings represents re-usable pieces of shipping information, relating to timing. It is designed for publication on an URL that may be referenced via the [[shippingSettingsLink]] property of a [[OfferShippingDetails]]. Several occurrences can be published, distinguished (and identified/referenced) by their different values for [[transitTimeLabel]]." ;
        rdfs:label       "DeliveryTimeSettings" ;
        rdfs:subClassOf  schema:StructuredValue .

schema:causeOf  a     rdf:Property ;
        rdfs:comment  "The condition, complication, symptom, sign, etc. caused." ;
        rdfs:label    "causeOf" .

schema:eligibleTransactionVolume
        a             rdf:Property ;
        rdfs:comment  "The transaction volume, in a monetary unit, for which the offer or price specification is valid, e.g. for indicating a minimal purchasing volume, to express free shipping above a certain order volume, or to limit the acceptance of credit cards to purchases to a certain minimal amount." ;
        rdfs:label    "eligibleTransactionVolume" .

schema:Book  a           rdfs:Class ;
        rdfs:comment     "A book." ;
        rdfs:label       "Book" ;
        rdfs:subClassOf  schema:CreativeWork .

schema:characterName  a  rdf:Property ;
        rdfs:comment  "The name of a character played in some acting or performing role, i.e. in a PerformanceRole." ;
        rdfs:label    "characterName" .

schema:illustrator  a  rdf:Property ;
        rdfs:comment  "The illustrator of the book." ;
        rdfs:label    "illustrator" .

schema:SeaBodyOfWater
        a                rdfs:Class ;
        rdfs:comment     "A sea (for example, the Caspian sea)." ;
        rdfs:label       "SeaBodyOfWater" ;
        rdfs:subClassOf  schema:BodyOfWater .

schema:hasDigitalDocumentPermission
        a             rdf:Property ;
        rdfs:comment  "A permission related to the access to this document (e.g. permission to read or write an electronic document). For a public document, specify a grantee with an Audience with audienceType equal to \"public\"." ;
        rdfs:label    "hasDigitalDocumentPermission" .

schema:geoMidpoint  a  rdf:Property ;
        rdfs:comment  "Indicates the GeoCoordinates at the centre of a GeoShape e.g. GeoCircle." ;
        rdfs:label    "geoMidpoint" .

schema:performer  a   rdf:Property ;
        rdfs:comment  "A performer at the event&#x2014;for example, a presenter, musician, musical group or actor." ;
        rdfs:label    "performer" .

schema:suggestedAnswer
        a             rdf:Property ;
        rdfs:comment  "An answer (possibly one of several, possibly incorrect) to a Question, e.g. on a Question/Answer site." ;
        rdfs:label    "suggestedAnswer" .

schema:isSimilarTo  a  rdf:Property ;
        rdfs:comment  "A pointer to another, functionally similar product (or multiple products)." ;
        rdfs:label    "isSimilarTo" .

schema:numberOfDoors  a  rdf:Property ;
        rdfs:comment  "The number of doors.\\n\\nTypical unit code(s): C62" ;
        rdfs:label    "numberOfDoors" .

schema:procedureType  a  rdf:Property ;
        rdfs:comment  "The type of procedure, for example Surgical, Noninvasive, or Percutaneous." ;
        rdfs:label    "procedureType" .

schema:Game  a           rdfs:Class ;
        rdfs:comment     "The Game type represents things which are games. These are typically rule-governed recreational activities, e.g. role-playing games in which players assume the role of characters in a fictional setting." ;
        rdfs:label       "Game" ;
        rdfs:subClassOf  schema:CreativeWork .

schema:Dataset  a        rdfs:Class ;
        rdfs:comment     "A body of structured information describing some topic(s) of interest." ;
        rdfs:label       "Dataset" ;
        rdfs:subClassOf  schema:CreativeWork .

schema:hasMenuSection
        a             rdf:Property ;
        rdfs:comment  "A subgrouping of the menu (by dishes, course, serving time period, etc.)." ;
        rdfs:label    "hasMenuSection" .

dcmitype:Dataset  a  rdfs:Class .

schema:transitTime  a  rdf:Property ;
        rdfs:comment  "The typical delay the order has been sent for delivery and the goods reach the final customer. Typical properties: minValue, maxValue, unitCode (d for DAY)." ;
        rdfs:label    "transitTime" .

schema:Vein  a           rdfs:Class ;
        rdfs:comment     "A type of blood vessel that specifically carries blood to the heart." ;
        rdfs:label       "Vein" ;
        rdfs:subClassOf  schema:Vessel .

schema:drainsTo  a    rdf:Property ;
        rdfs:comment  "The vasculature that the vein drains into." ;
        rdfs:label    "drainsTo" .

schema:busNumber  a   rdf:Property ;
        rdfs:comment  "The unique identifier for the bus." ;
        rdfs:label    "busNumber" .

schema:SuspendAction  a  rdfs:Class ;
        rdfs:comment     "The act of momentarily pausing a device or application (e.g. pause music playback or pause a timer)." ;
        rdfs:label       "SuspendAction" ;
        rdfs:subClassOf  schema:ControlAction .

schema:passengerPriorityStatus
        a             rdf:Property ;
        rdfs:comment  "The priority status assigned to a passenger for security or boarding (e.g. FastTrack or Priority)." ;
        rdfs:label    "passengerPriorityStatus" .

schema:TaxiReservation
        a                rdfs:Class ;
        rdfs:comment     "A reservation for a taxi.\\n\\nNote: This type is for information about actual reservations, e.g. in confirmation emails or HTML pages with individual confirmations of reservations. For offers of tickets, use [[Offer]]." ;
        rdfs:label       "TaxiReservation" ;
        rdfs:subClassOf  schema:Reservation .

schema:interactionType
        a             rdf:Property ;
        rdfs:comment  "The Action representing the type of interaction. For up votes, +1s, etc. use [[LikeAction]]. For down votes use [[DislikeAction]]. Otherwise, use the most specific Action." ;
        rdfs:label    "interactionType" .

schema:Obstetric  a      rdfs:Class ;
        rdfs:comment     "A specific branch of medical science that specializes in the care of women during the prenatal and postnatal care and with the delivery of the child." ;
        rdfs:label       "Obstetric" ;
        rdfs:subClassOf  schema:MedicalBusiness .

schema:MedicineSystem
        a                rdfs:Class ;
        rdfs:comment     "Systems of medical practice." ;
        rdfs:label       "MedicineSystem" ;
        rdfs:subClassOf  schema:MedicalEnumeration .

schema:additionalProperty
        a             rdf:Property ;
        rdfs:comment  "A property-value pair representing an additional characteristics of the entitity, e.g. a product feature or another characteristic for which there is no matching property in schema.org.\\n\\nNote: Publishers should be aware that applications designed to use specific schema.org properties (e.g. http://schema.org/width, http://schema.org/color, http://schema.org/gtin13, ...) will typically expect such data to be provided using those properties, rather than using the generic property/value mechanism.\n" ;
        rdfs:label    "additionalProperty" .

schema:distance  a    rdf:Property ;
        rdfs:comment  "The distance travelled, e.g. exercising or travelling." ;
        rdfs:label    "distance" .

schema:AMRadioChannel
        a                rdfs:Class ;
        rdfs:comment     "A radio channel that uses AM." ;
        rdfs:label       "AMRadioChannel" ;
        rdfs:subClassOf  schema:RadioChannel .

schema:dateCreated  a  rdf:Property ;
        rdfs:comment  "The date on which the CreativeWork was created or the item was added to a DataFeed." ;
        rdfs:label    "dateCreated" .

schema:BusinessEntityType
        a                rdfs:Class ;
        rdfs:comment     "A business entity type is a conceptual entity representing the legal form, the size, the main line of business, the position in the value chain, or any combination thereof, of an organization or business person.\\n\\nCommonly used values:\\n\\n* http://purl.org/goodrelations/v1#Business\\n* http://purl.org/goodrelations/v1#Enduser\\n* http://purl.org/goodrelations/v1#PublicInstitution\\n* http://purl.org/goodrelations/v1#Reseller\n\t  " ;
        rdfs:label       "BusinessEntityType" ;
        rdfs:subClassOf  schema:Enumeration .

schema:ElectronicsStore
        a                rdfs:Class ;
        rdfs:comment     "An electronics store." ;
        rdfs:label       "ElectronicsStore" ;
        rdfs:subClassOf  schema:Store .

schema:CommunityHealth
        a                rdfs:Class ;
        rdfs:comment     "A field of public health focusing on improving health characteristics of a defined population in relation with their geographical or environment areas." ;
        rdfs:label       "CommunityHealth" ;
        rdfs:subClassOf  schema:MedicalBusiness .

schema:duns  a              rdf:Property ;
        rdfs:comment        "The Dun & Bradstreet DUNS number for identifying an organization or business person." ;
        rdfs:label          "duns" ;
        rdfs:subPropertyOf  schema:identifier .

schema:byArtist  a    rdf:Property ;
        rdfs:comment  "The artist that performed this album or recording." ;
        rdfs:label    "byArtist" .

schema:geoDisjoint  a  rdf:Property ;
        rdfs:comment  "Represents spatial relations in which two geometries (or the places they represent) are topologically disjoint: they have no point in common. They form a set of disconnected geometries.\" (a symmetric relationship, as defined in [DE-9IM](https://en.wikipedia.org/wiki/DE-9IM))" ;
        rdfs:label    "geoDisjoint" .

schema:businessDays  a  rdf:Property ;
        rdfs:comment  "Days of the week when the merchant typically operates, indicated via opening hours markup." ;
        rdfs:label    "businessDays" .

schema:recipeCuisine  a  rdf:Property ;
        rdfs:comment  "The cuisine of the recipe (for example, French or Ethiopian)." ;
        rdfs:label    "recipeCuisine" .

schema:countriesSupported
        a             rdf:Property ;
        rdfs:comment  "Countries for which the application is supported. You can also provide the two-letter ISO 3166-1 alpha-2 country code." ;
        rdfs:label    "countriesSupported" .

schema:includedDataCatalog
        a             rdf:Property ;
        rdfs:comment  "A data catalog which contains this dataset (this property was previously 'catalog', preferred name is now 'includedInDataCatalog')." ;
        rdfs:label    "includedDataCatalog" .

schema:ethicsPolicy  a  rdf:Property ;
        rdfs:comment  "Statement about ethics policy, e.g. of a [[NewsMediaOrganization]] regarding journalistic and publishing practices, or of a [[Restaurant]], a page describing food source policies. In the case of a [[NewsMediaOrganization]], an ethicsPolicy is typically a statement describing the personal, organizational, and corporate standards of behavior expected by the organization." ;
        rdfs:label    "ethicsPolicy" .

schema:Airport  a        rdfs:Class ;
        rdfs:comment     "An airport." ;
        rdfs:label       "Airport" ;
        rdfs:subClassOf  schema:CivicStructure .

schema:Aquarium  a       rdfs:Class ;
        rdfs:comment     "Aquarium." ;
        rdfs:label       "Aquarium" ;
        rdfs:subClassOf  schema:CivicStructure .

schema:departurePlatform
        a             rdf:Property ;
        rdfs:comment  "The platform from which the train departs." ;
        rdfs:label    "departurePlatform" .

schema:State  a          rdfs:Class ;
        rdfs:comment     "A state or province of a country." ;
        rdfs:label       "State" ;
        rdfs:subClassOf  schema:AdministrativeArea .

schema:Atlas  a          rdfs:Class ;
        rdfs:comment     "A collection or bound volume of maps, charts, plates or tables, physical or in media form illustrating any subject." ;
        rdfs:label       "Atlas" ;
        rdfs:subClassOf  schema:CreativeWork .

schema:DeliveryMethod
        a                rdfs:Class ;
        rdfs:comment     "A delivery method is a standardized procedure for transferring the product or service to the destination of fulfillment chosen by the customer. Delivery methods are characterized by the means of transportation used, and by the organization or group that is the contracting party for the sending organization or person.\\n\\nCommonly used values:\\n\\n* http://purl.org/goodrelations/v1#DeliveryModeDirectDownload\\n* http://purl.org/goodrelations/v1#DeliveryModeFreight\\n* http://purl.org/goodrelations/v1#DeliveryModeMail\\n* http://purl.org/goodrelations/v1#DeliveryModeOwnFleet\\n* http://purl.org/goodrelations/v1#DeliveryModePickUp\\n* http://purl.org/goodrelations/v1#DHL\\n* http://purl.org/goodrelations/v1#FederalExpress\\n* http://purl.org/goodrelations/v1#UPS\n        " ;
        rdfs:label       "DeliveryMethod" ;
        rdfs:subClassOf  schema:Enumeration .

schema:ContactPointOption
        a                rdfs:Class ;
        rdfs:comment     "Enumerated options related to a ContactPoint." ;
        rdfs:label       "ContactPointOption" ;
        rdfs:subClassOf  schema:Enumeration .

schema:multipleValues
        a             rdf:Property ;
        rdfs:comment  "Whether multiple values are allowed for the property.  Default is false." ;
        rdfs:label    "multipleValues" .

schema:featureList  a  rdf:Property ;
        rdfs:comment  "Features or modules provided by this application (and possibly required by other applications)." ;
        rdfs:label    "featureList" .

schema:InsuranceAgency
        a                rdfs:Class ;
        rdfs:comment     "An Insurance agency." ;
        rdfs:label       "InsuranceAgency" ;
        rdfs:subClassOf  schema:FinancialService .

schema:SportsEvent  a    rdfs:Class ;
        rdfs:comment     "Event type: Sports event." ;
        rdfs:label       "SportsEvent" ;
        rdfs:subClassOf  schema:Event .

schema:branchOf  a    rdf:Property ;
        rdfs:comment  "The larger organization that this local business is a branch of, if any. Not to be confused with (anatomical)[[branch]]." ;
        rdfs:label    "branchOf" .

schema:EmployerAggregateRating
        a                rdfs:Class ;
        rdfs:comment     "An aggregate rating of an Organization related to its role as an employer." ;
        rdfs:label       "EmployerAggregateRating" ;
        rdfs:subClassOf  schema:AggregateRating .

schema:coverageEndTime
        a             rdf:Property ;
        rdfs:comment  "The time when the live blog will stop covering the Event. Note that coverage may continue after the Event concludes." ;
        rdfs:label    "coverageEndTime" .

schema:musicGroupMember
        a             rdf:Property ;
        rdfs:comment  "A member of a music group&#x2014;for example, John, Paul, George, or Ringo." ;
        rdfs:label    "musicGroupMember" .

schema:collectionSize
        a             rdf:Property ;
        rdfs:comment  "The number of items in the [[Collection]]."@en ;
        rdfs:label    "collectionSize"@en .

schema:legislationDate
        a                   rdf:Property ;
        rdfs:comment        "The date of adoption or signature of the legislation. This is the date at which the text is officially aknowledged to be a legislation, even though it might not even be published or in force." ;
        rdfs:label          "legislationDate" ;
        rdfs:subPropertyOf  schema:dateCreated .

schema:GolfCourse  a     rdfs:Class ;
        rdfs:comment     "A golf course." ;
        rdfs:label       "GolfCourse" ;
        rdfs:subClassOf  schema:SportsActivityLocation .

schema:serviceOutput  a  rdf:Property ;
        rdfs:comment  "The tangible thing generated by the service, e.g. a passport, permit, etc." ;
        rdfs:label    "serviceOutput" .

schema:OfferShippingDetails
        a                rdfs:Class ;
        rdfs:comment     "OfferShippingDetails represents information about shipping destinations.\n\nMultiple of these entities can be used to represent different shipping rates for different destinations:\n\nOne entity for Alaska/Hawaii. A different one for continental US.A different one for all France.\n\nMultiple of these entities can be used to represent different shipping costs and delivery times.\n\nTwo entities that are identical but differ in rate and time:\n\ne.g. Cheaper and slower: $5 in 5-7days\nor Fast and expensive: $15 in 1-2 days." ;
        rdfs:label       "OfferShippingDetails" ;
        rdfs:subClassOf  schema:StructuredValue .

schema:LegalValueLevel
        a                rdfs:Class ;
        rdfs:comment     "A list of possible levels for the legal validity of a legislation." ;
        rdfs:label       "LegalValueLevel" ;
        rdfs:subClassOf  schema:Enumeration .

schema:EducationalOrganization
        a                rdfs:Class ;
        rdfs:comment     "An educational organization." ;
        rdfs:label       "EducationalOrganization" ;
        rdfs:subClassOf  schema:CivicStructure , schema:Organization .

schema:InfectiousDisease
        a                rdfs:Class ;
        rdfs:comment     "An infectious disease is a clinically evident human disease resulting from the presence of pathogenic microbial agents, like pathogenic viruses, pathogenic bacteria, fungi, protozoa, multicellular parasites, and prions. To be considered an infectious disease, such pathogens are known to be able to cause this disease." ;
        rdfs:label       "InfectiousDisease" ;
        rdfs:subClassOf  schema:MedicalCondition .

schema:EducationalOccupationalCredential
        a                rdfs:Class ;
        rdfs:comment     "An educational or occupational credential. A diploma, academic degree, certification, qualification, badge, etc., that may be awarded to a person or other entity that meets the requirements defined by the credentialer." ;
        rdfs:label       "EducationalOccupationalCredential" ;
        rdfs:subClassOf  schema:CreativeWork .

schema:ratingValue  a  rdf:Property ;
        rdfs:comment  "The rating for the content.\\n\\nUsage guidelines:\\n\\n* Use values from 0123456789 (Unicode 'DIGIT ZERO' (U+0030) to 'DIGIT NINE' (U+0039)) rather than superficially similiar Unicode symbols.\\n* Use '.' (Unicode 'FULL STOP' (U+002E)) rather than ',' to indicate a decimal point. Avoid using these symbols as a readability separator." ;
        rdfs:label    "ratingValue" .

schema:CorrectionComment
        a                rdfs:Class ;
        rdfs:comment     "A [[comment]] that corrects [[CreativeWork]]." ;
        rdfs:label       "CorrectionComment" ;
        rdfs:subClassOf  schema:Comment .

schema:lesser  a      rdf:Property ;
        rdfs:comment  "This ordering relation for qualitative values indicates that the subject is lesser than the object." ;
        rdfs:label    "lesser" .

schema:itemListElement
        a             rdf:Property ;
        rdfs:comment  "For itemListElement values, you can use simple strings (e.g. \"Peter\", \"Paul\", \"Mary\"), existing entities, or use ListItem.\\n\\nText values are best if the elements in the list are plain strings. Existing entities are best for a simple, unordered list of existing things in your data. ListItem is used with ordered lists when you want to provide additional context about the element in that list or when the same item might be in different places in different lists.\\n\\nNote: The order of elements in your mark-up is not sufficient for indicating the order or elements.  Use ListItem with a 'position' property in such cases." ;
        rdfs:label    "itemListElement" .

schema:GameServer  a     rdfs:Class ;
        rdfs:comment     "Server that provides game interaction in a multiplayer game." ;
        rdfs:label       "GameServer" ;
        rdfs:subClassOf  schema:Intangible .

schema:Brewery  a        rdfs:Class ;
        rdfs:comment     "Brewery." ;
        rdfs:label       "Brewery" ;
        rdfs:subClassOf  schema:FoodEstablishment .

schema:handlingTime  a  rdf:Property ;
        rdfs:comment  "The typical delay between the receipt of the order and the goods either leaving the warehouse or being prepared for pickup, in case the delivery method is on site pickup. Typical properties: minValue, maxValue, unitCode (d for DAY).  This is by common convention assumed to mean business days (if a unitCode is used, coded as \"d\"), i.e. only counting days when the business normally operates." ;
        rdfs:label    "handlingTime" .

schema:includesAttraction
        a             rdf:Property ;
        rdfs:comment  "Attraction located at destination." ;
        rdfs:label    "includesAttraction" .

schema:FMRadioChannel
        a                rdfs:Class ;
        rdfs:comment     "A radio channel that uses FM." ;
        rdfs:label       "FMRadioChannel" ;
        rdfs:subClassOf  schema:RadioChannel .

schema:SportingGoodsStore
        a                rdfs:Class ;
        rdfs:comment     "A sporting goods store." ;
        rdfs:label       "SportingGoodsStore" ;
        rdfs:subClassOf  schema:Store .

ns1:closeMatch  a  rdf:Property .

schema:beforeMedia  a  rdf:Property ;
        rdfs:comment  "A media object representing the circumstances before performing this direction." ;
        rdfs:label    "beforeMedia" .

schema:taxID  a             rdf:Property ;
        rdfs:comment        "The Tax / Fiscal ID of the organization or person, e.g. the TIN in the US or the CIF/NIF in Spain." ;
        rdfs:label          "taxID" ;
        rdfs:subPropertyOf  schema:identifier .

schema:healthPlanPharmacyCategory
        a             rdf:Property ;
        rdfs:comment  "The category or type of pharmacy associated with this cost sharing." ;
        rdfs:label    "healthPlanPharmacyCategory" .

schema:temporal  a    rdf:Property ;
        rdfs:comment  "The \"temporal\" property can be used in cases where more specific properties\n(e.g. [[temporalCoverage]], [[dateCreated]], [[dateModified]], [[datePublished]]) are not known to be appropriate." ;
        rdfs:label    "temporal" .

schema:departureGate  a  rdf:Property ;
        rdfs:comment  "Identifier of the flight's departure gate." ;
        rdfs:label    "departureGate" .

schema:MenuItem  a       rdfs:Class ;
        rdfs:comment     "A food or drink item listed in a menu or menu section." ;
        rdfs:label       "MenuItem" ;
        rdfs:subClassOf  schema:Intangible .

schema:geoOverlaps  a  rdf:Property ;
        rdfs:comment  "Represents a relationship between two geometries (or the places they represent), relating a geometry to another that geospatially overlaps it, i.e. they have some but not all points in common. As defined in [DE-9IM](https://en.wikipedia.org/wiki/DE-9IM)." ;
        rdfs:label    "geoOverlaps" .

schema:appearance  a        rdf:Property ;
        rdfs:comment        "Indicates an occurence of a [[Claim]] in some [[CreativeWork]]." ;
        rdfs:label          "appearance" ;
        rdfs:subPropertyOf  schema:workExample .

schema:coverageStartTime
        a             rdf:Property ;
        rdfs:comment  "The time when the live blog will begin covering the Event. Note that coverage may begin before the Event's start time. The LiveBlogPosting may also be created before coverage begins." ;
        rdfs:label    "coverageStartTime" .

schema:hasMeasurement
        a             rdf:Property ;
        rdfs:comment  "A product measurement, for example the inseam of pants, the wheel size of a bicycle, or the gauge of a screw. Usually an exact measurement, but can also be a range of measurements for adjustable products, for example belts and ski bindings." ;
        rdfs:label    "hasMeasurement" .

schema:relatedCondition
        a             rdf:Property ;
        rdfs:comment  "A medical condition associated with this anatomy." ;
        rdfs:label    "relatedCondition" .

schema:RVPark  a         rdfs:Class ;
        rdfs:comment     "A place offering space for \"Recreational Vehicles\", Caravans, mobile homes and the like." ;
        rdfs:label       "RVPark" ;
        rdfs:subClassOf  schema:CivicStructure .

schema:MusicPlaylist  a  rdfs:Class ;
        rdfs:comment     "A collection of music tracks in playlist form." ;
        rdfs:label       "MusicPlaylist" ;
        rdfs:subClassOf  schema:CreativeWork .

schema:BorrowAction  a   rdfs:Class ;
        rdfs:comment     "The act of obtaining an object under an agreement to return it at a later date. Reciprocal of LendAction.\\n\\nRelated actions:\\n\\n* [[LendAction]]: Reciprocal of BorrowAction." ;
        rdfs:label       "BorrowAction" ;
        rdfs:subClassOf  schema:TransferAction .

schema:ComputerLanguage
        a                rdfs:Class ;
        rdfs:comment     "This type covers computer programming languages such as Scheme and Lisp, as well as other language-like computer representations. Natural languages are best represented with the [[Language]] type." ;
        rdfs:label       "ComputerLanguage" ;
        rdfs:subClassOf  schema:Intangible .

schema:typicalCreditsPerTerm
        a             rdf:Property ;
        rdfs:comment  "The number of credits or units a full-time student would be expected to take in 1 term however 'term' is defined by the institution." ;
        rdfs:label    "typicalCreditsPerTerm" .

schema:SportsOrganization
        a                rdfs:Class ;
        rdfs:comment     "Represents the collection of all sports organizations, including sports teams, governing bodies, and sports associations." ;
        rdfs:label       "SportsOrganization" ;
        rdfs:subClassOf  schema:Organization .

schema:BrokerageAccount
        a                rdfs:Class ;
        rdfs:comment     "An account that allows an investor to deposit funds and place investment orders with a licensed broker or brokerage firm." ;
        rdfs:label       "BrokerageAccount" ;
        rdfs:subClassOf  schema:InvestmentOrDeposit .

schema:ReportedDoseSchedule
        a                rdfs:Class ;
        rdfs:comment     "A patient-reported or observed dosing schedule for a drug or supplement." ;
        rdfs:label       "ReportedDoseSchedule" ;
        rdfs:subClassOf  schema:DoseSchedule .

schema:realEstateAgent
        a                   rdf:Property ;
        rdfs:comment        "A sub property of participant. The real estate agent involved in the action." ;
        rdfs:label          "realEstateAgent" ;
        rdfs:subPropertyOf  schema:participant .

schema:overdosage  a  rdf:Property ;
        rdfs:comment  "Any information related to overdose on a drug, including signs or symptoms, treatments, contact information for emergency response." ;
        rdfs:label    "overdosage" .

schema:TouristDestination
        a                rdfs:Class ;
        rdfs:comment     "A tourist destination. In principle any [[Place]] can be a [[TouristDestination]] from a [[City]], Region or [[Country]] to an [[AmusementPark]] or [[Hotel]]. This Type can be used on its own to describe a general [[TouristDestination]], or be used as an [[additionalType]] to add tourist relevant properties to any other [[Place]].  A [[TouristDestination]] is defined as a [[Place]] that contains, or is colocated with, one or more [[TouristAttraction]]s, often linked by a similar theme or interest to a particular [[touristType]]. The [UNWTO](http://www2.unwto.org/) defines Destination (main destination of a tourism trip) as the place visited that is central to the decision to take the trip.\n  (See examples below)." ;
        rdfs:label       "TouristDestination" ;
        rdfs:subClassOf  schema:Place .

schema:bankAccountType
        a             rdf:Property ;
        rdfs:comment  "The type of a bank account." ;
        rdfs:label    "bankAccountType" .

schema:cvdNumVent  a  rdf:Property ;
        rdfs:comment  "numvent - MECHANICAL VENTILATORS: Total number of ventilators available." ;
        rdfs:label    "cvdNumVent" .

schema:TypeAndQuantityNode
        a                rdfs:Class ;
        rdfs:comment     "A structured value indicating the quantity, unit of measurement, and business function of goods included in a bundle offer." ;
        rdfs:label       "TypeAndQuantityNode" ;
        rdfs:subClassOf  schema:StructuredValue .

schema:shippingDestination
        a             rdf:Property ;
        rdfs:comment  "indicates (possibly multiple) shipping destinations. These can be defined in several ways e.g. postalCode ranges." ;
        rdfs:label    "shippingDestination" .

schema:codeSampleType
        a             rdf:Property ;
        rdfs:comment  "What type of code sample: full (compile ready) solution, code snippet, inline code, scripts, template." ;
        rdfs:label    "codeSampleType" .

schema:usesHealthPlanIdStandard
        a             rdf:Property ;
        rdfs:comment  "The standard for interpreting thePlan ID. The preferred is \"HIOS\". See the Centers for Medicare & Medicaid Services for more details." ;
        rdfs:label    "usesHealthPlanIdStandard" .

schema:guideline  a   rdf:Property ;
        rdfs:comment  "A medical guideline related to this entity." ;
        rdfs:label    "guideline" .

schema:geoWithin  a   rdf:Property ;
        rdfs:comment  "Represents a relationship between two geometries (or the places they represent), relating a geometry to one that contains it, i.e. it is inside (i.e. within) its interior. As defined in [DE-9IM](https://en.wikipedia.org/wiki/DE-9IM)." ;
        rdfs:label    "geoWithin" .

schema:BloodTest  a      rdfs:Class ;
        rdfs:comment     "A medical test performed on a sample of a patient's blood." ;
        rdfs:label       "BloodTest" ;
        rdfs:subClassOf  schema:MedicalTest .

schema:Legislation  a    rdfs:Class ;
        rdfs:comment     "A legal document such as an act, decree, bill, etc. (enforceable or not) or a component of a legal act (like an article)." ;
        rdfs:label       "Legislation" ;
        rdfs:subClassOf  schema:CreativeWork .

schema:knowsAbout  a  rdf:Property ;
        rdfs:comment  "Of a [[Person]], and less typically of an [[Organization]], to indicate a topic that is known about - suggesting possible expertise but not implying it. We do not distinguish skill levels here, or relate this to educational content, events, objectives or [[JobPosting]] descriptions." ;
        rdfs:label    "knowsAbout" .

schema:JewelryStore  a   rdfs:Class ;
        rdfs:comment     "A jewelry store." ;
        rdfs:label       "JewelryStore" ;
        rdfs:subClassOf  schema:Store .

schema:hasPOS  a      rdf:Property ;
        rdfs:comment  "Points-of-Sales operated by the organization or person." ;
        rdfs:label    "hasPOS" .

schema:includesHealthPlanFormulary
        a             rdf:Property ;
        rdfs:comment  "Formularies covered by this plan." ;
        rdfs:label    "includesHealthPlanFormulary" .

schema:rangeIncludes  a  rdf:Property ;
        rdfs:comment  "Relates a property to a class that constitutes (one of) the expected type(s) for values of the property." ;
        rdfs:label    "rangeIncludes" .

schema:PalliativeProcedure
        a                rdfs:Class ;
        rdfs:comment     "A medical procedure intended primarily for palliative purposes, aimed at relieving the symptoms of an underlying health condition." ;
        rdfs:label       "PalliativeProcedure" ;
        rdfs:subClassOf  schema:MedicalTherapy , schema:MedicalProcedure .

schema:inAlbum  a     rdf:Property ;
        rdfs:comment  "The album to which this recording belongs." ;
        rdfs:label    "inAlbum" .

schema:cvdNumC19HospPats
        a             rdf:Property ;
        rdfs:comment  "numc19hosppats - HOSPITALIZED: Patients currently hospitalized in an inpatient care location who have suspected or confirmed COVID-19." ;
        rdfs:label    "cvdNumC19HospPats" .

schema:editor  a      rdf:Property ;
        rdfs:comment  "Specifies the Person who edited the CreativeWork." ;
        rdfs:label    "editor" .

schema:honorificPrefix
        a             rdf:Property ;
        rdfs:comment  "An honorific prefix preceding a Person's name such as Dr/Mrs/Mr." ;
        rdfs:label    "honorificPrefix" .

schema:mainEntity  a        rdf:Property ;
        rdfs:comment        "Indicates the primary entity described in some page or other CreativeWork." ;
        rdfs:label          "mainEntity" ;
        rdfs:subPropertyOf  schema:about .

schema:DiagnosticLab  a  rdfs:Class ;
        rdfs:comment     "A medical laboratory that offers on-site or off-site diagnostic services." ;
        rdfs:label       "DiagnosticLab" ;
        rdfs:subClassOf  schema:MedicalOrganization .

schema:DietNutrition  a  rdfs:Class ;
        rdfs:comment     "Dietetic and nutrition as a medical specialty." ;
        rdfs:label       "DietNutrition" ;
        rdfs:subClassOf  schema:MedicalBusiness .

schema:musicBy  a     rdf:Property ;
        rdfs:comment  "The composer of the soundtrack." ;
        rdfs:label    "musicBy" .

schema:question  a          rdf:Property ;
        rdfs:comment        "A sub property of object. A question." ;
        rdfs:label          "question" ;
        rdfs:subPropertyOf  schema:object .

schema:cvdNumC19MechVentPats
        a             rdf:Property ;
        rdfs:comment  "numc19mechventpats - HOSPITALIZED and VENTILATED: Patients hospitalized in an NHSN inpatient care location who have suspected or confirmed COVID-19 and are on a mechanical ventilator." ;
        rdfs:label    "cvdNumC19MechVentPats" .

schema:LegislativeBuilding
        a                rdfs:Class ;
        rdfs:comment     "A legislative building&#x2014;for example, the state capitol." ;
        rdfs:label       "LegislativeBuilding" ;
        rdfs:subClassOf  schema:GovernmentBuilding .

schema:articleSection
        a             rdf:Property ;
        rdfs:comment  "Articles may belong to one or more 'sections' in a magazine or newspaper, such as Sports, Lifestyle, etc." ;
        rdfs:label    "articleSection" .

schema:expertConsiderations
        a             rdf:Property ;
        rdfs:comment  "Medical expert advice related to the plan." ;
        rdfs:label    "expertConsiderations" .

schema:Role  a           rdfs:Class ;
        rdfs:comment     "Represents additional information about a relationship or property. For example a Role can be used to say that a 'member' role linking some SportsTeam to a player occurred during a particular time period. Or that a Person's 'actor' role in a Movie was for some particular characterName. Such properties can be attached to a Role entity, which is then associated with the main entities using ordinary properties like 'member' or 'actor'.\\n\\nSee also [blog post](http://blog.schema.org/2014/06/introducing-role.html)." ;
        rdfs:label       "Role" ;
        rdfs:subClassOf  schema:Intangible .

schema:eligibilityToWorkRequirement
        a             rdf:Property ;
        rdfs:comment  "The legal requirements such as citizenship, visa and other documentation required for an applicant to this job." ;
        rdfs:label    "eligibilityToWorkRequirement" .

schema:HealthAndBeautyBusiness
        a                rdfs:Class ;
        rdfs:comment     "Health and beauty." ;
        rdfs:label       "HealthAndBeautyBusiness" ;
        rdfs:subClassOf  schema:LocalBusiness .

schema:FundingScheme  a  rdfs:Class ;
        rdfs:comment     "A FundingScheme combines organizational, project and policy aspects of grant-based funding\n    that sets guidelines, principles and mechanisms to support other kinds of projects and activities.\n    Funding is typically organized via [[Grant]] funding. Examples of funding schemes: Swiss Priority Programmes (SPPs); EU Framework 7 (FP7); Horizon 2020; the NIH-R01 Grant Program; Wellcome institutional strategic support fund. For large scale public sector funding, the management and administration of grant awards is often handled by other, dedicated, organizations - [[FundingAgency]]s such as ERC, REA, ..." ;
        rdfs:label       "FundingScheme" ;
        rdfs:subClassOf  schema:Organization .

schema:HealthPlanFormulary
        a                rdfs:Class ;
        rdfs:comment     "For a given health insurance plan, the specification for costs and coverage of prescription drugs. " ;
        rdfs:label       "HealthPlanFormulary" ;
        rdfs:subClassOf  schema:Intangible .

schema:TherapeuticProcedure
        a                rdfs:Class ;
        rdfs:comment     "A medical procedure intended primarily for therapeutic purposes, aimed at improving a health condition." ;
        rdfs:label       "TherapeuticProcedure" ;
        rdfs:subClassOf  schema:MedicalProcedure .

schema:healthPlanNetworkTier
        a             rdf:Property ;
        rdfs:comment  "The tier(s) for this network." ;
        rdfs:label    "healthPlanNetworkTier" .

schema:WearableMeasurementTypeEnumeration
        a                rdfs:Class ;
        rdfs:comment     "Enumerates common types of measurement for wearables products." ;
        rdfs:label       "WearableMeasurementTypeEnumeration" ;
        rdfs:subClassOf  schema:MeasurementTypeEnumeration .

schema:UserBlocks  a     rdfs:Class ;
        rdfs:comment     "UserInteraction and its subtypes is an old way of talking about users interacting with pages. It is generally better to use [[Action]]-based vocabulary, alongside types such as [[Comment]]." ;
        rdfs:label       "UserBlocks" ;
        rdfs:subClassOf  schema:UserInteraction .

schema:merchantReturnDays
        a             rdf:Property ;
        rdfs:comment  "The merchantReturnDays property indicates the number of days (from purchase) within which relevant merchant return policy is applicable." ;
        rdfs:label    "merchantReturnDays" .

schema:BookStore  a      rdfs:Class ;
        rdfs:comment     "A bookstore." ;
        rdfs:label       "BookStore" ;
        rdfs:subClassOf  schema:Store .

schema:recommendedIntake
        a             rdf:Property ;
        rdfs:comment  "Recommended intake of this supplement for a given population as defined by a specific recommending authority." ;
        rdfs:label    "recommendedIntake" .

schema:Dentist  a        rdfs:Class ;
        rdfs:comment     "A dentist." ;
        rdfs:label       "Dentist" ;
        rdfs:subClassOf  schema:MedicalBusiness , schema:LocalBusiness , schema:MedicalOrganization .

schema:inLanguage  a  rdf:Property ;
        rdfs:comment  "The language of the content or performance or used in an action. Please use one of the language codes from the [IETF BCP 47 standard](http://tools.ietf.org/html/bcp47). See also [[availableLanguage]]." ;
        rdfs:label    "inLanguage" .

schema:ProgramMembership
        a                rdfs:Class ;
        rdfs:comment     "Used to describe membership in a loyalty programs (e.g. \"StarAliance\"), traveler clubs (e.g. \"AAA\"), purchase clubs (\"Safeway Club\"), etc." ;
        rdfs:label       "ProgramMembership" ;
        rdfs:subClassOf  schema:Intangible .

schema:doesNotShip  a  rdf:Property ;
        rdfs:comment  "Indicates when shipping to a particular [[shippingDestination]] is not available." ;
        rdfs:label    "doesNotShip" .

schema:targetProduct  a  rdf:Property ;
        rdfs:comment  "Target Operating System / Product to which the code applies.  If applies to several versions, just the product name can be used." ;
        rdfs:label    "targetProduct" .

schema:reservationFor
        a             rdf:Property ;
        rdfs:comment  "The thing -- flight, event, restaurant,etc. being reserved." ;
        rdfs:label    "reservationFor" .

schema:reviews  a     rdf:Property ;
        rdfs:comment  "Review of the item." ;
        rdfs:label    "reviews" .

schema:playMode  a    rdf:Property ;
        rdfs:comment  "Indicates whether this game is multi-player, co-op or single-player.  The game can be marked as multi-player, co-op and single-player at the same time." ;
        rdfs:label    "playMode" .

schema:Nursing  a        rdfs:Class ;
        rdfs:comment     "A health profession of a person formally educated and trained in the care of the sick or infirm person." ;
        rdfs:label       "Nursing" ;
        rdfs:subClassOf  schema:MedicalBusiness .

schema:numberOfBedrooms
        a             rdf:Property ;
        rdfs:comment  "The total integer number of bedrooms in a some [[Accommodation]], [[ApartmentComplex]] or [[FloorPlan]]." ;
        rdfs:label    "numberOfBedrooms" .

schema:ComedyEvent  a    rdfs:Class ;
        rdfs:comment     "Event type: Comedy event." ;
        rdfs:label       "ComedyEvent" ;
        rdfs:subClassOf  schema:Event .

schema:Blog  a           rdfs:Class ;
        rdfs:comment     "A blog." ;
        rdfs:label       "Blog" ;
        rdfs:subClassOf  schema:CreativeWork .

schema:addressRegion  a  rdf:Property ;
        rdfs:comment  "The region in which the locality is, and which is in the country. For example, California or another appropriate first-level [Administrative division](https://en.wikipedia.org/wiki/List_of_administrative_divisions_by_country) " ;
        rdfs:label    "addressRegion" .

schema:publicationType
        a             rdf:Property ;
        rdfs:comment  "The type of the medical article, taken from the US NLM MeSH publication type catalog. See also [MeSH documentation](http://www.nlm.nih.gov/mesh/pubtypes.html)." ;
        rdfs:label    "publicationType" .

schema:serviceArea  a  rdf:Property ;
        rdfs:comment  "The geographic area where the service is provided." ;
        rdfs:label    "serviceArea" .

schema:AnatomicalStructure
        a                rdfs:Class ;
        rdfs:comment     "Any part of the human body, typically a component of an anatomical system. Organs, tissues, and cells are all anatomical structures." ;
        rdfs:label       "AnatomicalStructure" ;
        rdfs:subClassOf  schema:MedicalEntity .

schema:DeactivateAction
        a                rdfs:Class ;
        rdfs:comment     "The act of stopping or deactivating a device or application (e.g. stopping a timer or turning off a flashlight)." ;
        rdfs:label       "DeactivateAction" ;
        rdfs:subClassOf  schema:ControlAction .

schema:DrugPrescriptionStatus
        a                rdfs:Class ;
        rdfs:comment     "Indicates whether this drug is available by prescription or over-the-counter." ;
        rdfs:label       "DrugPrescriptionStatus" ;
        rdfs:subClassOf  schema:MedicalEnumeration .

schema:ResearchProject
        a                rdfs:Class ;
        rdfs:comment     "A Research project." ;
        rdfs:label       "ResearchProject" ;
        rdfs:subClassOf  schema:Project .

schema:permitAudience
        a             rdf:Property ;
        rdfs:comment  "The target audience for this permit." ;
        rdfs:label    "permitAudience" .

schema:drug  a        rdf:Property ;
        rdfs:comment  "Specifying a drug or medicine used in a medication procedure." ;
        rdfs:label    "drug" .

schema:knowsLanguage  a  rdf:Property ;
        rdfs:comment  "Of a [[Person]], and less typically of an [[Organization]], to indicate a known language. We do not distinguish skill levels or reading/writing/speaking/signing here. Use language codes from the [IETF BCP 47 standard](http://tools.ietf.org/html/bcp47)." ;
        rdfs:label    "knowsLanguage" .

schema:activeIngredient
        a             rdf:Property ;
        rdfs:comment  "An active ingredient, typically chemical compounds and/or biologic substances." ;
        rdfs:label    "activeIngredient" .

schema:additionalName
        a             rdf:Property ;
        rdfs:comment  "An additional name for a Person, can be used for a middle name." ;
        rdfs:label    "additionalName" .

schema:CovidTestingFacility
        a                rdfs:Class ;
        rdfs:comment     "A CovidTestingFacility is a [[MedicalClinic]] where testing for the COVID-19 Coronavirus\n      disease is available. If the facility is being made available from an established [[Pharmacy]], [[Hotel]], or other\n      non-medical organization, multiple types can be listed. This makes it easier to re-use existing schema.org information\n      about that place e.g. contact info, address, opening hours. Note that in an emergency, such information may not always be reliable.\n      " ;
        rdfs:label       "CovidTestingFacility" ;
        rdfs:subClassOf  schema:MedicalClinic .

schema:EatAction  a      rdfs:Class ;
        rdfs:comment     "The act of swallowing solid objects." ;
        rdfs:label       "EatAction" ;
        rdfs:subClassOf  schema:ConsumeAction .

schema:RadioStation  a   rdfs:Class ;
        rdfs:comment     "A radio station." ;
        rdfs:label       "RadioStation" ;
        rdfs:subClassOf  schema:LocalBusiness .

schema:publication  a  rdf:Property ;
        rdfs:comment  "A publication event associated with the item." ;
        rdfs:label    "publication" .

schema:HairSalon  a      rdfs:Class ;
        rdfs:comment     "A hair salon." ;
        rdfs:label       "HairSalon" ;
        rdfs:subClassOf  schema:HealthAndBeautyBusiness .

schema:contentUrl  a  rdf:Property ;
        rdfs:comment  "Actual bytes of the media object, for example the image file or video file." ;
        rdfs:label    "contentUrl" .

schema:titleEIDR  a         rdf:Property ;
        rdfs:comment        "An [EIDR](https://eidr.org/) (Entertainment Identifier Registry) [[identifier]] representing at the most general/abstract level, a work of film or television.\n\nFor example, the motion picture known as \"Ghostbusters\" has a titleEIDR of  \"10.5240/7EC7-228A-510A-053E-CBB8-J\". This title (or work) may have several variants, which EIDR calls \"edits\". See [[editEIDR]].\n\nSince schema.org types like [[Movie]] and [[TVEpisode]] can be used for both works and their multiple expressions, it is possible to use [[titleEIDR]] alone (for a general description), or alongside [[editEIDR]] for a more edit-specific description.\n" ;
        rdfs:label          "titleEIDR" ;
        rdfs:subPropertyOf  schema:identifier .

schema:dateline  a    rdf:Property ;
        rdfs:comment  "A [dateline](https://en.wikipedia.org/wiki/Dateline) is a brief piece of text included in news articles that describes where and when the story was written or filed though the date is often omitted. Sometimes only a placename is provided.\n\nStructured representations of dateline-related information can also be expressed more explicitly using [[locationCreated]] (which represents where a work was created e.g. where a news report was written).  For location depicted or described in the content, use [[contentLocation]].\n\nDateline summaries are oriented more towards human readers than towards automated processing, and can vary substantially. Some examples: \"BEIRUT, Lebanon, June 2.\", \"Paris, France\", \"December 19, 2017 11:43AM Reporting from Washington\", \"Beijing/Moscow\", \"QUEZON CITY, Philippines\".\n      " ;
        rdfs:label    "dateline" .

schema:OccupationalExperienceRequirements
        a                rdfs:Class ;
        rdfs:comment     "Indicates employment-related experience requirements, e.g. [[monthsOfExperience]]." ;
        rdfs:label       "OccupationalExperienceRequirements" ;
        rdfs:subClassOf  schema:Intangible .

schema:differentialDiagnosis
        a             rdf:Property ;
        rdfs:comment  "One of a set of differential diagnoses for the condition. Specifically, a closely-related or competing diagnosis typically considered later in the cognitive process whereby this medical condition is distinguished from others most likely responsible for a similar collection of signs and symptoms to reach the most parsimonious diagnosis or diagnoses in a patient." ;
        rdfs:label    "differentialDiagnosis" .

schema:cvdNumICUBeds  a  rdf:Property ;
        rdfs:comment  "numicubeds - ICU BEDS: Total number of staffed inpatient intensive care unit (ICU) beds." ;
        rdfs:label    "cvdNumICUBeds" .

schema:BusOrCoach  a     rdfs:Class ;
        rdfs:comment     "A bus (also omnibus or autobus) is a road vehicle designed to carry passengers. Coaches are luxury busses, usually in service for long distance travel." ;
        rdfs:label       "BusOrCoach" ;
        rdfs:subClassOf  schema:Vehicle .

schema:TradeAction  a    rdfs:Class ;
        rdfs:comment     "The act of participating in an exchange of goods and services for monetary compensation. An agent trades an object, product or service with a participant in exchange for a one time or periodic payment." ;
        rdfs:label       "TradeAction" ;
        rdfs:subClassOf  schema:Action .

schema:ResumeAction  a   rdfs:Class ;
        rdfs:comment     "The act of resuming a device or application which was formerly paused (e.g. resume music playback or resume a timer)." ;
        rdfs:label       "ResumeAction" ;
        rdfs:subClassOf  schema:ControlAction .

schema:recordingOf  a  rdf:Property ;
        rdfs:comment  "The composition this track is a recording of." ;
        rdfs:label    "recordingOf" .

schema:MusicRelease  a   rdfs:Class ;
        rdfs:comment     "A MusicRelease is a specific release of a music album." ;
        rdfs:label       "MusicRelease" ;
        rdfs:subClassOf  schema:MusicPlaylist .

schema:codeRepository
        a             rdf:Property ;
        rdfs:comment  "Link to the repository where the un-compiled, human readable code and related code is located (SVN, github, CodePlex)." ;
        rdfs:label    "codeRepository" .

schema:AggregateRating
        a                rdfs:Class ;
        rdfs:comment     "The average rating based on multiple ratings or reviews." ;
        rdfs:label       "AggregateRating" ;
        rdfs:subClassOf  schema:Rating .

schema:isGift  a      rdf:Property ;
        rdfs:comment  "Was the offer accepted as a gift for someone other than the buyer." ;
        rdfs:label    "isGift" .

schema:MeasurementTypeEnumeration
        a                rdfs:Class ;
        rdfs:comment     "Enumeration of common measurement types (or dimensions), for example \"chest\" for a person, \"inseam\" for pants, \"gauge\" for screws, or \"wheel\" for bicycles." ;
        rdfs:label       "MeasurementTypeEnumeration" ;
        rdfs:subClassOf  schema:Enumeration .

schema:MarryAction  a    rdfs:Class ;
        rdfs:comment     "The act of marrying a person." ;
        rdfs:label       "MarryAction" ;
        rdfs:subClassOf  schema:InteractAction .

schema:subTrip  a     rdf:Property ;
        rdfs:comment  "Identifies a [[Trip]] that is a subTrip of this Trip.  For example Day 1, Day 2, etc. of a multi-day trip." ;
        rdfs:label    "subTrip" .

schema:departureTerminal
        a             rdf:Property ;
        rdfs:comment  "Identifier of the flight's departure terminal." ;
        rdfs:label    "departureTerminal" .

schema:isicV4  a      rdf:Property ;
        rdfs:comment  "The International Standard of Industrial Classification of All Economic Activities (ISIC), Revision 4 code for a particular organization, business person, or place." ;
        rdfs:label    "isicV4" .

schema:loanPaymentFrequency
        a             rdf:Property ;
        rdfs:comment  "Frequency of payments due, i.e. number of months between payments. This is defined as a frequency, i.e. the reciprocal of a period of time." ;
        rdfs:label    "loanPaymentFrequency" .

schema:gameLocation  a  rdf:Property ;
        rdfs:comment  "Real or fictional location of the game (or part of game)." ;
        rdfs:label    "gameLocation" .

schema:renegotiableLoan
        a             rdf:Property ;
        rdfs:comment  "Whether the terms for payment of interest can be renegotiated during the life of the loan." ;
        rdfs:label    "renegotiableLoan" .

schema:driveWheelConfiguration
        a             rdf:Property ;
        rdfs:comment  "The drive wheel configuration, i.e. which roadwheels will receive torque from the vehicle's engine via the drivetrain." ;
        rdfs:label    "driveWheelConfiguration" .

schema:Trip  a           rdfs:Class ;
        rdfs:comment     "A trip or journey. An itinerary of visits to one or more places." ;
        rdfs:label       "Trip" ;
        rdfs:subClassOf  schema:Intangible .

schema:Researcher  a     rdfs:Class ;
        rdfs:comment     "Researchers." ;
        rdfs:label       "Researcher" ;
        rdfs:subClassOf  schema:Audience .

schema:marginOfError  a  rdf:Property ;
        rdfs:comment  "A marginOfError for an [[Observation]]." ;
        rdfs:label    "marginOfError" .

schema:landlord  a          rdf:Property ;
        rdfs:comment        "A sub property of participant. The owner of the real estate property." ;
        rdfs:label          "landlord" ;
        rdfs:subPropertyOf  schema:participant .

schema:identifyingExam
        a             rdf:Property ;
        rdfs:comment  "A physical examination that can identify this sign." ;
        rdfs:label    "identifyingExam" .

schema:broadcastAffiliateOf
        a             rdf:Property ;
        rdfs:comment  "The media network(s) whose content is broadcast on this station." ;
        rdfs:label    "broadcastAffiliateOf" .

schema:additionalVariable
        a             rdf:Property ;
        rdfs:comment  "Any additional component of the exercise prescription that may need to be articulated to the patient. This may include the order of exercises, the number of repetitions of movement, quantitative distance, progressions over time, etc." ;
        rdfs:label    "additionalVariable" .

schema:subReservation
        a             rdf:Property ;
        rdfs:comment  "The individual reservations included in the package. Typically a repeated property." ;
        rdfs:label    "subReservation" .

schema:winner  a            rdf:Property ;
        rdfs:comment        "A sub property of participant. The winner of the action." ;
        rdfs:label          "winner" ;
        rdfs:subPropertyOf  schema:participant .

schema:datePosted  a  rdf:Property ;
        rdfs:comment  "Publication date of an online listing." ;
        rdfs:label    "datePosted" .
